<?xml version="1.0"?>
<rdf:RDF xmlns="http://purl.obolibrary.org/obo/aio/aio-full.owl#"
     xml:base="http://purl.obolibrary.org/obo/aio/aio-full.owl"
     xmlns:BFO="http://purl.obolibrary.org/obo/BFO_"
     xmlns:IAO="http://purl.obolibrary.org/obo/IAO_"
     xmlns:aio="https://w3id.org/aio/"
     xmlns:obo="http://purl.obolibrary.org/obo/"
     xmlns:owl="http://www.w3.org/2002/07/owl#"
     xmlns:rdf="http://www.w3.org/1999/02/22-rdf-syntax-ns#"
     xmlns:xml="http://www.w3.org/XML/1998/namespace"
     xmlns:xsd="http://www.w3.org/2001/XMLSchema#"
     xmlns:rdfs="http://www.w3.org/2000/01/rdf-schema#"
     xmlns:dcterms="http://purl.org/dc/terms/"
     xmlns:oboInOwl="http://www.geneontology.org/formats/oboInOwl#">
    <owl:Ontology rdf:about="http://purl.obolibrary.org/obo/aio/aio-full.owl">
        <owl:versionIRI rdf:resource="http://purl.obolibrary.org/obo/aio/releases/2024-06-26/aio-full.owl"/>
        <dcterms:description>This ontology models classes and relationships describing deep learning networks, their component layers and activation functions, as well as potential biases.</dcterms:description>
        <dcterms:license rdf:resource="http://creativecommons.org/licenses/by/4.0/"/>
        <dcterms:title>Artificial Intelligence Ontology</dcterms:title>
        <owl:versionInfo>2024-06-26</owl:versionInfo>
    </owl:Ontology>
    


    <!-- 
    ///////////////////////////////////////////////////////////////////////////////////////
    //
    // Annotation properties
    //
    ///////////////////////////////////////////////////////////////////////////////////////
     -->

    


    <!-- http://purl.obolibrary.org/obo/IAO_0000115 -->

    <owl:AnnotationProperty rdf:about="http://purl.obolibrary.org/obo/IAO_0000115">
        <obo:IAO_0000115>The official definition, explaining the meaning of a class or property. Shall be Aristotelian, formalized and normalized. Can be augmented with colloquial definitions.</obo:IAO_0000115>
        <rdfs:label>definition</rdfs:label>
    </owl:AnnotationProperty>
    


    <!-- http://purl.org/dc/terms/description -->

    <owl:AnnotationProperty rdf:about="http://purl.org/dc/terms/description">
        <obo:IAO_0000115>Description may include but is not limited to: an abstract, table of contents, reference to a graphical representation of content or a free-text account of the content.</obo:IAO_0000115>
        <rdfs:label>description</rdfs:label>
    </owl:AnnotationProperty>
    


    <!-- http://purl.org/dc/terms/license -->

    <owl:AnnotationProperty rdf:about="http://purl.org/dc/terms/license">
        <obo:IAO_0000115>A legal document giving official permission to do something with the resource.</obo:IAO_0000115>
        <rdfs:label>license</rdfs:label>
    </owl:AnnotationProperty>
    


    <!-- http://purl.org/dc/terms/title -->

    <owl:AnnotationProperty rdf:about="http://purl.org/dc/terms/title">
        <obo:IAO_0000115>A name given to the resource.</obo:IAO_0000115>
        <rdfs:label>title</rdfs:label>
    </owl:AnnotationProperty>
    


    <!-- http://www.geneontology.org/formats/oboInOwl#SubsetProperty -->

    <owl:AnnotationProperty rdf:about="http://www.geneontology.org/formats/oboInOwl#SubsetProperty">
        <rdfs:label xml:lang="en">subset_property</rdfs:label>
    </owl:AnnotationProperty>
    


    <!-- http://www.geneontology.org/formats/oboInOwl#hasDbXref -->

    <owl:AnnotationProperty rdf:about="http://www.geneontology.org/formats/oboInOwl#hasDbXref"/>
    


    <!-- http://www.geneontology.org/formats/oboInOwl#hasExactSynonym -->

    <owl:AnnotationProperty rdf:about="http://www.geneontology.org/formats/oboInOwl#hasExactSynonym"/>
    


    <!-- http://www.geneontology.org/formats/oboInOwl#hasRelatedSynonym -->

    <owl:AnnotationProperty rdf:about="http://www.geneontology.org/formats/oboInOwl#hasRelatedSynonym"/>
    


    <!-- http://www.geneontology.org/formats/oboInOwl#inSubset -->

    <owl:AnnotationProperty rdf:about="http://www.geneontology.org/formats/oboInOwl#inSubset"/>
    


    <!-- https://w3id.org/aio/BiasSubset -->

    <owl:AnnotationProperty rdf:about="https://w3id.org/aio/BiasSubset">
        <rdfs:comment xml:lang="en">Bias Subset</rdfs:comment>
        <rdfs:subPropertyOf rdf:resource="http://www.geneontology.org/formats/oboInOwl#SubsetProperty"/>
    </owl:AnnotationProperty>
    


    <!-- https://w3id.org/aio/ClassSubset -->

    <owl:AnnotationProperty rdf:about="https://w3id.org/aio/ClassSubset">
        <rdfs:comment xml:lang="en">Class Subset</rdfs:comment>
        <rdfs:subPropertyOf rdf:resource="http://www.geneontology.org/formats/oboInOwl#SubsetProperty"/>
    </owl:AnnotationProperty>
    


    <!-- https://w3id.org/aio/FunctionSubset -->

    <owl:AnnotationProperty rdf:about="https://w3id.org/aio/FunctionSubset">
        <rdfs:comment xml:lang="en">Function Subset</rdfs:comment>
        <rdfs:subPropertyOf rdf:resource="http://www.geneontology.org/formats/oboInOwl#SubsetProperty"/>
    </owl:AnnotationProperty>
    


    <!-- https://w3id.org/aio/LayerSubset -->

    <owl:AnnotationProperty rdf:about="https://w3id.org/aio/LayerSubset">
        <rdfs:comment xml:lang="en">Layer Subset</rdfs:comment>
        <rdfs:subPropertyOf rdf:resource="http://www.geneontology.org/formats/oboInOwl#SubsetProperty"/>
    </owl:AnnotationProperty>
    


    <!-- https://w3id.org/aio/MachineLearningSubset -->

    <owl:AnnotationProperty rdf:about="https://w3id.org/aio/MachineLearningSubset">
        <rdfs:comment xml:lang="en">Machine Learning Subset</rdfs:comment>
        <rdfs:subPropertyOf rdf:resource="http://www.geneontology.org/formats/oboInOwl#SubsetProperty"/>
    </owl:AnnotationProperty>
    


    <!-- https://w3id.org/aio/ModelSubset -->

    <owl:AnnotationProperty rdf:about="https://w3id.org/aio/ModelSubset">
        <rdfs:comment xml:lang="en">Model Subset</rdfs:comment>
        <rdfs:subPropertyOf rdf:resource="http://www.geneontology.org/formats/oboInOwl#SubsetProperty"/>
    </owl:AnnotationProperty>
    


    <!-- https://w3id.org/aio/NetworkSubset -->

    <owl:AnnotationProperty rdf:about="https://w3id.org/aio/NetworkSubset">
        <rdfs:comment xml:lang="en">Network Subset</rdfs:comment>
        <rdfs:subPropertyOf rdf:resource="http://www.geneontology.org/formats/oboInOwl#SubsetProperty"/>
    </owl:AnnotationProperty>
    


    <!-- https://w3id.org/aio/PreprocessingSubset -->

    <owl:AnnotationProperty rdf:about="https://w3id.org/aio/PreprocessingSubset">
        <rdfs:comment xml:lang="en">Preprocessing Subset</rdfs:comment>
        <rdfs:subPropertyOf rdf:resource="http://www.geneontology.org/formats/oboInOwl#SubsetProperty"/>
    </owl:AnnotationProperty>
    


    <!-- 
    ///////////////////////////////////////////////////////////////////////////////////////
    //
    // Object Properties
    //
    ///////////////////////////////////////////////////////////////////////////////////////
     -->

    


    <!-- http://purl.obolibrary.org/obo/BFO_0000050 -->

    <owl:ObjectProperty rdf:about="http://purl.obolibrary.org/obo/BFO_0000050">
        <obo:IAO_0000115 xml:lang="en">A core relation that holds between a part and its whole</obo:IAO_0000115>
        <rdfs:label xml:lang="en">part of</rdfs:label>
    </owl:ObjectProperty>
    


    <!-- http://purl.obolibrary.org/obo/BFO_0000051 -->

    <owl:ObjectProperty rdf:about="http://purl.obolibrary.org/obo/BFO_0000051"/>
    


    <!-- 
    ///////////////////////////////////////////////////////////////////////////////////////
    //
    // Data properties
    //
    ///////////////////////////////////////////////////////////////////////////////////////
     -->

    


    <!-- http://purl.obolibrary.org/obo/BFO_0000051 -->

    <owl:DatatypeProperty rdf:about="http://purl.obolibrary.org/obo/BFO_0000051"/>
    


    <!-- 
    ///////////////////////////////////////////////////////////////////////////////////////
    //
    // Classes
    //
    ///////////////////////////////////////////////////////////////////////////////////////
     -->

    


    <!-- https://w3id.org/aio/AbstractRNNCell -->

    <owl:Class rdf:about="https://w3id.org/aio/AbstractRNNCell">
        <rdfs:subClassOf rdf:resource="https://w3id.org/aio/Layer"/>
        <obo:IAO_0000115>An abstract layer object representing an RNN cell that is the base class for implementing RNN cells with custom behavior.</obo:IAO_0000115>
        <oboInOwl:inSubset rdf:resource="https://w3id.org/aio/LayerSubset"/>
        <rdfs:label>AbstractRNNCell</rdfs:label>
    </owl:Class>
    <owl:Axiom>
        <owl:annotatedSource rdf:resource="https://w3id.org/aio/AbstractRNNCell"/>
        <owl:annotatedProperty rdf:resource="http://purl.obolibrary.org/obo/IAO_0000115"/>
        <owl:annotatedTarget>An abstract layer object representing an RNN cell that is the base class for implementing RNN cells with custom behavior.</owl:annotatedTarget>
        <oboInOwl:hasDbXref rdf:resource="https://www.tensorflow.org/api_docs/python/tf/keras/layers/AbstractRNNCell"/>
    </owl:Axiom>
    


    <!-- https://w3id.org/aio/ActivationLayer -->

    <owl:Class rdf:about="https://w3id.org/aio/ActivationLayer">
        <rdfs:subClassOf rdf:resource="https://w3id.org/aio/Layer"/>
        <obo:IAO_0000115>A layer that applies an activation function to an output.</obo:IAO_0000115>
        <oboInOwl:inSubset rdf:resource="https://w3id.org/aio/LayerSubset"/>
        <rdfs:comment>Applies an activation function to an output.</rdfs:comment>
        <rdfs:label>Activation Layer</rdfs:label>
    </owl:Class>
    <owl:Axiom>
        <owl:annotatedSource rdf:resource="https://w3id.org/aio/ActivationLayer"/>
        <owl:annotatedProperty rdf:resource="http://purl.obolibrary.org/obo/IAO_0000115"/>
        <owl:annotatedTarget>A layer that applies an activation function to an output.</owl:annotatedTarget>
        <oboInOwl:hasDbXref rdf:resource="https://www.tensorflow.org/api_docs/python/tf/keras/layers/Activation"/>
    </owl:Axiom>
    


    <!-- https://w3id.org/aio/ActiveLearning -->

    <owl:Class rdf:about="https://w3id.org/aio/ActiveLearning">
        <rdfs:subClassOf rdf:resource="https://w3id.org/aio/MachineLearning"/>
        <obo:IAO_0000115>A type of machine learning focused on methods that interactively query a user or another information source to label new data points with the desired outputs.</obo:IAO_0000115>
        <oboInOwl:hasExactSynonym>Query Learning</oboInOwl:hasExactSynonym>
        <oboInOwl:inSubset rdf:resource="https://w3id.org/aio/MachineLearningSubset"/>
        <rdfs:label>Active Learning</rdfs:label>
    </owl:Class>
    <owl:Axiom>
        <owl:annotatedSource rdf:resource="https://w3id.org/aio/ActiveLearning"/>
        <owl:annotatedProperty rdf:resource="http://purl.obolibrary.org/obo/IAO_0000115"/>
        <owl:annotatedTarget>A type of machine learning focused on methods that interactively query a user or another information source to label new data points with the desired outputs.</owl:annotatedTarget>
        <oboInOwl:hasDbXref rdf:resource="https://en.wikipedia.org/wiki/Active_learning_(machine_learning)"/>
    </owl:Axiom>
    


    <!-- https://w3id.org/aio/ActivityBias -->

    <owl:Class rdf:about="https://w3id.org/aio/ActivityBias">
        <rdfs:subClassOf rdf:resource="https://w3id.org/aio/UseAndInterpretationBias"/>
        <obo:IAO_0000115>A use and interpretation bias occurring when systems/platforms get training data from their most active users rather than less active or inactive users.</obo:IAO_0000115>
        <oboInOwl:inSubset rdf:resource="https://w3id.org/aio/BiasSubset"/>
        <rdfs:label>Activity Bias</rdfs:label>
    </owl:Class>
    <owl:Axiom>
        <owl:annotatedSource rdf:resource="https://w3id.org/aio/ActivityBias"/>
        <owl:annotatedProperty rdf:resource="http://purl.obolibrary.org/obo/IAO_0000115"/>
        <owl:annotatedTarget>A use and interpretation bias occurring when systems/platforms get training data from their most active users rather than less active or inactive users.</owl:annotatedTarget>
        <oboInOwl:hasDbXref rdf:resource="https://en.wikipedia.org/wiki/Interpretive_bias"/>
    </owl:Axiom>
    


    <!-- https://w3id.org/aio/ActivityRegularizationLayer -->

    <owl:Class rdf:about="https://w3id.org/aio/ActivityRegularizationLayer">
        <rdfs:subClassOf rdf:resource="https://w3id.org/aio/RegularizationLayer"/>
        <obo:IAO_0000115>A regularization layer that applies an update to the cost function based on input activity.</obo:IAO_0000115>
        <oboInOwl:inSubset rdf:resource="https://w3id.org/aio/LayerSubset"/>
        <rdfs:label>ActivityRegularization Layer</rdfs:label>
    </owl:Class>
    <owl:Axiom>
        <owl:annotatedSource rdf:resource="https://w3id.org/aio/ActivityRegularizationLayer"/>
        <owl:annotatedProperty rdf:resource="http://purl.obolibrary.org/obo/IAO_0000115"/>
        <owl:annotatedTarget>A regularization layer that applies an update to the cost function based on input activity.</owl:annotatedTarget>
        <oboInOwl:hasDbXref rdf:resource="https://www.tensorflow.org/api_docs/python/tf/keras/layers/ActivityRegularization"/>
    </owl:Axiom>
    


    <!-- https://w3id.org/aio/AdaptiveAvgPool1DLayer -->

    <owl:Class rdf:about="https://w3id.org/aio/AdaptiveAvgPool1DLayer">
        <rdfs:subClassOf rdf:resource="https://w3id.org/aio/PoolingLayer"/>
        <obo:IAO_0000115>A pooling layer that applies a 1D adaptive average pooling over an input signal composed of several input planes.</obo:IAO_0000115>
        <oboInOwl:hasExactSynonym>AdaptiveAvgPool1D</oboInOwl:hasExactSynonym>
        <oboInOwl:inSubset rdf:resource="https://w3id.org/aio/LayerSubset"/>
        <rdfs:label>AdaptiveAvgPool1D Layer</rdfs:label>
    </owl:Class>
    <owl:Axiom>
        <owl:annotatedSource rdf:resource="https://w3id.org/aio/AdaptiveAvgPool1DLayer"/>
        <owl:annotatedProperty rdf:resource="http://purl.obolibrary.org/obo/IAO_0000115"/>
        <owl:annotatedTarget>A pooling layer that applies a 1D adaptive average pooling over an input signal composed of several input planes.</owl:annotatedTarget>
        <oboInOwl:hasDbXref rdf:resource="https://pytorch.org/docs/stable/nn.html#pooling-layers"/>
    </owl:Axiom>
    


    <!-- https://w3id.org/aio/AdaptiveAvgPool2DLayer -->

    <owl:Class rdf:about="https://w3id.org/aio/AdaptiveAvgPool2DLayer">
        <rdfs:subClassOf rdf:resource="https://w3id.org/aio/PoolingLayer"/>
        <obo:IAO_0000115>A pooling layer that applies a 2D adaptive average pooling over an input signal composed of several input planes.</obo:IAO_0000115>
        <oboInOwl:hasExactSynonym>AdaptiveAvgPool2D</oboInOwl:hasExactSynonym>
        <oboInOwl:inSubset rdf:resource="https://w3id.org/aio/LayerSubset"/>
        <rdfs:label>AdaptiveAvgPool2D Layer</rdfs:label>
    </owl:Class>
    <owl:Axiom>
        <owl:annotatedSource rdf:resource="https://w3id.org/aio/AdaptiveAvgPool2DLayer"/>
        <owl:annotatedProperty rdf:resource="http://purl.obolibrary.org/obo/IAO_0000115"/>
        <owl:annotatedTarget>A pooling layer that applies a 2D adaptive average pooling over an input signal composed of several input planes.</owl:annotatedTarget>
        <oboInOwl:hasDbXref rdf:resource="https://pytorch.org/docs/stable/nn.html#pooling-layers"/>
    </owl:Axiom>
    


    <!-- https://w3id.org/aio/AdaptiveAvgPool3DLayer -->

    <owl:Class rdf:about="https://w3id.org/aio/AdaptiveAvgPool3DLayer">
        <rdfs:subClassOf rdf:resource="https://w3id.org/aio/PoolingLayer"/>
        <obo:IAO_0000115>A pooling layer that applies a 3D adaptive average pooling over an input signal composed of several input planes.</obo:IAO_0000115>
        <oboInOwl:hasExactSynonym>AdaptiveAvgPool3D</oboInOwl:hasExactSynonym>
        <oboInOwl:inSubset rdf:resource="https://w3id.org/aio/LayerSubset"/>
        <rdfs:label>AdaptiveAvgPool3D Layer</rdfs:label>
    </owl:Class>
    <owl:Axiom>
        <owl:annotatedSource rdf:resource="https://w3id.org/aio/AdaptiveAvgPool3DLayer"/>
        <owl:annotatedProperty rdf:resource="http://purl.obolibrary.org/obo/IAO_0000115"/>
        <owl:annotatedTarget>A pooling layer that applies a 3D adaptive average pooling over an input signal composed of several input planes.</owl:annotatedTarget>
        <oboInOwl:hasDbXref rdf:resource="https://pytorch.org/docs/stable/nn.html#pooling-layers"/>
    </owl:Axiom>
    


    <!-- https://w3id.org/aio/AdaptiveMaxPool1DLayer -->

    <owl:Class rdf:about="https://w3id.org/aio/AdaptiveMaxPool1DLayer">
        <rdfs:subClassOf rdf:resource="https://w3id.org/aio/PoolingLayer"/>
        <obo:IAO_0000115>A pooling layer that applies a 1D adaptive max pooling over an input signal composed of several input planes.</obo:IAO_0000115>
        <oboInOwl:hasExactSynonym>AdaptiveMaxPool1D</oboInOwl:hasExactSynonym>
        <oboInOwl:inSubset rdf:resource="https://w3id.org/aio/LayerSubset"/>
        <rdfs:label>AdaptiveMaxPool1D Layer</rdfs:label>
    </owl:Class>
    <owl:Axiom>
        <owl:annotatedSource rdf:resource="https://w3id.org/aio/AdaptiveMaxPool1DLayer"/>
        <owl:annotatedProperty rdf:resource="http://purl.obolibrary.org/obo/IAO_0000115"/>
        <owl:annotatedTarget>A pooling layer that applies a 1D adaptive max pooling over an input signal composed of several input planes.</owl:annotatedTarget>
        <oboInOwl:hasDbXref rdf:resource="https://pytorch.org/docs/stable/nn.html#pooling-layers"/>
    </owl:Axiom>
    


    <!-- https://w3id.org/aio/AdaptiveMaxPool2DLayer -->

    <owl:Class rdf:about="https://w3id.org/aio/AdaptiveMaxPool2DLayer">
        <rdfs:subClassOf rdf:resource="https://w3id.org/aio/PoolingLayer"/>
        <obo:IAO_0000115>A pooling layer that applies a 2D adaptive max pooling over an input signal composed of several input planes.</obo:IAO_0000115>
        <oboInOwl:hasExactSynonym>AdaptiveMaxPool2D</oboInOwl:hasExactSynonym>
        <oboInOwl:inSubset rdf:resource="https://w3id.org/aio/LayerSubset"/>
        <rdfs:label>AdaptiveMaxPool2D Layer</rdfs:label>
    </owl:Class>
    <owl:Axiom>
        <owl:annotatedSource rdf:resource="https://w3id.org/aio/AdaptiveMaxPool2DLayer"/>
        <owl:annotatedProperty rdf:resource="http://purl.obolibrary.org/obo/IAO_0000115"/>
        <owl:annotatedTarget>A pooling layer that applies a 2D adaptive max pooling over an input signal composed of several input planes.</owl:annotatedTarget>
        <oboInOwl:hasDbXref rdf:resource="https://pytorch.org/docs/stable/nn.html#pooling-layers"/>
    </owl:Axiom>
    


    <!-- https://w3id.org/aio/AdaptiveMaxPool3DLayer -->

    <owl:Class rdf:about="https://w3id.org/aio/AdaptiveMaxPool3DLayer">
        <rdfs:subClassOf rdf:resource="https://w3id.org/aio/PoolingLayer"/>
        <obo:IAO_0000115>A pooling layer that applies a 3D adaptive max pooling over an input signal composed of several input planes.</obo:IAO_0000115>
        <oboInOwl:hasExactSynonym>AdaptiveMaxPool3D</oboInOwl:hasExactSynonym>
        <oboInOwl:inSubset rdf:resource="https://w3id.org/aio/LayerSubset"/>
        <rdfs:label>AdaptiveMaxPool3D Layer</rdfs:label>
    </owl:Class>
    <owl:Axiom>
        <owl:annotatedSource rdf:resource="https://w3id.org/aio/AdaptiveMaxPool3DLayer"/>
        <owl:annotatedProperty rdf:resource="http://purl.obolibrary.org/obo/IAO_0000115"/>
        <owl:annotatedTarget>A pooling layer that applies a 3D adaptive max pooling over an input signal composed of several input planes.</owl:annotatedTarget>
        <oboInOwl:hasDbXref rdf:resource="https://pytorch.org/docs/stable/nn.html#pooling-layers"/>
    </owl:Axiom>
    


    <!-- https://w3id.org/aio/AddLayer -->

    <owl:Class rdf:about="https://w3id.org/aio/AddLayer">
        <rdfs:subClassOf rdf:resource="https://w3id.org/aio/MergingLayer"/>
        <obo:IAO_0000115>A merging layer that adds a list of inputs taking as input a list of tensors all of the same shape.</obo:IAO_0000115>
        <oboInOwl:inSubset rdf:resource="https://w3id.org/aio/LayerSubset"/>
        <rdfs:comment>Layer that adds a list of inputs. It takes as input a list of tensors, all of the same shape, and returns a single tensor (also of the same shape).</rdfs:comment>
        <rdfs:label>Add Layer</rdfs:label>
    </owl:Class>
    <owl:Axiom>
        <owl:annotatedSource rdf:resource="https://w3id.org/aio/AddLayer"/>
        <owl:annotatedProperty rdf:resource="http://purl.obolibrary.org/obo/IAO_0000115"/>
        <owl:annotatedTarget>A merging layer that adds a list of inputs taking as input a list of tensors all of the same shape.</owl:annotatedTarget>
        <oboInOwl:hasDbXref rdf:resource="https://www.tensorflow.org/api_docs/python/tf/keras/layers/Add"/>
    </owl:Axiom>
    


    <!-- https://w3id.org/aio/AdditionLayer -->

    <owl:Class rdf:about="https://w3id.org/aio/AdditionLayer">
        <rdfs:subClassOf rdf:resource="https://w3id.org/aio/Layer"/>
        <obo:IAO_0000115>A layer that adds inputs from one or more other layers to cells or neurons of a target layer.</obo:IAO_0000115>
        <oboInOwl:inSubset rdf:resource="https://w3id.org/aio/LayerSubset"/>
        <rdfs:label>Addition Layer</rdfs:label>
    </owl:Class>
    


    <!-- https://w3id.org/aio/AdditiveAttentionLayer -->

    <owl:Class rdf:about="https://w3id.org/aio/AdditiveAttentionLayer">
        <rdfs:subClassOf rdf:resource="https://w3id.org/aio/AttentionLayer"/>
        <obo:IAO_0000115>An attention layer that implements additive attention also known as Bahdanau-style attention.</obo:IAO_0000115>
        <oboInOwl:inSubset rdf:resource="https://w3id.org/aio/LayerSubset"/>
        <rdfs:comment>Additive attention layer, a.k.a. Bahdanau-style attention.</rdfs:comment>
        <rdfs:label>AdditiveAttention Layer</rdfs:label>
    </owl:Class>
    <owl:Axiom>
        <owl:annotatedSource rdf:resource="https://w3id.org/aio/AdditiveAttentionLayer"/>
        <owl:annotatedProperty rdf:resource="http://purl.obolibrary.org/obo/IAO_0000115"/>
        <owl:annotatedTarget>An attention layer that implements additive attention also known as Bahdanau-style attention.</owl:annotatedTarget>
        <oboInOwl:hasDbXref rdf:resource="https://www.tensorflow.org/api_docs/python/tf/keras/layers/AdditiveAttention"/>
    </owl:Axiom>
    


    <!-- https://w3id.org/aio/AlphaDropoutLayer -->

    <owl:Class rdf:about="https://w3id.org/aio/AlphaDropoutLayer">
        <rdfs:subClassOf rdf:resource="https://w3id.org/aio/RegularizationLayer"/>
        <obo:IAO_0000115>A regularization layer that applies Alpha Dropout to the input keeping mean and variance of inputs to ensure self-normalizing property.</obo:IAO_0000115>
        <oboInOwl:inSubset rdf:resource="https://w3id.org/aio/LayerSubset"/>
        <rdfs:comment>Applies Alpha Dropout to the input. Alpha Dropout is a Dropout that keeps mean and variance of inputs to their original values, in order to ensure the self-normalizing property even after this dropout. Alpha Dropout fits well to Scaled Exponential Linear Units by randomly setting activations to the negative saturation value.</rdfs:comment>
        <rdfs:label>AlphaDropout Layer</rdfs:label>
    </owl:Class>
    <owl:Axiom>
        <owl:annotatedSource rdf:resource="https://w3id.org/aio/AlphaDropoutLayer"/>
        <owl:annotatedProperty rdf:resource="http://purl.obolibrary.org/obo/IAO_0000115"/>
        <owl:annotatedTarget>A regularization layer that applies Alpha Dropout to the input keeping mean and variance of inputs to ensure self-normalizing property.</owl:annotatedTarget>
        <oboInOwl:hasDbXref rdf:resource="https://www.tensorflow.org/api_docs/python/tf/keras/layers/AlphaDropout"/>
    </owl:Axiom>
    


    <!-- https://w3id.org/aio/AmplificationBias -->

    <owl:Class rdf:about="https://w3id.org/aio/AmplificationBias">
        <rdfs:subClassOf rdf:resource="https://w3id.org/aio/ProcessingBias"/>
        <obo:IAO_0000115>A processing bias arising when the distribution over prediction outputs is skewed compared to the prior distribution of the prediction target.</obo:IAO_0000115>
        <oboInOwl:inSubset rdf:resource="https://w3id.org/aio/BiasSubset"/>
        <rdfs:label>Amplification Bias</rdfs:label>
    </owl:Class>
    <owl:Axiom>
        <owl:annotatedSource rdf:resource="https://w3id.org/aio/AmplificationBias"/>
        <owl:annotatedProperty rdf:resource="http://purl.obolibrary.org/obo/IAO_0000115"/>
        <owl:annotatedTarget>A processing bias arising when the distribution over prediction outputs is skewed compared to the prior distribution of the prediction target.</owl:annotatedTarget>
        <oboInOwl:hasDbXref rdf:resource="https://royalsocietypublishing.org/doi/10.1098/rspb.2019.0165#d1e5237"/>
    </owl:Axiom>
    


    <!-- https://w3id.org/aio/AnchoringBias -->

    <owl:Class rdf:about="https://w3id.org/aio/AnchoringBias">
        <rdfs:subClassOf rdf:resource="https://w3id.org/aio/IndividualBias"/>
        <obo:IAO_0000115>A cognitive bias characterized by the influence of a reference point or anchor on decisions leading to insufficient adjustment from that anchor point.</obo:IAO_0000115>
        <oboInOwl:inSubset rdf:resource="https://w3id.org/aio/BiasSubset"/>
        <rdfs:label>Anchoring Bias</rdfs:label>
    </owl:Class>
    <owl:Axiom>
        <owl:annotatedSource rdf:resource="https://w3id.org/aio/AnchoringBias"/>
        <owl:annotatedProperty rdf:resource="http://purl.obolibrary.org/obo/IAO_0000115"/>
        <owl:annotatedTarget>A cognitive bias characterized by the influence of a reference point or anchor on decisions leading to insufficient adjustment from that anchor point.</owl:annotatedTarget>
        <oboInOwl:hasDbXref rdf:resource="https://doi.org/10.6028/NIST.SP.1270"/>
    </owl:Axiom>
    


    <!-- https://w3id.org/aio/AnnotatorReportingBias -->

    <owl:Class rdf:about="https://w3id.org/aio/AnnotatorReportingBias">
        <rdfs:subClassOf rdf:resource="https://w3id.org/aio/IndividualBias"/>
        <obo:IAO_0000115>An individual bias occurring when users rely on automation as a heuristic replacement for their own information seeking and processing.</obo:IAO_0000115>
        <oboInOwl:inSubset rdf:resource="https://w3id.org/aio/BiasSubset"/>
        <rdfs:label>Annotator Reporting Bias</rdfs:label>
    </owl:Class>
    <owl:Axiom>
        <owl:annotatedSource rdf:resource="https://w3id.org/aio/AnnotatorReportingBias"/>
        <owl:annotatedProperty rdf:resource="http://purl.obolibrary.org/obo/IAO_0000115"/>
        <owl:annotatedTarget>An individual bias occurring when users rely on automation as a heuristic replacement for their own information seeking and processing.</owl:annotatedTarget>
        <oboInOwl:hasDbXref rdf:resource="https://doi.org/10.6028/NIST.SP.1270"/>
    </owl:Axiom>
    


    <!-- https://w3id.org/aio/ArtificialNeuralNetwork -->

    <owl:Class rdf:about="https://w3id.org/aio/ArtificialNeuralNetwork">
        <rdfs:subClassOf rdf:resource="https://w3id.org/aio/Network"/>
        <obo:IAO_0000115>A network based on a collection of connected units called artificial neurons modeled after biological neurons.</obo:IAO_0000115>
        <oboInOwl:hasExactSynonym>ANN</oboInOwl:hasExactSynonym>
        <oboInOwl:hasExactSynonym>NN</oboInOwl:hasExactSynonym>
        <oboInOwl:inSubset rdf:resource="https://w3id.org/aio/NetworkSubset"/>
        <rdfs:comment>An artificial neural network (ANN) is based on a collection of connected units or nodes called artificial neurons, modeled after biological neurons, with connections transmitting signals processed by non-linear functions.</rdfs:comment>
        <rdfs:label>Artificial Neural Network</rdfs:label>
    </owl:Class>
    <owl:Axiom>
        <owl:annotatedSource rdf:resource="https://w3id.org/aio/ArtificialNeuralNetwork"/>
        <owl:annotatedProperty rdf:resource="http://purl.obolibrary.org/obo/IAO_0000115"/>
        <owl:annotatedTarget>A network based on a collection of connected units called artificial neurons modeled after biological neurons.</owl:annotatedTarget>
        <oboInOwl:hasDbXref rdf:resource="https://en.wikipedia.org/wiki/Artificial_neural_network"/>
    </owl:Axiom>
    


    <!-- https://w3id.org/aio/AssociationRuleLearning -->

    <owl:Class rdf:about="https://w3id.org/aio/AssociationRuleLearning">
        <rdfs:subClassOf rdf:resource="https://w3id.org/aio/SupervisedLearning"/>
        <obo:IAO_0000115>A supervised learning method focused on a rule-based approach for discovering interesting relations between variables in large databases.</obo:IAO_0000115>
        <oboInOwl:inSubset rdf:resource="https://w3id.org/aio/MachineLearningSubset"/>
        <rdfs:label>Association Rule Learning</rdfs:label>
    </owl:Class>
    <owl:Axiom>
        <owl:annotatedSource rdf:resource="https://w3id.org/aio/AssociationRuleLearning"/>
        <owl:annotatedProperty rdf:resource="http://purl.obolibrary.org/obo/IAO_0000115"/>
        <owl:annotatedTarget>A supervised learning method focused on a rule-based approach for discovering interesting relations between variables in large databases.</owl:annotatedTarget>
        <oboInOwl:hasDbXref rdf:resource="https://en.wikipedia.org/wiki/Association_rule_learning"/>
    </owl:Axiom>
    


    <!-- https://w3id.org/aio/AttentionLayer -->

    <owl:Class rdf:about="https://w3id.org/aio/AttentionLayer">
        <rdfs:subClassOf rdf:resource="https://w3id.org/aio/Layer"/>
        <obo:IAO_0000115>A layer that implements dot-product attention also known as Luong-style attention.</obo:IAO_0000115>
        <oboInOwl:inSubset rdf:resource="https://w3id.org/aio/LayerSubset"/>
        <rdfs:comment>Dot-product attention layer, a.k.a. Luong-style attention.</rdfs:comment>
        <rdfs:label>Attention Layer</rdfs:label>
    </owl:Class>
    <owl:Axiom>
        <owl:annotatedSource rdf:resource="https://w3id.org/aio/AttentionLayer"/>
        <owl:annotatedProperty rdf:resource="http://purl.obolibrary.org/obo/IAO_0000115"/>
        <owl:annotatedTarget>A layer that implements dot-product attention also known as Luong-style attention.</owl:annotatedTarget>
        <oboInOwl:hasDbXref rdf:resource="https://www.tensorflow.org/api_docs/python/tf/keras/layers/Attention"/>
    </owl:Axiom>
    


    <!-- https://w3id.org/aio/AutoEncoderNetwork -->

    <owl:Class rdf:about="https://w3id.org/aio/AutoEncoderNetwork">
        <rdfs:subClassOf rdf:resource="https://w3id.org/aio/UnsupervisedPretrainedNetwork"/>
        <rdfs:subClassOf>
            <owl:Restriction>
                <owl:onProperty rdf:resource="http://purl.obolibrary.org/obo/BFO_0000051"/>
                <owl:someValuesFrom rdf:resource="https://w3id.org/aio/HiddenLayer"/>
            </owl:Restriction>
        </rdfs:subClassOf>
        <rdfs:subClassOf>
            <owl:Restriction>
                <owl:onProperty rdf:resource="http://purl.obolibrary.org/obo/BFO_0000051"/>
                <owl:someValuesFrom rdf:resource="https://w3id.org/aio/MatchedInputOutputLayer"/>
            </owl:Restriction>
        </rdfs:subClassOf>
        <obo:IAO_0000115>An unsupervised pretrained network that learns efficient codings of unlabeled data by training to ignore insignificant data and regenerate input from encoding.</obo:IAO_0000115>
        <oboInOwl:hasExactSynonym>AE</oboInOwl:hasExactSynonym>
        <oboInOwl:inSubset rdf:resource="https://w3id.org/aio/NetworkSubset"/>
        <rdfs:comment>Layers: Input, Hidden, Matched Output-Input</rdfs:comment>
        <rdfs:label>Auto Encoder Network</rdfs:label>
    </owl:Class>
    <owl:Axiom>
        <owl:annotatedSource rdf:resource="https://w3id.org/aio/AutoEncoderNetwork"/>
        <owl:annotatedProperty rdf:resource="http://purl.obolibrary.org/obo/IAO_0000115"/>
        <owl:annotatedTarget>An unsupervised pretrained network that learns efficient codings of unlabeled data by training to ignore insignificant data and regenerate input from encoding.</owl:annotatedTarget>
        <oboInOwl:hasDbXref rdf:resource="https://en.wikipedia.org/wiki/Autoencoder"/>
    </owl:Axiom>
    


    <!-- https://w3id.org/aio/AutomationComplacencyBias -->

    <owl:Class rdf:about="https://w3id.org/aio/AutomationComplacencyBias">
        <rdfs:subClassOf rdf:resource="https://w3id.org/aio/IndividualBias"/>
        <obo:IAO_0000115>A bias characterized by over-reliance on automated systems leading to attenuated human skills.</obo:IAO_0000115>
        <oboInOwl:hasExactSynonym>Automation Complaceny</oboInOwl:hasExactSynonym>
        <oboInOwl:inSubset rdf:resource="https://w3id.org/aio/BiasSubset"/>
        <rdfs:comment>Over-reliance on automated systems, leading to attenuated human skills, such as with spelling and autocorrect.</rdfs:comment>
        <rdfs:label>Automation Complacency Bias</rdfs:label>
    </owl:Class>
    <owl:Axiom>
        <owl:annotatedSource rdf:resource="https://w3id.org/aio/AutomationComplacencyBias"/>
        <owl:annotatedProperty rdf:resource="http://purl.obolibrary.org/obo/IAO_0000115"/>
        <owl:annotatedTarget>A bias characterized by over-reliance on automated systems leading to attenuated human skills.</owl:annotatedTarget>
        <oboInOwl:hasDbXref rdf:resource="https://doi.org/10.6028/NIST.SP.1270"/>
    </owl:Axiom>
    


    <!-- https://w3id.org/aio/AutoregressiveConditionalHeteroskedasticity -->

    <owl:Class rdf:about="https://w3id.org/aio/AutoregressiveConditionalHeteroskedasticity">
        <rdfs:subClassOf rdf:resource="https://w3id.org/aio/Model"/>
        <obo:IAO_0000115>A model that describes the variance of the current error term as a function of the previous periods&apos; error terms, capturing volatility clustering. Used for time series data.</obo:IAO_0000115>
        <oboInOwl:hasExactSynonym>ARCH</oboInOwl:hasExactSynonym>
        <oboInOwl:inSubset rdf:resource="https://w3id.org/aio/ModelSubset"/>
        <rdfs:label>Autoregressive Conditional Heteroskedasticity</rdfs:label>
    </owl:Class>
    


    <!-- https://w3id.org/aio/AutoregressiveDistributedLag -->

    <owl:Class rdf:about="https://w3id.org/aio/AutoregressiveDistributedLag">
        <rdfs:subClassOf rdf:resource="https://w3id.org/aio/Model"/>
        <obo:IAO_0000115>A model that includes lagged values of both the dependent variable and one or more independent variables, capturing dynamic relationships over time. Used in time series analysis.</obo:IAO_0000115>
        <oboInOwl:hasExactSynonym>ARDL</oboInOwl:hasExactSynonym>
        <oboInOwl:inSubset rdf:resource="https://w3id.org/aio/ModelSubset"/>
        <rdfs:label>Autoregressive Distributed Lag</rdfs:label>
    </owl:Class>
    


    <!-- https://w3id.org/aio/AutoregressiveIntegratedMovingAverage -->

    <owl:Class rdf:about="https://w3id.org/aio/AutoregressiveIntegratedMovingAverage">
        <rdfs:subClassOf rdf:resource="https://w3id.org/aio/Model"/>
        <obo:IAO_0000115>A model which combines autoregression (AR), differencing (I), and moving average (MA) components. Used for analyzing and forecasting time series data.</obo:IAO_0000115>
        <oboInOwl:hasExactSynonym>ARIMA</oboInOwl:hasExactSynonym>
        <oboInOwl:inSubset rdf:resource="https://w3id.org/aio/ModelSubset"/>
        <rdfs:label>Autoregressive Integrated Moving Average</rdfs:label>
    </owl:Class>
    


    <!-- https://w3id.org/aio/AutoregressiveLanguageModel -->

    <owl:Class rdf:about="https://w3id.org/aio/AutoregressiveLanguageModel">
        <rdfs:subClassOf rdf:resource="https://w3id.org/aio/LanguageModel"/>
        <obo:IAO_0000115>A language model that generates text sequentially predicting one token at a time based on the previously generated tokens excelling at natural language generation tasks by modeling the probability distribution over sequences of tokens.</obo:IAO_0000115>
        <oboInOwl:hasRelatedSynonym>generative language model</oboInOwl:hasRelatedSynonym>
        <oboInOwl:hasRelatedSynonym>sequence-to-sequence model</oboInOwl:hasRelatedSynonym>
        <oboInOwl:inSubset rdf:resource="https://w3id.org/aio/ModelSubset"/>
        <rdfs:label>Autoregressive Language Model</rdfs:label>
    </owl:Class>
    


    <!-- https://w3id.org/aio/AutoregressiveMovingAverage -->

    <owl:Class rdf:about="https://w3id.org/aio/AutoregressiveMovingAverage">
        <rdfs:subClassOf rdf:resource="https://w3id.org/aio/Model"/>
        <obo:IAO_0000115>A model that combines autoregressive (AR) and moving average (MA) components to represent time series data, suitable for stationary series without the need for differencing.</obo:IAO_0000115>
        <oboInOwl:hasExactSynonym>ARMA</oboInOwl:hasExactSynonym>
        <oboInOwl:inSubset rdf:resource="https://w3id.org/aio/ModelSubset"/>
        <rdfs:label>Autoregressive Moving Average</rdfs:label>
    </owl:Class>
    


    <!-- https://w3id.org/aio/AvailabilityHeuristicBias -->

    <owl:Class rdf:about="https://w3id.org/aio/AvailabilityHeuristicBias">
        <rdfs:subClassOf rdf:resource="https://w3id.org/aio/IndividualBias"/>
        <obo:IAO_0000115>A cognitive bias characterized by a mental shortcut where easily recalled information is overweighted in judgment and decision-making.</obo:IAO_0000115>
        <oboInOwl:hasExactSynonym>Availability Bias</oboInOwl:hasExactSynonym>
        <oboInOwl:hasExactSynonym>Availability Heuristic</oboInOwl:hasExactSynonym>
        <oboInOwl:inSubset rdf:resource="https://w3id.org/aio/BiasSubset"/>
        <rdfs:label>Availability Heuristic Bias</rdfs:label>
    </owl:Class>
    <owl:Axiom>
        <owl:annotatedSource rdf:resource="https://w3id.org/aio/AvailabilityHeuristicBias"/>
        <owl:annotatedProperty rdf:resource="http://purl.obolibrary.org/obo/IAO_0000115"/>
        <owl:annotatedTarget>A cognitive bias characterized by a mental shortcut where easily recalled information is overweighted in judgment and decision-making.</owl:annotatedTarget>
        <oboInOwl:hasDbXref rdf:resource="https://doi.org/10.6028/NIST.SP.1270"/>
    </owl:Axiom>
    


    <!-- https://w3id.org/aio/AverageLayer -->

    <owl:Class rdf:about="https://w3id.org/aio/AverageLayer">
        <rdfs:subClassOf rdf:resource="https://w3id.org/aio/MergingLayer"/>
        <obo:IAO_0000115>A merging layer that averages a list of inputs element-wise taking as input a list of tensors all of the same shape.</obo:IAO_0000115>
        <oboInOwl:inSubset rdf:resource="https://w3id.org/aio/LayerSubset"/>
        <rdfs:comment>Layer that averages a list of inputs element-wise. It takes as input a list of tensors, all of the same shape, and returns a single tensor (also of the same shape).</rdfs:comment>
        <rdfs:label>Average Layer</rdfs:label>
    </owl:Class>
    <owl:Axiom>
        <owl:annotatedSource rdf:resource="https://w3id.org/aio/AverageLayer"/>
        <owl:annotatedProperty rdf:resource="http://purl.obolibrary.org/obo/IAO_0000115"/>
        <owl:annotatedTarget>A merging layer that averages a list of inputs element-wise taking as input a list of tensors all of the same shape.</owl:annotatedTarget>
        <oboInOwl:hasDbXref rdf:resource="https://www.tensorflow.org/api_docs/python/tf/keras/layers/Average"/>
    </owl:Axiom>
    


    <!-- https://w3id.org/aio/AveragePooling1DLayer -->

    <owl:Class rdf:about="https://w3id.org/aio/AveragePooling1DLayer">
        <rdfs:subClassOf rdf:resource="https://w3id.org/aio/PoolingLayer"/>
        <obo:IAO_0000115>A pooling layer that performs average pooling for temporal data.</obo:IAO_0000115>
        <oboInOwl:hasExactSynonym>AvgPool1D</oboInOwl:hasExactSynonym>
        <oboInOwl:inSubset rdf:resource="https://w3id.org/aio/LayerSubset"/>
        <rdfs:comment>Average pooling for temporal data. Downsamples the input representation by taking the average value over the window defined by pool_size. The window is shifted by strides. The resulting output when using &quot;valid&quot; padding option has a shape of: output_shape = (input_shape - pool_size + 1) / strides). The resulting output shape when using the &quot;same&quot; padding option is: output_shape = input_shape / strides.</rdfs:comment>
        <rdfs:label>AveragePooling1D Layer</rdfs:label>
    </owl:Class>
    <owl:Axiom>
        <owl:annotatedSource rdf:resource="https://w3id.org/aio/AveragePooling1DLayer"/>
        <owl:annotatedProperty rdf:resource="http://purl.obolibrary.org/obo/IAO_0000115"/>
        <owl:annotatedTarget>A pooling layer that performs average pooling for temporal data.</owl:annotatedTarget>
        <oboInOwl:hasDbXref rdf:resource="https://www.tensorflow.org/api_docs/python/tf/keras/layers/AveragePooling1D"/>
    </owl:Axiom>
    


    <!-- https://w3id.org/aio/AveragePooling2DLayer -->

    <owl:Class rdf:about="https://w3id.org/aio/AveragePooling2DLayer">
        <rdfs:subClassOf rdf:resource="https://w3id.org/aio/PoolingLayer"/>
        <obo:IAO_0000115>A pooling layer that performs average pooling for spatial data.</obo:IAO_0000115>
        <oboInOwl:hasExactSynonym>AvgPool2D</oboInOwl:hasExactSynonym>
        <oboInOwl:inSubset rdf:resource="https://w3id.org/aio/LayerSubset"/>
        <rdfs:comment>Average pooling operation for spatial data. Downsamples the input along its spatial dimensions (height and width) by taking the average value over an input window (of size defined by pool_size) for each channel of the input. The window is shifted by strides along each dimension. The resulting output when using &quot;valid&quot; padding option has a shape (number of rows or columns) of: output_shape = math.floor((input_shape - pool_size) / strides) + 1 (when input_shape &gt;= pool_size). The resulting output shape when using the &quot;same&quot; padding option is: output_shape = math.floor((input_shape - 1) / strides) + 1.</rdfs:comment>
        <rdfs:label>AveragePooling2D Layer</rdfs:label>
    </owl:Class>
    <owl:Axiom>
        <owl:annotatedSource rdf:resource="https://w3id.org/aio/AveragePooling2DLayer"/>
        <owl:annotatedProperty rdf:resource="http://purl.obolibrary.org/obo/IAO_0000115"/>
        <owl:annotatedTarget>A pooling layer that performs average pooling for spatial data.</owl:annotatedTarget>
        <oboInOwl:hasDbXref rdf:resource="https://www.tensorflow.org/api_docs/python/tf/keras/layers/AveragePooling2D"/>
    </owl:Axiom>
    


    <!-- https://w3id.org/aio/AveragePooling3DLayer -->

    <owl:Class rdf:about="https://w3id.org/aio/AveragePooling3DLayer">
        <rdfs:subClassOf rdf:resource="https://w3id.org/aio/PoolingLayer"/>
        <obo:IAO_0000115>A pooling layer that performs average pooling for 3D data (spatial or spatio-temporal).</obo:IAO_0000115>
        <oboInOwl:hasExactSynonym>AvgPool3D</oboInOwl:hasExactSynonym>
        <oboInOwl:inSubset rdf:resource="https://w3id.org/aio/LayerSubset"/>
        <rdfs:comment>Average pooling operation for 3D data (spatial or spatio-temporal). Downsamples the input along its spatial dimensions (depth, height, and width) by taking the average value over an input window (of size defined by pool_size) for each channel of the input. The window is shifted by strides along each dimension.</rdfs:comment>
        <rdfs:label>AveragePooling3D Layer</rdfs:label>
    </owl:Class>
    <owl:Axiom>
        <owl:annotatedSource rdf:resource="https://w3id.org/aio/AveragePooling3DLayer"/>
        <owl:annotatedProperty rdf:resource="http://purl.obolibrary.org/obo/IAO_0000115"/>
        <owl:annotatedTarget>A pooling layer that performs average pooling for 3D data (spatial or spatio-temporal).</owl:annotatedTarget>
        <oboInOwl:hasDbXref rdf:resource="https://www.tensorflow.org/api_docs/python/tf/keras/layers/AveragePooling3D"/>
    </owl:Axiom>
    


    <!-- https://w3id.org/aio/AvgPool1DLayer -->

    <owl:Class rdf:about="https://w3id.org/aio/AvgPool1DLayer">
        <rdfs:subClassOf rdf:resource="https://w3id.org/aio/PoolingLayer"/>
        <obo:IAO_0000115>A pooling layer that applies a 1D average pooling over an input signal composed of several input planes.</obo:IAO_0000115>
        <oboInOwl:hasExactSynonym>AvgPool1D</oboInOwl:hasExactSynonym>
        <oboInOwl:inSubset rdf:resource="https://w3id.org/aio/LayerSubset"/>
        <rdfs:label>AvgPool1D Layer</rdfs:label>
    </owl:Class>
    <owl:Axiom>
        <owl:annotatedSource rdf:resource="https://w3id.org/aio/AvgPool1DLayer"/>
        <owl:annotatedProperty rdf:resource="http://purl.obolibrary.org/obo/IAO_0000115"/>
        <owl:annotatedTarget>A pooling layer that applies a 1D average pooling over an input signal composed of several input planes.</owl:annotatedTarget>
        <oboInOwl:hasDbXref rdf:resource="https://pytorch.org/docs/stable/nn.html#pooling-layers"/>
    </owl:Axiom>
    


    <!-- https://w3id.org/aio/AvgPool2DLayer -->

    <owl:Class rdf:about="https://w3id.org/aio/AvgPool2DLayer">
        <rdfs:subClassOf rdf:resource="https://w3id.org/aio/PoolingLayer"/>
        <obo:IAO_0000115>A pooling layer that applies a 2D average pooling over an input signal composed of several input planes.</obo:IAO_0000115>
        <oboInOwl:hasExactSynonym>AvgPool2D</oboInOwl:hasExactSynonym>
        <oboInOwl:inSubset rdf:resource="https://w3id.org/aio/LayerSubset"/>
        <rdfs:label>AvgPool2D Layer</rdfs:label>
    </owl:Class>
    <owl:Axiom>
        <owl:annotatedSource rdf:resource="https://w3id.org/aio/AvgPool2DLayer"/>
        <owl:annotatedProperty rdf:resource="http://purl.obolibrary.org/obo/IAO_0000115"/>
        <owl:annotatedTarget>A pooling layer that applies a 2D average pooling over an input signal composed of several input planes.</owl:annotatedTarget>
        <oboInOwl:hasDbXref rdf:resource="https://pytorch.org/docs/stable/nn.html#pooling-layers"/>
    </owl:Axiom>
    


    <!-- https://w3id.org/aio/AvgPool3DLayer -->

    <owl:Class rdf:about="https://w3id.org/aio/AvgPool3DLayer">
        <rdfs:subClassOf rdf:resource="https://w3id.org/aio/PoolingLayer"/>
        <obo:IAO_0000115>A pooling layer that applies a 3D average pooling over an input signal composed of several input planes.</obo:IAO_0000115>
        <oboInOwl:hasExactSynonym>AvgPool3D</oboInOwl:hasExactSynonym>
        <oboInOwl:inSubset rdf:resource="https://w3id.org/aio/LayerSubset"/>
        <rdfs:label>AvgPool3D Layer</rdfs:label>
    </owl:Class>
    <owl:Axiom>
        <owl:annotatedSource rdf:resource="https://w3id.org/aio/AvgPool3DLayer"/>
        <owl:annotatedProperty rdf:resource="http://purl.obolibrary.org/obo/IAO_0000115"/>
        <owl:annotatedTarget>A pooling layer that applies a 3D average pooling over an input signal composed of several input planes.</owl:annotatedTarget>
        <oboInOwl:hasDbXref rdf:resource="https://pytorch.org/docs/stable/nn.html#pooling-layers"/>
    </owl:Axiom>
    


    <!-- https://w3id.org/aio/BackfedInputLayer -->

    <owl:Class rdf:about="https://w3id.org/aio/BackfedInputLayer">
        <rdfs:subClassOf rdf:resource="https://w3id.org/aio/InputLayer"/>
        <obo:IAO_0000115>An input layer that receives values from another layer.</obo:IAO_0000115>
        <oboInOwl:inSubset rdf:resource="https://w3id.org/aio/LayerSubset"/>
        <rdfs:label>Backfed Input Layer</rdfs:label>
    </owl:Class>
    


    <!-- https://w3id.org/aio/BatchNorm1DLayer -->

    <owl:Class rdf:about="https://w3id.org/aio/BatchNorm1DLayer">
        <rdfs:subClassOf rdf:resource="https://w3id.org/aio/BatchNormalizationLayer"/>
        <obo:IAO_0000115>A batch normalization layer that applies Batch Normalization over a 2D or 3D input.</obo:IAO_0000115>
        <oboInOwl:hasExactSynonym>BatchNorm1D</oboInOwl:hasExactSynonym>
        <oboInOwl:inSubset rdf:resource="https://w3id.org/aio/LayerSubset"/>
        <rdfs:comment>Applies Batch Normalization over a 2D or 3D input as described in the paper Batch Normalization: Accelerating Deep Network Training by Reducing Internal Covariate Shift .</rdfs:comment>
        <rdfs:label>BatchNorm1D Layer</rdfs:label>
    </owl:Class>
    <owl:Axiom>
        <owl:annotatedSource rdf:resource="https://w3id.org/aio/BatchNorm1DLayer"/>
        <owl:annotatedProperty rdf:resource="http://purl.obolibrary.org/obo/IAO_0000115"/>
        <owl:annotatedTarget>A batch normalization layer that applies Batch Normalization over a 2D or 3D input.</owl:annotatedTarget>
        <oboInOwl:hasDbXref rdf:resource="https://pytorch.org/docs/stable/nn.html#normalization-layers"/>
    </owl:Axiom>
    


    <!-- https://w3id.org/aio/BatchNorm2DLayer -->

    <owl:Class rdf:about="https://w3id.org/aio/BatchNorm2DLayer">
        <rdfs:subClassOf rdf:resource="https://w3id.org/aio/BatchNormalizationLayer"/>
        <obo:IAO_0000115>A batch normalization layer that applies Batch Normalization over a 4D input.</obo:IAO_0000115>
        <oboInOwl:hasExactSynonym>BatchNorm2D</oboInOwl:hasExactSynonym>
        <oboInOwl:inSubset rdf:resource="https://w3id.org/aio/LayerSubset"/>
        <rdfs:comment>Applies Batch Normalization over a 4D input (a mini-batch of 2D inputs with additional channel dimension) as described in the paper Batch Normalization: Accelerating Deep Network Training by Reducing Internal Covariate Shift .</rdfs:comment>
        <rdfs:label>BatchNorm2D Layer</rdfs:label>
    </owl:Class>
    <owl:Axiom>
        <owl:annotatedSource rdf:resource="https://w3id.org/aio/BatchNorm2DLayer"/>
        <owl:annotatedProperty rdf:resource="http://purl.obolibrary.org/obo/IAO_0000115"/>
        <owl:annotatedTarget>A batch normalization layer that applies Batch Normalization over a 4D input.</owl:annotatedTarget>
        <oboInOwl:hasDbXref rdf:resource="https://pytorch.org/docs/stable/nn.html#normalization-layers"/>
    </owl:Axiom>
    


    <!-- https://w3id.org/aio/BatchNorm3DLayer -->

    <owl:Class rdf:about="https://w3id.org/aio/BatchNorm3DLayer">
        <rdfs:subClassOf rdf:resource="https://w3id.org/aio/BatchNormalizationLayer"/>
        <obo:IAO_0000115>A batch normalization layer that applies Batch Normalization over a 5D input.</obo:IAO_0000115>
        <oboInOwl:hasExactSynonym>BatchNorm3D</oboInOwl:hasExactSynonym>
        <oboInOwl:inSubset rdf:resource="https://w3id.org/aio/LayerSubset"/>
        <rdfs:comment>Applies Batch Normalization over a 5D input (a mini-batch of 3D inputs with additional channel dimension) as described in the paper Batch Normalization: Accelerating Deep Network Training by Reducing Internal Covariate Shift .</rdfs:comment>
        <rdfs:label>BatchNorm3D Layer</rdfs:label>
    </owl:Class>
    <owl:Axiom>
        <owl:annotatedSource rdf:resource="https://w3id.org/aio/BatchNorm3DLayer"/>
        <owl:annotatedProperty rdf:resource="http://purl.obolibrary.org/obo/IAO_0000115"/>
        <owl:annotatedTarget>A batch normalization layer that applies Batch Normalization over a 5D input.</owl:annotatedTarget>
        <oboInOwl:hasDbXref rdf:resource="https://pytorch.org/docs/stable/nn.html#normalization-layers"/>
    </owl:Axiom>
    


    <!-- https://w3id.org/aio/BatchNormalizationLayer -->

    <owl:Class rdf:about="https://w3id.org/aio/BatchNormalizationLayer">
        <rdfs:subClassOf rdf:resource="https://w3id.org/aio/NormalizationLayer"/>
        <obo:IAO_0000115>A normalization layer that normalizes its inputs applying a transformation that maintains the mean close to 0 and the standard deviation close to 1.</obo:IAO_0000115>
        <oboInOwl:hasExactSynonym>BatchNorm</oboInOwl:hasExactSynonym>
        <oboInOwl:inSubset rdf:resource="https://w3id.org/aio/LayerSubset"/>
        <rdfs:comment>Layer that normalizes its inputs. Batch normalization applies a transformation that maintains the mean output close to 0 and the output standard deviation close to 1. Importantly, batch normalization works differently during training and during inference. During training (i.e. when using fit() or when calling the layer/model with the argument training=True), the layer normalizes its output using the mean and standard deviation of the current batch of inputs. That is to say, for each channel being normalized, the layer returns gamma * (batch - mean(batch)) / sqrt(var(batch) + epsilon) + beta, where: epsilon is small constant (configurable as part of the constructor arguments), gamma is a learned scaling factor (initialized as 1), which can be disabled by passing scale=False to the constructor. beta is a learned offset factor (initialized as 0), which can be disabled by passing center=False to the constructor. During inference (i.e. when using evaluate() or predict() or when calling the layer/model with the argument training=False (which is the default), the layer normalizes its output using a moving average of the mean and standard deviation of the batches it has seen during training. That is to say, it returns gamma * (batch - self.moving_mean) / sqrt(self.moving_var + epsilon) + beta. self.moving_mean and self.moving_var are non-trainable variables that are updated each time the layer in called in training mode, as such: moving_mean = moving_mean * momentum + mean(batch) * (1 - momentum) moving_var = moving_var * momentum + var(batch) * (1 - momentum).</rdfs:comment>
        <rdfs:label>BatchNormalization Layer</rdfs:label>
    </owl:Class>
    <owl:Axiom>
        <owl:annotatedSource rdf:resource="https://w3id.org/aio/BatchNormalizationLayer"/>
        <owl:annotatedProperty rdf:resource="http://purl.obolibrary.org/obo/IAO_0000115"/>
        <owl:annotatedTarget>A normalization layer that normalizes its inputs applying a transformation that maintains the mean close to 0 and the standard deviation close to 1.</owl:annotatedTarget>
        <oboInOwl:hasDbXref rdf:resource="https://www.tensorflow.org/api_docs/python/tf/keras/layers/BatchNormalization"/>
    </owl:Axiom>
    


    <!-- https://w3id.org/aio/BayesianNetwork -->

    <owl:Class rdf:about="https://w3id.org/aio/BayesianNetwork">
        <rdfs:subClassOf rdf:resource="https://w3id.org/aio/Network"/>
        <obo:IAO_0000115>A network that is a probabilistic graphical model representing variables and their conditional dependencies via a directed acyclic graph.</obo:IAO_0000115>
        <oboInOwl:inSubset rdf:resource="https://w3id.org/aio/NetworkSubset"/>
        <rdfs:label>Bayesian Network</rdfs:label>
    </owl:Class>
    <owl:Axiom>
        <owl:annotatedSource rdf:resource="https://w3id.org/aio/BayesianNetwork"/>
        <owl:annotatedProperty rdf:resource="http://purl.obolibrary.org/obo/IAO_0000115"/>
        <owl:annotatedTarget>A network that is a probabilistic graphical model representing variables and their conditional dependencies via a directed acyclic graph.</owl:annotatedTarget>
        <oboInOwl:hasDbXref rdf:resource="https://en.wikipedia.org/wiki/Bayesian_network"/>
    </owl:Axiom>
    


    <!-- https://w3id.org/aio/BehavioralBias -->

    <owl:Class rdf:about="https://w3id.org/aio/BehavioralBias">
        <rdfs:subClassOf rdf:resource="https://w3id.org/aio/IndividualBias"/>
        <obo:IAO_0000115>An individual bias characterized by systematic distortions in user behavior across platforms or contexts or across users represented in different datasets.</obo:IAO_0000115>
        <oboInOwl:inSubset rdf:resource="https://w3id.org/aio/BiasSubset"/>
        <rdfs:comment>Systematic distortions in user behavior across platforms or contexts, or across users represented in different datasets.</rdfs:comment>
        <rdfs:label>Behavioral Bias</rdfs:label>
    </owl:Class>
    <owl:Axiom>
        <owl:annotatedSource rdf:resource="https://w3id.org/aio/BehavioralBias"/>
        <owl:annotatedProperty rdf:resource="http://purl.obolibrary.org/obo/IAO_0000115"/>
        <owl:annotatedTarget>An individual bias characterized by systematic distortions in user behavior across platforms or contexts or across users represented in different datasets.</owl:annotatedTarget>
        <oboInOwl:hasDbXref rdf:resource="https://doi.org/10.6028/NIST.SP.1270"/>
    </owl:Axiom>
    


    <!-- https://w3id.org/aio/Bias -->

    <owl:Class rdf:about="https://w3id.org/aio/Bias">
        <rdfs:subClassOf rdf:resource="http://www.w3.org/2002/07/owl#Thing"/>
        <obo:IAO_0000115>A systematic error introduced into sampling or testing by selecting or encouraging one outcome or answer over others.</obo:IAO_0000115>
        <oboInOwl:inSubset rdf:resource="https://w3id.org/aio/BiasSubset"/>
        <rdfs:label>Bias</rdfs:label>
    </owl:Class>
    <owl:Axiom>
        <owl:annotatedSource rdf:resource="https://w3id.org/aio/Bias"/>
        <owl:annotatedProperty rdf:resource="http://purl.obolibrary.org/obo/IAO_0000115"/>
        <owl:annotatedTarget>A systematic error introduced into sampling or testing by selecting or encouraging one outcome or answer over others.</owl:annotatedTarget>
        <oboInOwl:hasDbXref rdf:resource="https://www.merriam-webster.com/dictionary/bias"/>
    </owl:Axiom>
    


    <!-- https://w3id.org/aio/Biclustering -->

    <owl:Class rdf:about="https://w3id.org/aio/Biclustering">
        <rdfs:subClassOf rdf:resource="https://w3id.org/aio/MachineLearning"/>
        <obo:IAO_0000115>A machine learning task focused on methods that simultaneously cluster the rows and columns of a matrix to identify submatrices with coherent patterns.</obo:IAO_0000115>
        <oboInOwl:hasExactSynonym>Block Clustering</oboInOwl:hasExactSynonym>
        <oboInOwl:hasExactSynonym>Co-clustering</oboInOwl:hasExactSynonym>
        <oboInOwl:hasExactSynonym>Joint Clustering</oboInOwl:hasExactSynonym>
        <oboInOwl:hasExactSynonym>Two-mode Clustering</oboInOwl:hasExactSynonym>
        <oboInOwl:hasExactSynonym>Two-way Clustering</oboInOwl:hasExactSynonym>
        <oboInOwl:inSubset rdf:resource="https://w3id.org/aio/MachineLearningSubset"/>
        <rdfs:label>Biclustering</rdfs:label>
    </owl:Class>
    <owl:Axiom>
        <owl:annotatedSource rdf:resource="https://w3id.org/aio/Biclustering"/>
        <owl:annotatedProperty rdf:resource="http://purl.obolibrary.org/obo/IAO_0000115"/>
        <owl:annotatedTarget>A machine learning task focused on methods that simultaneously cluster the rows and columns of a matrix to identify submatrices with coherent patterns.</owl:annotatedTarget>
        <oboInOwl:hasDbXref rdf:resource="https://en.wikipedia.org/wiki/Biclustering"/>
    </owl:Axiom>
    


    <!-- https://w3id.org/aio/BidirectionalLayer -->

    <owl:Class rdf:about="https://w3id.org/aio/BidirectionalLayer">
        <rdfs:subClassOf rdf:resource="https://w3id.org/aio/RecurrentLayer"/>
        <obo:IAO_0000115>A recurrent layer that is a bidirectional wrapper for RNNs.</obo:IAO_0000115>
        <oboInOwl:inSubset rdf:resource="https://w3id.org/aio/LayerSubset"/>
        <rdfs:comment>Bidirectional wrapper for RNNs.</rdfs:comment>
        <rdfs:label>Bidirectional Layer</rdfs:label>
    </owl:Class>
    <owl:Axiom>
        <owl:annotatedSource rdf:resource="https://w3id.org/aio/BidirectionalLayer"/>
        <owl:annotatedProperty rdf:resource="http://purl.obolibrary.org/obo/IAO_0000115"/>
        <owl:annotatedTarget>A recurrent layer that is a bidirectional wrapper for RNNs.</owl:annotatedTarget>
        <oboInOwl:hasDbXref rdf:resource="https://www.tensorflow.org/api_docs/python/tf/keras/layers/Bidirectional"/>
    </owl:Axiom>
    


    <!-- https://w3id.org/aio/BidirectionalTransformerLanguageModel -->

    <owl:Class rdf:about="https://w3id.org/aio/BidirectionalTransformerLanguageModel">
        <rdfs:subClassOf rdf:resource="https://w3id.org/aio/TransformerLanguageModel"/>
        <obo:IAO_0000115>A transformer language model such as BERT that uses the transformer architecture to build deep bidirectional representations by predicting masked tokens based on their context.</obo:IAO_0000115>
        <oboInOwl:hasExactSynonym>BERT</oboInOwl:hasExactSynonym>
        <oboInOwl:hasExactSynonym>Bidirectional Transformer LM</oboInOwl:hasExactSynonym>
        <oboInOwl:inSubset rdf:resource="https://w3id.org/aio/ModelSubset"/>
        <rdfs:label>Bidirectional Transformer Language Model</rdfs:label>
    </owl:Class>
    <owl:Axiom>
        <owl:annotatedSource rdf:resource="https://w3id.org/aio/BidirectionalTransformerLanguageModel"/>
        <owl:annotatedProperty rdf:resource="http://purl.obolibrary.org/obo/IAO_0000115"/>
        <owl:annotatedTarget>A transformer language model such as BERT that uses the transformer architecture to build deep bidirectional representations by predicting masked tokens based on their context.</owl:annotatedTarget>
        <oboInOwl:hasDbXref rdf:resource="https://arxiv.org/abs/1810.04805"/>
        <oboInOwl:hasDbXref rdf:resource="https://en.wikipedia.org/wiki/BERT_(language_model)"/>
    </owl:Axiom>
    


    <!-- https://w3id.org/aio/BinaryClassification -->

    <owl:Class rdf:about="https://w3id.org/aio/BinaryClassification">
        <rdfs:subClassOf rdf:resource="https://w3id.org/aio/Classification"/>
        <obo:IAO_0000115>A machine learning task focused on methods that classify elements into two groups based on a classification rule.</obo:IAO_0000115>
        <oboInOwl:inSubset rdf:resource="https://w3id.org/aio/MachineLearningSubset"/>
        <rdfs:label>Binary Classification</rdfs:label>
    </owl:Class>
    <owl:Axiom>
        <owl:annotatedSource rdf:resource="https://w3id.org/aio/BinaryClassification"/>
        <owl:annotatedProperty rdf:resource="http://purl.obolibrary.org/obo/IAO_0000115"/>
        <owl:annotatedTarget>A machine learning task focused on methods that classify elements into two groups based on a classification rule.</owl:annotatedTarget>
        <oboInOwl:hasDbXref rdf:resource="https://en.wikipedia.org/wiki/Binary_classification"/>
    </owl:Axiom>
    


    <!-- https://w3id.org/aio/BoltzmannMachineNetwork -->

    <owl:Class rdf:about="https://w3id.org/aio/BoltzmannMachineNetwork">
        <rdfs:subClassOf rdf:resource="https://w3id.org/aio/SymmetricallyConnectedNetwork"/>
        <rdfs:subClassOf>
            <owl:Restriction>
                <owl:onProperty rdf:resource="http://purl.obolibrary.org/obo/BFO_0000051"/>
                <owl:someValuesFrom rdf:resource="https://w3id.org/aio/BackfedInputLayer"/>
            </owl:Restriction>
        </rdfs:subClassOf>
        <rdfs:subClassOf>
            <owl:Restriction>
                <owl:onProperty rdf:resource="http://purl.obolibrary.org/obo/BFO_0000051"/>
                <owl:someValuesFrom rdf:resource="https://w3id.org/aio/ProbabilisticHiddenLayer"/>
            </owl:Restriction>
        </rdfs:subClassOf>
        <obo:IAO_0000115>A symmetrically connected network that is a type of stochastic recurrent neural network and Markov random field.</obo:IAO_0000115>
        <oboInOwl:hasExactSynonym>BM</oboInOwl:hasExactSynonym>
        <oboInOwl:hasExactSynonym>Sherrington–Kirkpatrick model with external field</oboInOwl:hasExactSynonym>
        <oboInOwl:hasExactSynonym>stochastic Hopfield network with hidden units</oboInOwl:hasExactSynonym>
        <oboInOwl:hasExactSynonym>stochastic Ising-Lenz-Little model</oboInOwl:hasExactSynonym>
        <oboInOwl:inSubset rdf:resource="https://w3id.org/aio/NetworkSubset"/>
        <rdfs:comment>Layers: Backfed Input, Probabilistic Hidden</rdfs:comment>
        <rdfs:label>Boltzmann Machine Network</rdfs:label>
    </owl:Class>
    <owl:Axiom>
        <owl:annotatedSource rdf:resource="https://w3id.org/aio/BoltzmannMachineNetwork"/>
        <owl:annotatedProperty rdf:resource="http://purl.obolibrary.org/obo/IAO_0000115"/>
        <owl:annotatedTarget>A symmetrically connected network that is a type of stochastic recurrent neural network and Markov random field.</owl:annotatedTarget>
        <oboInOwl:hasDbXref rdf:resource="https://en.wikipedia.org/wiki/Boltzmann_machine"/>
    </owl:Axiom>
    


    <!-- https://w3id.org/aio/CategoricalFeaturesPreprocessingLayer -->

    <owl:Class rdf:about="https://w3id.org/aio/CategoricalFeaturesPreprocessingLayer">
        <rdfs:subClassOf rdf:resource="https://w3id.org/aio/Layer"/>
        <obo:IAO_0000115>A layer that performs categorical data preprocessing operations.</obo:IAO_0000115>
        <oboInOwl:inSubset rdf:resource="https://w3id.org/aio/LayerSubset"/>
        <rdfs:label>Categorical Features Preprocessing Layer</rdfs:label>
    </owl:Class>
    <owl:Axiom>
        <owl:annotatedSource rdf:resource="https://w3id.org/aio/CategoricalFeaturesPreprocessingLayer"/>
        <owl:annotatedProperty rdf:resource="http://purl.obolibrary.org/obo/IAO_0000115"/>
        <owl:annotatedTarget>A layer that performs categorical data preprocessing operations.</owl:annotatedTarget>
        <oboInOwl:hasDbXref rdf:resource="https://keras.io/guides/preprocessing_layers/"/>
    </owl:Axiom>
    


    <!-- https://w3id.org/aio/CategoryEncodingLayer -->

    <owl:Class rdf:about="https://w3id.org/aio/CategoryEncodingLayer">
        <rdfs:subClassOf rdf:resource="https://w3id.org/aio/CategoricalFeaturesPreprocessingLayer"/>
        <obo:IAO_0000115>A categorical features preprocessing layer that encodes integer features providing options for condensing data into a categorical encoding.</obo:IAO_0000115>
        <oboInOwl:inSubset rdf:resource="https://w3id.org/aio/LayerSubset"/>
        <rdfs:comment>A preprocessing layer which encodes integer features. This layer provides options for condensing data into a categorical encoding when the total number of tokens are known in advance. It accepts integer values as inputs, and it outputs a dense or sparse representation of those inputs. For integer inputs where the total number of tokens is not known, use tf.keras.layers.IntegerLookup instead.</rdfs:comment>
        <rdfs:label>CategoryEncoding Layer</rdfs:label>
    </owl:Class>
    <owl:Axiom>
        <owl:annotatedSource rdf:resource="https://w3id.org/aio/CategoryEncodingLayer"/>
        <owl:annotatedProperty rdf:resource="http://purl.obolibrary.org/obo/IAO_0000115"/>
        <owl:annotatedTarget>A categorical features preprocessing layer that encodes integer features providing options for condensing data into a categorical encoding.</owl:annotatedTarget>
        <oboInOwl:hasDbXref rdf:resource="https://www.tensorflow.org/api_docs/python/tf/keras/layers/CategoryEncoding"/>
    </owl:Axiom>
    


    <!-- https://w3id.org/aio/CausalGraphicalModel -->

    <owl:Class rdf:about="https://w3id.org/aio/CausalGraphicalModel">
        <rdfs:subClassOf rdf:resource="https://w3id.org/aio/ProbabilisticGraphicalModel"/>
        <obo:IAO_0000115>A probabilistic graphical model used to encode assumptions about the data-generating process.</obo:IAO_0000115>
        <oboInOwl:hasExactSynonym>Casaul Bayesian Network</oboInOwl:hasExactSynonym>
        <oboInOwl:hasExactSynonym>Casaul Graph</oboInOwl:hasExactSynonym>
        <oboInOwl:hasExactSynonym>DAG</oboInOwl:hasExactSynonym>
        <oboInOwl:hasExactSynonym>Directed Acyclic Graph</oboInOwl:hasExactSynonym>
        <oboInOwl:hasExactSynonym>Path Diagram</oboInOwl:hasExactSynonym>
        <oboInOwl:inSubset rdf:resource="https://w3id.org/aio/MachineLearningSubset"/>
        <rdfs:label>Causal Graphical Model</rdfs:label>
    </owl:Class>
    <owl:Axiom>
        <owl:annotatedSource rdf:resource="https://w3id.org/aio/CausalGraphicalModel"/>
        <owl:annotatedProperty rdf:resource="http://purl.obolibrary.org/obo/IAO_0000115"/>
        <owl:annotatedTarget>A probabilistic graphical model used to encode assumptions about the data-generating process.</owl:annotatedTarget>
        <oboInOwl:hasDbXref rdf:resource="https://en.wikipedia.org/wiki/Causal_graph"/>
    </owl:Axiom>
    


    <!-- https://w3id.org/aio/CausalLLM -->

    <owl:Class rdf:about="https://w3id.org/aio/CausalLLM">
        <rdfs:subClassOf rdf:resource="https://w3id.org/aio/LargeLanguageModel"/>
        <obo:IAO_0000115>A large language model that only attends to previous tokens in the sequence when generating text modeling the probability distribution autoregressively from left-to-right or causally.</obo:IAO_0000115>
        <oboInOwl:hasExactSynonym>Causal Large Language Model</oboInOwl:hasExactSynonym>
        <oboInOwl:hasRelatedSynonym>autoregressive</oboInOwl:hasRelatedSynonym>
        <oboInOwl:hasRelatedSynonym>unidirectional</oboInOwl:hasRelatedSynonym>
        <oboInOwl:inSubset rdf:resource="https://w3id.org/aio/ModelSubset"/>
        <rdfs:label>Causal LLM</rdfs:label>
    </owl:Class>
    


    <!-- https://w3id.org/aio/CenterCropLayer -->

    <owl:Class rdf:about="https://w3id.org/aio/CenterCropLayer">
        <rdfs:subClassOf rdf:resource="https://w3id.org/aio/ImagePreprocessingLayer"/>
        <obo:IAO_0000115>An image preprocessing layer that crops the central portion of images to a target size.</obo:IAO_0000115>
        <oboInOwl:inSubset rdf:resource="https://w3id.org/aio/LayerSubset"/>
        <rdfs:comment>A preprocessing layer which crops images. This layers crops the central portion of the images to a target size. If an image is smaller than the target size, it will be resized and cropped so as to return the largest possible window in the image that matches the target aspect ratio. Input pixel values can be of any range (e.g. [0., 1.) or [0, 255]) and of interger or floating point dtype. By default, the layer will output floats.</rdfs:comment>
        <rdfs:label>CenterCrop Layer</rdfs:label>
    </owl:Class>
    <owl:Axiom>
        <owl:annotatedSource rdf:resource="https://w3id.org/aio/CenterCropLayer"/>
        <owl:annotatedProperty rdf:resource="http://purl.obolibrary.org/obo/IAO_0000115"/>
        <owl:annotatedTarget>An image preprocessing layer that crops the central portion of images to a target size.</owl:annotatedTarget>
        <oboInOwl:hasDbXref rdf:resource="https://www.tensorflow.org/api_docs/python/tf/keras/layers/CenterCrop"/>
    </owl:Axiom>
    


    <!-- https://w3id.org/aio/Classification -->

    <owl:Class rdf:about="https://w3id.org/aio/Classification">
        <rdfs:subClassOf rdf:resource="https://w3id.org/aio/SupervisedLearning"/>
        <obo:IAO_0000115>A supervised learning task focused on methods that distinguish and distribute kinds of &quot;things&quot; into different groups.</obo:IAO_0000115>
        <oboInOwl:inSubset rdf:resource="https://w3id.org/aio/MachineLearningSubset"/>
        <rdfs:comment>Methods that distinguish and distribute kinds of &quot;things&quot; into different groups.</rdfs:comment>
        <rdfs:label>Classification</rdfs:label>
    </owl:Class>
    <owl:Axiom>
        <owl:annotatedSource rdf:resource="https://w3id.org/aio/Classification"/>
        <owl:annotatedProperty rdf:resource="http://purl.obolibrary.org/obo/IAO_0000115"/>
        <owl:annotatedTarget>A supervised learning task focused on methods that distinguish and distribute kinds of &quot;things&quot; into different groups.</owl:annotatedTarget>
        <oboInOwl:hasDbXref rdf:resource="https://en.wikipedia.org/wiki/Classification_(general_theory)"/>
    </owl:Axiom>
    


    <!-- https://w3id.org/aio/Cleaning -->

    <owl:Class rdf:about="https://w3id.org/aio/Cleaning">
        <rdfs:subClassOf rdf:resource="https://w3id.org/aio/DataPreparation"/>
        <obo:IAO_0000115>The process of removing noise inconsistencies and irrelevant information from data to enhance its quality and prepare it for analysis or further processing.</obo:IAO_0000115>
        <oboInOwl:hasExactSynonym>Data Cleansing</oboInOwl:hasExactSynonym>
        <oboInOwl:hasExactSynonym>Standardization</oboInOwl:hasExactSynonym>
        <oboInOwl:hasRelatedSynonym>Data cleaning</oboInOwl:hasRelatedSynonym>
        <oboInOwl:hasRelatedSynonym>Text normalization</oboInOwl:hasRelatedSynonym>
        <oboInOwl:inSubset rdf:resource="https://w3id.org/aio/PreprocessingSubset"/>
        <rdfs:label>Cleaning</rdfs:label>
    </owl:Class>
    


    <!-- https://w3id.org/aio/Clustering -->

    <owl:Class rdf:about="https://w3id.org/aio/Clustering">
        <rdfs:subClassOf rdf:resource="https://w3id.org/aio/MachineLearning"/>
        <obo:IAO_0000115>A machine learning task focused on methods that group a set of objects such that objects in the same group are more similar to each other than to those in other groups.</obo:IAO_0000115>
        <oboInOwl:hasExactSynonym>Cluster analysis</oboInOwl:hasExactSynonym>
        <oboInOwl:inSubset rdf:resource="https://w3id.org/aio/MachineLearningSubset"/>
        <rdfs:label>Clustering</rdfs:label>
    </owl:Class>
    <owl:Axiom>
        <owl:annotatedSource rdf:resource="https://w3id.org/aio/Clustering"/>
        <owl:annotatedProperty rdf:resource="http://purl.obolibrary.org/obo/IAO_0000115"/>
        <owl:annotatedTarget>A machine learning task focused on methods that group a set of objects such that objects in the same group are more similar to each other than to those in other groups.</owl:annotatedTarget>
        <oboInOwl:hasDbXref rdf:resource="https://en.wikipedia.org/wiki/Cluster_analysis"/>
    </owl:Axiom>
    


    <!-- https://w3id.org/aio/CognitiveBias -->

    <owl:Class rdf:about="https://w3id.org/aio/CognitiveBias">
        <rdfs:subClassOf rdf:resource="https://w3id.org/aio/IndividualBias"/>
        <obo:IAO_0000115>A systematic deviation from rational judgment and decision-making including adaptive mental shortcuts known as heuristics.</obo:IAO_0000115>
        <oboInOwl:inSubset rdf:resource="https://w3id.org/aio/BiasSubset"/>
        <rdfs:label>Cognitive Bias</rdfs:label>
    </owl:Class>
    <owl:Axiom>
        <owl:annotatedSource rdf:resource="https://w3id.org/aio/CognitiveBias"/>
        <owl:annotatedProperty rdf:resource="http://purl.obolibrary.org/obo/IAO_0000115"/>
        <owl:annotatedTarget>A systematic deviation from rational judgment and decision-making including adaptive mental shortcuts known as heuristics.</owl:annotatedTarget>
        <oboInOwl:hasDbXref rdf:resource="https://doi.org/10.6028/NIST.SP.1270"/>
    </owl:Axiom>
    


    <!-- https://w3id.org/aio/CompositionalGeneralizationLLM -->

    <owl:Class rdf:about="https://w3id.org/aio/CompositionalGeneralizationLLM">
        <rdfs:subClassOf rdf:resource="https://w3id.org/aio/LargeLanguageModel"/>
        <obo:IAO_0000115>A large language model that is trained to understand and recombine the underlying compositional structures in language enabling better generalization to novel combinations and out-of-distribution examples.</obo:IAO_0000115>
        <oboInOwl:hasExactSynonym>Compositional Generalization Large Language Model</oboInOwl:hasExactSynonym>
        <oboInOwl:hasRelatedSynonym>out-of-distribution generalization</oboInOwl:hasRelatedSynonym>
        <oboInOwl:hasRelatedSynonym>systematic generalization</oboInOwl:hasRelatedSynonym>
        <oboInOwl:inSubset rdf:resource="https://w3id.org/aio/ModelSubset"/>
        <rdfs:label>Compositional Generalization LLM</rdfs:label>
    </owl:Class>
    


    <!-- https://w3id.org/aio/ComputationalBias -->

    <owl:Class rdf:about="https://w3id.org/aio/ComputationalBias">
        <rdfs:subClassOf rdf:resource="https://w3id.org/aio/Bias"/>
        <obo:IAO_0000115>A bias caused by differences between results and facts in the process of data analysis (including the source of data the estimator chose) and analysis methods.</obo:IAO_0000115>
        <oboInOwl:hasExactSynonym>Statistical Bias</oboInOwl:hasExactSynonym>
        <oboInOwl:inSubset rdf:resource="https://w3id.org/aio/BiasSubset"/>
        <rdfs:label>Computational Bias</rdfs:label>
    </owl:Class>
    <owl:Axiom>
        <owl:annotatedSource rdf:resource="https://w3id.org/aio/ComputationalBias"/>
        <owl:annotatedProperty rdf:resource="http://purl.obolibrary.org/obo/IAO_0000115"/>
        <owl:annotatedTarget>A bias caused by differences between results and facts in the process of data analysis (including the source of data the estimator chose) and analysis methods.</owl:annotatedTarget>
        <oboInOwl:hasDbXref rdf:resource="https://doi.org/10.6028/NIST.SP.1270"/>
    </owl:Axiom>
    


    <!-- https://w3id.org/aio/ConcatenateLayer -->

    <owl:Class rdf:about="https://w3id.org/aio/ConcatenateLayer">
        <rdfs:subClassOf rdf:resource="https://w3id.org/aio/MergingLayer"/>
        <obo:IAO_0000115>A merging layer that concatenates a list of inputs taking as input a list of tensors all of the same shape except for the concatenation axis.</obo:IAO_0000115>
        <oboInOwl:inSubset rdf:resource="https://w3id.org/aio/LayerSubset"/>
        <rdfs:comment>Layer that concatenates a list of inputs. It takes as input a list of tensors, all of the same shape except for the concatenation axis, and returns a single tensor that is the concatenation of all inputs.</rdfs:comment>
        <rdfs:label>Concatenate Layer</rdfs:label>
    </owl:Class>
    <owl:Axiom>
        <owl:annotatedSource rdf:resource="https://w3id.org/aio/ConcatenateLayer"/>
        <owl:annotatedProperty rdf:resource="http://purl.obolibrary.org/obo/IAO_0000115"/>
        <owl:annotatedTarget>A merging layer that concatenates a list of inputs taking as input a list of tensors all of the same shape except for the concatenation axis.</owl:annotatedTarget>
        <oboInOwl:hasDbXref rdf:resource="https://www.tensorflow.org/api_docs/python/tf/keras/layers/Concatenate"/>
    </owl:Axiom>
    


    <!-- https://w3id.org/aio/ConceptDriftBias -->

    <owl:Class rdf:about="https://w3id.org/aio/ConceptDriftBias">
        <rdfs:subClassOf rdf:resource="https://w3id.org/aio/UseAndInterpretationBias"/>
        <obo:IAO_0000115>A use and interpretation bias due to the use of a system outside its planned domain of application causing performance gaps between laboratory settings and the real world.</obo:IAO_0000115>
        <oboInOwl:hasExactSynonym>Concept Drift</oboInOwl:hasExactSynonym>
        <oboInOwl:inSubset rdf:resource="https://w3id.org/aio/BiasSubset"/>
        <rdfs:label>Concept Drift Bias</rdfs:label>
    </owl:Class>
    <owl:Axiom>
        <owl:annotatedSource rdf:resource="https://w3id.org/aio/ConceptDriftBias"/>
        <owl:annotatedProperty rdf:resource="http://purl.obolibrary.org/obo/IAO_0000115"/>
        <owl:annotatedTarget>A use and interpretation bias due to the use of a system outside its planned domain of application causing performance gaps between laboratory settings and the real world.</owl:annotatedTarget>
        <oboInOwl:hasDbXref rdf:resource="https://doi.org/10.6028/NIST.SP.1270"/>
    </owl:Axiom>
    


    <!-- https://w3id.org/aio/ConfirmationBias -->

    <owl:Class rdf:about="https://w3id.org/aio/ConfirmationBias">
        <rdfs:subClassOf rdf:resource="https://w3id.org/aio/IndividualBias"/>
        <obo:IAO_0000115>A cognitive bias characterized by the tendency to prefer information that confirms existing beliefs influencing the search for interpretation of and recall of information.</obo:IAO_0000115>
        <oboInOwl:inSubset rdf:resource="https://w3id.org/aio/BiasSubset"/>
        <rdfs:comment>The tendency to prefer information that confirms existing beliefs, influencing the search for, interpretation of, and recall of information.</rdfs:comment>
        <rdfs:label>Confirmation Bias</rdfs:label>
    </owl:Class>
    <owl:Axiom>
        <owl:annotatedSource rdf:resource="https://w3id.org/aio/ConfirmationBias"/>
        <owl:annotatedProperty rdf:resource="http://purl.obolibrary.org/obo/IAO_0000115"/>
        <owl:annotatedTarget>A cognitive bias characterized by the tendency to prefer information that confirms existing beliefs influencing the search for interpretation of and recall of information.</owl:annotatedTarget>
        <oboInOwl:hasDbXref rdf:resource="https://doi.org/10.6028/NIST.SP.1270"/>
    </owl:Axiom>
    


    <!-- https://w3id.org/aio/ConsumerBias -->

    <owl:Class rdf:about="https://w3id.org/aio/ConsumerBias">
        <rdfs:subClassOf rdf:resource="https://w3id.org/aio/IndividualBias"/>
        <obo:IAO_0000115>A bias arising when an algorithm or platform provides users a venue to express their biases occurring from either side in a digital interaction.</obo:IAO_0000115>
        <oboInOwl:inSubset rdf:resource="https://w3id.org/aio/BiasSubset"/>
        <rdfs:label>Consumer Bias</rdfs:label>
    </owl:Class>
    <owl:Axiom>
        <owl:annotatedSource rdf:resource="https://w3id.org/aio/ConsumerBias"/>
        <owl:annotatedProperty rdf:resource="http://purl.obolibrary.org/obo/IAO_0000115"/>
        <owl:annotatedTarget>A bias arising when an algorithm or platform provides users a venue to express their biases occurring from either side in a digital interaction.</owl:annotatedTarget>
        <oboInOwl:hasDbXref rdf:resource="https://doi.org/10.6028/NIST.SP.1270"/>
    </owl:Axiom>
    


    <!-- https://w3id.org/aio/ContentProductionBias -->

    <owl:Class rdf:about="https://w3id.org/aio/ContentProductionBias">
        <rdfs:subClassOf rdf:resource="https://w3id.org/aio/UseAndInterpretationBias"/>
        <obo:IAO_0000115>A use and interpretation bias arising from structural lexical semantic and syntactic differences in user-generated content.</obo:IAO_0000115>
        <oboInOwl:inSubset rdf:resource="https://w3id.org/aio/BiasSubset"/>
        <rdfs:comment>Bias from structural, lexical, semantic, and syntactic differences in user-generated content.</rdfs:comment>
        <rdfs:label>Content Production Bias</rdfs:label>
    </owl:Class>
    <owl:Axiom>
        <owl:annotatedSource rdf:resource="https://w3id.org/aio/ContentProductionBias"/>
        <owl:annotatedProperty rdf:resource="http://purl.obolibrary.org/obo/IAO_0000115"/>
        <owl:annotatedTarget>A use and interpretation bias arising from structural lexical semantic and syntactic differences in user-generated content.</owl:annotatedTarget>
        <oboInOwl:hasDbXref rdf:resource="https://doi.org/10.6028/NIST.SP.1270"/>
    </owl:Axiom>
    


    <!-- https://w3id.org/aio/ContinualLearning -->

    <owl:Class rdf:about="https://w3id.org/aio/ContinualLearning">
        <rdfs:subClassOf rdf:resource="https://w3id.org/aio/DeepNeuralNetwork"/>
        <obo:IAO_0000115>A deep neural network that learns sequential tasks without forgetting knowledge from preceding tasks and without access to old task data during new task training.</obo:IAO_0000115>
        <oboInOwl:hasExactSynonym>Incremental Learning</oboInOwl:hasExactSynonym>
        <oboInOwl:hasExactSynonym>Life-Long Learning</oboInOwl:hasExactSynonym>
        <oboInOwl:inSubset rdf:resource="https://w3id.org/aio/NetworkSubset"/>
        <rdfs:comment>Learning a model for sequential tasks without forgetting knowledge from preceding tasks, with no access to old task data during new task training.</rdfs:comment>
        <rdfs:label>Continual Learning</rdfs:label>
    </owl:Class>
    <owl:Axiom>
        <owl:annotatedSource rdf:resource="https://w3id.org/aio/ContinualLearning"/>
        <owl:annotatedProperty rdf:resource="http://purl.obolibrary.org/obo/IAO_0000115"/>
        <owl:annotatedTarget>A deep neural network that learns sequential tasks without forgetting knowledge from preceding tasks and without access to old task data during new task training.</owl:annotatedTarget>
        <oboInOwl:hasDbXref rdf:resource="https://paperswithcode.com/task/continual-learning"/>
    </owl:Axiom>
    


    <!-- https://w3id.org/aio/ContinualLearningLLM -->

    <owl:Class rdf:about="https://w3id.org/aio/ContinualLearningLLM">
        <rdfs:subClassOf rdf:resource="https://w3id.org/aio/LargeLanguageModel"/>
        <obo:IAO_0000115>A large language model that continually acquires new knowledge and skills over time without forgetting previously learned information allowing the model to adapt and expand its capabilities as new data becomes available.</obo:IAO_0000115>
        <oboInOwl:hasExactSynonym>CL-Large Language Model</oboInOwl:hasExactSynonym>
        <oboInOwl:hasExactSynonym>Continual Learning Large Language Model</oboInOwl:hasExactSynonym>
        <oboInOwl:hasRelatedSynonym>catastrophic forgetting</oboInOwl:hasRelatedSynonym>
        <oboInOwl:hasRelatedSynonym>lifelong learning</oboInOwl:hasRelatedSynonym>
        <oboInOwl:inSubset rdf:resource="https://w3id.org/aio/ModelSubset"/>
        <rdfs:label>Continual Learning LLM</rdfs:label>
    </owl:Class>
    


    <!-- https://w3id.org/aio/ContrastiveLearning -->

    <owl:Class rdf:about="https://w3id.org/aio/ContrastiveLearning">
        <rdfs:subClassOf rdf:resource="https://w3id.org/aio/DeepNeuralNetwork"/>
        <obo:IAO_0000115>A deep neural network self-supervised learning approach that learns to distinguish between similar and dissimilar data samples.</obo:IAO_0000115>
        <oboInOwl:inSubset rdf:resource="https://w3id.org/aio/NetworkSubset"/>
        <rdfs:comment>Contrastive learning is a self-supervised learning approach in which the model learns to distinguish between similar and dissimilar pairs of data samples. By maximizing the similarity between positive pairs (similar samples) and minimizing the similarity between negative pairs (dissimilar samples), the model learns to capture meaningful representations of the data. This method is particularly effective for representation learning and is widely used in tasks such as image classification, clustering, and retrieval. Contrastive learning techniques often employ loss functions such as the contrastive loss or the triplet loss to achieve these objectives.</rdfs:comment>
        <rdfs:label>Contrastive Learning</rdfs:label>
    </owl:Class>
    <owl:Axiom>
        <owl:annotatedSource rdf:resource="https://w3id.org/aio/ContrastiveLearning"/>
        <owl:annotatedProperty rdf:resource="http://purl.obolibrary.org/obo/IAO_0000115"/>
        <owl:annotatedTarget>A deep neural network self-supervised learning approach that learns to distinguish between similar and dissimilar data samples.</owl:annotatedTarget>
        <oboInOwl:hasDbXref rdf:resource="https://arxiv.org/abs/2202.14037"/>
    </owl:Axiom>
    


    <!-- https://w3id.org/aio/ContrastiveLearningLLM -->

    <owl:Class rdf:about="https://w3id.org/aio/ContrastiveLearningLLM">
        <rdfs:subClassOf rdf:resource="https://w3id.org/aio/LargeLanguageModel"/>
        <obo:IAO_0000115>A large language model that is trained to pull semantically similar samples closer together and push dissimilar samples apart in the representation space learning high-quality features useful for downstream tasks.</obo:IAO_0000115>
        <oboInOwl:hasRelatedSynonym>Representation learning</oboInOwl:hasRelatedSynonym>
        <oboInOwl:inSubset rdf:resource="https://w3id.org/aio/ModelSubset"/>
        <rdfs:label>Contrastive Learning LLM</rdfs:label>
    </owl:Class>
    


    <!-- https://w3id.org/aio/ControllableLLM -->

    <owl:Class rdf:about="https://w3id.org/aio/ControllableLLM">
        <rdfs:subClassOf rdf:resource="https://w3id.org/aio/LargeLanguageModel"/>
        <obo:IAO_0000115>A large language model that allows for explicit control over certain attributes of the generated text such as style tone topic or other desired characteristics through conditioning or specialized training objectives.</obo:IAO_0000115>
        <oboInOwl:hasExactSynonym>Controllable Large Language Model</oboInOwl:hasExactSynonym>
        <oboInOwl:hasRelatedSynonym>conditional generation</oboInOwl:hasRelatedSynonym>
        <oboInOwl:hasRelatedSynonym>guided generation</oboInOwl:hasRelatedSynonym>
        <oboInOwl:inSubset rdf:resource="https://w3id.org/aio/ModelSubset"/>
        <rdfs:comment>A controllable LLM allows for explicit control over certain attributes of the generated text, such as style, tone, topic, or other desired characteristics, through conditioning or specialized training objectives.</rdfs:comment>
        <rdfs:label>Controllable LLM</rdfs:label>
    </owl:Class>
    


    <!-- https://w3id.org/aio/ConvLSTM1DLayer -->

    <owl:Class rdf:about="https://w3id.org/aio/ConvLSTM1DLayer">
        <rdfs:subClassOf rdf:resource="https://w3id.org/aio/ConvolutionalLayer"/>
        <obo:IAO_0000115>A convolutional layer that implements a 1D Convolutional LSTM similar to an LSTM but with convolutional input and recurrent transformations.</obo:IAO_0000115>
        <oboInOwl:inSubset rdf:resource="https://w3id.org/aio/LayerSubset"/>
        <rdfs:comment>1D Convolutional LSTM. Similar to an LSTM layer, but the input transformations and recurrent transformations are both convolutional.</rdfs:comment>
        <rdfs:label>ConvLSTM1D Layer</rdfs:label>
    </owl:Class>
    <owl:Axiom>
        <owl:annotatedSource rdf:resource="https://w3id.org/aio/ConvLSTM1DLayer"/>
        <owl:annotatedProperty rdf:resource="http://purl.obolibrary.org/obo/IAO_0000115"/>
        <owl:annotatedTarget>A convolutional layer that implements a 1D Convolutional LSTM similar to an LSTM but with convolutional input and recurrent transformations.</owl:annotatedTarget>
        <oboInOwl:hasDbXref rdf:resource="https://www.tensorflow.org/api_docs/python/tf/keras/layers/ConvLSTM1D"/>
    </owl:Axiom>
    


    <!-- https://w3id.org/aio/ConvLSTM2DLayer -->

    <owl:Class rdf:about="https://w3id.org/aio/ConvLSTM2DLayer">
        <rdfs:subClassOf rdf:resource="https://w3id.org/aio/ConvolutionalLayer"/>
        <obo:IAO_0000115>A convolutional layer that implements a 2D Convolutional LSTM similar to an LSTM but with convolutional input and recurrent transformations.</obo:IAO_0000115>
        <oboInOwl:inSubset rdf:resource="https://w3id.org/aio/LayerSubset"/>
        <rdfs:comment>2D Convolutional LSTM. Similar to an LSTM layer, but the input transformations and recurrent transformations are both convolutional.</rdfs:comment>
        <rdfs:label>ConvLSTM2D Layer</rdfs:label>
    </owl:Class>
    <owl:Axiom>
        <owl:annotatedSource rdf:resource="https://w3id.org/aio/ConvLSTM2DLayer"/>
        <owl:annotatedProperty rdf:resource="http://purl.obolibrary.org/obo/IAO_0000115"/>
        <owl:annotatedTarget>A convolutional layer that implements a 2D Convolutional LSTM similar to an LSTM but with convolutional input and recurrent transformations.</owl:annotatedTarget>
        <oboInOwl:hasDbXref rdf:resource="https://www.tensorflow.org/api_docs/python/tf/keras/layers/ConvLSTM2D"/>
    </owl:Axiom>
    


    <!-- https://w3id.org/aio/ConvLSTM3DLayer -->

    <owl:Class rdf:about="https://w3id.org/aio/ConvLSTM3DLayer">
        <rdfs:subClassOf rdf:resource="https://w3id.org/aio/ConvolutionalLayer"/>
        <obo:IAO_0000115>A convolutional layer that implements a 3D Convolutional LSTM similar to an LSTM but with convolutional input and recurrent transformations.</obo:IAO_0000115>
        <oboInOwl:inSubset rdf:resource="https://w3id.org/aio/LayerSubset"/>
        <rdfs:comment>3D Convolutional LSTM. Similar to an LSTM layer, but the input transformations and recurrent transformations are both convolutional.</rdfs:comment>
        <rdfs:label>ConvLSTM3D Layer</rdfs:label>
    </owl:Class>
    <owl:Axiom>
        <owl:annotatedSource rdf:resource="https://w3id.org/aio/ConvLSTM3DLayer"/>
        <owl:annotatedProperty rdf:resource="http://purl.obolibrary.org/obo/IAO_0000115"/>
        <owl:annotatedTarget>A convolutional layer that implements a 3D Convolutional LSTM similar to an LSTM but with convolutional input and recurrent transformations.</owl:annotatedTarget>
        <oboInOwl:hasDbXref rdf:resource="https://www.tensorflow.org/api_docs/python/tf/keras/layers/ConvLSTM3D"/>
    </owl:Axiom>
    


    <!-- https://w3id.org/aio/Convolution1DLayer -->

    <owl:Class rdf:about="https://w3id.org/aio/Convolution1DLayer">
        <rdfs:subClassOf rdf:resource="https://w3id.org/aio/ConvolutionalLayer"/>
        <obo:IAO_0000115>A layer that implements 1D convolution (e.g. temporal convolution).</obo:IAO_0000115>
        <oboInOwl:hasExactSynonym>Conv1D</oboInOwl:hasExactSynonym>
        <oboInOwl:hasExactSynonym>Conv1D Layer</oboInOwl:hasExactSynonym>
        <oboInOwl:hasExactSynonym>Convolution1D</oboInOwl:hasExactSynonym>
        <oboInOwl:hasExactSynonym>nn.Conv1D</oboInOwl:hasExactSynonym>
        <oboInOwl:inSubset rdf:resource="https://w3id.org/aio/LayerSubset"/>
        <rdfs:label>Convolution1D Layer</rdfs:label>
    </owl:Class>
    <owl:Axiom>
        <owl:annotatedSource rdf:resource="https://w3id.org/aio/Convolution1DLayer"/>
        <owl:annotatedProperty rdf:resource="http://purl.obolibrary.org/obo/IAO_0000115"/>
        <owl:annotatedTarget>A layer that implements 1D convolution (e.g. temporal convolution).</owl:annotatedTarget>
        <oboInOwl:hasDbXref rdf:resource="https://www.tensorflow.org/api_docs/python/tf/keras/layers/Conv1D"/>
    </owl:Axiom>
    


    <!-- https://w3id.org/aio/Convolution1DTransposeLayer -->

    <owl:Class rdf:about="https://w3id.org/aio/Convolution1DTransposeLayer">
        <rdfs:subClassOf rdf:resource="https://w3id.org/aio/ConvolutionalLayer"/>
        <obo:IAO_0000115>A layer that implements transposed 1D convolution sometimes called deconvolution.</obo:IAO_0000115>
        <oboInOwl:hasExactSynonym>Conv1DTranspose Layer</oboInOwl:hasExactSynonym>
        <oboInOwl:hasExactSynonym>ConvTranspose1D</oboInOwl:hasExactSynonym>
        <oboInOwl:hasExactSynonym>Convolution1DTranspose</oboInOwl:hasExactSynonym>
        <oboInOwl:hasExactSynonym>nn.ConvTranspose1D</oboInOwl:hasExactSynonym>
        <oboInOwl:inSubset rdf:resource="https://w3id.org/aio/LayerSubset"/>
        <rdfs:comment>Transposed convolution layer (sometimes called Deconvolution). The need for transposed convolutions generally arises from the desire to use a transformation going in the opposite direction of a normal convolution, i.e., from something that has the shape of the output of some convolution to something that has the shape of its input while maintaining a connectivity pattern that is compatible with said convolution. When using this layer as the first layer in a model, provide the keyword argument input_shape (tuple of integers or None, does not include the sample axis), e.g. input_shape=(128, 3) for data with 128 time steps and 3 channels.</rdfs:comment>
        <rdfs:label>Convolution1DTranspose Layer</rdfs:label>
    </owl:Class>
    <owl:Axiom>
        <owl:annotatedSource rdf:resource="https://w3id.org/aio/Convolution1DTransposeLayer"/>
        <owl:annotatedProperty rdf:resource="http://purl.obolibrary.org/obo/IAO_0000115"/>
        <owl:annotatedTarget>A layer that implements transposed 1D convolution sometimes called deconvolution.</owl:annotatedTarget>
        <oboInOwl:hasDbXref rdf:resource="https://www.tensorflow.org/api_docs/python/tf/keras/layers/Conv1DTranspose"/>
    </owl:Axiom>
    


    <!-- https://w3id.org/aio/Convolution2DLayer -->

    <owl:Class rdf:about="https://w3id.org/aio/Convolution2DLayer">
        <rdfs:subClassOf rdf:resource="https://w3id.org/aio/ConvolutionalLayer"/>
        <obo:IAO_0000115>A layer that implements 2D convolution (e.g. spatial convolution over images).</obo:IAO_0000115>
        <oboInOwl:hasExactSynonym>Conv2D</oboInOwl:hasExactSynonym>
        <oboInOwl:hasExactSynonym>Conv2D Layer</oboInOwl:hasExactSynonym>
        <oboInOwl:hasExactSynonym>Convolution2D</oboInOwl:hasExactSynonym>
        <oboInOwl:hasExactSynonym>nn.Conv2D</oboInOwl:hasExactSynonym>
        <oboInOwl:inSubset rdf:resource="https://w3id.org/aio/LayerSubset"/>
        <rdfs:comment>2D convolution layer (e.g. spatial convolution over images). This layer creates a convolution kernel that is convolved with the layer input to produce a tensor of outputs. If use_bias is True, a bias vector is created and added to the outputs. Finally, if activation is not None, it is applied to the outputs as well. When using this layer as the first layer in a model, provide the keyword argument input_shape (tuple of integers or None, does not include the sample axis), e.g. input_shape=(128, 128, 3) for 128x128 RGB pictures in data_format=&quot;channels_last&quot;. You can use None when a dimension has variable size.</rdfs:comment>
        <rdfs:label>Convolution2D Layer</rdfs:label>
    </owl:Class>
    <owl:Axiom>
        <owl:annotatedSource rdf:resource="https://w3id.org/aio/Convolution2DLayer"/>
        <owl:annotatedProperty rdf:resource="http://purl.obolibrary.org/obo/IAO_0000115"/>
        <owl:annotatedTarget>A layer that implements 2D convolution (e.g. spatial convolution over images).</owl:annotatedTarget>
        <oboInOwl:hasDbXref rdf:resource="https://www.tensorflow.org/api_docs/python/tf/keras/layers/Conv2D"/>
    </owl:Axiom>
    


    <!-- https://w3id.org/aio/Convolution2DTransposeLayer -->

    <owl:Class rdf:about="https://w3id.org/aio/Convolution2DTransposeLayer">
        <rdfs:subClassOf rdf:resource="https://w3id.org/aio/ConvolutionalLayer"/>
        <obo:IAO_0000115>A layer that implements transposed 2D convolution</obo:IAO_0000115>
        <oboInOwl:hasExactSynonym>Conv2DTranspose Layer</oboInOwl:hasExactSynonym>
        <oboInOwl:hasExactSynonym>ConvTranspose2D</oboInOwl:hasExactSynonym>
        <oboInOwl:hasExactSynonym>Convolution2DTranspose</oboInOwl:hasExactSynonym>
        <oboInOwl:hasExactSynonym>nn.ConvTranspose2D</oboInOwl:hasExactSynonym>
        <oboInOwl:inSubset rdf:resource="https://w3id.org/aio/LayerSubset"/>
        <rdfs:comment>Transposed convolution layer (sometimes called Deconvolution).</rdfs:comment>
        <rdfs:label>Convolution2DTranspose Layer</rdfs:label>
    </owl:Class>
    <owl:Axiom>
        <owl:annotatedSource rdf:resource="https://w3id.org/aio/Convolution2DTransposeLayer"/>
        <owl:annotatedProperty rdf:resource="http://purl.obolibrary.org/obo/IAO_0000115"/>
        <owl:annotatedTarget>A layer that implements transposed 2D convolution</owl:annotatedTarget>
        <oboInOwl:hasDbXref rdf:resource="https://www.tensorflow.org/api_docs/python/tf/keras/layers/Conv2DTranspose"/>
    </owl:Axiom>
    


    <!-- https://w3id.org/aio/Convolution3DLayer -->

    <owl:Class rdf:about="https://w3id.org/aio/Convolution3DLayer">
        <rdfs:subClassOf rdf:resource="https://w3id.org/aio/ConvolutionalLayer"/>
        <obo:IAO_0000115>A layer that implements 3D convolution (e.g. spatial convolution over volumes).</obo:IAO_0000115>
        <oboInOwl:hasExactSynonym>Conv3D</oboInOwl:hasExactSynonym>
        <oboInOwl:hasExactSynonym>Conv3D Layer</oboInOwl:hasExactSynonym>
        <oboInOwl:hasExactSynonym>Convolution3D</oboInOwl:hasExactSynonym>
        <oboInOwl:hasExactSynonym>nn.Conv3D</oboInOwl:hasExactSynonym>
        <oboInOwl:inSubset rdf:resource="https://w3id.org/aio/LayerSubset"/>
        <rdfs:comment>3D convolution layer (e.g. spatial convolution over volumes). This layer creates a convolution kernel that is convolved with the layer input to produce a tensor of outputs. If use_bias is True, a bias vector is created and added to the outputs. Finally, if activation is not None, it is applied to the outputs as well. When using this layer as the first layer in a model, provide the keyword argument input_shape (tuple of integers or None, does not include the sample axis), e.g. input_shape=(128, 128, 128, 1) for 128x128x128 volumes with a single channel, in data_format=&quot;channels_last&quot;.</rdfs:comment>
        <rdfs:label>Convolution3D Layer</rdfs:label>
    </owl:Class>
    <owl:Axiom>
        <owl:annotatedSource rdf:resource="https://w3id.org/aio/Convolution3DLayer"/>
        <owl:annotatedProperty rdf:resource="http://purl.obolibrary.org/obo/IAO_0000115"/>
        <owl:annotatedTarget>A layer that implements 3D convolution (e.g. spatial convolution over volumes).</owl:annotatedTarget>
        <oboInOwl:hasDbXref rdf:resource="https://www.tensorflow.org/api_docs/python/tf/keras/layers/Conv3D"/>
    </owl:Axiom>
    


    <!-- https://w3id.org/aio/Convolution3DTransposeLayer -->

    <owl:Class rdf:about="https://w3id.org/aio/Convolution3DTransposeLayer">
        <rdfs:subClassOf rdf:resource="https://w3id.org/aio/ConvolutionalLayer"/>
        <obo:IAO_0000115>A layer that implements transposed 3D convolution</obo:IAO_0000115>
        <oboInOwl:hasExactSynonym>Conv3DTranspose Layer</oboInOwl:hasExactSynonym>
        <oboInOwl:hasExactSynonym>ConvTranspose3D</oboInOwl:hasExactSynonym>
        <oboInOwl:hasExactSynonym>Convolution3DTranspose</oboInOwl:hasExactSynonym>
        <oboInOwl:hasExactSynonym>nn.ConvTranspose3D</oboInOwl:hasExactSynonym>
        <oboInOwl:inSubset rdf:resource="https://w3id.org/aio/LayerSubset"/>
        <rdfs:comment>Transposed convolution layer (sometimes called Deconvolution). The need for transposed convolutions generally arises from the desire to use a transformation going in the opposite direction of a normal convolution, i.e., from something that has the shape of the output of some convolution to something that has the shape of its input while maintaining a connectivity pattern that is compatible with said convolution. When using this layer as the first layer in a model, provide the keyword argument input_shape (tuple of integers or None, does not include the sample axis), e.g. input_shape=(128, 128, 128, 3) for a 128x128x128 volume with 3 channels if data_format=&quot;channels_last&quot;.</rdfs:comment>
        <rdfs:label>Convolution3DTranspose Layer</rdfs:label>
    </owl:Class>
    <owl:Axiom>
        <owl:annotatedSource rdf:resource="https://w3id.org/aio/Convolution3DTransposeLayer"/>
        <owl:annotatedProperty rdf:resource="http://purl.obolibrary.org/obo/IAO_0000115"/>
        <owl:annotatedTarget>A layer that implements transposed 3D convolution</owl:annotatedTarget>
        <oboInOwl:hasDbXref rdf:resource="https://www.tensorflow.org/api_docs/python/tf/keras/layers/Conv3DTranspose"/>
    </owl:Axiom>
    


    <!-- https://w3id.org/aio/ConvolutionalLayer -->

    <owl:Class rdf:about="https://w3id.org/aio/ConvolutionalLayer">
        <rdfs:subClassOf rdf:resource="https://w3id.org/aio/Layer"/>
        <obo:IAO_0000115>A layer that contains a set of filters (or kernels) parameters of which are to be learned throughout the training.</obo:IAO_0000115>
        <oboInOwl:inSubset rdf:resource="https://w3id.org/aio/LayerSubset"/>
        <rdfs:comment>A convolutional layer is the main building block of a CNN. It contains a set of filters (or kernels), parameters of which are to be learned throughout the training. The size of the filters is usually smaller than the actual image. Each filter convolves with the image and creates an activation map.</rdfs:comment>
        <rdfs:label>Convolutional Layer</rdfs:label>
    </owl:Class>
    <owl:Axiom>
        <owl:annotatedSource rdf:resource="https://w3id.org/aio/ConvolutionalLayer"/>
        <owl:annotatedProperty rdf:resource="http://purl.obolibrary.org/obo/IAO_0000115"/>
        <owl:annotatedTarget>A layer that contains a set of filters (or kernels) parameters of which are to be learned throughout the training.</owl:annotatedTarget>
        <oboInOwl:hasDbXref rdf:resource="https://www.sciencedirect.com/topics/engineering/convolutional-layer"/>
    </owl:Axiom>
    


    <!-- https://w3id.org/aio/Cropping1DLayer -->

    <owl:Class rdf:about="https://w3id.org/aio/Cropping1DLayer">
        <rdfs:subClassOf rdf:resource="https://w3id.org/aio/ReshapingLayer"/>
        <obo:IAO_0000115>A layer that crops along the time dimension (axis 1) for 1D input.</obo:IAO_0000115>
        <oboInOwl:inSubset rdf:resource="https://w3id.org/aio/LayerSubset"/>
        <rdfs:comment>Cropping layer for 1D input (e.g. temporal sequence). It crops along the time dimension (axis 1).</rdfs:comment>
        <rdfs:label>Cropping1D Layer</rdfs:label>
    </owl:Class>
    <owl:Axiom>
        <owl:annotatedSource rdf:resource="https://w3id.org/aio/Cropping1DLayer"/>
        <owl:annotatedProperty rdf:resource="http://purl.obolibrary.org/obo/IAO_0000115"/>
        <owl:annotatedTarget>A layer that crops along the time dimension (axis 1) for 1D input.</owl:annotatedTarget>
        <oboInOwl:hasDbXref rdf:resource="https://www.tensorflow.org/api_docs/python/tf/keras/layers/Cropping1D"/>
    </owl:Axiom>
    


    <!-- https://w3id.org/aio/Cropping2DLayer -->

    <owl:Class rdf:about="https://w3id.org/aio/Cropping2DLayer">
        <rdfs:subClassOf rdf:resource="https://w3id.org/aio/Layer"/>
        <obo:IAO_0000115>A layer that crops along spatial dimensions (i.e. height and width) for 2D input.</obo:IAO_0000115>
        <oboInOwl:inSubset rdf:resource="https://w3id.org/aio/LayerSubset"/>
        <rdfs:comment>Cropping layer for 2D input (e.g. picture). It crops along spatial dimensions, i.e. height and width.</rdfs:comment>
        <rdfs:label>Cropping2D Layer</rdfs:label>
    </owl:Class>
    <owl:Axiom>
        <owl:annotatedSource rdf:resource="https://w3id.org/aio/Cropping2DLayer"/>
        <owl:annotatedProperty rdf:resource="http://purl.obolibrary.org/obo/IAO_0000115"/>
        <owl:annotatedTarget>A layer that crops along spatial dimensions (i.e. height and width) for 2D input.</owl:annotatedTarget>
        <oboInOwl:hasDbXref rdf:resource="https://www.tensorflow.org/api_docs/python/tf/keras/layers/Cropping2D"/>
    </owl:Axiom>
    


    <!-- https://w3id.org/aio/Cropping3DLayer -->

    <owl:Class rdf:about="https://w3id.org/aio/Cropping3DLayer">
        <rdfs:subClassOf rdf:resource="https://w3id.org/aio/Layer"/>
        <obo:IAO_0000115>A layer that crops along spatial dimensions (depth</obo:IAO_0000115>
        <oboInOwl:inSubset rdf:resource="https://w3id.org/aio/LayerSubset"/>
        <rdfs:comment>Cropping layer for 3D data (e.g. spatial or spatio-temporal).</rdfs:comment>
        <rdfs:label>Cropping3D Layer</rdfs:label>
    </owl:Class>
    <owl:Axiom>
        <owl:annotatedSource rdf:resource="https://w3id.org/aio/Cropping3DLayer"/>
        <owl:annotatedProperty rdf:resource="http://purl.obolibrary.org/obo/IAO_0000115"/>
        <owl:annotatedTarget>A layer that crops along spatial dimensions (depth</owl:annotatedTarget>
        <oboInOwl:hasDbXref rdf:resource="https://www.tensorflow.org/api_docs/python/tf/keras/layers/Cropping3D"/>
    </owl:Axiom>
    


    <!-- https://w3id.org/aio/CrossDomainLLM -->

    <owl:Class rdf:about="https://w3id.org/aio/CrossDomainLLM">
        <rdfs:subClassOf rdf:resource="https://w3id.org/aio/LargeLanguageModel"/>
        <obo:IAO_0000115>A LLM that performs well across a wide range of domains without significant loss in performance, facilitated by advanced domain adaptation techniques.</obo:IAO_0000115>
        <oboInOwl:hasExactSynonym>Domain-General LLM</oboInOwl:hasExactSynonym>
        <oboInOwl:hasRelatedSynonym>cross-domain transfer</oboInOwl:hasRelatedSynonym>
        <oboInOwl:hasRelatedSynonym>domain adaptation</oboInOwl:hasRelatedSynonym>
        <oboInOwl:inSubset rdf:resource="https://w3id.org/aio/ModelSubset"/>
        <rdfs:label>Cross-Domain LLM</rdfs:label>
    </owl:Class>
    


    <!-- https://w3id.org/aio/CurriculumLearning -->

    <owl:Class rdf:about="https://w3id.org/aio/CurriculumLearning">
        <rdfs:subClassOf rdf:resource="https://w3id.org/aio/TrainingStrategies"/>
        <obo:IAO_0000115>A training strategy in machine learning where models are trained on data in a meaningful order starting with simpler examples and gradually increasing the complexity to improve learning efficiency and model performance.</obo:IAO_0000115>
        <oboInOwl:hasExactSynonym>Sequential Learning</oboInOwl:hasExactSynonym>
        <oboInOwl:hasExactSynonym>Structured Learning</oboInOwl:hasExactSynonym>
        <oboInOwl:hasRelatedSynonym>Complexity grading</oboInOwl:hasRelatedSynonym>
        <oboInOwl:hasRelatedSynonym>Sequential learning</oboInOwl:hasRelatedSynonym>
        <oboInOwl:inSubset rdf:resource="https://w3id.org/aio/PreprocessingSubset"/>
        <rdfs:label>Curriculum Learning</rdfs:label>
    </owl:Class>
    


    <!-- https://w3id.org/aio/CurriculumLearningLLM -->

    <owl:Class rdf:about="https://w3id.org/aio/CurriculumLearningLLM">
        <rdfs:subClassOf rdf:resource="https://w3id.org/aio/LargeLanguageModel"/>
        <obo:IAO_0000115>A large language model that is trained by presenting learning examples in a meaningful order from simple to complex mimicking the learning trajectory followed by humans.</obo:IAO_0000115>
        <oboInOwl:hasRelatedSynonym>Learning progression</oboInOwl:hasRelatedSynonym>
        <oboInOwl:inSubset rdf:resource="https://w3id.org/aio/ModelSubset"/>
        <rdfs:label>Curriculum Learning LLM</rdfs:label>
    </owl:Class>
    


    <!-- https://w3id.org/aio/DataAugmentation -->

    <owl:Class rdf:about="https://w3id.org/aio/DataAugmentation">
        <rdfs:subClassOf rdf:resource="https://w3id.org/aio/DataEnhancement"/>
        <obo:IAO_0000115>A technique used to increase the diversity and quantity of training data by applying various transformations such as rotation scaling flipping and cropping to existing data samples enhancing the robustness and performance of machine learning models.</obo:IAO_0000115>
        <oboInOwl:hasExactSynonym>Data Enrichment</oboInOwl:hasExactSynonym>
        <oboInOwl:hasExactSynonym>Data Expansion</oboInOwl:hasExactSynonym>
        <oboInOwl:hasRelatedSynonym>Paraphrasing</oboInOwl:hasRelatedSynonym>
        <oboInOwl:hasRelatedSynonym>Synonym replacement</oboInOwl:hasRelatedSynonym>
        <oboInOwl:inSubset rdf:resource="https://w3id.org/aio/PreprocessingSubset"/>
        <rdfs:label>Data Augmentation</rdfs:label>
    </owl:Class>
    


    <!-- https://w3id.org/aio/DataDredgingBias -->

    <owl:Class rdf:about="https://w3id.org/aio/DataDredgingBias">
        <rdfs:subClassOf rdf:resource="https://w3id.org/aio/UseAndInterpretationBias"/>
        <obo:IAO_0000115>A use and interpretation bias where testing many hypotheses in a dataset may yield apparent statistical significance even when results are nonsignificant.</obo:IAO_0000115>
        <oboInOwl:hasExactSynonym>Data Dredging</oboInOwl:hasExactSynonym>
        <oboInOwl:inSubset rdf:resource="https://w3id.org/aio/BiasSubset"/>
        <rdfs:label>Data Dredging Bias</rdfs:label>
    </owl:Class>
    <owl:Axiom>
        <owl:annotatedSource rdf:resource="https://w3id.org/aio/DataDredgingBias"/>
        <owl:annotatedProperty rdf:resource="http://purl.obolibrary.org/obo/IAO_0000115"/>
        <owl:annotatedTarget>A use and interpretation bias where testing many hypotheses in a dataset may yield apparent statistical significance even when results are nonsignificant.</owl:annotatedTarget>
        <oboInOwl:hasDbXref rdf:resource="https://doi.org/10.6028/NIST.SP.1270"/>
    </owl:Axiom>
    


    <!-- https://w3id.org/aio/DataEnhancement -->

    <owl:Class rdf:about="https://w3id.org/aio/DataEnhancement">
        <rdfs:subClassOf rdf:resource="https://w3id.org/aio/Preprocessing"/>
        <obo:IAO_0000115>Techniques used to improve the quality diversity and volume of data available for training machine learning models such as data augmentation synthesis and enrichment to enhance model robustness and accuracy.</obo:IAO_0000115>
        <oboInOwl:inSubset rdf:resource="https://w3id.org/aio/PreprocessingSubset"/>
        <rdfs:label>DataEnhancement</rdfs:label>
    </owl:Class>
    


    <!-- https://w3id.org/aio/DataGenerationBias -->

    <owl:Class rdf:about="https://w3id.org/aio/DataGenerationBias">
        <rdfs:subClassOf rdf:resource="https://w3id.org/aio/SelectionAndSamplingBias"/>
        <obo:IAO_0000115>A selection and sampling bias arising from adding synthetic or redundant data samples to a dataset.</obo:IAO_0000115>
        <oboInOwl:inSubset rdf:resource="https://w3id.org/aio/BiasSubset"/>
        <rdfs:comment>Bias from adding synthetic or redundant data samples to a dataset.</rdfs:comment>
        <rdfs:label>Data Generation Bias</rdfs:label>
    </owl:Class>
    <owl:Axiom>
        <owl:annotatedSource rdf:resource="https://w3id.org/aio/DataGenerationBias"/>
        <owl:annotatedProperty rdf:resource="http://purl.obolibrary.org/obo/IAO_0000115"/>
        <owl:annotatedTarget>A selection and sampling bias arising from adding synthetic or redundant data samples to a dataset.</owl:annotatedTarget>
        <oboInOwl:hasDbXref rdf:resource="https://en.wikipedia.org/wiki/Selection_bias"/>
    </owl:Axiom>
    


    <!-- https://w3id.org/aio/DataImputation -->

    <owl:Class rdf:about="https://w3id.org/aio/DataImputation">
        <rdfs:subClassOf rdf:resource="https://w3id.org/aio/MachineLearning"/>
        <obo:IAO_0000115>A machine learning task focused on methods that replace missing data with substituted values.</obo:IAO_0000115>
        <oboInOwl:inSubset rdf:resource="https://w3id.org/aio/MachineLearningSubset"/>
        <rdfs:comment>Methods that replace missing data with substituted values.</rdfs:comment>
        <rdfs:label>Data Imputation</rdfs:label>
    </owl:Class>
    <owl:Axiom>
        <owl:annotatedSource rdf:resource="https://w3id.org/aio/DataImputation"/>
        <owl:annotatedProperty rdf:resource="http://purl.obolibrary.org/obo/IAO_0000115"/>
        <owl:annotatedTarget>A machine learning task focused on methods that replace missing data with substituted values.</owl:annotatedTarget>
        <oboInOwl:hasDbXref rdf:resource="https://en.wikipedia.org/wiki/Imputation_(statistics)"/>
    </owl:Axiom>
    


    <!-- https://w3id.org/aio/DataPreparation -->

    <owl:Class rdf:about="https://w3id.org/aio/DataPreparation">
        <rdfs:subClassOf rdf:resource="https://w3id.org/aio/Preprocessing"/>
        <obo:IAO_0000115>The process of cleaning transforming and organizing raw data into a suitable format for analysis and modeling ensuring the quality and relevance of the data for machine learning tasks.</obo:IAO_0000115>
        <oboInOwl:hasExactSynonym>Data Assembly</oboInOwl:hasExactSynonym>
        <oboInOwl:hasExactSynonym>Data Curation</oboInOwl:hasExactSynonym>
        <oboInOwl:hasExactSynonym>Data Processing</oboInOwl:hasExactSynonym>
        <oboInOwl:inSubset rdf:resource="https://w3id.org/aio/PreprocessingSubset"/>
        <rdfs:label>Data Preparation</rdfs:label>
    </owl:Class>
    


    <!-- https://w3id.org/aio/DatatoTextLLM -->

    <owl:Class rdf:about="https://w3id.org/aio/DatatoTextLLM">
        <rdfs:subClassOf rdf:resource="https://w3id.org/aio/LargeLanguageModel"/>
        <obo:IAO_0000115>A LLM that generates natural language descriptions from structured data sources like tables, graphs, and knowledge bases, requiring grounding in meaning representations.</obo:IAO_0000115>
        <oboInOwl:hasExactSynonym>Meaning representation</oboInOwl:hasExactSynonym>
        <oboInOwl:inSubset rdf:resource="https://w3id.org/aio/ModelSubset"/>
        <rdfs:label>Data-to-Text LLM</rdfs:label>
    </owl:Class>
    


    <!-- https://w3id.org/aio/DecisionTree -->

    <owl:Class rdf:about="https://w3id.org/aio/DecisionTree">
        <rdfs:subClassOf rdf:resource="https://w3id.org/aio/Classification"/>
        <obo:IAO_0000115>A machine learning model that uses a tree-like model of decisions and their possible consequences including chance event outcomes resource costs and utilities.</obo:IAO_0000115>
        <oboInOwl:inSubset rdf:resource="https://w3id.org/aio/MachineLearningSubset"/>
        <rdfs:comment>A decision support tool that uses a tree-like model of decisions and their possible consequences, including chance event outcomes, resource costs, and utilities.</rdfs:comment>
        <rdfs:label>Decision Tree</rdfs:label>
    </owl:Class>
    <owl:Axiom>
        <owl:annotatedSource rdf:resource="https://w3id.org/aio/DecisionTree"/>
        <owl:annotatedProperty rdf:resource="http://purl.obolibrary.org/obo/IAO_0000115"/>
        <owl:annotatedTarget>A machine learning model that uses a tree-like model of decisions and their possible consequences including chance event outcomes resource costs and utilities.</owl:annotatedTarget>
        <oboInOwl:hasDbXref rdf:resource="https://en.wikipedia.org/wiki/Decision_tree"/>
    </owl:Axiom>
    


    <!-- https://w3id.org/aio/DecoderLLM -->

    <owl:Class rdf:about="https://w3id.org/aio/DecoderLLM">
        <rdfs:subClassOf rdf:resource="https://w3id.org/aio/LargeLanguageModel"/>
        <obo:IAO_0000115>A large language model that uses a decoder-only architecture consisting of only a decoder trained to predict the next token in a sequence given the previous tokens.</obo:IAO_0000115>
        <oboInOwl:inSubset rdf:resource="https://w3id.org/aio/ModelSubset"/>
        <rdfs:comment>A decoder-only architecture consisting of only a decoder, trained to predict the next token in a sequence given the previous tokens. Unlike the encoder-decoder architecture, it does not have an explicit encoder and encodes information implicitly in the hidden state of the decoder, updated at each step of the generation process.</rdfs:comment>
        <rdfs:label>Decoder LLM</rdfs:label>
    </owl:Class>
    <owl:Axiom>
        <owl:annotatedSource rdf:resource="https://w3id.org/aio/DecoderLLM"/>
        <owl:annotatedProperty rdf:resource="http://purl.obolibrary.org/obo/IAO_0000115"/>
        <owl:annotatedTarget>A large language model that uses a decoder-only architecture consisting of only a decoder trained to predict the next token in a sequence given the previous tokens.</owl:annotatedTarget>
        <oboInOwl:hasDbXref rdf:resource="https://www.practicalai.io/understanding-transformer-model-architectures/#:~:text=Encoder"/>
    </owl:Axiom>
    


    <!-- https://w3id.org/aio/DeconvolutionalNetwork -->

    <owl:Class rdf:about="https://w3id.org/aio/DeconvolutionalNetwork">
        <rdfs:subClassOf rdf:resource="https://w3id.org/aio/DeepNeuralNetwork"/>
        <rdfs:subClassOf>
            <owl:Restriction>
                <owl:onProperty rdf:resource="http://purl.obolibrary.org/obo/BFO_0000051"/>
                <owl:someValuesFrom rdf:resource="https://w3id.org/aio/ConvolutionalLayer"/>
            </owl:Restriction>
        </rdfs:subClassOf>
        <rdfs:subClassOf>
            <owl:Restriction>
                <owl:onProperty rdf:resource="http://purl.obolibrary.org/obo/BFO_0000051"/>
                <owl:someValuesFrom rdf:resource="https://w3id.org/aio/InputLayer"/>
            </owl:Restriction>
        </rdfs:subClassOf>
        <rdfs:subClassOf>
            <owl:Restriction>
                <owl:onProperty rdf:resource="http://purl.obolibrary.org/obo/BFO_0000051"/>
                <owl:someValuesFrom rdf:resource="https://w3id.org/aio/KernelLayer"/>
            </owl:Restriction>
        </rdfs:subClassOf>
        <rdfs:subClassOf>
            <owl:Restriction>
                <owl:onProperty rdf:resource="http://purl.obolibrary.org/obo/BFO_0000051"/>
                <owl:someValuesFrom rdf:resource="https://w3id.org/aio/OutputLayer"/>
            </owl:Restriction>
        </rdfs:subClassOf>
        <rdfs:subClassOf>
            <owl:Restriction>
                <owl:onProperty rdf:resource="http://purl.obolibrary.org/obo/BFO_0000051"/>
                <owl:someValuesFrom rdf:resource="https://w3id.org/aio/PoolingLayer"/>
            </owl:Restriction>
        </rdfs:subClassOf>
        <obo:IAO_0000115>A deep neural network that uses deconvolution for unsupervised construction of hierarchical image representations.</obo:IAO_0000115>
        <oboInOwl:hasExactSynonym>DN</oboInOwl:hasExactSynonym>
        <oboInOwl:inSubset rdf:resource="https://w3id.org/aio/NetworkSubset"/>
        <rdfs:comment>Layers: Input, Kernel, Convolutional/Pool, Output</rdfs:comment>
        <rdfs:label>Deconvolutional Network</rdfs:label>
    </owl:Class>
    <owl:Axiom>
        <owl:annotatedSource rdf:resource="https://w3id.org/aio/DeconvolutionalNetwork"/>
        <owl:annotatedProperty rdf:resource="http://purl.obolibrary.org/obo/IAO_0000115"/>
        <owl:annotatedTarget>A deep neural network that uses deconvolution for unsupervised construction of hierarchical image representations.</owl:annotatedTarget>
        <oboInOwl:hasDbXref rdf:resource="https://ieeexplore.ieee.org/document/5539957"/>
    </owl:Axiom>
    


    <!-- https://w3id.org/aio/DeepActiveLearning -->

    <owl:Class rdf:about="https://w3id.org/aio/DeepActiveLearning">
        <rdfs:subClassOf rdf:resource="https://w3id.org/aio/DeepNeuralNetwork"/>
        <obo:IAO_0000115>A deep neural network that combines deep learning and active learning to maximize model performance while annotating the fewest samples possible.</obo:IAO_0000115>
        <oboInOwl:hasExactSynonym>DeepAL</oboInOwl:hasExactSynonym>
        <oboInOwl:inSubset rdf:resource="https://w3id.org/aio/NetworkSubset"/>
        <rdfs:label>Deep Active Learning</rdfs:label>
    </owl:Class>
    <owl:Axiom>
        <owl:annotatedSource rdf:resource="https://w3id.org/aio/DeepActiveLearning"/>
        <owl:annotatedProperty rdf:resource="http://purl.obolibrary.org/obo/IAO_0000115"/>
        <owl:annotatedTarget>A deep neural network that combines deep learning and active learning to maximize model performance while annotating the fewest samples possible.</owl:annotatedTarget>
        <oboInOwl:hasDbXref rdf:resource="https://arxiv.org/pdf/2009.00236.pdf"/>
    </owl:Axiom>
    


    <!-- https://w3id.org/aio/DeepBeliefNetwork -->

    <owl:Class rdf:about="https://w3id.org/aio/DeepBeliefNetwork">
        <rdfs:subClassOf rdf:resource="https://w3id.org/aio/UnsupervisedPretrainedNetwork"/>
        <rdfs:subClassOf>
            <owl:Restriction>
                <owl:onProperty rdf:resource="http://purl.obolibrary.org/obo/BFO_0000051"/>
                <owl:someValuesFrom rdf:resource="https://w3id.org/aio/BackfedInputLayer"/>
            </owl:Restriction>
        </rdfs:subClassOf>
        <rdfs:subClassOf>
            <owl:Restriction>
                <owl:onProperty rdf:resource="http://purl.obolibrary.org/obo/BFO_0000051"/>
                <owl:someValuesFrom rdf:resource="https://w3id.org/aio/MatchedInputOutputLayer"/>
            </owl:Restriction>
        </rdfs:subClassOf>
        <rdfs:subClassOf>
            <owl:Restriction>
                <owl:onProperty rdf:resource="http://purl.obolibrary.org/obo/BFO_0000051"/>
                <owl:someValuesFrom rdf:resource="https://w3id.org/aio/ProbabilisticHiddenLayer"/>
            </owl:Restriction>
        </rdfs:subClassOf>
        <obo:IAO_0000115>An unsupervised pretrained network composed of multiple layers of latent variables that learns to probabilistically reconstruct inputs and perform classification.</obo:IAO_0000115>
        <oboInOwl:hasExactSynonym>DBN</oboInOwl:hasExactSynonym>
        <oboInOwl:inSubset rdf:resource="https://w3id.org/aio/NetworkSubset"/>
        <rdfs:comment>Layers: Backfed Input, Probabilistic Hidden, Hidden, Matched Output-Input</rdfs:comment>
        <rdfs:label>Deep Belief Network</rdfs:label>
    </owl:Class>
    <owl:Axiom>
        <owl:annotatedSource rdf:resource="https://w3id.org/aio/DeepBeliefNetwork"/>
        <owl:annotatedProperty rdf:resource="http://purl.obolibrary.org/obo/IAO_0000115"/>
        <owl:annotatedTarget>An unsupervised pretrained network composed of multiple layers of latent variables that learns to probabilistically reconstruct inputs and perform classification.</owl:annotatedTarget>
        <oboInOwl:hasDbXref rdf:resource="https://en.wikipedia.org/wiki/Deep_belief_network"/>
    </owl:Axiom>
    


    <!-- https://w3id.org/aio/DeepConvolutionalInverseGraphicsNetwork -->

    <owl:Class rdf:about="https://w3id.org/aio/DeepConvolutionalInverseGraphicsNetwork">
        <rdfs:subClassOf rdf:resource="https://w3id.org/aio/AutoEncoderNetwork"/>
        <rdfs:subClassOf>
            <owl:Restriction>
                <owl:onProperty rdf:resource="http://purl.obolibrary.org/obo/BFO_0000051"/>
                <owl:someValuesFrom rdf:resource="https://w3id.org/aio/ConvolutionalLayer"/>
            </owl:Restriction>
        </rdfs:subClassOf>
        <rdfs:subClassOf>
            <owl:Restriction>
                <owl:onProperty rdf:resource="http://purl.obolibrary.org/obo/BFO_0000051"/>
                <owl:someValuesFrom rdf:resource="https://w3id.org/aio/KernelLayer"/>
            </owl:Restriction>
        </rdfs:subClassOf>
        <rdfs:subClassOf>
            <owl:Restriction>
                <owl:onProperty rdf:resource="http://purl.obolibrary.org/obo/BFO_0000051"/>
                <owl:someValuesFrom rdf:resource="https://w3id.org/aio/OutputLayer"/>
            </owl:Restriction>
        </rdfs:subClassOf>
        <rdfs:subClassOf>
            <owl:Restriction>
                <owl:onProperty rdf:resource="http://purl.obolibrary.org/obo/BFO_0000051"/>
                <owl:someValuesFrom rdf:resource="https://w3id.org/aio/PoolingLayer"/>
            </owl:Restriction>
        </rdfs:subClassOf>
        <rdfs:subClassOf>
            <owl:Restriction>
                <owl:onProperty rdf:resource="http://purl.obolibrary.org/obo/BFO_0000051"/>
                <owl:someValuesFrom rdf:resource="https://w3id.org/aio/ProbabilisticHiddenLayer"/>
            </owl:Restriction>
        </rdfs:subClassOf>
        <obo:IAO_0000115>An autoencoder network that learns interpretable disentangled image representations through convolution and de-convolution layers trained with the stochastic gradient variational Bayes algorithm.</obo:IAO_0000115>
        <oboInOwl:hasExactSynonym>DCIGN</oboInOwl:hasExactSynonym>
        <oboInOwl:inSubset rdf:resource="https://w3id.org/aio/NetworkSubset"/>
        <rdfs:comment>Layers: Input, Kernel, Convolutional/Pool, Probabilistic Hidden, Convolutional/Pool, Kernel, Output</rdfs:comment>
        <rdfs:label>Deep Convolutional Inverse Graphics Network</rdfs:label>
    </owl:Class>
    


    <!-- https://w3id.org/aio/DeepConvolutionalNetwork -->

    <owl:Class rdf:about="https://w3id.org/aio/DeepConvolutionalNetwork">
        <rdfs:subClassOf rdf:resource="https://w3id.org/aio/DeepNeuralNetwork"/>
        <rdfs:subClassOf>
            <owl:Restriction>
                <owl:onProperty rdf:resource="http://purl.obolibrary.org/obo/BFO_0000051"/>
                <owl:someValuesFrom rdf:resource="https://w3id.org/aio/ConvolutionalLayer"/>
            </owl:Restriction>
        </rdfs:subClassOf>
        <rdfs:subClassOf>
            <owl:Restriction>
                <owl:onProperty rdf:resource="http://purl.obolibrary.org/obo/BFO_0000051"/>
                <owl:someValuesFrom rdf:resource="https://w3id.org/aio/HiddenLayer"/>
            </owl:Restriction>
        </rdfs:subClassOf>
        <rdfs:subClassOf>
            <owl:Restriction>
                <owl:onProperty rdf:resource="http://purl.obolibrary.org/obo/BFO_0000051"/>
                <owl:someValuesFrom rdf:resource="https://w3id.org/aio/InputLayer"/>
            </owl:Restriction>
        </rdfs:subClassOf>
        <rdfs:subClassOf>
            <owl:Restriction>
                <owl:onProperty rdf:resource="http://purl.obolibrary.org/obo/BFO_0000051"/>
                <owl:someValuesFrom rdf:resource="https://w3id.org/aio/KernelLayer"/>
            </owl:Restriction>
        </rdfs:subClassOf>
        <rdfs:subClassOf>
            <owl:Restriction>
                <owl:onProperty rdf:resource="http://purl.obolibrary.org/obo/BFO_0000051"/>
                <owl:someValuesFrom rdf:resource="https://w3id.org/aio/OutputLayer"/>
            </owl:Restriction>
        </rdfs:subClassOf>
        <rdfs:subClassOf>
            <owl:Restriction>
                <owl:onProperty rdf:resource="http://purl.obolibrary.org/obo/BFO_0000051"/>
                <owl:someValuesFrom rdf:resource="https://w3id.org/aio/PoolingLayer"/>
            </owl:Restriction>
        </rdfs:subClassOf>
        <obo:IAO_0000115>A deep neural network specialized for analyzing visual imagery using shared-weight architecture and translation-equivariant feature maps.</obo:IAO_0000115>
        <oboInOwl:hasExactSynonym>CNN</oboInOwl:hasExactSynonym>
        <oboInOwl:hasExactSynonym>ConvNet</oboInOwl:hasExactSynonym>
        <oboInOwl:hasExactSynonym>Convolutional Neural Network</oboInOwl:hasExactSynonym>
        <oboInOwl:hasExactSynonym>DCN</oboInOwl:hasExactSynonym>
        <oboInOwl:inSubset rdf:resource="https://w3id.org/aio/NetworkSubset"/>
        <rdfs:comment>Layers: Input, Kernel, Convolutional/Pool, Hidden, Output</rdfs:comment>
        <rdfs:label>Deep Convolutional Network</rdfs:label>
    </owl:Class>
    <owl:Axiom>
        <owl:annotatedSource rdf:resource="https://w3id.org/aio/DeepConvolutionalNetwork"/>
        <owl:annotatedProperty rdf:resource="http://purl.obolibrary.org/obo/IAO_0000115"/>
        <owl:annotatedTarget>A deep neural network specialized for analyzing visual imagery using shared-weight architecture and translation-equivariant feature maps.</owl:annotatedTarget>
        <oboInOwl:hasDbXref rdf:resource="https://en.wikipedia.org/wiki/Convolutional_neural_network"/>
    </owl:Axiom>
    


    <!-- https://w3id.org/aio/DeepFeedForwardNetwork -->

    <owl:Class rdf:about="https://w3id.org/aio/DeepFeedForwardNetwork">
        <rdfs:subClassOf rdf:resource="https://w3id.org/aio/DeepNeuralNetwork"/>
        <rdfs:subClassOf>
            <owl:Restriction>
                <owl:onProperty rdf:resource="http://purl.obolibrary.org/obo/BFO_0000051"/>
                <owl:someValuesFrom rdf:resource="https://w3id.org/aio/HiddenLayer"/>
            </owl:Restriction>
        </rdfs:subClassOf>
        <rdfs:subClassOf>
            <owl:Restriction>
                <owl:onProperty rdf:resource="http://purl.obolibrary.org/obo/BFO_0000051"/>
                <owl:someValuesFrom rdf:resource="https://w3id.org/aio/InputLayer"/>
            </owl:Restriction>
        </rdfs:subClassOf>
        <rdfs:subClassOf>
            <owl:Restriction>
                <owl:onProperty rdf:resource="http://purl.obolibrary.org/obo/BFO_0000051"/>
                <owl:someValuesFrom rdf:resource="https://w3id.org/aio/OutputLayer"/>
            </owl:Restriction>
        </rdfs:subClassOf>
        <obo:IAO_0000115>A deep neural network that processes information in one direction—from input nodes through hidden nodes to output nodes—without cycles or loops.</obo:IAO_0000115>
        <oboInOwl:hasExactSynonym>DFF</oboInOwl:hasExactSynonym>
        <oboInOwl:hasExactSynonym>MLP</oboInOwl:hasExactSynonym>
        <oboInOwl:hasExactSynonym>Multilayer Perceptoron</oboInOwl:hasExactSynonym>
        <oboInOwl:inSubset rdf:resource="https://w3id.org/aio/NetworkSubset"/>
        <rdfs:comment>Layers: Input, Hidden, Output</rdfs:comment>
        <rdfs:label>Deep Feed-Forward Network</rdfs:label>
    </owl:Class>
    <owl:Axiom>
        <owl:annotatedSource rdf:resource="https://w3id.org/aio/DeepFeedForwardNetwork"/>
        <owl:annotatedProperty rdf:resource="http://purl.obolibrary.org/obo/IAO_0000115"/>
        <owl:annotatedTarget>A deep neural network that processes information in one direction—from input nodes through hidden nodes to output nodes—without cycles or loops.</owl:annotatedTarget>
        <oboInOwl:hasDbXref rdf:resource="https://en.wikipedia.org/wiki/Feedforward_neural_network"/>
    </owl:Axiom>
    


    <!-- https://w3id.org/aio/DeepNeuralNetwork -->

    <owl:Class rdf:about="https://w3id.org/aio/DeepNeuralNetwork">
        <rdfs:subClassOf rdf:resource="https://w3id.org/aio/ArtificialNeuralNetwork"/>
        <obo:IAO_0000115>An artificial neural network characterized by multiple hidden layers between the input and output layers.</obo:IAO_0000115>
        <oboInOwl:hasExactSynonym>DNN</oboInOwl:hasExactSynonym>
        <oboInOwl:inSubset rdf:resource="https://w3id.org/aio/NetworkSubset"/>
        <rdfs:comment>A deep neural network (DNN) is a type of artificial neural network (ANN) characterized by multiple hidden layers between the input and output layers. Each layer consists of interconnected neurons that process and transmit information. DNNs can model complex patterns and representations in data through their hierarchical structure, where each layer extracts increasingly abstract features from the input. DNNs are widely used in various applications, including image and speech recognition, natural language processing, and more, due to their ability to learn and generalize from large amounts of data.</rdfs:comment>
        <rdfs:label>Deep Neural Network</rdfs:label>
    </owl:Class>
    


    <!-- https://w3id.org/aio/DeepTransferLearning -->

    <owl:Class rdf:about="https://w3id.org/aio/DeepTransferLearning">
        <rdfs:subClassOf rdf:resource="https://w3id.org/aio/DeepNeuralNetwork"/>
        <obo:IAO_0000115>A deep neural network that relaxes the hypothesis that training data must be independent and identically distributed with test data to address insufficient training data.</obo:IAO_0000115>
        <oboInOwl:inSubset rdf:resource="https://w3id.org/aio/NetworkSubset"/>
        <rdfs:label>Deep Transfer Learning</rdfs:label>
    </owl:Class>
    <owl:Axiom>
        <owl:annotatedSource rdf:resource="https://w3id.org/aio/DeepTransferLearning"/>
        <owl:annotatedProperty rdf:resource="http://purl.obolibrary.org/obo/IAO_0000115"/>
        <owl:annotatedTarget>A deep neural network that relaxes the hypothesis that training data must be independent and identically distributed with test data to address insufficient training data.</owl:annotatedTarget>
        <oboInOwl:hasDbXref rdf:resource="https://arxiv.org/abs/1808.01974"/>
    </owl:Axiom>
    


    <!-- https://w3id.org/aio/DenoisingAutoEncoder -->

    <owl:Class rdf:about="https://w3id.org/aio/DenoisingAutoEncoder">
        <rdfs:subClassOf rdf:resource="https://w3id.org/aio/AutoEncoderNetwork"/>
        <rdfs:subClassOf>
            <owl:Restriction>
                <owl:onProperty rdf:resource="http://purl.obolibrary.org/obo/BFO_0000051"/>
                <owl:someValuesFrom rdf:resource="https://w3id.org/aio/NoisyInputLayer"/>
            </owl:Restriction>
        </rdfs:subClassOf>
        <obo:IAO_0000115>An autoencoder network trained to reconstruct the original undistorted input from a partially corrupted input.</obo:IAO_0000115>
        <oboInOwl:hasExactSynonym>DAE</oboInOwl:hasExactSynonym>
        <oboInOwl:hasExactSynonym>Denoising Autoencoder</oboInOwl:hasExactSynonym>
        <oboInOwl:inSubset rdf:resource="https://w3id.org/aio/NetworkSubset"/>
        <rdfs:comment>Layers: Noisy Input, Hidden, Matched Output-Input</rdfs:comment>
        <rdfs:label>Denoising Auto Encoder</rdfs:label>
    </owl:Class>
    <owl:Axiom>
        <owl:annotatedSource rdf:resource="https://w3id.org/aio/DenoisingAutoEncoder"/>
        <owl:annotatedProperty rdf:resource="http://purl.obolibrary.org/obo/IAO_0000115"/>
        <owl:annotatedTarget>An autoencoder network trained to reconstruct the original undistorted input from a partially corrupted input.</owl:annotatedTarget>
        <oboInOwl:hasDbXref rdf:resource="https://doi.org/10.1145/1390156.1390294"/>
    </owl:Axiom>
    


    <!-- https://w3id.org/aio/DenseFeaturesLayer -->

    <owl:Class rdf:about="https://w3id.org/aio/DenseFeaturesLayer">
        <rdfs:subClassOf rdf:resource="https://w3id.org/aio/Layer"/>
        <obo:IAO_0000115>A layer that produces a dense tensor based on given feature columns.</obo:IAO_0000115>
        <oboInOwl:inSubset rdf:resource="https://w3id.org/aio/LayerSubset"/>
        <rdfs:comment>A layer that produces a dense Tensor based on given feature_columns. Generally a single example in training data is described with FeatureColumns. At the first layer of the model, this column oriented data should be converted to a single Tensor. This layer can be called multiple times with different features. This is the V2 version of this layer that uses name_scopes to create variables instead of variable_scopes. But this approach currently lacks support for partitioned variables. In that case, use the V1 version instead.</rdfs:comment>
        <rdfs:label>DenseFeatures Layer</rdfs:label>
    </owl:Class>
    <owl:Axiom>
        <owl:annotatedSource rdf:resource="https://w3id.org/aio/DenseFeaturesLayer"/>
        <owl:annotatedProperty rdf:resource="http://purl.obolibrary.org/obo/IAO_0000115"/>
        <owl:annotatedTarget>A layer that produces a dense tensor based on given feature columns.</owl:annotatedTarget>
        <oboInOwl:hasDbXref rdf:resource="https://www.tensorflow.org/api_docs/python/tf/keras/layers/DenseFeatures"/>
    </owl:Axiom>
    


    <!-- https://w3id.org/aio/DenseLayer -->

    <owl:Class rdf:about="https://w3id.org/aio/DenseLayer">
        <rdfs:subClassOf rdf:resource="https://w3id.org/aio/Layer"/>
        <obo:IAO_0000115>A layer that is a regular densely-connected neural network layer.</obo:IAO_0000115>
        <oboInOwl:inSubset rdf:resource="https://w3id.org/aio/LayerSubset"/>
        <rdfs:comment>Just your regular densely-connected NN layer.</rdfs:comment>
        <rdfs:label>Dense Layer</rdfs:label>
    </owl:Class>
    <owl:Axiom>
        <owl:annotatedSource rdf:resource="https://w3id.org/aio/DenseLayer"/>
        <owl:annotatedProperty rdf:resource="http://purl.obolibrary.org/obo/IAO_0000115"/>
        <owl:annotatedTarget>A layer that is a regular densely-connected neural network layer.</owl:annotatedTarget>
        <oboInOwl:hasDbXref rdf:resource="https://www.tensorflow.org/api_docs/python/tf/keras/layers/Dense"/>
    </owl:Axiom>
    


    <!-- https://w3id.org/aio/DeploymentBias -->

    <owl:Class rdf:about="https://w3id.org/aio/DeploymentBias">
        <rdfs:subClassOf rdf:resource="https://w3id.org/aio/GroupBias"/>
        <obo:IAO_0000115>A bias arising when systems are used as decision aids for humans since the human intermediary may act on predictions in ways that are typically not modeled in the system.</obo:IAO_0000115>
        <oboInOwl:inSubset rdf:resource="https://w3id.org/aio/BiasSubset"/>
        <rdfs:label>Deployment Bias</rdfs:label>
    </owl:Class>
    <owl:Axiom>
        <owl:annotatedSource rdf:resource="https://w3id.org/aio/DeploymentBias"/>
        <owl:annotatedProperty rdf:resource="http://purl.obolibrary.org/obo/IAO_0000115"/>
        <owl:annotatedTarget>A bias arising when systems are used as decision aids for humans since the human intermediary may act on predictions in ways that are typically not modeled in the system.</owl:annotatedTarget>
        <oboInOwl:hasDbXref rdf:resource="https://doi.org/10.6028/NIST.SP.1270"/>
    </owl:Axiom>
    


    <!-- https://w3id.org/aio/DepthwiseConv1DLayer -->

    <owl:Class rdf:about="https://w3id.org/aio/DepthwiseConv1DLayer">
        <rdfs:subClassOf rdf:resource="https://w3id.org/aio/ConvolutionalLayer"/>
        <obo:IAO_0000115>A layer that performs depthwise 1D convolution</obo:IAO_0000115>
        <oboInOwl:inSubset rdf:resource="https://w3id.org/aio/LayerSubset"/>
        <rdfs:comment>Depthwise 1D convolution. Depthwise convolution is a type of convolution in which each input channel is convolved with a different kernel (called a depthwise kernel). You can understand depthwise convolution as the first step in a depthwise separable convolution. It is implemented via the following steps: Split the input into individual channels. Convolve each channel with an individual depthwise kernel with depth_multiplier output channels. Concatenate the convolved outputs along the channels axis. Unlike a regular 1D convolution, depthwise convolution does not mix information across different input channels. The depth_multiplier argument determines how many filter are applied to one input channel. As such, it controls the amount of output channels that are generated per input channel in the depthwise step.</rdfs:comment>
        <rdfs:label>DepthwiseConv1D Layer</rdfs:label>
    </owl:Class>
    <owl:Axiom>
        <owl:annotatedSource rdf:resource="https://w3id.org/aio/DepthwiseConv1DLayer"/>
        <owl:annotatedProperty rdf:resource="http://purl.obolibrary.org/obo/IAO_0000115"/>
        <owl:annotatedTarget>A layer that performs depthwise 1D convolution</owl:annotatedTarget>
        <oboInOwl:hasDbXref rdf:resource="https://www.tensorflow.org/api_docs/python/tf/keras/layers/DepthwiseConv1D"/>
    </owl:Axiom>
    


    <!-- https://w3id.org/aio/DepthwiseConv2DLayer -->

    <owl:Class rdf:about="https://w3id.org/aio/DepthwiseConv2DLayer">
        <rdfs:subClassOf rdf:resource="https://w3id.org/aio/ConvolutionalLayer"/>
        <obo:IAO_0000115>A layer that performs depthwise 2D convolution</obo:IAO_0000115>
        <oboInOwl:inSubset rdf:resource="https://w3id.org/aio/LayerSubset"/>
        <rdfs:comment>Depthwise 2D convolution.</rdfs:comment>
        <rdfs:label>DepthwiseConv2D Layer</rdfs:label>
    </owl:Class>
    <owl:Axiom>
        <owl:annotatedSource rdf:resource="https://w3id.org/aio/DepthwiseConv2DLayer"/>
        <owl:annotatedProperty rdf:resource="http://purl.obolibrary.org/obo/IAO_0000115"/>
        <owl:annotatedTarget>A layer that performs depthwise 2D convolution</owl:annotatedTarget>
        <oboInOwl:hasDbXref rdf:resource="https://www.tensorflow.org/api_docs/python/tf/keras/layers/DepthwiseConv2D"/>
    </owl:Axiom>
    


    <!-- https://w3id.org/aio/DetectionBias -->

    <owl:Class rdf:about="https://w3id.org/aio/DetectionBias">
        <rdfs:subClassOf rdf:resource="https://w3id.org/aio/SelectionAndSamplingBias"/>
        <obo:IAO_0000115>A selection and sampling bias characterized by systematic differences between groups in how outcomes are determined potentially over- or underestimating effect size.</obo:IAO_0000115>
        <oboInOwl:inSubset rdf:resource="https://w3id.org/aio/BiasSubset"/>
        <rdfs:comment>Systematic differences between groups in how outcomes are determined, potentially over- or underestimating effect size.</rdfs:comment>
        <rdfs:label>Detection Bias</rdfs:label>
    </owl:Class>
    <owl:Axiom>
        <owl:annotatedSource rdf:resource="https://w3id.org/aio/DetectionBias"/>
        <owl:annotatedProperty rdf:resource="http://purl.obolibrary.org/obo/IAO_0000115"/>
        <owl:annotatedTarget>A selection and sampling bias characterized by systematic differences between groups in how outcomes are determined potentially over- or underestimating effect size.</owl:annotatedTarget>
        <oboInOwl:hasDbXref rdf:resource="https://doi.org/10.6028/NIST.SP.1270"/>
    </owl:Axiom>
    


    <!-- https://w3id.org/aio/DialogueLLM -->

    <owl:Class rdf:about="https://w3id.org/aio/DialogueLLM">
        <rdfs:subClassOf rdf:resource="https://w3id.org/aio/LargeLanguageModel"/>
        <obo:IAO_0000115>A large language model that is optimized for engaging in multi-turn conversations understanding context and generating relevant coherent responses continuously over many dialogue turns.</obo:IAO_0000115>
        <oboInOwl:hasExactSynonym>Dialogue Large Language Model</oboInOwl:hasExactSynonym>
        <oboInOwl:hasRelatedSynonym>conversational AI</oboInOwl:hasRelatedSynonym>
        <oboInOwl:hasRelatedSynonym>multi-turn dialogue</oboInOwl:hasRelatedSynonym>
        <oboInOwl:inSubset rdf:resource="https://w3id.org/aio/ModelSubset"/>
        <rdfs:label>Dialogue LLM</rdfs:label>
    </owl:Class>
    


    <!-- https://w3id.org/aio/DifferentiableLLM -->

    <owl:Class rdf:about="https://w3id.org/aio/DifferentiableLLM">
        <rdfs:subClassOf rdf:resource="https://w3id.org/aio/LargeLanguageModel"/>
        <obo:IAO_0000115>A large language model that has an architecture amenable to full end-to-end training via backpropagation without relying on teacher forcing or unlikelihood training objectives.</obo:IAO_0000115>
        <oboInOwl:hasExactSynonym>Differentiable Large Language Model</oboInOwl:hasExactSynonym>
        <oboInOwl:hasRelatedSynonym>end-to-end training</oboInOwl:hasRelatedSynonym>
        <oboInOwl:hasRelatedSynonym>fully backpropagable</oboInOwl:hasRelatedSynonym>
        <oboInOwl:inSubset rdf:resource="https://w3id.org/aio/ModelSubset"/>
        <rdfs:label>Differentiable LLM</rdfs:label>
    </owl:Class>
    


    <!-- https://w3id.org/aio/DimensionalityReduction -->

    <owl:Class rdf:about="https://w3id.org/aio/DimensionalityReduction">
        <rdfs:subClassOf rdf:resource="https://w3id.org/aio/UnsupervisedLearning"/>
        <obo:IAO_0000115>A machine learning task focused on the process of transforming data from a high-dimensional space into a lower-dimensional space while retaining meaningful properties of the original data.</obo:IAO_0000115>
        <oboInOwl:hasExactSynonym>Dimension Reduction</oboInOwl:hasExactSynonym>
        <oboInOwl:inSubset rdf:resource="https://w3id.org/aio/MachineLearningSubset"/>
        <rdfs:label>Dimensionality Reduction</rdfs:label>
    </owl:Class>
    <owl:Axiom>
        <owl:annotatedSource rdf:resource="https://w3id.org/aio/DimensionalityReduction"/>
        <owl:annotatedProperty rdf:resource="http://purl.obolibrary.org/obo/IAO_0000115"/>
        <owl:annotatedTarget>A machine learning task focused on the process of transforming data from a high-dimensional space into a lower-dimensional space while retaining meaningful properties of the original data.</owl:annotatedTarget>
        <oboInOwl:hasDbXref rdf:resource="https://en.wikipedia.org/wiki/Dimensionality_reduction"/>
    </owl:Axiom>
    


    <!-- https://w3id.org/aio/DiscretizationLayer -->

    <owl:Class rdf:about="https://w3id.org/aio/DiscretizationLayer">
        <rdfs:subClassOf rdf:resource="https://w3id.org/aio/NumericalFeaturesPreprocessingLayer"/>
        <obo:IAO_0000115>A preprocessing layer which buckets continuous features by ranges.</obo:IAO_0000115>
        <oboInOwl:inSubset rdf:resource="https://w3id.org/aio/LayerSubset"/>
        <rdfs:label>Discretization Layer</rdfs:label>
    </owl:Class>
    <owl:Axiom>
        <owl:annotatedSource rdf:resource="https://w3id.org/aio/DiscretizationLayer"/>
        <owl:annotatedProperty rdf:resource="http://purl.obolibrary.org/obo/IAO_0000115"/>
        <owl:annotatedTarget>A preprocessing layer which buckets continuous features by ranges.</owl:annotatedTarget>
        <oboInOwl:hasDbXref rdf:resource="https://www.tensorflow.org/api_docs/python/tf/keras/layers/Discretization"/>
    </owl:Axiom>
    


    <!-- https://w3id.org/aio/Distillation -->

    <owl:Class rdf:about="https://w3id.org/aio/Distillation">
        <rdfs:subClassOf rdf:resource="https://w3id.org/aio/Preprocessing"/>
        <obo:IAO_0000115>The process of training a smaller model to replicate the behavior of a larger model aiming to compress the knowledge into a more compact form without significant loss of performance.</obo:IAO_0000115>
        <oboInOwl:hasExactSynonym>Purification</oboInOwl:hasExactSynonym>
        <oboInOwl:hasExactSynonym>Refining</oboInOwl:hasExactSynonym>
        <oboInOwl:hasRelatedSynonym>Knowledge compression</oboInOwl:hasRelatedSynonym>
        <oboInOwl:hasRelatedSynonym>Teacher-student model</oboInOwl:hasRelatedSynonym>
        <oboInOwl:inSubset rdf:resource="https://w3id.org/aio/PreprocessingSubset"/>
        <rdfs:label>Distillation</rdfs:label>
    </owl:Class>
    <owl:Axiom>
        <owl:annotatedSource rdf:resource="https://w3id.org/aio/Distillation"/>
        <owl:annotatedProperty rdf:resource="http://purl.obolibrary.org/obo/IAO_0000115"/>
        <owl:annotatedTarget>The process of training a smaller model to replicate the behavior of a larger model aiming to compress the knowledge into a more compact form without significant loss of performance.</owl:annotatedTarget>
        <oboInOwl:hasDbXref rdf:resource="https://doi.org/10.48550/arXiv.2105.13093"/>
    </owl:Axiom>
    


    <!-- https://w3id.org/aio/DomainAdaptedLLM -->

    <owl:Class rdf:about="https://w3id.org/aio/DomainAdaptedLLM">
        <rdfs:subClassOf rdf:resource="https://w3id.org/aio/LargeLanguageModel"/>
        <obo:IAO_0000115>A LLM which is pre-trained on a broad corpus and then fine-tuned on domain-specific data to specialize its capabilities for particular domains or applications, like scientific literature or code generation.</obo:IAO_0000115>
        <oboInOwl:hasExactSynonym>Domain-Adapted Large Language Model</oboInOwl:hasExactSynonym>
        <oboInOwl:hasRelatedSynonym>domain robustness</oboInOwl:hasRelatedSynonym>
        <oboInOwl:hasRelatedSynonym>transfer learning</oboInOwl:hasRelatedSynonym>
        <oboInOwl:inSubset rdf:resource="https://w3id.org/aio/ModelSubset"/>
        <rdfs:label>Domain-Adapted LLM</rdfs:label>
    </owl:Class>
    


    <!-- https://w3id.org/aio/DotLayer -->

    <owl:Class rdf:about="https://w3id.org/aio/DotLayer">
        <rdfs:subClassOf rdf:resource="https://w3id.org/aio/Layer"/>
        <obo:IAO_0000115>A layer that computes a dot product between samples in two tensors.</obo:IAO_0000115>
        <oboInOwl:inSubset rdf:resource="https://w3id.org/aio/LayerSubset"/>
        <rdfs:comment>Layer that computes a dot product between samples in two tensors. E.g. if applied to a list of two tensors a and b of shape (batch_size, n), the output will be a tensor of shape (batch_size, 1) where each entry i will be the dot product between a[i] and b[i].</rdfs:comment>
        <rdfs:label>Dot Layer</rdfs:label>
    </owl:Class>
    <owl:Axiom>
        <owl:annotatedSource rdf:resource="https://w3id.org/aio/DotLayer"/>
        <owl:annotatedProperty rdf:resource="http://purl.obolibrary.org/obo/IAO_0000115"/>
        <owl:annotatedTarget>A layer that computes a dot product between samples in two tensors.</owl:annotatedTarget>
        <oboInOwl:hasDbXref rdf:resource="https://www.tensorflow.org/api_docs/python/tf/keras/layers/Dot"/>
    </owl:Axiom>
    


    <!-- https://w3id.org/aio/DropoutLayer -->

    <owl:Class rdf:about="https://w3id.org/aio/DropoutLayer">
        <rdfs:subClassOf rdf:resource="https://w3id.org/aio/RegularizationLayer"/>
        <obo:IAO_0000115>A regularization layer that applies Dropout to the input</obo:IAO_0000115>
        <oboInOwl:inSubset rdf:resource="https://w3id.org/aio/LayerSubset"/>
        <rdfs:comment>Applies Dropout to the input. The Dropout layer randomly sets input units to 0 with a frequency of rate at each step during training time, which helps prevent overfitting. Inputs not set to 0 are scaled up by 1/(1 - rate) such that the sum over all inputs is unchanged. Note that the Dropout layer only applies when training is set to True such that no values are dropped during inference. When using model.fit, training will be appropriately set to True automatically, and in other contexts, you can set the kwarg explicitly to True when calling the layer. (This is in contrast to setting trainable=False for a Dropout layer. trainable does not affect the layer&apos;s behavior, as Dropout does not have any variables/weights that can be frozen during training.)</rdfs:comment>
        <rdfs:label>Dropout Layer</rdfs:label>
    </owl:Class>
    <owl:Axiom>
        <owl:annotatedSource rdf:resource="https://w3id.org/aio/DropoutLayer"/>
        <owl:annotatedProperty rdf:resource="http://purl.obolibrary.org/obo/IAO_0000115"/>
        <owl:annotatedTarget>A regularization layer that applies Dropout to the input</owl:annotatedTarget>
        <oboInOwl:hasDbXref rdf:resource="https://www.tensorflow.org/api_docs/python/tf/keras/layers/Dropout"/>
    </owl:Axiom>
    


    <!-- https://w3id.org/aio/DunningKrugerEffectBias -->

    <owl:Class rdf:about="https://w3id.org/aio/DunningKrugerEffectBias">
        <rdfs:subClassOf rdf:resource="https://w3id.org/aio/CognitiveBias"/>
        <obo:IAO_0000115>A cognitive bias in which people with low ability in an area overestimate that ability. Often measured by comparing self-assessment with objective performance.</obo:IAO_0000115>
        <oboInOwl:hasExactSynonym>Dunning-Kruger Effect</oboInOwl:hasExactSynonym>
        <oboInOwl:inSubset rdf:resource="https://w3id.org/aio/BiasSubset"/>
        <rdfs:label>Dunning-Kruger Effect Bias</rdfs:label>
    </owl:Class>
    <owl:Axiom>
        <owl:annotatedSource rdf:resource="https://w3id.org/aio/DunningKrugerEffectBias"/>
        <owl:annotatedProperty rdf:resource="http://purl.obolibrary.org/obo/IAO_0000115"/>
        <owl:annotatedTarget>A cognitive bias in which people with low ability in an area overestimate that ability. Often measured by comparing self-assessment with objective performance.</owl:annotatedTarget>
        <oboInOwl:hasDbXref rdf:resource="https://doi.org/10.6028/NIST.SP.1270"/>
    </owl:Axiom>
    


    <!-- https://w3id.org/aio/DynamicConditionalCorrelation -->

    <owl:Class rdf:about="https://w3id.org/aio/DynamicConditionalCorrelation">
        <rdfs:subClassOf rdf:resource="https://w3id.org/aio/Model"/>
        <obo:IAO_0000115>A model that allows for time-varying correlations between different time series, used in financial econometrics to model and forecast covariances.</obo:IAO_0000115>
        <oboInOwl:hasExactSynonym>DCC</oboInOwl:hasExactSynonym>
        <oboInOwl:inSubset rdf:resource="https://w3id.org/aio/ModelSubset"/>
        <rdfs:label>Dynamic Conditional Correlation</rdfs:label>
    </owl:Class>
    


    <!-- https://w3id.org/aio/ELUFunction -->

    <owl:Class rdf:about="https://w3id.org/aio/ELUFunction">
        <rdfs:subClassOf rdf:resource="https://w3id.org/aio/Function"/>
        <obo:IAO_0000115>An activation function that is x if x &gt; 0 and alpha * (exp(x) - 1) if x &lt; 0 where alpha controls the value to which an ELU saturates for negative net inputs.</obo:IAO_0000115>
        <oboInOwl:hasExactSynonym>ELU</oboInOwl:hasExactSynonym>
        <oboInOwl:hasExactSynonym>Exponential Linear Unit</oboInOwl:hasExactSynonym>
        <oboInOwl:inSubset rdf:resource="https://w3id.org/aio/FunctionSubset"/>
        <rdfs:comment>The exponential linear unit (ELU) with alpha &gt; 0 is: x if x &gt; 0 and alpha * (exp(x) - 1) if x &lt; 0 The ELU hyperparameter alpha controls the value to which an ELU saturates for negative net inputs. ELUs diminish the vanishing gradient effect. ELUs have negative values which pushes the mean of the activations closer to zero. Mean activations that are closer to zero enable faster Learning as they bring the gradient closer to the natural gradient. ELUs saturate to a negative value when the argument gets smaller. Saturation means a small derivative which decreases the variation and the information that is propagated to the next layer.</rdfs:comment>
        <rdfs:label>ELU Function</rdfs:label>
    </owl:Class>
    <owl:Axiom>
        <owl:annotatedSource rdf:resource="https://w3id.org/aio/ELUFunction"/>
        <owl:annotatedProperty rdf:resource="http://purl.obolibrary.org/obo/IAO_0000115"/>
        <owl:annotatedTarget>An activation function that is x if x &gt; 0 and alpha * (exp(x) - 1) if x &lt; 0 where alpha controls the value to which an ELU saturates for negative net inputs.</owl:annotatedTarget>
        <oboInOwl:hasDbXref rdf:resource="https://www.tensorflow.org/api_docs/python/tf/keras/activations/elu"/>
    </owl:Axiom>
    


    <!-- https://w3id.org/aio/ELULayer -->

    <owl:Class rdf:about="https://w3id.org/aio/ELULayer">
        <rdfs:subClassOf rdf:resource="https://w3id.org/aio/ActivationLayer"/>
        <obo:IAO_0000115>An activation layer that applies the Exponential Linear Unit (ELU) function element-wise.</obo:IAO_0000115>
        <oboInOwl:inSubset rdf:resource="https://w3id.org/aio/LayerSubset"/>
        <rdfs:comment>Exponential Linear Unit.</rdfs:comment>
        <rdfs:label>ELU Layer</rdfs:label>
    </owl:Class>
    <owl:Axiom>
        <owl:annotatedSource rdf:resource="https://w3id.org/aio/ELULayer"/>
        <owl:annotatedProperty rdf:resource="http://purl.obolibrary.org/obo/IAO_0000115"/>
        <owl:annotatedTarget>An activation layer that applies the Exponential Linear Unit (ELU) function element-wise.</owl:annotatedTarget>
        <oboInOwl:hasDbXref rdf:resource="https://www.tensorflow.org/api_docs/python/tf/keras/layers/ELU"/>
    </owl:Axiom>
    


    <!-- https://w3id.org/aio/EchoStateNetwork -->

    <owl:Class rdf:about="https://w3id.org/aio/EchoStateNetwork">
        <rdfs:subClassOf rdf:resource="https://w3id.org/aio/RecurrentNeuralNetwork"/>
        <rdfs:subClassOf>
            <owl:Restriction>
                <owl:onProperty rdf:resource="http://purl.obolibrary.org/obo/BFO_0000051"/>
                <owl:someValuesFrom rdf:resource="https://w3id.org/aio/InputLayer"/>
            </owl:Restriction>
        </rdfs:subClassOf>
        <rdfs:subClassOf>
            <owl:Restriction>
                <owl:onProperty rdf:resource="http://purl.obolibrary.org/obo/BFO_0000051"/>
                <owl:someValuesFrom rdf:resource="https://w3id.org/aio/OutputLayer"/>
            </owl:Restriction>
        </rdfs:subClassOf>
        <rdfs:subClassOf>
            <owl:Restriction>
                <owl:onProperty rdf:resource="http://purl.obolibrary.org/obo/BFO_0000051"/>
                <owl:someValuesFrom rdf:resource="https://w3id.org/aio/RecurrentLayer"/>
            </owl:Restriction>
        </rdfs:subClassOf>
        <obo:IAO_0000115>A recurrent neural network with a recurrent hidden layer and sparsely connected hidden neurons that learns output weights to produce temporal patterns.</obo:IAO_0000115>
        <oboInOwl:hasExactSynonym>ESN</oboInOwl:hasExactSynonym>
        <oboInOwl:inSubset rdf:resource="https://w3id.org/aio/NetworkSubset"/>
        <rdfs:comment>Layers: Input, Recurrent, Output</rdfs:comment>
        <rdfs:label>Echo State Network</rdfs:label>
    </owl:Class>
    <owl:Axiom>
        <owl:annotatedSource rdf:resource="https://w3id.org/aio/EchoStateNetwork"/>
        <owl:annotatedProperty rdf:resource="http://purl.obolibrary.org/obo/IAO_0000115"/>
        <owl:annotatedTarget>A recurrent neural network with a recurrent hidden layer and sparsely connected hidden neurons that learns output weights to produce temporal patterns.</owl:annotatedTarget>
        <oboInOwl:hasDbXref rdf:resource="https://en.wikipedia.org/wiki/Echo_state_network"/>
    </owl:Axiom>
    


    <!-- https://w3id.org/aio/EcologicalFallacyBias -->

    <owl:Class rdf:about="https://w3id.org/aio/EcologicalFallacyBias">
        <rdfs:subClassOf rdf:resource="https://w3id.org/aio/SelectionAndSamplingBias"/>
        <obo:IAO_0000115>A selection and sampling bias occurring when an inference about an individual is made based on their group membership.</obo:IAO_0000115>
        <oboInOwl:hasExactSynonym>Ecological Fallacy</oboInOwl:hasExactSynonym>
        <oboInOwl:inSubset rdf:resource="https://w3id.org/aio/BiasSubset"/>
        <rdfs:label>Ecological Fallacy Bias</rdfs:label>
    </owl:Class>
    <owl:Axiom>
        <owl:annotatedSource rdf:resource="https://w3id.org/aio/EcologicalFallacyBias"/>
        <owl:annotatedProperty rdf:resource="http://purl.obolibrary.org/obo/IAO_0000115"/>
        <owl:annotatedTarget>A selection and sampling bias occurring when an inference about an individual is made based on their group membership.</owl:annotatedTarget>
        <oboInOwl:hasDbXref rdf:resource="https://doi.org/10.6028/NIST.SP.1270"/>
    </owl:Axiom>
    


    <!-- https://w3id.org/aio/EmbeddingLayer -->

    <owl:Class rdf:about="https://w3id.org/aio/EmbeddingLayer">
        <rdfs:subClassOf rdf:resource="https://w3id.org/aio/Layer"/>
        <obo:IAO_0000115>A layer that turns positive integers (indexes) into dense vectors of fixed size.</obo:IAO_0000115>
        <oboInOwl:inSubset rdf:resource="https://w3id.org/aio/LayerSubset"/>
        <rdfs:label>Embedding Layer</rdfs:label>
    </owl:Class>
    <owl:Axiom>
        <owl:annotatedSource rdf:resource="https://w3id.org/aio/EmbeddingLayer"/>
        <owl:annotatedProperty rdf:resource="http://purl.obolibrary.org/obo/IAO_0000115"/>
        <owl:annotatedTarget>A layer that turns positive integers (indexes) into dense vectors of fixed size.</owl:annotatedTarget>
        <oboInOwl:hasDbXref rdf:resource="https://www.tensorflow.org/api_docs/python/tf/keras/layers/Embedding"/>
    </owl:Axiom>
    


    <!-- https://w3id.org/aio/EmbodiedLLM -->

    <owl:Class rdf:about="https://w3id.org/aio/EmbodiedLLM">
        <rdfs:subClassOf rdf:resource="https://w3id.org/aio/LargeLanguageModel"/>
        <obo:IAO_0000115>A large language model that integrates language with other modalities like vision audio and robotics to enable grounded language understanding in real-world environments.</obo:IAO_0000115>
        <oboInOwl:hasExactSynonym>Embodied Large Language Model</oboInOwl:hasExactSynonym>
        <oboInOwl:hasRelatedSynonym>multimodal grounding</oboInOwl:hasRelatedSynonym>
        <oboInOwl:inSubset rdf:resource="https://w3id.org/aio/ModelSubset"/>
        <rdfs:comment>An embodied LLM integrates language with other modalities like vision, audio, and robotics to enable grounded language understanding in real-world environments.</rdfs:comment>
        <rdfs:label>Embodied LLM</rdfs:label>
    </owl:Class>
    


    <!-- https://w3id.org/aio/EmergentBias -->

    <owl:Class rdf:about="https://w3id.org/aio/EmergentBias">
        <rdfs:subClassOf rdf:resource="https://w3id.org/aio/UseAndInterpretationBias"/>
        <obo:IAO_0000115>A use and interpretation bias resulting from the use and reliance on algorithms across new or unanticipated contexts.</obo:IAO_0000115>
        <oboInOwl:inSubset rdf:resource="https://w3id.org/aio/BiasSubset"/>
        <rdfs:label>Emergent Bias</rdfs:label>
    </owl:Class>
    <owl:Axiom>
        <owl:annotatedSource rdf:resource="https://w3id.org/aio/EmergentBias"/>
        <owl:annotatedProperty rdf:resource="http://purl.obolibrary.org/obo/IAO_0000115"/>
        <owl:annotatedTarget>A use and interpretation bias resulting from the use and reliance on algorithms across new or unanticipated contexts.</owl:annotatedTarget>
        <oboInOwl:hasDbXref rdf:resource="https://doi.org/10.6028/NIST.SP.1270"/>
    </owl:Axiom>
    


    <!-- https://w3id.org/aio/EncoderDecoderLLM -->

    <owl:Class rdf:about="https://w3id.org/aio/EncoderDecoderLLM">
        <rdfs:subClassOf rdf:resource="https://w3id.org/aio/LargeLanguageModel"/>
        <obo:IAO_0000115>The LLM introduced in the &quot;Attention Is All You Need&quot; paper. The encoder processes the input sequence to generate a hidden representation summarizing the input information, while the decoder uses this hidden representation to generate the desired output sequence.</obo:IAO_0000115>
        <oboInOwl:inSubset rdf:resource="https://w3id.org/aio/ModelSubset"/>
        <rdfs:label>Encoder-Decoder LLM</rdfs:label>
    </owl:Class>
    <owl:Axiom>
        <owl:annotatedSource rdf:resource="https://w3id.org/aio/EncoderDecoderLLM"/>
        <owl:annotatedProperty rdf:resource="http://purl.obolibrary.org/obo/IAO_0000115"/>
        <owl:annotatedTarget>The LLM introduced in the &quot;Attention Is All You Need&quot; paper. The encoder processes the input sequence to generate a hidden representation summarizing the input information, while the decoder uses this hidden representation to generate the desired output sequence.</owl:annotatedTarget>
        <oboInOwl:hasDbXref rdf:resource="https://www.practicalai.io/understanding-transformer-model-architectures/#:~:text=Encoder"/>
    </owl:Axiom>
    


    <!-- https://w3id.org/aio/EncoderLLM -->

    <owl:Class rdf:about="https://w3id.org/aio/EncoderLLM">
        <rdfs:subClassOf rdf:resource="https://w3id.org/aio/LargeLanguageModel"/>
        <obo:IAO_0000115>A large language model that uses an encoder-only architecture to encode the input sequence into a fixed-length representation which is then used as input to a classifier or regressor for prediction.</obo:IAO_0000115>
        <oboInOwl:inSubset rdf:resource="https://w3id.org/aio/ModelSubset"/>
        <rdfs:comment>An encoder-only architecture that encodes the input sequence into a fixed-length representation, which is then used as input to a classifier or regressor for prediction. The model has a pre-trained general-purpose encoder that requires fine-tuning for specific tasks.</rdfs:comment>
        <rdfs:label>Encoder LLM</rdfs:label>
    </owl:Class>
    <owl:Axiom>
        <owl:annotatedSource rdf:resource="https://w3id.org/aio/EncoderLLM"/>
        <owl:annotatedProperty rdf:resource="http://purl.obolibrary.org/obo/IAO_0000115"/>
        <owl:annotatedTarget>A large language model that uses an encoder-only architecture to encode the input sequence into a fixed-length representation which is then used as input to a classifier or regressor for prediction.</owl:annotatedTarget>
        <oboInOwl:hasDbXref rdf:resource="https://www.practicalai.io/understanding-transformer-model-architectures/#:~:text=Encoder"/>
    </owl:Axiom>
    


    <!-- https://w3id.org/aio/EnergyBasedLLM -->

    <owl:Class rdf:about="https://w3id.org/aio/EnergyBasedLLM">
        <rdfs:subClassOf rdf:resource="https://w3id.org/aio/LargeLanguageModel"/>
        <obo:IAO_0000115>A LLM which models the explicit probability density over token sequences using an energy function, rather than an autoregressive factorization. This can improve modeling of long-range dependencies and global coherence.</obo:IAO_0000115>
        <oboInOwl:hasExactSynonym>Energy-Based Large Language Model</oboInOwl:hasExactSynonym>
        <oboInOwl:hasRelatedSynonym>energy scoring</oboInOwl:hasRelatedSynonym>
        <oboInOwl:hasRelatedSynonym>explicit density modeling</oboInOwl:hasRelatedSynonym>
        <oboInOwl:inSubset rdf:resource="https://w3id.org/aio/ModelSubset"/>
        <rdfs:label>Energy-Based LLM</rdfs:label>
    </owl:Class>
    


    <!-- https://w3id.org/aio/EnsembleLearning -->

    <owl:Class rdf:about="https://w3id.org/aio/EnsembleLearning">
        <rdfs:subClassOf rdf:resource="https://w3id.org/aio/MachineLearning"/>
        <obo:IAO_0000115>A type of machine learning focused on methods that use multiple learning algorithms to achieve better predictive performance than any of the constituent algorithms alone.</obo:IAO_0000115>
        <oboInOwl:inSubset rdf:resource="https://w3id.org/aio/MachineLearningSubset"/>
        <rdfs:label>Ensemble Learning</rdfs:label>
    </owl:Class>
    <owl:Axiom>
        <owl:annotatedSource rdf:resource="https://w3id.org/aio/EnsembleLearning"/>
        <owl:annotatedProperty rdf:resource="http://purl.obolibrary.org/obo/IAO_0000115"/>
        <owl:annotatedTarget>A type of machine learning focused on methods that use multiple learning algorithms to achieve better predictive performance than any of the constituent algorithms alone.</owl:annotatedTarget>
        <oboInOwl:hasDbXref rdf:resource="https://en.wikipedia.org/wiki/Ensemble_learning"/>
    </owl:Axiom>
    


    <!-- https://w3id.org/aio/ErrorPropagationBias -->

    <owl:Class rdf:about="https://w3id.org/aio/ErrorPropagationBias">
        <rdfs:subClassOf rdf:resource="https://w3id.org/aio/ProcessingBias"/>
        <obo:IAO_0000115>A processing bias characterized by the effect of variables&apos; uncertainties (or errors more specifically random errors) on the uncertainty of a function based on them.</obo:IAO_0000115>
        <oboInOwl:hasExactSynonym>Error Propagation</oboInOwl:hasExactSynonym>
        <oboInOwl:inSubset rdf:resource="https://w3id.org/aio/BiasSubset"/>
        <rdfs:label>Error Propagation Bias</rdfs:label>
    </owl:Class>
    <owl:Axiom>
        <owl:annotatedSource rdf:resource="https://w3id.org/aio/ErrorPropagationBias"/>
        <owl:annotatedProperty rdf:resource="http://purl.obolibrary.org/obo/IAO_0000115"/>
        <owl:annotatedTarget>A processing bias characterized by the effect of variables&apos; uncertainties (or errors more specifically random errors) on the uncertainty of a function based on them.</owl:annotatedTarget>
        <oboInOwl:hasDbXref rdf:resource="https://doi.org/10.6028/NIST.SP.1270"/>
    </owl:Axiom>
    


    <!-- https://w3id.org/aio/EthicalLLM -->

    <owl:Class rdf:about="https://w3id.org/aio/EthicalLLM">
        <rdfs:subClassOf rdf:resource="https://w3id.org/aio/LargeLanguageModel"/>
        <obo:IAO_0000115>A large language model that is trained to uphold certain ethical principles values or rules in its language generation to increase safety and trustworthiness.</obo:IAO_0000115>
        <oboInOwl:hasExactSynonym>Ethical Large Language Model</oboInOwl:hasExactSynonym>
        <oboInOwl:hasRelatedSynonym>constituitional AI</oboInOwl:hasRelatedSynonym>
        <oboInOwl:hasRelatedSynonym>value alignment</oboInOwl:hasRelatedSynonym>
        <oboInOwl:inSubset rdf:resource="https://w3id.org/aio/ModelSubset"/>
        <rdfs:label>Ethical LLM</rdfs:label>
    </owl:Class>
    


    <!-- https://w3id.org/aio/EvaluationBias -->

    <owl:Class rdf:about="https://w3id.org/aio/EvaluationBias">
        <rdfs:subClassOf rdf:resource="https://w3id.org/aio/SelectionAndSamplingBias"/>
        <obo:IAO_0000115>A selection and sampling bias arising when testing populations do not equally represent user populations or when inappropriate performance metrics are used.</obo:IAO_0000115>
        <oboInOwl:inSubset rdf:resource="https://w3id.org/aio/BiasSubset"/>
        <rdfs:label>Evaluation Bias</rdfs:label>
    </owl:Class>
    <owl:Axiom>
        <owl:annotatedSource rdf:resource="https://w3id.org/aio/EvaluationBias"/>
        <owl:annotatedProperty rdf:resource="http://purl.obolibrary.org/obo/IAO_0000115"/>
        <owl:annotatedTarget>A selection and sampling bias arising when testing populations do not equally represent user populations or when inappropriate performance metrics are used.</owl:annotatedTarget>
        <oboInOwl:hasDbXref rdf:resource="https://doi.org/10.6028/NIST.SP.1270"/>
    </owl:Axiom>
    


    <!-- https://w3id.org/aio/EvolutionaryLLM -->

    <owl:Class rdf:about="https://w3id.org/aio/EvolutionaryLLM">
        <rdfs:subClassOf rdf:resource="https://w3id.org/aio/LargeLanguageModel"/>
        <obo:IAO_0000115>A large language model that applies principles of evolutionary computation to optimize its structure and parameters evolving over time to improve performance.</obo:IAO_0000115>
        <oboInOwl:hasExactSynonym>Evolutionary Language Model</oboInOwl:hasExactSynonym>
        <oboInOwl:hasRelatedSynonym>evolutionary algorithms</oboInOwl:hasRelatedSynonym>
        <oboInOwl:hasRelatedSynonym>genetic programming</oboInOwl:hasRelatedSynonym>
        <oboInOwl:inSubset rdf:resource="https://w3id.org/aio/ModelSubset"/>
        <rdfs:label>Evolutionary LLM</rdfs:label>
    </owl:Class>
    


    <!-- https://w3id.org/aio/ExclusionBias -->

    <owl:Class rdf:about="https://w3id.org/aio/ExclusionBias">
        <rdfs:subClassOf rdf:resource="https://w3id.org/aio/SelectionAndSamplingBias"/>
        <obo:IAO_0000115>A selection and sampling bias occurring when specific groups of user populations are excluded from testing and analysis.</obo:IAO_0000115>
        <oboInOwl:inSubset rdf:resource="https://w3id.org/aio/BiasSubset"/>
        <rdfs:label>Exclusion Bias</rdfs:label>
    </owl:Class>
    <owl:Axiom>
        <owl:annotatedSource rdf:resource="https://w3id.org/aio/ExclusionBias"/>
        <owl:annotatedProperty rdf:resource="http://purl.obolibrary.org/obo/IAO_0000115"/>
        <owl:annotatedTarget>A selection and sampling bias occurring when specific groups of user populations are excluded from testing and analysis.</owl:annotatedTarget>
        <oboInOwl:hasDbXref rdf:resource="https://doi.org/10.6028/NIST.SP.1270"/>
    </owl:Axiom>
    


    <!-- https://w3id.org/aio/ExplainableLLM -->

    <owl:Class rdf:about="https://w3id.org/aio/ExplainableLLM">
        <rdfs:subClassOf rdf:resource="https://w3id.org/aio/LargeLanguageModel"/>
        <obo:IAO_0000115>A large language model that is designed to provide insights into its decision-making process making it easier for users to understand and trust the model&apos;s outputs by incorporating mechanisms for interpreting and explaining its predictions in human-understandable terms.</obo:IAO_0000115>
        <oboInOwl:hasExactSynonym>Explainable Language Model</oboInOwl:hasExactSynonym>
        <oboInOwl:hasExactSynonym>XAI LLM</oboInOwl:hasExactSynonym>
        <oboInOwl:hasRelatedSynonym>interpretability</oboInOwl:hasRelatedSynonym>
        <oboInOwl:hasRelatedSynonym>model understanding</oboInOwl:hasRelatedSynonym>
        <oboInOwl:inSubset rdf:resource="https://w3id.org/aio/ModelSubset"/>
        <rdfs:label>Explainable LLM</rdfs:label>
    </owl:Class>
    


    <!-- https://w3id.org/aio/ExponentialFunction -->

    <owl:Class rdf:about="https://w3id.org/aio/ExponentialFunction">
        <rdfs:subClassOf rdf:resource="https://w3id.org/aio/Function"/>
        <obo:IAO_0000115>An activation function that is the mathematical function denoted by f(x)=exp or e^{x}.</obo:IAO_0000115>
        <oboInOwl:inSubset rdf:resource="https://w3id.org/aio/FunctionSubset"/>
        <rdfs:comment>The exponential function is a mathematical function denoted by f(x)=exp or e^{x}.</rdfs:comment>
        <rdfs:label>Exponential Function</rdfs:label>
    </owl:Class>
    <owl:Axiom>
        <owl:annotatedSource rdf:resource="https://w3id.org/aio/ExponentialFunction"/>
        <owl:annotatedProperty rdf:resource="http://purl.obolibrary.org/obo/IAO_0000115"/>
        <owl:annotatedTarget>An activation function that is the mathematical function denoted by f(x)=exp or e^{x}.</owl:annotatedTarget>
        <oboInOwl:hasDbXref rdf:resource="https://www.tensorflow.org/api_docs/python/tf/keras/activations/exponential"/>
    </owl:Axiom>
    


    <!-- https://w3id.org/aio/ExponentialSmoothingStateSpaceModel -->

    <owl:Class rdf:about="https://w3id.org/aio/ExponentialSmoothingStateSpaceModel">
        <rdfs:subClassOf rdf:resource="https://w3id.org/aio/Model"/>
        <obo:IAO_0000115>A model that combines exponential smoothing with state space modeling, allowing for the inclusion of both trend and seasonal components. Used in  forecasting.</obo:IAO_0000115>
        <oboInOwl:hasExactSynonym>ETS</oboInOwl:hasExactSynonym>
        <oboInOwl:inSubset rdf:resource="https://w3id.org/aio/ModelSubset"/>
        <rdfs:label>Exponential Smoothing State Space Model</rdfs:label>
    </owl:Class>
    


    <!-- https://w3id.org/aio/ExtremeLearningMachine -->

    <owl:Class rdf:about="https://w3id.org/aio/ExtremeLearningMachine">
        <rdfs:subClassOf rdf:resource="https://w3id.org/aio/FeedbackNetwork"/>
        <obo:IAO_0000115>A feedback network with randomly assigned hidden nodes that are not updated during training.</obo:IAO_0000115>
        <oboInOwl:hasExactSynonym>ELM</oboInOwl:hasExactSynonym>
        <oboInOwl:inSubset rdf:resource="https://w3id.org/aio/NetworkSubset"/>
        <rdfs:comment>Layers: Input, Hidden, Output</rdfs:comment>
        <rdfs:label>Extreme Learning Machine</rdfs:label>
    </owl:Class>
    <owl:Axiom>
        <owl:annotatedSource rdf:resource="https://w3id.org/aio/ExtremeLearningMachine"/>
        <owl:annotatedProperty rdf:resource="http://purl.obolibrary.org/obo/IAO_0000115"/>
        <owl:annotatedTarget>A feedback network with randomly assigned hidden nodes that are not updated during training.</owl:annotatedTarget>
        <oboInOwl:hasDbXref rdf:resource="https://en.wikipedia.org/wiki/Extreme_Learning_machine"/>
    </owl:Axiom>
    


    <!-- https://w3id.org/aio/FactoredLanguageModel -->

    <owl:Class rdf:about="https://w3id.org/aio/FactoredLanguageModel">
        <rdfs:subClassOf rdf:resource="https://w3id.org/aio/LanguageModel"/>
        <obo:IAO_0000115>A language model that views each word as a vector of multiple factors such as part-of-speech morphology and semantics to improve language modeling.</obo:IAO_0000115>
        <oboInOwl:hasExactSynonym>Factorized Language Model</oboInOwl:hasExactSynonym>
        <oboInOwl:inSubset rdf:resource="https://w3id.org/aio/ModelSubset"/>
        <rdfs:label>Factored Language Model</rdfs:label>
    </owl:Class>
    <owl:Axiom>
        <owl:annotatedSource rdf:resource="https://w3id.org/aio/FactoredLanguageModel"/>
        <owl:annotatedProperty rdf:resource="http://purl.obolibrary.org/obo/IAO_0000115"/>
        <owl:annotatedTarget>A language model that views each word as a vector of multiple factors such as part-of-speech morphology and semantics to improve language modeling.</owl:annotatedTarget>
        <oboInOwl:hasDbXref rdf:resource="https://en.wikipedia.org/wiki/Factored_language_model"/>
    </owl:Axiom>
    


    <!-- https://w3id.org/aio/FactorizedLLM -->

    <owl:Class rdf:about="https://w3id.org/aio/FactorizedLLM">
        <rdfs:subClassOf rdf:resource="https://w3id.org/aio/LargeLanguageModel"/>
        <obo:IAO_0000115>A large language model that decomposes the full language modeling task into multiple sub-components or experts that each focus on a subset of the information enabling more efficient scaling.</obo:IAO_0000115>
        <oboInOwl:hasExactSynonym>Factorized Large Language Model</oboInOwl:hasExactSynonym>
        <oboInOwl:hasExactSynonym>Factorized Learning Assisted with Large Language Model</oboInOwl:hasExactSynonym>
        <oboInOwl:hasRelatedSynonym>Conditional masking</oboInOwl:hasRelatedSynonym>
        <oboInOwl:hasRelatedSynonym>Product of experts</oboInOwl:hasRelatedSynonym>
        <oboInOwl:inSubset rdf:resource="https://w3id.org/aio/ModelSubset"/>
        <rdfs:label>Factorized LLM</rdfs:label>
    </owl:Class>
    <owl:Axiom>
        <owl:annotatedSource rdf:resource="https://w3id.org/aio/FactorizedLLM"/>
        <owl:annotatedProperty rdf:resource="http://purl.obolibrary.org/obo/IAO_0000115"/>
        <owl:annotatedTarget>A large language model that decomposes the full language modeling task into multiple sub-components or experts that each focus on a subset of the information enabling more efficient scaling.</owl:annotatedTarget>
        <oboInOwl:hasDbXref rdf:resource="https://doi.org/10.48550/arXiv.2403.12556"/>
    </owl:Axiom>
    


    <!-- https://w3id.org/aio/FeatureExtraction -->

    <owl:Class rdf:about="https://w3id.org/aio/FeatureExtraction">
        <rdfs:subClassOf rdf:resource="https://w3id.org/aio/DataEnhancement"/>
        <obo:IAO_0000115>The process of transforming raw data into a set of measurable characteristics that can be used as input for machine learning algorithms enhancing the ability to make accurate predictions.</obo:IAO_0000115>
        <oboInOwl:hasExactSynonym>Attribute Extraction</oboInOwl:hasExactSynonym>
        <oboInOwl:hasExactSynonym>Feature Isolation</oboInOwl:hasExactSynonym>
        <oboInOwl:hasRelatedSynonym>Semantic embeddings</oboInOwl:hasRelatedSynonym>
        <oboInOwl:hasRelatedSynonym>Syntactic information</oboInOwl:hasRelatedSynonym>
        <oboInOwl:inSubset rdf:resource="https://w3id.org/aio/PreprocessingSubset"/>
        <rdfs:label>Feature Extraction</rdfs:label>
    </owl:Class>
    


    <!-- https://w3id.org/aio/FederatedLLM -->

    <owl:Class rdf:about="https://w3id.org/aio/FederatedLLM">
        <rdfs:subClassOf rdf:resource="https://w3id.org/aio/LargeLanguageModel"/>
        <obo:IAO_0000115>A large language model that is trained in a decentralized manner across multiple devices or silos without directly sharing private data enabling collaborative training while preserving data privacy and security.</obo:IAO_0000115>
        <oboInOwl:hasExactSynonym>Federated Large Language Model</oboInOwl:hasExactSynonym>
        <oboInOwl:hasRelatedSynonym>decentralized training</oboInOwl:hasRelatedSynonym>
        <oboInOwl:hasRelatedSynonym>privacy-preserving</oboInOwl:hasRelatedSynonym>
        <oboInOwl:inSubset rdf:resource="https://w3id.org/aio/ModelSubset"/>
        <rdfs:label>Federated LLM</rdfs:label>
    </owl:Class>
    


    <!-- https://w3id.org/aio/FederatedLearning -->

    <owl:Class rdf:about="https://w3id.org/aio/FederatedLearning">
        <rdfs:subClassOf rdf:resource="https://w3id.org/aio/DeepNeuralNetwork"/>
        <obo:IAO_0000115>A deep neural network trained across decentralized edge devices or servers holding local data samples without exchanging them.</obo:IAO_0000115>
        <oboInOwl:inSubset rdf:resource="https://w3id.org/aio/NetworkSubset"/>
        <rdfs:comment>Training an algorithm across multiple decentralized edge devices or servers holding local data samples without exchanging them.</rdfs:comment>
        <rdfs:label>Federated Learning</rdfs:label>
    </owl:Class>
    <owl:Axiom>
        <owl:annotatedSource rdf:resource="https://w3id.org/aio/FederatedLearning"/>
        <owl:annotatedProperty rdf:resource="http://purl.obolibrary.org/obo/IAO_0000115"/>
        <owl:annotatedTarget>A deep neural network trained across decentralized edge devices or servers holding local data samples without exchanging them.</owl:annotatedTarget>
        <oboInOwl:hasDbXref rdf:resource="https://en.wikipedia.org/wiki/Federated_learning"/>
    </owl:Axiom>
    


    <!-- https://w3id.org/aio/FeedbackLoopBias -->

    <owl:Class rdf:about="https://w3id.org/aio/FeedbackLoopBias">
        <rdfs:subClassOf rdf:resource="https://w3id.org/aio/UseAndInterpretationBias"/>
        <obo:IAO_0000115>A use and interpretation bias occurring when an algorithm learns from user behavior and feeds that behavior back into the model.</obo:IAO_0000115>
        <oboInOwl:inSubset rdf:resource="https://w3id.org/aio/BiasSubset"/>
        <rdfs:label>Feedback Loop Bias</rdfs:label>
    </owl:Class>
    <owl:Axiom>
        <owl:annotatedSource rdf:resource="https://w3id.org/aio/FeedbackLoopBias"/>
        <owl:annotatedProperty rdf:resource="http://purl.obolibrary.org/obo/IAO_0000115"/>
        <owl:annotatedTarget>A use and interpretation bias occurring when an algorithm learns from user behavior and feeds that behavior back into the model.</owl:annotatedTarget>
        <oboInOwl:hasDbXref rdf:resource="https://doi.org/10.6028/NIST.SP.1270"/>
    </owl:Axiom>
    


    <!-- https://w3id.org/aio/FeedbackNetwork -->

    <owl:Class rdf:about="https://w3id.org/aio/FeedbackNetwork">
        <rdfs:subClassOf rdf:resource="https://w3id.org/aio/ArtificialNeuralNetwork"/>
        <rdfs:subClassOf>
            <owl:Restriction>
                <owl:onProperty rdf:resource="http://purl.obolibrary.org/obo/BFO_0000051"/>
                <owl:someValuesFrom rdf:resource="https://w3id.org/aio/HiddenLayer"/>
            </owl:Restriction>
        </rdfs:subClassOf>
        <rdfs:subClassOf>
            <owl:Restriction>
                <owl:onProperty rdf:resource="http://purl.obolibrary.org/obo/BFO_0000051"/>
                <owl:someValuesFrom rdf:resource="https://w3id.org/aio/InputLayer"/>
            </owl:Restriction>
        </rdfs:subClassOf>
        <rdfs:subClassOf>
            <owl:Restriction>
                <owl:onProperty rdf:resource="http://purl.obolibrary.org/obo/BFO_0000051"/>
                <owl:someValuesFrom rdf:resource="https://w3id.org/aio/OutputLayer"/>
            </owl:Restriction>
        </rdfs:subClassOf>
        <obo:IAO_0000115>An artificial neural network that refines its representations iteratively based on feedback from previous outputs.</obo:IAO_0000115>
        <oboInOwl:hasExactSynonym>FBN</oboInOwl:hasExactSynonym>
        <oboInOwl:inSubset rdf:resource="https://w3id.org/aio/NetworkSubset"/>
        <rdfs:comment>Layers: Input, Hidden, Output, Hidden</rdfs:comment>
        <rdfs:label>Feedback Network</rdfs:label>
    </owl:Class>
    


    <!-- https://w3id.org/aio/FixedEffectsModel -->

    <owl:Class rdf:about="https://w3id.org/aio/FixedEffectsModel">
        <rdfs:subClassOf rdf:resource="https://w3id.org/aio/RegressionAnalysis"/>
        <obo:IAO_0000115>A regression analysis model in which the model parameters are fixed or non-random quantities.</obo:IAO_0000115>
        <oboInOwl:hasExactSynonym>FEM</oboInOwl:hasExactSynonym>
        <oboInOwl:inSubset rdf:resource="https://w3id.org/aio/MachineLearningSubset"/>
        <rdfs:label>Fixed Effects Model</rdfs:label>
    </owl:Class>
    <owl:Axiom>
        <owl:annotatedSource rdf:resource="https://w3id.org/aio/FixedEffectsModel"/>
        <owl:annotatedProperty rdf:resource="http://purl.obolibrary.org/obo/IAO_0000115"/>
        <owl:annotatedTarget>A regression analysis model in which the model parameters are fixed or non-random quantities.</owl:annotatedTarget>
        <oboInOwl:hasDbXref rdf:resource="https://en.wikipedia.org/wiki/Fixed_effects_model"/>
    </owl:Axiom>
    


    <!-- https://w3id.org/aio/FlattenLayer -->

    <owl:Class rdf:about="https://w3id.org/aio/FlattenLayer">
        <rdfs:subClassOf rdf:resource="https://w3id.org/aio/ReshapingLayer"/>
        <obo:IAO_0000115>A layer that flattens the input</obo:IAO_0000115>
        <oboInOwl:inSubset rdf:resource="https://w3id.org/aio/LayerSubset"/>
        <rdfs:comment>Flattens the input. Does not affect the batch size.</rdfs:comment>
        <rdfs:label>Flatten Layer</rdfs:label>
    </owl:Class>
    <owl:Axiom>
        <owl:annotatedSource rdf:resource="https://w3id.org/aio/FlattenLayer"/>
        <owl:annotatedProperty rdf:resource="http://purl.obolibrary.org/obo/IAO_0000115"/>
        <owl:annotatedTarget>A layer that flattens the input</owl:annotatedTarget>
        <oboInOwl:hasDbXref rdf:resource="https://www.tensorflow.org/api_docs/python/tf/keras/layers/Flatten"/>
    </owl:Axiom>
    


    <!-- https://w3id.org/aio/FractionalMaxPool2DLayer -->

    <owl:Class rdf:about="https://w3id.org/aio/FractionalMaxPool2DLayer">
        <rdfs:subClassOf rdf:resource="https://w3id.org/aio/PoolingLayer"/>
        <obo:IAO_0000115>A pooling layer that applies a 2D fractional max pooling over an input signal composed of several input planes.</obo:IAO_0000115>
        <oboInOwl:hasExactSynonym>FractionalMaxPool2D</oboInOwl:hasExactSynonym>
        <oboInOwl:inSubset rdf:resource="https://w3id.org/aio/LayerSubset"/>
        <rdfs:label>FractionalMaxPool2D Layer</rdfs:label>
    </owl:Class>
    <owl:Axiom>
        <owl:annotatedSource rdf:resource="https://w3id.org/aio/FractionalMaxPool2DLayer"/>
        <owl:annotatedProperty rdf:resource="http://purl.obolibrary.org/obo/IAO_0000115"/>
        <owl:annotatedTarget>A pooling layer that applies a 2D fractional max pooling over an input signal composed of several input planes.</owl:annotatedTarget>
        <oboInOwl:hasDbXref rdf:resource="https://pytorch.org/docs/stable/nn.html#pooling-layers"/>
    </owl:Axiom>
    


    <!-- https://w3id.org/aio/FractionalMaxPool3DLayer -->

    <owl:Class rdf:about="https://w3id.org/aio/FractionalMaxPool3DLayer">
        <rdfs:subClassOf rdf:resource="https://w3id.org/aio/PoolingLayer"/>
        <obo:IAO_0000115>A pooling layer that applies a 3D fractional max pooling over an input signal composed of several input planes.</obo:IAO_0000115>
        <oboInOwl:hasExactSynonym>FractionalMaxPool3D</oboInOwl:hasExactSynonym>
        <oboInOwl:inSubset rdf:resource="https://w3id.org/aio/LayerSubset"/>
        <rdfs:label>FractionalMaxPool3D Layer</rdfs:label>
    </owl:Class>
    <owl:Axiom>
        <owl:annotatedSource rdf:resource="https://w3id.org/aio/FractionalMaxPool3DLayer"/>
        <owl:annotatedProperty rdf:resource="http://purl.obolibrary.org/obo/IAO_0000115"/>
        <owl:annotatedTarget>A pooling layer that applies a 3D fractional max pooling over an input signal composed of several input planes.</owl:annotatedTarget>
        <oboInOwl:hasDbXref rdf:resource="https://pytorch.org/docs/stable/nn.html#pooling-layers"/>
    </owl:Axiom>
    


    <!-- https://w3id.org/aio/Function -->

    <owl:Class rdf:about="https://w3id.org/aio/Function">
        <rdfs:subClassOf rdf:resource="http://www.w3.org/2002/07/owl#Thing"/>
        <obo:IAO_0000115>A mathematical rule that gives the value of a dependent variable corresponding to specified values of independent variables.</obo:IAO_0000115>
        <oboInOwl:inSubset rdf:resource="https://w3id.org/aio/ClassSubset"/>
        <rdfs:label>Function</rdfs:label>
    </owl:Class>
    <owl:Axiom>
        <owl:annotatedSource rdf:resource="https://w3id.org/aio/Function"/>
        <owl:annotatedProperty rdf:resource="http://purl.obolibrary.org/obo/IAO_0000115"/>
        <owl:annotatedTarget>A mathematical rule that gives the value of a dependent variable corresponding to specified values of independent variables.</owl:annotatedTarget>
        <oboInOwl:hasDbXref rdf:resource="https://www.sciencedirect.com/topics/mathematics/mathematical-function"/>
    </owl:Axiom>
    


    <!-- https://w3id.org/aio/FundingBias -->

    <owl:Class rdf:about="https://w3id.org/aio/FundingBias">
        <rdfs:subClassOf rdf:resource="https://w3id.org/aio/GroupBias"/>
        <obo:IAO_0000115>A bias arising when biased results are reported to support or satisfy the funding agency or financial supporter of a research study.</obo:IAO_0000115>
        <oboInOwl:inSubset rdf:resource="https://w3id.org/aio/BiasSubset"/>
        <rdfs:label>Funding Bias</rdfs:label>
    </owl:Class>
    <owl:Axiom>
        <owl:annotatedSource rdf:resource="https://w3id.org/aio/FundingBias"/>
        <owl:annotatedProperty rdf:resource="http://purl.obolibrary.org/obo/IAO_0000115"/>
        <owl:annotatedTarget>A bias arising when biased results are reported to support or satisfy the funding agency or financial supporter of a research study.</owl:annotatedTarget>
        <oboInOwl:hasDbXref rdf:resource="https://doi.org/10.6028/NIST.SP.1270"/>
    </owl:Axiom>
    


    <!-- https://w3id.org/aio/GELUFunction -->

    <owl:Class rdf:about="https://w3id.org/aio/GELUFunction">
        <rdfs:subClassOf rdf:resource="https://w3id.org/aio/Function"/>
        <obo:IAO_0000115>An activation function that computes x * P(X &lt;= x) where P(X) ~ N(0 1) weighting inputs by their value rather than gating inputs by their sign as in ReLU.</obo:IAO_0000115>
        <oboInOwl:hasExactSynonym>GELU</oboInOwl:hasExactSynonym>
        <oboInOwl:hasExactSynonym>Gaussian Error Linear Unit</oboInOwl:hasExactSynonym>
        <oboInOwl:inSubset rdf:resource="https://w3id.org/aio/FunctionSubset"/>
        <rdfs:comment>Gaussian error linear unit (GELU) computes x * P(X &lt;= x), where P(X) ~ N(0, 1). The (GELU) nonlinearity weights inputs by their value, rather than gates inputs by their sign as in ReLU.</rdfs:comment>
        <rdfs:label>GELU Function</rdfs:label>
    </owl:Class>
    <owl:Axiom>
        <owl:annotatedSource rdf:resource="https://w3id.org/aio/GELUFunction"/>
        <owl:annotatedProperty rdf:resource="http://purl.obolibrary.org/obo/IAO_0000115"/>
        <owl:annotatedTarget>An activation function that computes x * P(X &lt;= x) where P(X) ~ N(0 1) weighting inputs by their value rather than gating inputs by their sign as in ReLU.</owl:annotatedTarget>
        <oboInOwl:hasDbXref rdf:resource="https://www.tensorflow.org/api_docs/python/tf/keras/activations/gelu"/>
    </owl:Axiom>
    


    <!-- https://w3id.org/aio/GRUCellLayer -->

    <owl:Class rdf:about="https://w3id.org/aio/GRUCellLayer">
        <rdfs:subClassOf rdf:resource="https://w3id.org/aio/Layer"/>
        <obo:IAO_0000115>A layer that processes one step within the whole time sequence input for a GRU layer.</obo:IAO_0000115>
        <oboInOwl:inSubset rdf:resource="https://w3id.org/aio/LayerSubset"/>
        <rdfs:comment>Cell class for the GRU layer. This class processes one step within the whole time sequence input, whereas tf.keras.layer.GRU processes the whole sequence.</rdfs:comment>
        <rdfs:label>GRUCell Layer</rdfs:label>
    </owl:Class>
    <owl:Axiom>
        <owl:annotatedSource rdf:resource="https://w3id.org/aio/GRUCellLayer"/>
        <owl:annotatedProperty rdf:resource="http://purl.obolibrary.org/obo/IAO_0000115"/>
        <owl:annotatedTarget>A layer that processes one step within the whole time sequence input for a GRU layer.</owl:annotatedTarget>
        <oboInOwl:hasDbXref rdf:resource="https://www.tensorflow.org/api_docs/python/tf/keras/layers/GRUCell"/>
    </owl:Axiom>
    


    <!-- https://w3id.org/aio/GRULayer -->

    <owl:Class rdf:about="https://w3id.org/aio/GRULayer">
        <rdfs:subClassOf rdf:resource="https://w3id.org/aio/RecurrentLayer"/>
        <obo:IAO_0000115>A recurrent layer that implements the Gated Recurrent Unit architecture.</obo:IAO_0000115>
        <oboInOwl:inSubset rdf:resource="https://w3id.org/aio/LayerSubset"/>
        <rdfs:comment>Gated Recurrent Unit - Cho et al. 2014. Based on available runtime hardware and constraints, this layer will choose different implementations (cuDNN-based or pure-TensorFlow) to maximize the performance. If a GPU is available and all the arguments to the layer meet the requirement of the cuDNN kernel (see below for details), the layer will use a fast cuDNN implementation. The requirements to use the cuDNN implementation are: activation == tanh, recurrent_activation == sigmoid, recurrent_dropout == 0, unroll is False, use_bias is True, reset_after is True. Inputs, if use masking, are strictly right-padded. Eager execution is enabled in the outermost context. There are two variants of the GRU implementation. The default one is based on v3 and has reset gate applied to hidden state before matrix multiplication. The other one is based on original and has the order reversed. The second variant is compatible with CuDNNGRU (GPU-only) and allows inference on CPU. Thus it has separate biases for kernel and recurrent_kernel. To use this variant, set reset_after=True and recurrent_activation=&apos;sigmoid&apos;.</rdfs:comment>
        <rdfs:label>GRU Layer</rdfs:label>
    </owl:Class>
    <owl:Axiom>
        <owl:annotatedSource rdf:resource="https://w3id.org/aio/GRULayer"/>
        <owl:annotatedProperty rdf:resource="http://purl.obolibrary.org/obo/IAO_0000115"/>
        <owl:annotatedTarget>A recurrent layer that implements the Gated Recurrent Unit architecture.</owl:annotatedTarget>
        <oboInOwl:hasDbXref rdf:resource="https://www.tensorflow.org/api_docs/python/tf/keras/layers/GRU"/>
    </owl:Axiom>
    


    <!-- https://w3id.org/aio/GatedRecurrentUnit -->

    <owl:Class rdf:about="https://w3id.org/aio/GatedRecurrentUnit">
        <rdfs:subClassOf rdf:resource="https://w3id.org/aio/LongShortTermMemory"/>
        <obo:IAO_0000115>A long short-term memory network that is a gating mechanism in recurrent neural networks similar to LSTMs but with fewer parameters and no output gate.</obo:IAO_0000115>
        <oboInOwl:hasExactSynonym>GRU</oboInOwl:hasExactSynonym>
        <oboInOwl:inSubset rdf:resource="https://w3id.org/aio/NetworkSubset"/>
        <rdfs:comment>Layers: Input, Memory Cell, Output</rdfs:comment>
        <rdfs:label>Gated Recurrent Unit</rdfs:label>
    </owl:Class>
    <owl:Axiom>
        <owl:annotatedSource rdf:resource="https://w3id.org/aio/GatedRecurrentUnit"/>
        <owl:annotatedProperty rdf:resource="http://purl.obolibrary.org/obo/IAO_0000115"/>
        <owl:annotatedTarget>A long short-term memory network that is a gating mechanism in recurrent neural networks similar to LSTMs but with fewer parameters and no output gate.</owl:annotatedTarget>
        <oboInOwl:hasDbXref rdf:resource="https://en.wikipedia.org/wiki/Gated_recurrent_unit"/>
    </owl:Axiom>
    


    <!-- https://w3id.org/aio/GaussianDropoutLayer -->

    <owl:Class rdf:about="https://w3id.org/aio/GaussianDropoutLayer">
        <rdfs:subClassOf rdf:resource="https://w3id.org/aio/RegularizationLayer"/>
        <obo:IAO_0000115>A regularization layer that applies multiplicative 1-centered Gaussian noise.</obo:IAO_0000115>
        <oboInOwl:inSubset rdf:resource="https://w3id.org/aio/LayerSubset"/>
        <rdfs:comment>Apply multiplicative 1-centered Gaussian noise. As it is a regularization layer, it is only active at training time.</rdfs:comment>
        <rdfs:label>GaussianDropout Layer</rdfs:label>
    </owl:Class>
    <owl:Axiom>
        <owl:annotatedSource rdf:resource="https://w3id.org/aio/GaussianDropoutLayer"/>
        <owl:annotatedProperty rdf:resource="http://purl.obolibrary.org/obo/IAO_0000115"/>
        <owl:annotatedTarget>A regularization layer that applies multiplicative 1-centered Gaussian noise.</owl:annotatedTarget>
        <oboInOwl:hasDbXref rdf:resource="https://www.tensorflow.org/api_docs/python/tf/keras/layers/GaussianDropout"/>
    </owl:Axiom>
    


    <!-- https://w3id.org/aio/GaussianNoiseLayer -->

    <owl:Class rdf:about="https://w3id.org/aio/GaussianNoiseLayer">
        <rdfs:subClassOf rdf:resource="https://w3id.org/aio/RegularizationLayer"/>
        <obo:IAO_0000115>A regularization layer that applies additive zero-centered Gaussian noise.</obo:IAO_0000115>
        <oboInOwl:inSubset rdf:resource="https://w3id.org/aio/LayerSubset"/>
        <rdfs:comment>Apply additive zero-centered Gaussian noise. This is useful to mitigate overfitting (you could see it as a form of random data augmentation). Gaussian Noise (GS) is a natural choice as corruption process for real valued inputs. As it is a regularization layer, it is only active at training time.</rdfs:comment>
        <rdfs:label>GaussianNoise Layer</rdfs:label>
    </owl:Class>
    <owl:Axiom>
        <owl:annotatedSource rdf:resource="https://w3id.org/aio/GaussianNoiseLayer"/>
        <owl:annotatedProperty rdf:resource="http://purl.obolibrary.org/obo/IAO_0000115"/>
        <owl:annotatedTarget>A regularization layer that applies additive zero-centered Gaussian noise.</owl:annotatedTarget>
        <oboInOwl:hasDbXref rdf:resource="https://www.tensorflow.org/api_docs/python/tf/keras/layers/GaussianNoise"/>
    </owl:Axiom>
    


    <!-- https://w3id.org/aio/GeneralizedAutoregressiveConditionalHeteroskedasticity -->

    <owl:Class rdf:about="https://w3id.org/aio/GeneralizedAutoregressiveConditionalHeteroskedasticity">
        <rdfs:subClassOf rdf:resource="https://w3id.org/aio/Model"/>
        <obo:IAO_0000115>A model that incorporates lagged conditional variances, allowing for more flexibility in modeling time-varying volatility.</obo:IAO_0000115>
        <oboInOwl:hasExactSynonym>GARCH</oboInOwl:hasExactSynonym>
        <oboInOwl:inSubset rdf:resource="https://w3id.org/aio/ModelSubset"/>
        <rdfs:label>Generalized Autoregressive Conditional Heteroskedasticity</rdfs:label>
    </owl:Class>
    


    <!-- https://w3id.org/aio/GeneralizedFewshotLearning -->

    <owl:Class rdf:about="https://w3id.org/aio/GeneralizedFewshotLearning">
        <rdfs:subClassOf rdf:resource="https://w3id.org/aio/DeepNeuralNetwork"/>
        <obo:IAO_0000115>A deep neural network that learns novel classes from few samples per class, preventing catastrophic forgetting of base classes and ensuring classifier calibration.</obo:IAO_0000115>
        <oboInOwl:hasExactSynonym>GFSL</oboInOwl:hasExactSynonym>
        <oboInOwl:inSubset rdf:resource="https://w3id.org/aio/NetworkSubset"/>
        <rdfs:label>Generalized Few-shot Learning</rdfs:label>
    </owl:Class>
    <owl:Axiom>
        <owl:annotatedSource rdf:resource="https://w3id.org/aio/GeneralizedFewshotLearning"/>
        <owl:annotatedProperty rdf:resource="http://purl.obolibrary.org/obo/IAO_0000115"/>
        <owl:annotatedTarget>A deep neural network that learns novel classes from few samples per class, preventing catastrophic forgetting of base classes and ensuring classifier calibration.</owl:annotatedTarget>
        <oboInOwl:hasDbXref rdf:resource="https://paperswithcode.com/paper/generalized-and-incremental-few-shot-learning/review/"/>
    </owl:Axiom>
    


    <!-- https://w3id.org/aio/GeneralizedLinearModel -->

    <owl:Class rdf:about="https://w3id.org/aio/GeneralizedLinearModel">
        <rdfs:subClassOf rdf:resource="https://w3id.org/aio/RegressionAnalysis"/>
        <obo:IAO_0000115>A machine learning model that generalizes linear regression by relating the linear model to the response variable via a link function and allowing the variance of each measurement to be a function of its predicted value.</obo:IAO_0000115>
        <oboInOwl:hasExactSynonym>GLM</oboInOwl:hasExactSynonym>
        <oboInOwl:inSubset rdf:resource="https://w3id.org/aio/MachineLearningSubset"/>
        <rdfs:label>Generalized Linear Model</rdfs:label>
    </owl:Class>
    <owl:Axiom>
        <owl:annotatedSource rdf:resource="https://w3id.org/aio/GeneralizedLinearModel"/>
        <owl:annotatedProperty rdf:resource="http://purl.obolibrary.org/obo/IAO_0000115"/>
        <owl:annotatedTarget>A machine learning model that generalizes linear regression by relating the linear model to the response variable via a link function and allowing the variance of each measurement to be a function of its predicted value.</owl:annotatedTarget>
        <oboInOwl:hasDbXref rdf:resource="https://en.wikipedia.org/wiki/Generalized_linear_model"/>
    </owl:Axiom>
    


    <!-- https://w3id.org/aio/GenerativeAdversarialNetwork -->

    <owl:Class rdf:about="https://w3id.org/aio/GenerativeAdversarialNetwork">
        <rdfs:subClassOf rdf:resource="https://w3id.org/aio/UnsupervisedPretrainedNetwork"/>
        <rdfs:subClassOf>
            <owl:Restriction>
                <owl:onProperty rdf:resource="http://purl.obolibrary.org/obo/BFO_0000051"/>
                <owl:someValuesFrom rdf:resource="https://w3id.org/aio/BackfedInputLayer"/>
            </owl:Restriction>
        </rdfs:subClassOf>
        <rdfs:subClassOf>
            <owl:Restriction>
                <owl:onProperty rdf:resource="http://purl.obolibrary.org/obo/BFO_0000051"/>
                <owl:someValuesFrom rdf:resource="https://w3id.org/aio/HiddenLayer"/>
            </owl:Restriction>
        </rdfs:subClassOf>
        <rdfs:subClassOf>
            <owl:Restriction>
                <owl:onProperty rdf:resource="http://purl.obolibrary.org/obo/BFO_0000051"/>
                <owl:someValuesFrom rdf:resource="https://w3id.org/aio/MatchedInputOutputLayer"/>
            </owl:Restriction>
        </rdfs:subClassOf>
        <obo:IAO_0000115>An unsupervised pretrained network framework where two neural networks contest in a game to generate new data with the same statistics as the training set.</obo:IAO_0000115>
        <oboInOwl:hasExactSynonym>GAN</oboInOwl:hasExactSynonym>
        <oboInOwl:inSubset rdf:resource="https://w3id.org/aio/NetworkSubset"/>
        <rdfs:comment>Layers: Backfed Input, Hidden, Matched Output-Input, Hidden, Matched Output-Input</rdfs:comment>
        <rdfs:label>Generative Adversarial Network</rdfs:label>
    </owl:Class>
    <owl:Axiom>
        <owl:annotatedSource rdf:resource="https://w3id.org/aio/GenerativeAdversarialNetwork"/>
        <owl:annotatedProperty rdf:resource="http://purl.obolibrary.org/obo/IAO_0000115"/>
        <owl:annotatedTarget>An unsupervised pretrained network framework where two neural networks contest in a game to generate new data with the same statistics as the training set.</owl:annotatedTarget>
        <oboInOwl:hasDbXref rdf:resource="https://en.wikipedia.org/wiki/Generative_adversarial_network"/>
    </owl:Axiom>
    


    <!-- https://w3id.org/aio/GenerativeAdversarialNetworkAugmentedLLM -->

    <owl:Class rdf:about="https://w3id.org/aio/GenerativeAdversarialNetworkAugmentedLLM">
        <rdfs:subClassOf rdf:resource="https://w3id.org/aio/LargeLanguageModel"/>
        <obo:IAO_0000115>A LLM which incorporates a generative adversarial network (GAN) into its training process, using a discriminator network to provide a signal for generating more realistic and coherent text. This adversarial training can improve the quality and diversity of generated text.</obo:IAO_0000115>
        <oboInOwl:hasExactSynonym>GAN-Large Language Model</oboInOwl:hasExactSynonym>
        <oboInOwl:hasExactSynonym>Generative Adversarial Network-Augmented Large Language Model</oboInOwl:hasExactSynonym>
        <oboInOwl:hasRelatedSynonym>adversarial training</oboInOwl:hasRelatedSynonym>
        <oboInOwl:hasRelatedSynonym>text generation</oboInOwl:hasRelatedSynonym>
        <oboInOwl:inSubset rdf:resource="https://w3id.org/aio/ModelSubset"/>
        <rdfs:label>Generative Adversarial Network-Augmented LLM</rdfs:label>
    </owl:Class>
    


    <!-- https://w3id.org/aio/GenerativeCommonsenseLLM -->

    <owl:Class rdf:about="https://w3id.org/aio/GenerativeCommonsenseLLM">
        <rdfs:subClassOf rdf:resource="https://w3id.org/aio/LargeLanguageModel"/>
        <obo:IAO_0000115>A large language model that is trained to understand and model basic physics causality and common sense about how the real world works.</obo:IAO_0000115>
        <oboInOwl:hasExactSynonym>Generative Commonsense Large Language Model</oboInOwl:hasExactSynonym>
        <oboInOwl:hasExactSynonym>World Model</oboInOwl:hasExactSynonym>
        <oboInOwl:hasRelatedSynonym>causal modeling</oboInOwl:hasRelatedSynonym>
        <oboInOwl:hasRelatedSynonym>physical reasoning</oboInOwl:hasRelatedSynonym>
        <oboInOwl:inSubset rdf:resource="https://w3id.org/aio/ModelSubset"/>
        <rdfs:label>Generative Commonsense LLM</rdfs:label>
    </owl:Class>
    <owl:Axiom>
        <owl:annotatedSource rdf:resource="https://w3id.org/aio/GenerativeCommonsenseLLM"/>
        <owl:annotatedProperty rdf:resource="http://purl.obolibrary.org/obo/IAO_0000115"/>
        <owl:annotatedTarget>A large language model that is trained to understand and model basic physics causality and common sense about how the real world works.</owl:annotatedTarget>
        <oboInOwl:hasDbXref rdf:resource="https://arxiv.org/abs/2306.12672"/>
    </owl:Axiom>
    


    <!-- https://w3id.org/aio/GenerativeLanguageInterface -->

    <owl:Class rdf:about="https://w3id.org/aio/GenerativeLanguageInterface">
        <rdfs:subClassOf rdf:resource="https://w3id.org/aio/LanguageModel"/>
        <obo:IAO_0000115>A language model that enables users to engage in an interactive dialogue with an LLM providing feedback to guide and refine the generated outputs iteratively.</obo:IAO_0000115>
        <oboInOwl:hasRelatedSynonym>Interactive generation</oboInOwl:hasRelatedSynonym>
        <oboInOwl:inSubset rdf:resource="https://w3id.org/aio/ModelSubset"/>
        <rdfs:label>Generative Language Interface</rdfs:label>
    </owl:Class>
    


    <!-- https://w3id.org/aio/GlobalAveragePooling1DLayer -->

    <owl:Class rdf:about="https://w3id.org/aio/GlobalAveragePooling1DLayer">
        <rdfs:subClassOf rdf:resource="https://w3id.org/aio/PoolingLayer"/>
        <obo:IAO_0000115>A pooling layer that performs global average pooling operation for temporal data.</obo:IAO_0000115>
        <oboInOwl:hasExactSynonym>GlobalAvgPool1D</oboInOwl:hasExactSynonym>
        <oboInOwl:inSubset rdf:resource="https://w3id.org/aio/LayerSubset"/>
        <rdfs:comment>Global average pooling operation for temporal data.</rdfs:comment>
        <rdfs:label>GlobalAveragePooling1D Layer</rdfs:label>
    </owl:Class>
    <owl:Axiom>
        <owl:annotatedSource rdf:resource="https://w3id.org/aio/GlobalAveragePooling1DLayer"/>
        <owl:annotatedProperty rdf:resource="http://purl.obolibrary.org/obo/IAO_0000115"/>
        <owl:annotatedTarget>A pooling layer that performs global average pooling operation for temporal data.</owl:annotatedTarget>
        <oboInOwl:hasDbXref rdf:resource="https://www.tensorflow.org/api_docs/python/tf/keras/layers/GlobalAveragePooling1D"/>
    </owl:Axiom>
    


    <!-- https://w3id.org/aio/GlobalAveragePooling2DLayer -->

    <owl:Class rdf:about="https://w3id.org/aio/GlobalAveragePooling2DLayer">
        <rdfs:subClassOf rdf:resource="https://w3id.org/aio/PoolingLayer"/>
        <obo:IAO_0000115>A pooling layer that performs global average pooling operation for spatial data.</obo:IAO_0000115>
        <oboInOwl:hasExactSynonym>GlobalAvgPool2D</oboInOwl:hasExactSynonym>
        <oboInOwl:inSubset rdf:resource="https://w3id.org/aio/LayerSubset"/>
        <rdfs:comment>Global average pooling operation for spatial data.</rdfs:comment>
        <rdfs:label>GlobalAveragePooling2D Layer</rdfs:label>
    </owl:Class>
    <owl:Axiom>
        <owl:annotatedSource rdf:resource="https://w3id.org/aio/GlobalAveragePooling2DLayer"/>
        <owl:annotatedProperty rdf:resource="http://purl.obolibrary.org/obo/IAO_0000115"/>
        <owl:annotatedTarget>A pooling layer that performs global average pooling operation for spatial data.</owl:annotatedTarget>
        <oboInOwl:hasDbXref rdf:resource="https://www.tensorflow.org/api_docs/python/tf/keras/layers/GlobalAveragePooling2D"/>
    </owl:Axiom>
    


    <!-- https://w3id.org/aio/GlobalAveragePooling3DLayer -->

    <owl:Class rdf:about="https://w3id.org/aio/GlobalAveragePooling3DLayer">
        <rdfs:subClassOf rdf:resource="https://w3id.org/aio/PoolingLayer"/>
        <obo:IAO_0000115>A pooling layer that performs global average pooling operation for 3D data.</obo:IAO_0000115>
        <oboInOwl:hasExactSynonym>GlobalAvgPool3D</oboInOwl:hasExactSynonym>
        <oboInOwl:inSubset rdf:resource="https://w3id.org/aio/LayerSubset"/>
        <rdfs:comment>Global Average pooling operation for 3D data.</rdfs:comment>
        <rdfs:label>GlobalAveragePooling3D Layer</rdfs:label>
    </owl:Class>
    <owl:Axiom>
        <owl:annotatedSource rdf:resource="https://w3id.org/aio/GlobalAveragePooling3DLayer"/>
        <owl:annotatedProperty rdf:resource="http://purl.obolibrary.org/obo/IAO_0000115"/>
        <owl:annotatedTarget>A pooling layer that performs global average pooling operation for 3D data.</owl:annotatedTarget>
        <oboInOwl:hasDbXref rdf:resource="https://www.tensorflow.org/api_docs/python/tf/keras/layers/GlobalAveragePooling3D"/>
    </owl:Axiom>
    


    <!-- https://w3id.org/aio/GlobalMaxPooling1DLayer -->

    <owl:Class rdf:about="https://w3id.org/aio/GlobalMaxPooling1DLayer">
        <rdfs:subClassOf rdf:resource="https://w3id.org/aio/PoolingLayer"/>
        <obo:IAO_0000115>A pooling layer that performs global max pooling operation for temporal data.</obo:IAO_0000115>
        <oboInOwl:hasExactSynonym>GlobalMaxPool1D</oboInOwl:hasExactSynonym>
        <oboInOwl:inSubset rdf:resource="https://w3id.org/aio/LayerSubset"/>
        <rdfs:comment>Global max pooling operation for 1D temporal data.</rdfs:comment>
        <rdfs:label>GlobalMaxPooling1D Layer</rdfs:label>
    </owl:Class>
    <owl:Axiom>
        <owl:annotatedSource rdf:resource="https://w3id.org/aio/GlobalMaxPooling1DLayer"/>
        <owl:annotatedProperty rdf:resource="http://purl.obolibrary.org/obo/IAO_0000115"/>
        <owl:annotatedTarget>A pooling layer that performs global max pooling operation for temporal data.</owl:annotatedTarget>
        <oboInOwl:hasDbXref rdf:resource="https://www.tensorflow.org/api_docs/python/tf/keras/layers/GlobalMaxPool1D"/>
    </owl:Axiom>
    


    <!-- https://w3id.org/aio/GlobalMaxPooling2DLayer -->

    <owl:Class rdf:about="https://w3id.org/aio/GlobalMaxPooling2DLayer">
        <rdfs:subClassOf rdf:resource="https://w3id.org/aio/PoolingLayer"/>
        <obo:IAO_0000115>A pooling layer that performs global max pooling operation for spatial data.</obo:IAO_0000115>
        <oboInOwl:hasExactSynonym>GlobalMaxPool2D</oboInOwl:hasExactSynonym>
        <oboInOwl:inSubset rdf:resource="https://w3id.org/aio/LayerSubset"/>
        <rdfs:comment>Global max pooling operation for spatial data.</rdfs:comment>
        <rdfs:label>GlobalMaxPooling2D Layer</rdfs:label>
    </owl:Class>
    <owl:Axiom>
        <owl:annotatedSource rdf:resource="https://w3id.org/aio/GlobalMaxPooling2DLayer"/>
        <owl:annotatedProperty rdf:resource="http://purl.obolibrary.org/obo/IAO_0000115"/>
        <owl:annotatedTarget>A pooling layer that performs global max pooling operation for spatial data.</owl:annotatedTarget>
        <oboInOwl:hasDbXref rdf:resource="https://www.tensorflow.org/api_docs/python/tf/keras/layers/GlobalMaxPool2D"/>
    </owl:Axiom>
    


    <!-- https://w3id.org/aio/GlobalMaxPooling3DLayer -->

    <owl:Class rdf:about="https://w3id.org/aio/GlobalMaxPooling3DLayer">
        <rdfs:subClassOf rdf:resource="https://w3id.org/aio/PoolingLayer"/>
        <obo:IAO_0000115>A pooling layer that performs global max pooling operation for 3D data.</obo:IAO_0000115>
        <oboInOwl:hasExactSynonym>GlobalMaxPool3D</oboInOwl:hasExactSynonym>
        <oboInOwl:inSubset rdf:resource="https://w3id.org/aio/LayerSubset"/>
        <rdfs:comment>Global Max pooling operation for 3D data.</rdfs:comment>
        <rdfs:label>GlobalMaxPooling3D Layer</rdfs:label>
    </owl:Class>
    <owl:Axiom>
        <owl:annotatedSource rdf:resource="https://w3id.org/aio/GlobalMaxPooling3DLayer"/>
        <owl:annotatedProperty rdf:resource="http://purl.obolibrary.org/obo/IAO_0000115"/>
        <owl:annotatedTarget>A pooling layer that performs global max pooling operation for 3D data.</owl:annotatedTarget>
        <oboInOwl:hasDbXref rdf:resource="https://www.tensorflow.org/api_docs/python/tf/keras/layers/GlobalMaxPool3D"/>
    </owl:Axiom>
    


    <!-- https://w3id.org/aio/GraphConvolutionalNetwork -->

    <owl:Class rdf:about="https://w3id.org/aio/GraphConvolutionalNetwork">
        <rdfs:subClassOf rdf:resource="https://w3id.org/aio/DeepNeuralNetwork"/>
        <rdfs:subClassOf>
            <owl:Restriction>
                <owl:onProperty rdf:resource="http://purl.obolibrary.org/obo/BFO_0000051"/>
                <owl:someValuesFrom rdf:resource="https://w3id.org/aio/HiddenLayer"/>
            </owl:Restriction>
        </rdfs:subClassOf>
        <rdfs:subClassOf>
            <owl:Restriction>
                <owl:onProperty rdf:resource="http://purl.obolibrary.org/obo/BFO_0000051"/>
                <owl:someValuesFrom rdf:resource="https://w3id.org/aio/InputLayer"/>
            </owl:Restriction>
        </rdfs:subClassOf>
        <rdfs:subClassOf>
            <owl:Restriction>
                <owl:onProperty rdf:resource="http://purl.obolibrary.org/obo/BFO_0000051"/>
                <owl:someValuesFrom rdf:resource="https://w3id.org/aio/OutputLayer"/>
            </owl:Restriction>
        </rdfs:subClassOf>
        <obo:IAO_0000115>A deep neural network that operates directly on graph structures utilizing structural information.</obo:IAO_0000115>
        <oboInOwl:hasExactSynonym>GCN</oboInOwl:hasExactSynonym>
        <oboInOwl:inSubset rdf:resource="https://w3id.org/aio/NetworkSubset"/>
        <rdfs:comment>Layers: Input, Hidden, Hidden, Output</rdfs:comment>
        <rdfs:label>Graph Convolutional Network</rdfs:label>
    </owl:Class>
    <owl:Axiom>
        <owl:annotatedSource rdf:resource="https://w3id.org/aio/GraphConvolutionalNetwork"/>
        <owl:annotatedProperty rdf:resource="http://purl.obolibrary.org/obo/IAO_0000115"/>
        <owl:annotatedTarget>A deep neural network that operates directly on graph structures utilizing structural information.</owl:annotatedTarget>
        <oboInOwl:hasDbXref rdf:resource="https://arxiv.org/abs/1609.02907"/>
    </owl:Axiom>
    


    <!-- https://w3id.org/aio/GraphConvolutionalPolicyNetwork -->

    <owl:Class rdf:about="https://w3id.org/aio/GraphConvolutionalPolicyNetwork">
        <rdfs:subClassOf rdf:resource="https://w3id.org/aio/GraphConvolutionalNetwork"/>
        <rdfs:subClassOf>
            <owl:Restriction>
                <owl:onProperty rdf:resource="http://purl.obolibrary.org/obo/BFO_0000051"/>
                <owl:someValuesFrom rdf:resource="https://w3id.org/aio/PolicyLayer"/>
            </owl:Restriction>
        </rdfs:subClassOf>
        <obo:IAO_0000115>A graph convolutional network that generates goal-directed graphs using reinforcement learning and optimizing for rewards and adversarial loss.</obo:IAO_0000115>
        <oboInOwl:hasExactSynonym>GPCN</oboInOwl:hasExactSynonym>
        <oboInOwl:inSubset rdf:resource="https://w3id.org/aio/NetworkSubset"/>
        <rdfs:comment>Layers: Input, Hidden, Hidden, Policy, Output</rdfs:comment>
        <rdfs:label>Graph Convolutional Policy Network</rdfs:label>
    </owl:Class>
    <owl:Axiom>
        <owl:annotatedSource rdf:resource="https://w3id.org/aio/GraphConvolutionalPolicyNetwork"/>
        <owl:annotatedProperty rdf:resource="http://purl.obolibrary.org/obo/IAO_0000115"/>
        <owl:annotatedTarget>A graph convolutional network that generates goal-directed graphs using reinforcement learning and optimizing for rewards and adversarial loss.</owl:annotatedTarget>
        <oboInOwl:hasDbXref rdf:resource="https://arxiv.org/abs/1806.02473"/>
    </owl:Axiom>
    


    <!-- https://w3id.org/aio/GraphLanguageModel -->

    <owl:Class rdf:about="https://w3id.org/aio/GraphLanguageModel">
        <rdfs:subClassOf rdf:resource="https://w3id.org/aio/LanguageModel"/>
        <obo:IAO_0000115>A language model that operates over structured inputs or outputs represented as graphs enabling reasoning over explicit relational knowledge representations during language tasks.</obo:IAO_0000115>
        <oboInOwl:hasExactSynonym>Graph LM</oboInOwl:hasExactSynonym>
        <oboInOwl:hasRelatedSynonym>Structured representations</oboInOwl:hasRelatedSynonym>
        <oboInOwl:inSubset rdf:resource="https://w3id.org/aio/ModelSubset"/>
        <rdfs:label>Graph Language Model</rdfs:label>
    </owl:Class>
    <owl:Axiom>
        <owl:annotatedSource rdf:resource="https://w3id.org/aio/GraphLanguageModel"/>
        <owl:annotatedProperty rdf:resource="http://purl.obolibrary.org/obo/IAO_0000115"/>
        <owl:annotatedTarget>A language model that operates over structured inputs or outputs represented as graphs enabling reasoning over explicit relational knowledge representations during language tasks.</owl:annotatedTarget>
        <oboInOwl:hasDbXref rdf:resource="https://arxiv.org/abs/2401.07105"/>
    </owl:Axiom>
    


    <!-- https://w3id.org/aio/GroupBias -->

    <owl:Class rdf:about="https://w3id.org/aio/GroupBias">
        <rdfs:subClassOf rdf:resource="https://w3id.org/aio/HumanBias"/>
        <obo:IAO_0000115>A bias characterized by favoring members of one&apos;s in-group over out-group members expressed in evaluation resource allocation and other ways.</obo:IAO_0000115>
        <oboInOwl:hasExactSynonym>In-group Favoritism</oboInOwl:hasExactSynonym>
        <oboInOwl:hasExactSynonym>In-group bias</oboInOwl:hasExactSynonym>
        <oboInOwl:hasExactSynonym>In-group preference</oboInOwl:hasExactSynonym>
        <oboInOwl:hasExactSynonym>In-group–out-group Bias</oboInOwl:hasExactSynonym>
        <oboInOwl:hasExactSynonym>Intergroup bias</oboInOwl:hasExactSynonym>
        <oboInOwl:inSubset rdf:resource="https://w3id.org/aio/BiasSubset"/>
        <rdfs:comment>Favoring members of one&apos;s in-group over out-group members, expressed in evaluation, resource allocation, and other ways.</rdfs:comment>
        <rdfs:label>Group Bias</rdfs:label>
    </owl:Class>
    <owl:Axiom>
        <owl:annotatedSource rdf:resource="https://w3id.org/aio/GroupBias"/>
        <owl:annotatedProperty rdf:resource="http://purl.obolibrary.org/obo/IAO_0000115"/>
        <owl:annotatedTarget>A bias characterized by favoring members of one&apos;s in-group over out-group members expressed in evaluation resource allocation and other ways.</owl:annotatedTarget>
        <oboInOwl:hasDbXref rdf:resource="https://en.wikipedia.org/wiki/In-group_favoritism"/>
    </owl:Axiom>
    


    <!-- https://w3id.org/aio/GroupNormLayer -->

    <owl:Class rdf:about="https://w3id.org/aio/GroupNormLayer">
        <rdfs:subClassOf rdf:resource="https://w3id.org/aio/NormalizationLayer"/>
        <obo:IAO_0000115>A normalization layer that applies Group Normalization over a mini-batch of inputs.</obo:IAO_0000115>
        <oboInOwl:hasExactSynonym>GroupNorm</oboInOwl:hasExactSynonym>
        <oboInOwl:inSubset rdf:resource="https://w3id.org/aio/LayerSubset"/>
        <rdfs:comment>Applies Group Normalization over a mini-batch of inputs as described in the paper Group Normalization</rdfs:comment>
        <rdfs:label>GroupNorm Layer</rdfs:label>
    </owl:Class>
    <owl:Axiom>
        <owl:annotatedSource rdf:resource="https://w3id.org/aio/GroupNormLayer"/>
        <owl:annotatedProperty rdf:resource="http://purl.obolibrary.org/obo/IAO_0000115"/>
        <owl:annotatedTarget>A normalization layer that applies Group Normalization over a mini-batch of inputs.</owl:annotatedTarget>
        <oboInOwl:hasDbXref rdf:resource="https://pytorch.org/docs/stable/nn.html#normalization-layers"/>
    </owl:Axiom>
    


    <!-- https://w3id.org/aio/GroupthinkBias -->

    <owl:Class rdf:about="https://w3id.org/aio/GroupthinkBias">
        <rdfs:subClassOf rdf:resource="https://w3id.org/aio/GroupBias"/>
        <obo:IAO_0000115>A psychological phenomenon where people in a group make non-optimal decisions due to a desire to conform or fear of dissent.</obo:IAO_0000115>
        <oboInOwl:hasExactSynonym>Groupthink</oboInOwl:hasExactSynonym>
        <oboInOwl:inSubset rdf:resource="https://w3id.org/aio/BiasSubset"/>
        <rdfs:label>Groupthink Bias</rdfs:label>
    </owl:Class>
    <owl:Axiom>
        <owl:annotatedSource rdf:resource="https://w3id.org/aio/GroupthinkBias"/>
        <owl:annotatedProperty rdf:resource="http://purl.obolibrary.org/obo/IAO_0000115"/>
        <owl:annotatedTarget>A psychological phenomenon where people in a group make non-optimal decisions due to a desire to conform or fear of dissent.</owl:annotatedTarget>
        <oboInOwl:hasDbXref rdf:resource="https://doi.org/10.6028/NIST.SP.1270"/>
    </owl:Axiom>
    


    <!-- https://w3id.org/aio/HardSigmoidFunction -->

    <owl:Class rdf:about="https://w3id.org/aio/HardSigmoidFunction">
        <rdfs:subClassOf rdf:resource="https://w3id.org/aio/Function"/>
        <obo:IAO_0000115>An activation function that is a faster approximation of the sigmoid activation using a piecewise linear approximation.</obo:IAO_0000115>
        <oboInOwl:inSubset rdf:resource="https://w3id.org/aio/FunctionSubset"/>
        <rdfs:comment>A faster approximation of the sigmoid activation. Piecewise linear approximation of the sigmoid function. Ref: &apos;https://en.wikipedia.org/wiki/Hard_sigmoid&apos;</rdfs:comment>
        <rdfs:label>Hard Sigmoid Function</rdfs:label>
    </owl:Class>
    <owl:Axiom>
        <owl:annotatedSource rdf:resource="https://w3id.org/aio/HardSigmoidFunction"/>
        <owl:annotatedProperty rdf:resource="http://purl.obolibrary.org/obo/IAO_0000115"/>
        <owl:annotatedTarget>An activation function that is a faster approximation of the sigmoid activation using a piecewise linear approximation.</owl:annotatedTarget>
        <oboInOwl:hasDbXref rdf:resource="https://www.tensorflow.org/api_docs/python/tf/keras/activations/hard_sigmoid"/>
    </owl:Axiom>
    


    <!-- https://w3id.org/aio/HashingLayer -->

    <owl:Class rdf:about="https://w3id.org/aio/HashingLayer">
        <rdfs:subClassOf rdf:resource="https://w3id.org/aio/CategoricalFeaturesPreprocessingLayer"/>
        <obo:IAO_0000115>A categorical features preprocessing layer which hashes and bins categorical features.</obo:IAO_0000115>
        <oboInOwl:inSubset rdf:resource="https://w3id.org/aio/LayerSubset"/>
        <rdfs:comment>A preprocessing layer which hashes and bins categorical features. This layer transforms categorical inputs to hashed output. It element-wise converts a ints or strings to ints in a fixed range. The stable hash function uses tensorflow::ops::Fingerprint to produce the same output consistently across all platforms. This layer uses FarmHash64 by default, which provides a consistent hashed output across different platforms and is stable across invocations, regardless of device and context, by mixing the input bits thoroughly. If you want to obfuscate the hashed output, you can also pass a random salt argument in the constructor. In that case, the layer will use the SipHash64 hash function, with the salt value serving as additional input to the hash function.</rdfs:comment>
        <rdfs:label>Hashing Layer</rdfs:label>
    </owl:Class>
    <owl:Axiom>
        <owl:annotatedSource rdf:resource="https://w3id.org/aio/HashingLayer"/>
        <owl:annotatedProperty rdf:resource="http://purl.obolibrary.org/obo/IAO_0000115"/>
        <owl:annotatedTarget>A categorical features preprocessing layer which hashes and bins categorical features.</owl:annotatedTarget>
        <oboInOwl:hasDbXref rdf:resource="https://www.tensorflow.org/api_docs/python/tf/keras/layers/Hashing"/>
    </owl:Axiom>
    


    <!-- https://w3id.org/aio/HiddenLayer -->

    <owl:Class rdf:about="https://w3id.org/aio/HiddenLayer">
        <rdfs:subClassOf rdf:resource="https://w3id.org/aio/Layer"/>
        <obo:IAO_0000115>A layer located between the input and output that performs nonlinear transformations of the inputs entered into the network.</obo:IAO_0000115>
        <oboInOwl:inSubset rdf:resource="https://w3id.org/aio/LayerSubset"/>
        <rdfs:comment>A hidden layer is located between the input and output of the algorithm, in which the function applies weights to the inputs and directs them through an activation function as the output. In short, the hidden layers perform nonlinear transformations of the inputs entered into the network. Hidden layers vary depending on the function of the neural network, and similarly, the layers may vary depending on their associated weights.</rdfs:comment>
        <rdfs:label>Hidden Layer</rdfs:label>
    </owl:Class>
    <owl:Axiom>
        <owl:annotatedSource rdf:resource="https://w3id.org/aio/HiddenLayer"/>
        <owl:annotatedProperty rdf:resource="http://purl.obolibrary.org/obo/IAO_0000115"/>
        <owl:annotatedTarget>A layer located between the input and output that performs nonlinear transformations of the inputs entered into the network.</owl:annotatedTarget>
        <oboInOwl:hasDbXref rdf:resource="https://deepai.org/machine-Learning-glossary-and-terms/hidden-layer-machine-Learning"/>
    </owl:Axiom>
    


    <!-- https://w3id.org/aio/HierarchicalClassification -->

    <owl:Class rdf:about="https://w3id.org/aio/HierarchicalClassification">
        <rdfs:subClassOf rdf:resource="https://w3id.org/aio/Classification"/>
        <obo:IAO_0000115>A classification task focused on methods that group things according to a hierarchy.</obo:IAO_0000115>
        <oboInOwl:inSubset rdf:resource="https://w3id.org/aio/MachineLearningSubset"/>
        <rdfs:comment>Methods that group things according to a hierarchy.</rdfs:comment>
        <rdfs:label>Hierarchical Classification</rdfs:label>
    </owl:Class>
    <owl:Axiom>
        <owl:annotatedSource rdf:resource="https://w3id.org/aio/HierarchicalClassification"/>
        <owl:annotatedProperty rdf:resource="http://purl.obolibrary.org/obo/IAO_0000115"/>
        <owl:annotatedTarget>A classification task focused on methods that group things according to a hierarchy.</owl:annotatedTarget>
        <oboInOwl:hasDbXref rdf:resource="https://en.wikipedia.org/wiki/Hierarchical_classification"/>
    </owl:Axiom>
    


    <!-- https://w3id.org/aio/HierarchicalClustering -->

    <owl:Class rdf:about="https://w3id.org/aio/HierarchicalClustering">
        <rdfs:subClassOf rdf:resource="https://w3id.org/aio/Clustering"/>
        <obo:IAO_0000115>A clustering method that builds a hierarchy of clusters.</obo:IAO_0000115>
        <oboInOwl:hasExactSynonym>HCL</oboInOwl:hasExactSynonym>
        <oboInOwl:inSubset rdf:resource="https://w3id.org/aio/MachineLearningSubset"/>
        <rdfs:comment>Methods that build a hierarchy of clusters.</rdfs:comment>
        <rdfs:label>Hierarchical Clustering</rdfs:label>
    </owl:Class>
    <owl:Axiom>
        <owl:annotatedSource rdf:resource="https://w3id.org/aio/HierarchicalClustering"/>
        <owl:annotatedProperty rdf:resource="http://purl.obolibrary.org/obo/IAO_0000115"/>
        <owl:annotatedTarget>A clustering method that builds a hierarchy of clusters.</owl:annotatedTarget>
        <oboInOwl:hasDbXref rdf:resource="https://en.wikipedia.org/wiki/Hierarchical_clustering"/>
    </owl:Axiom>
    


    <!-- https://w3id.org/aio/HierarchicalLanguageModel -->

    <owl:Class rdf:about="https://w3id.org/aio/HierarchicalLanguageModel">
        <rdfs:subClassOf rdf:resource="https://w3id.org/aio/LanguageModel"/>
        <obo:IAO_0000115>A language model that represents language at multiple levels of granularity learning hierarchical representations that capture both low-level patterns and high-level abstractions.</obo:IAO_0000115>
        <oboInOwl:hasExactSynonym>Hierarchical LM</oboInOwl:hasExactSynonym>
        <oboInOwl:hasRelatedSynonym>multi-scale representations</oboInOwl:hasRelatedSynonym>
        <oboInOwl:inSubset rdf:resource="https://w3id.org/aio/ModelSubset"/>
        <rdfs:label>Hierarchical Language Model</rdfs:label>
    </owl:Class>
    <owl:Axiom>
        <owl:annotatedSource rdf:resource="https://w3id.org/aio/HierarchicalLanguageModel"/>
        <owl:annotatedProperty rdf:resource="http://purl.obolibrary.org/obo/IAO_0000115"/>
        <owl:annotatedTarget>A language model that represents language at multiple levels of granularity learning hierarchical representations that capture both low-level patterns and high-level abstractions.</owl:annotatedTarget>
        <oboInOwl:hasDbXref rdf:resource="https://doi.org/10.1016/j.ipm.2024.103698"/>
    </owl:Axiom>
    


    <!-- https://w3id.org/aio/HistoricalBias -->

    <owl:Class rdf:about="https://w3id.org/aio/HistoricalBias">
        <rdfs:subClassOf rdf:resource="https://w3id.org/aio/Bias"/>
        <obo:IAO_0000115>A bias characterized by long-standing biases encoded in society over time distinct from biases in historical description or interpretation.</obo:IAO_0000115>
        <oboInOwl:inSubset rdf:resource="https://w3id.org/aio/BiasSubset"/>
        <rdfs:comment>Long-standing biases encoded in society over time, distinct from biases in historical description or the interpretation of history, such as viewing the larger world from a Western or European perspective.</rdfs:comment>
        <rdfs:label>Historical Bias</rdfs:label>
    </owl:Class>
    <owl:Axiom>
        <owl:annotatedSource rdf:resource="https://w3id.org/aio/HistoricalBias"/>
        <owl:annotatedProperty rdf:resource="http://purl.obolibrary.org/obo/IAO_0000115"/>
        <owl:annotatedTarget>A bias characterized by long-standing biases encoded in society over time distinct from biases in historical description or interpretation.</owl:annotatedTarget>
        <oboInOwl:hasDbXref rdf:resource="https://doi.org/10.6028/NIST.SP.1270"/>
    </owl:Axiom>
    


    <!-- https://w3id.org/aio/HopfieldNetwork -->

    <owl:Class rdf:about="https://w3id.org/aio/HopfieldNetwork">
        <rdfs:subClassOf rdf:resource="https://w3id.org/aio/SymmetricallyConnectedNetwork"/>
        <rdfs:subClassOf>
            <owl:Restriction>
                <owl:onProperty rdf:resource="http://purl.obolibrary.org/obo/BFO_0000051"/>
                <owl:someValuesFrom rdf:resource="https://w3id.org/aio/BackfedInputLayer"/>
            </owl:Restriction>
        </rdfs:subClassOf>
        <obo:IAO_0000115>A symmetrically connected network that is a type of recurrent artificial neural network serving as a content-addressable memory system.</obo:IAO_0000115>
        <oboInOwl:hasExactSynonym>HN</oboInOwl:hasExactSynonym>
        <oboInOwl:hasExactSynonym>Ising model of a neural network</oboInOwl:hasExactSynonym>
        <oboInOwl:hasExactSynonym>Ising–Lenz–Little model</oboInOwl:hasExactSynonym>
        <oboInOwl:inSubset rdf:resource="https://w3id.org/aio/NetworkSubset"/>
        <rdfs:comment>Layers: Backfed input</rdfs:comment>
        <rdfs:label>Hopfield Network</rdfs:label>
    </owl:Class>
    <owl:Axiom>
        <owl:annotatedSource rdf:resource="https://w3id.org/aio/HopfieldNetwork"/>
        <owl:annotatedProperty rdf:resource="http://purl.obolibrary.org/obo/IAO_0000115"/>
        <owl:annotatedTarget>A symmetrically connected network that is a type of recurrent artificial neural network serving as a content-addressable memory system.</owl:annotatedTarget>
        <oboInOwl:hasDbXref rdf:resource="https://en.wikipedia.org/wiki/Hopfield_network"/>
    </owl:Axiom>
    


    <!-- https://w3id.org/aio/HostileAttributionBias -->

    <owl:Class rdf:about="https://w3id.org/aio/HostileAttributionBias">
        <rdfs:subClassOf rdf:resource="https://w3id.org/aio/UseAndInterpretationBias"/>
        <obo:IAO_0000115>A use and interpretation bias where individuals perceive benign or ambiguous behaviors as hostile.</obo:IAO_0000115>
        <oboInOwl:inSubset rdf:resource="https://w3id.org/aio/BiasSubset"/>
        <rdfs:comment>Bias where individuals perceive benign or ambiguous behaviors as hostile.</rdfs:comment>
        <rdfs:label>Hostile Attribution Bias</rdfs:label>
    </owl:Class>
    <owl:Axiom>
        <owl:annotatedSource rdf:resource="https://w3id.org/aio/HostileAttributionBias"/>
        <owl:annotatedProperty rdf:resource="http://purl.obolibrary.org/obo/IAO_0000115"/>
        <owl:annotatedTarget>A use and interpretation bias where individuals perceive benign or ambiguous behaviors as hostile.</owl:annotatedTarget>
        <oboInOwl:hasDbXref rdf:resource="https://en.wikipedia.org/wiki/Interpretive_bias"/>
    </owl:Axiom>
    


    <!-- https://w3id.org/aio/HumanBias -->

    <owl:Class rdf:about="https://w3id.org/aio/HumanBias">
        <rdfs:subClassOf rdf:resource="https://w3id.org/aio/Bias"/>
        <obo:IAO_0000115>A systematic error in human thought based on heuristic principles leading to simplified judgmental operations.</obo:IAO_0000115>
        <oboInOwl:inSubset rdf:resource="https://w3id.org/aio/BiasSubset"/>
        <rdfs:label>Human Bias</rdfs:label>
    </owl:Class>
    <owl:Axiom>
        <owl:annotatedSource rdf:resource="https://w3id.org/aio/HumanBias"/>
        <owl:annotatedProperty rdf:resource="http://purl.obolibrary.org/obo/IAO_0000115"/>
        <owl:annotatedTarget>A systematic error in human thought based on heuristic principles leading to simplified judgmental operations.</owl:annotatedTarget>
        <oboInOwl:hasDbXref rdf:resource="https://doi.org/10.6028/NIST.SP.1270"/>
    </owl:Axiom>
    


    <!-- https://w3id.org/aio/HumanReportingBias -->

    <owl:Class rdf:about="https://w3id.org/aio/HumanReportingBias">
        <rdfs:subClassOf rdf:resource="https://w3id.org/aio/IndividualBias"/>
        <obo:IAO_0000115>An individual bias that arises when users depend on automated systems as heuristic substitutes for their own information-seeking and processing efforts.</obo:IAO_0000115>
        <oboInOwl:inSubset rdf:resource="https://w3id.org/aio/BiasSubset"/>
        <rdfs:label>Human Reporting Bias</rdfs:label>
    </owl:Class>
    <owl:Axiom>
        <owl:annotatedSource rdf:resource="https://w3id.org/aio/HumanReportingBias"/>
        <owl:annotatedProperty rdf:resource="http://purl.obolibrary.org/obo/IAO_0000115"/>
        <owl:annotatedTarget>An individual bias that arises when users depend on automated systems as heuristic substitutes for their own information-seeking and processing efforts.</owl:annotatedTarget>
        <oboInOwl:hasDbXref rdf:resource="https://doi.org/10.6028/NIST.SP.1270"/>
    </owl:Axiom>
    


    <!-- https://w3id.org/aio/ImageAugmentationLayer -->

    <owl:Class rdf:about="https://w3id.org/aio/ImageAugmentationLayer">
        <rdfs:subClassOf rdf:resource="https://w3id.org/aio/Layer"/>
        <obo:IAO_0000115>A layer that performs image data preprocessing augmentations.</obo:IAO_0000115>
        <oboInOwl:inSubset rdf:resource="https://w3id.org/aio/LayerSubset"/>
        <rdfs:label>Image Augmentation Layer</rdfs:label>
    </owl:Class>
    <owl:Axiom>
        <owl:annotatedSource rdf:resource="https://w3id.org/aio/ImageAugmentationLayer"/>
        <owl:annotatedProperty rdf:resource="http://purl.obolibrary.org/obo/IAO_0000115"/>
        <owl:annotatedTarget>A layer that performs image data preprocessing augmentations.</owl:annotatedTarget>
        <oboInOwl:hasDbXref rdf:resource="https://keras.io/guides/preprocessing_layers/"/>
    </owl:Axiom>
    


    <!-- https://w3id.org/aio/ImagePreprocessingLayer -->

    <owl:Class rdf:about="https://w3id.org/aio/ImagePreprocessingLayer">
        <rdfs:subClassOf rdf:resource="https://w3id.org/aio/Layer"/>
        <obo:IAO_0000115>A layer that performs image data preprocessing operations.</obo:IAO_0000115>
        <oboInOwl:inSubset rdf:resource="https://w3id.org/aio/LayerSubset"/>
        <rdfs:label>Image Preprocessing Layer</rdfs:label>
    </owl:Class>
    <owl:Axiom>
        <owl:annotatedSource rdf:resource="https://w3id.org/aio/ImagePreprocessingLayer"/>
        <owl:annotatedProperty rdf:resource="http://purl.obolibrary.org/obo/IAO_0000115"/>
        <owl:annotatedTarget>A layer that performs image data preprocessing operations.</owl:annotatedTarget>
        <oboInOwl:hasDbXref rdf:resource="https://keras.io/guides/preprocessing_layers/"/>
    </owl:Axiom>
    


    <!-- https://w3id.org/aio/ImplicitBias -->

    <owl:Class rdf:about="https://w3id.org/aio/ImplicitBias">
        <rdfs:subClassOf rdf:resource="https://w3id.org/aio/IndividualBias"/>
        <obo:IAO_0000115>An individual bias characterized by unconscious beliefs attitudes feelings associations or stereotypes that affect information processing decision-making and actions.</obo:IAO_0000115>
        <oboInOwl:hasExactSynonym>Confirmatory Bias</oboInOwl:hasExactSynonym>
        <oboInOwl:inSubset rdf:resource="https://w3id.org/aio/BiasSubset"/>
        <rdfs:comment>Unconscious beliefs, attitudes, feelings, associations, or stereotypes that affect information processing, decision-making, and actions.</rdfs:comment>
        <rdfs:label>Implicit Bias</rdfs:label>
    </owl:Class>
    <owl:Axiom>
        <owl:annotatedSource rdf:resource="https://w3id.org/aio/ImplicitBias"/>
        <owl:annotatedProperty rdf:resource="http://purl.obolibrary.org/obo/IAO_0000115"/>
        <owl:annotatedTarget>An individual bias characterized by unconscious beliefs attitudes feelings associations or stereotypes that affect information processing decision-making and actions.</owl:annotatedTarget>
        <oboInOwl:hasDbXref rdf:resource="https://doi.org/10.6028/NIST.SP.1270"/>
    </owl:Axiom>
    


    <!-- https://w3id.org/aio/ImplicitLanguageModel -->

    <owl:Class rdf:about="https://w3id.org/aio/ImplicitLanguageModel">
        <rdfs:subClassOf rdf:resource="https://w3id.org/aio/LanguageModel"/>
        <obo:IAO_0000115>A language model that uses an energy function to score entire sequences instead of factorizing probabilities autoregressively better capturing global properties and long-range dependencies.</obo:IAO_0000115>
        <oboInOwl:hasExactSynonym>Implicit LM</oboInOwl:hasExactSynonym>
        <oboInOwl:hasRelatedSynonym>Energy-based models</oboInOwl:hasRelatedSynonym>
        <oboInOwl:hasRelatedSynonym>Token-level scoring</oboInOwl:hasRelatedSynonym>
        <oboInOwl:inSubset rdf:resource="https://w3id.org/aio/ModelSubset"/>
        <rdfs:label>Implicit Language Model</rdfs:label>
    </owl:Class>
    <owl:Axiom>
        <owl:annotatedSource rdf:resource="https://w3id.org/aio/ImplicitLanguageModel"/>
        <owl:annotatedProperty rdf:resource="http://purl.obolibrary.org/obo/IAO_0000115"/>
        <owl:annotatedTarget>A language model that uses an energy function to score entire sequences instead of factorizing probabilities autoregressively better capturing global properties and long-range dependencies.</owl:annotatedTarget>
        <oboInOwl:hasDbXref rdf:resource="https://arxiv.org/pdf/2303.16189"/>
    </owl:Axiom>
    


    <!-- https://w3id.org/aio/IncremenetalFewshotLearning -->

    <owl:Class rdf:about="https://w3id.org/aio/IncremenetalFewshotLearning">
        <rdfs:subClassOf rdf:resource="https://w3id.org/aio/DeepNeuralNetwork"/>
        <obo:IAO_0000115>A deep neural network trained on a base set of classes and then presented with novel classes, each with few labeled examples.</obo:IAO_0000115>
        <oboInOwl:hasExactSynonym>IFSL</oboInOwl:hasExactSynonym>
        <oboInOwl:inSubset rdf:resource="https://w3id.org/aio/NetworkSubset"/>
        <rdfs:label>Incremenetal Few-shot Learning</rdfs:label>
    </owl:Class>
    <owl:Axiom>
        <owl:annotatedSource rdf:resource="https://w3id.org/aio/IncremenetalFewshotLearning"/>
        <owl:annotatedProperty rdf:resource="http://purl.obolibrary.org/obo/IAO_0000115"/>
        <owl:annotatedTarget>A deep neural network trained on a base set of classes and then presented with novel classes, each with few labeled examples.</owl:annotatedTarget>
        <oboInOwl:hasDbXref rdf:resource="https://arxiv.org/abs/1810.07218"/>
    </owl:Axiom>
    


    <!-- https://w3id.org/aio/IndividualBias -->

    <owl:Class rdf:about="https://w3id.org/aio/IndividualBias">
        <rdfs:subClassOf rdf:resource="https://w3id.org/aio/Bias"/>
        <obo:IAO_0000115>A persistent point of view or limited list of such points of view applied by an individual.</obo:IAO_0000115>
        <oboInOwl:inSubset rdf:resource="https://w3id.org/aio/BiasSubset"/>
        <rdfs:label>Individual Bias</rdfs:label>
    </owl:Class>
    <owl:Axiom>
        <owl:annotatedSource rdf:resource="https://w3id.org/aio/IndividualBias"/>
        <owl:annotatedProperty rdf:resource="http://purl.obolibrary.org/obo/IAO_0000115"/>
        <owl:annotatedTarget>A persistent point of view or limited list of such points of view applied by an individual.</owl:annotatedTarget>
        <oboInOwl:hasDbXref rdf:resource="https://develop.consumerium.org/wiki/Individual_bias"/>
    </owl:Axiom>
    


    <!-- https://w3id.org/aio/InheritedBias -->

    <owl:Class rdf:about="https://w3id.org/aio/InheritedBias">
        <rdfs:subClassOf rdf:resource="https://w3id.org/aio/ProcessingBias"/>
        <obo:IAO_0000115>A processing bias arising when machine learning applications generate inputs for other machine learning algorithms passing on any existing bias.</obo:IAO_0000115>
        <oboInOwl:inSubset rdf:resource="https://w3id.org/aio/BiasSubset"/>
        <rdfs:label>Inherited Bias</rdfs:label>
    </owl:Class>
    <owl:Axiom>
        <owl:annotatedSource rdf:resource="https://w3id.org/aio/InheritedBias"/>
        <owl:annotatedProperty rdf:resource="http://purl.obolibrary.org/obo/IAO_0000115"/>
        <owl:annotatedTarget>A processing bias arising when machine learning applications generate inputs for other machine learning algorithms passing on any existing bias.</owl:annotatedTarget>
        <oboInOwl:hasDbXref rdf:resource="https://doi.org/10.6028/NIST.SP.1270"/>
    </owl:Axiom>
    


    <!-- https://w3id.org/aio/InputLayer -->

    <owl:Class rdf:about="https://w3id.org/aio/InputLayer">
        <rdfs:subClassOf rdf:resource="https://w3id.org/aio/Layer"/>
        <obo:IAO_0000115>A layer composed of artificial input neurons that brings the initial data into the system for further processing by subsequent layers.</obo:IAO_0000115>
        <oboInOwl:inSubset rdf:resource="https://w3id.org/aio/LayerSubset"/>
        <rdfs:comment>The input layer of a neural network is composed of artificial input neurons, and brings the initial data into the system for further processing by subsequent layers of artificial neurons. The input layer is the very beginning of the workflow for the artificial neural network.</rdfs:comment>
        <rdfs:label>Input Layer</rdfs:label>
    </owl:Class>
    <owl:Axiom>
        <owl:annotatedSource rdf:resource="https://w3id.org/aio/InputLayer"/>
        <owl:annotatedProperty rdf:resource="http://purl.obolibrary.org/obo/IAO_0000115"/>
        <owl:annotatedTarget>A layer composed of artificial input neurons that brings the initial data into the system for further processing by subsequent layers.</owl:annotatedTarget>
        <oboInOwl:hasDbXref rdf:resource="https://www.techopedia.com/definition/33262/input-layer-neural-networks"/>
    </owl:Axiom>
    


    <!-- https://w3id.org/aio/InputLayerLayer -->

    <owl:Class rdf:about="https://w3id.org/aio/InputLayerLayer">
        <rdfs:subClassOf rdf:resource="https://w3id.org/aio/Layer"/>
        <obo:IAO_0000115>A layer to be used as an entry point into a Network (a graph of layers).</obo:IAO_0000115>
        <oboInOwl:inSubset rdf:resource="https://w3id.org/aio/LayerSubset"/>
        <rdfs:label>InputLayer Layer</rdfs:label>
    </owl:Class>
    <owl:Axiom>
        <owl:annotatedSource rdf:resource="https://w3id.org/aio/InputLayerLayer"/>
        <owl:annotatedProperty rdf:resource="http://purl.obolibrary.org/obo/IAO_0000115"/>
        <owl:annotatedTarget>A layer to be used as an entry point into a Network (a graph of layers).</owl:annotatedTarget>
        <oboInOwl:hasDbXref rdf:resource="https://www.tensorflow.org/api_docs/python/tf/keras/layers/InputLayer"/>
    </owl:Axiom>
    


    <!-- https://w3id.org/aio/InputSpecLayer -->

    <owl:Class rdf:about="https://w3id.org/aio/InputSpecLayer">
        <rdfs:subClassOf rdf:resource="https://w3id.org/aio/Layer"/>
        <obo:IAO_0000115>A layer that specifies the rank</obo:IAO_0000115>
        <oboInOwl:inSubset rdf:resource="https://w3id.org/aio/LayerSubset"/>
        <rdfs:comment>Specifies the rank, dtype and shape of every input to a layer. Layers can expose (if appropriate) an input_spec attribute: an instance of InputSpec, or a nested structure of InputSpec instances (one per input tensor). These objects enable the layer to run input compatibility checks for input structure, input rank, input shape, and input dtype. A None entry in a shape is compatible with any dimension, a None shape is compatible with any shape.</rdfs:comment>
        <rdfs:label>InputSpec Layer</rdfs:label>
    </owl:Class>
    <owl:Axiom>
        <owl:annotatedSource rdf:resource="https://w3id.org/aio/InputSpecLayer"/>
        <owl:annotatedProperty rdf:resource="http://purl.obolibrary.org/obo/IAO_0000115"/>
        <owl:annotatedTarget>A layer that specifies the rank</owl:annotatedTarget>
        <oboInOwl:hasDbXref rdf:resource="https://www.tensorflow.org/api_docs/python/tf/keras/layers/InputSpec"/>
    </owl:Axiom>
    


    <!-- https://w3id.org/aio/InstanceNorm1DLayer -->

    <owl:Class rdf:about="https://w3id.org/aio/InstanceNorm1DLayer">
        <rdfs:subClassOf rdf:resource="https://w3id.org/aio/NormalizationLayer"/>
        <obo:IAO_0000115>A normalization layer that applies Instance Normalization over a 2D (unbatched) or 3D (batched) input.</obo:IAO_0000115>
        <oboInOwl:hasExactSynonym>InstanceNorm1D</oboInOwl:hasExactSynonym>
        <oboInOwl:inSubset rdf:resource="https://w3id.org/aio/LayerSubset"/>
        <rdfs:comment>Applies Instance Normalization over a 2D (unbatched) or 3D (batched) input as described in the paper Instance Normalization: The Missing Ingredient for Fast Stylization.</rdfs:comment>
        <rdfs:label>InstanceNorm1D Layer</rdfs:label>
    </owl:Class>
    <owl:Axiom>
        <owl:annotatedSource rdf:resource="https://w3id.org/aio/InstanceNorm1DLayer"/>
        <owl:annotatedProperty rdf:resource="http://purl.obolibrary.org/obo/IAO_0000115"/>
        <owl:annotatedTarget>A normalization layer that applies Instance Normalization over a 2D (unbatched) or 3D (batched) input.</owl:annotatedTarget>
        <oboInOwl:hasDbXref rdf:resource="https://pytorch.org/docs/stable/nn.html#normalization-layers"/>
    </owl:Axiom>
    


    <!-- https://w3id.org/aio/InstanceNorm2D -->

    <owl:Class rdf:about="https://w3id.org/aio/InstanceNorm2D">
        <rdfs:subClassOf rdf:resource="https://w3id.org/aio/NormalizationLayer"/>
        <obo:IAO_0000115>A normalization layer that applies Instance Normalization over a 4D input (a mini-batch of 2D inputs with additional channel dimension).</obo:IAO_0000115>
        <oboInOwl:inSubset rdf:resource="https://w3id.org/aio/LayerSubset"/>
        <rdfs:comment>Applies Instance Normalization over a 4D input (a mini-batch of 2D inputs with additional channel dimension) as described in the paper Instance Normalization: The Missing Ingredient for Fast Stylization.</rdfs:comment>
        <rdfs:label>InstanceNorm2D</rdfs:label>
    </owl:Class>
    <owl:Axiom>
        <owl:annotatedSource rdf:resource="https://w3id.org/aio/InstanceNorm2D"/>
        <owl:annotatedProperty rdf:resource="http://purl.obolibrary.org/obo/IAO_0000115"/>
        <owl:annotatedTarget>A normalization layer that applies Instance Normalization over a 4D input (a mini-batch of 2D inputs with additional channel dimension).</owl:annotatedTarget>
        <oboInOwl:hasDbXref rdf:resource="https://pytorch.org/docs/stable/nn.html#normalization-layers"/>
    </owl:Axiom>
    


    <!-- https://w3id.org/aio/InstanceNorm3DLayer -->

    <owl:Class rdf:about="https://w3id.org/aio/InstanceNorm3DLayer">
        <rdfs:subClassOf rdf:resource="https://w3id.org/aio/NormalizationLayer"/>
        <obo:IAO_0000115>A normalization layer that applies Instance Normalization over a 5D input (a mini-batch of 3D inputs with additional channel dimension).</obo:IAO_0000115>
        <oboInOwl:hasExactSynonym>InstanceNorm3D</oboInOwl:hasExactSynonym>
        <oboInOwl:inSubset rdf:resource="https://w3id.org/aio/LayerSubset"/>
        <rdfs:comment>Applies Instance Normalization over a 5D input (a mini-batch of 3D inputs with additional channel dimension) as described in the paper Instance Normalization: The Missing Ingredient for Fast Stylization.</rdfs:comment>
        <rdfs:label>InstanceNorm3D Layer</rdfs:label>
    </owl:Class>
    <owl:Axiom>
        <owl:annotatedSource rdf:resource="https://w3id.org/aio/InstanceNorm3DLayer"/>
        <owl:annotatedProperty rdf:resource="http://purl.obolibrary.org/obo/IAO_0000115"/>
        <owl:annotatedTarget>A normalization layer that applies Instance Normalization over a 5D input (a mini-batch of 3D inputs with additional channel dimension).</owl:annotatedTarget>
        <oboInOwl:hasDbXref rdf:resource="https://pytorch.org/docs/stable/nn.html#normalization-layers"/>
    </owl:Axiom>
    


    <!-- https://w3id.org/aio/InstitutionalBias -->

    <owl:Class rdf:about="https://w3id.org/aio/InstitutionalBias">
        <rdfs:subClassOf rdf:resource="https://w3id.org/aio/Bias"/>
        <obo:IAO_0000115>A bias exhibited at the level of entire institutions where practices or norms result in the favoring or disadvantaging of certain social groups.</obo:IAO_0000115>
        <oboInOwl:inSubset rdf:resource="https://w3id.org/aio/BiasSubset"/>
        <rdfs:comment>Bias exhibited at the level of entire institutions, where practices or norms result in the favoring or disadvantaging of certain social groups, such as institutional racism or sexism.</rdfs:comment>
        <rdfs:label>Institutional Bias</rdfs:label>
    </owl:Class>
    <owl:Axiom>
        <owl:annotatedSource rdf:resource="https://w3id.org/aio/InstitutionalBias"/>
        <owl:annotatedProperty rdf:resource="http://purl.obolibrary.org/obo/IAO_0000115"/>
        <owl:annotatedTarget>A bias exhibited at the level of entire institutions where practices or norms result in the favoring or disadvantaging of certain social groups.</owl:annotatedTarget>
        <oboInOwl:hasDbXref rdf:resource="https://doi.org/10.6028/NIST.SP.1270"/>
    </owl:Axiom>
    


    <!-- https://w3id.org/aio/InstructionTunedLLM -->

    <owl:Class rdf:about="https://w3id.org/aio/InstructionTunedLLM">
        <rdfs:subClassOf rdf:resource="https://w3id.org/aio/LargeLanguageModel"/>
        <obo:IAO_0000115>A LLM which is fine-tuned to follow natural language instructions accurately and safely, learning to map from instructions to desired model behavior in a more controlled and principled way.</obo:IAO_0000115>
        <oboInOwl:hasExactSynonym>Instruction-Tuned Large Language Model</oboInOwl:hasExactSynonym>
        <oboInOwl:hasRelatedSynonym>constitutional AI</oboInOwl:hasRelatedSynonym>
        <oboInOwl:hasRelatedSynonym>natural language instructions</oboInOwl:hasRelatedSynonym>
        <oboInOwl:inSubset rdf:resource="https://w3id.org/aio/ModelSubset"/>
        <rdfs:label>Instruction-Tuned LLM</rdfs:label>
    </owl:Class>
    


    <!-- https://w3id.org/aio/IntegerLookupLayer -->

    <owl:Class rdf:about="https://w3id.org/aio/IntegerLookupLayer">
        <rdfs:subClassOf rdf:resource="https://w3id.org/aio/CategoricalFeaturesPreprocessingLayer"/>
        <obo:IAO_0000115>A categorical features preprocessing layer that maps integer features to contiguous ranges.</obo:IAO_0000115>
        <oboInOwl:inSubset rdf:resource="https://w3id.org/aio/LayerSubset"/>
        <rdfs:label>IntegerLookup Layer</rdfs:label>
    </owl:Class>
    <owl:Axiom>
        <owl:annotatedSource rdf:resource="https://w3id.org/aio/IntegerLookupLayer"/>
        <owl:annotatedProperty rdf:resource="http://purl.obolibrary.org/obo/IAO_0000115"/>
        <owl:annotatedTarget>A categorical features preprocessing layer that maps integer features to contiguous ranges.</owl:annotatedTarget>
        <oboInOwl:hasDbXref rdf:resource="https://www.tensorflow.org/api_docs/python/tf/keras/layers/IntegerLookup"/>
    </owl:Axiom>
    


    <!-- https://w3id.org/aio/InterpretationBias -->

    <owl:Class rdf:about="https://w3id.org/aio/InterpretationBias">
        <rdfs:subClassOf rdf:resource="https://w3id.org/aio/IndividualBias"/>
        <obo:IAO_0000115>An individual bias where users interpret algorithmic outputs according to their internalized biases and views.</obo:IAO_0000115>
        <oboInOwl:inSubset rdf:resource="https://w3id.org/aio/BiasSubset"/>
        <rdfs:label>Interpretation Bias</rdfs:label>
    </owl:Class>
    <owl:Axiom>
        <owl:annotatedSource rdf:resource="https://w3id.org/aio/InterpretationBias"/>
        <owl:annotatedProperty rdf:resource="http://purl.obolibrary.org/obo/IAO_0000115"/>
        <owl:annotatedTarget>An individual bias where users interpret algorithmic outputs according to their internalized biases and views.</owl:annotatedTarget>
        <oboInOwl:hasDbXref rdf:resource="https://doi.org/10.6028/NIST.SP.1270"/>
    </owl:Axiom>
    


    <!-- https://w3id.org/aio/KernelLayer -->

    <owl:Class rdf:about="https://w3id.org/aio/KernelLayer">
        <rdfs:subClassOf rdf:resource="https://w3id.org/aio/Layer"/>
        <obo:IAO_0000115>A layer that obtains the dot product of input values or subsets of input values.</obo:IAO_0000115>
        <oboInOwl:inSubset rdf:resource="https://w3id.org/aio/LayerSubset"/>
        <rdfs:label>Kernel Layer</rdfs:label>
    </owl:Class>
    


    <!-- https://w3id.org/aio/KnearestNeighborAlgorithm -->

    <owl:Class rdf:about="https://w3id.org/aio/KnearestNeighborAlgorithm">
        <rdfs:subClassOf rdf:resource="https://w3id.org/aio/MachineLearning"/>
        <obo:IAO_0000115>A machine learning that groups objects by a plurality vote of its neighbors, assigning each object to the class most common among its k nearest neighbors.</obo:IAO_0000115>
        <oboInOwl:hasExactSynonym>K-NN</oboInOwl:hasExactSynonym>
        <oboInOwl:hasExactSynonym>KNN</oboInOwl:hasExactSynonym>
        <oboInOwl:inSubset rdf:resource="https://w3id.org/aio/MachineLearningSubset"/>
        <rdfs:label>K-nearest Neighbor Algorithm</rdfs:label>
    </owl:Class>
    <owl:Axiom>
        <owl:annotatedSource rdf:resource="https://w3id.org/aio/KnearestNeighborAlgorithm"/>
        <owl:annotatedProperty rdf:resource="http://purl.obolibrary.org/obo/IAO_0000115"/>
        <owl:annotatedTarget>A machine learning that groups objects by a plurality vote of its neighbors, assigning each object to the class most common among its k nearest neighbors.</owl:annotatedTarget>
        <oboInOwl:hasDbXref rdf:resource="https://en.wikipedia.org/wiki/K-nearest_neighbors_algorithm"/>
    </owl:Axiom>
    


    <!-- https://w3id.org/aio/KnearestNeighborClassificationAlgorithm -->

    <owl:Class rdf:about="https://w3id.org/aio/KnearestNeighborClassificationAlgorithm">
        <rdfs:subClassOf rdf:resource="https://w3id.org/aio/Classification"/>
        <rdfs:subClassOf rdf:resource="https://w3id.org/aio/Clustering"/>
        <obo:IAO_0000115>A classification and clustering that classifies objects by a plurality vote of its neighbors, assigning each object to the class most common among its k nearest neighbors.</obo:IAO_0000115>
        <oboInOwl:hasExactSynonym>K-NN</oboInOwl:hasExactSynonym>
        <oboInOwl:hasExactSynonym>KNN</oboInOwl:hasExactSynonym>
        <oboInOwl:inSubset rdf:resource="https://w3id.org/aio/MachineLearningSubset"/>
        <rdfs:label>K-nearest Neighbor Classification Algorithm</rdfs:label>
    </owl:Class>
    <owl:Axiom>
        <owl:annotatedSource rdf:resource="https://w3id.org/aio/KnearestNeighborClassificationAlgorithm"/>
        <owl:annotatedProperty rdf:resource="http://purl.obolibrary.org/obo/IAO_0000115"/>
        <owl:annotatedTarget>A classification and clustering that classifies objects by a plurality vote of its neighbors, assigning each object to the class most common among its k nearest neighbors.</owl:annotatedTarget>
        <oboInOwl:hasDbXref rdf:resource="https://en.wikipedia.org/wiki/K-nearest_neighbors_algorithm"/>
    </owl:Axiom>
    


    <!-- https://w3id.org/aio/KnearestNeighborRegressionAlgorithm -->

    <owl:Class rdf:about="https://w3id.org/aio/KnearestNeighborRegressionAlgorithm">
        <rdfs:subClassOf rdf:resource="https://w3id.org/aio/RegressionAnalysis"/>
        <obo:IAO_0000115>An regression analysis that assigns the average of the values of k nearest neighbors to objects.</obo:IAO_0000115>
        <oboInOwl:hasExactSynonym>K-NN</oboInOwl:hasExactSynonym>
        <oboInOwl:hasExactSynonym>KNN</oboInOwl:hasExactSynonym>
        <oboInOwl:inSubset rdf:resource="https://w3id.org/aio/MachineLearningSubset"/>
        <rdfs:label>K-nearest Neighbor Regression Algorithm</rdfs:label>
    </owl:Class>
    <owl:Axiom>
        <owl:annotatedSource rdf:resource="https://w3id.org/aio/KnearestNeighborRegressionAlgorithm"/>
        <owl:annotatedProperty rdf:resource="http://purl.obolibrary.org/obo/IAO_0000115"/>
        <owl:annotatedTarget>An regression analysis that assigns the average of the values of k nearest neighbors to objects.</owl:annotatedTarget>
        <oboInOwl:hasDbXref rdf:resource="https://en.wikipedia.org/wiki/K-nearest_neighbors_algorithm"/>
    </owl:Axiom>
    


    <!-- https://w3id.org/aio/KnowledgeGroundedLLM -->

    <owl:Class rdf:about="https://w3id.org/aio/KnowledgeGroundedLLM">
        <rdfs:subClassOf rdf:resource="https://w3id.org/aio/LargeLanguageModel"/>
        <obo:IAO_0000115>A LLM which incorporates external knowledge sources or knowledge bases into the model architecture, enabling it to generate more factually accurate and knowledge-aware text.</obo:IAO_0000115>
        <oboInOwl:hasExactSynonym>Knowledge-Grounded Large Language Model</oboInOwl:hasExactSynonym>
        <oboInOwl:hasRelatedSynonym>factual grounding</oboInOwl:hasRelatedSynonym>
        <oboInOwl:hasRelatedSynonym>knowledge integration</oboInOwl:hasRelatedSynonym>
        <oboInOwl:inSubset rdf:resource="https://w3id.org/aio/ModelSubset"/>
        <rdfs:label>Knowledge-Grounded LLM</rdfs:label>
    </owl:Class>
    


    <!-- https://w3id.org/aio/KnowledgeTransfer -->

    <owl:Class rdf:about="https://w3id.org/aio/KnowledgeTransfer">
        <rdfs:subClassOf rdf:resource="https://w3id.org/aio/TrainingStrategies"/>
        <obo:IAO_0000115>The process by which knowledge is passed from one entity such as a person organization or system to another facilitating learning and adaptation in the receiving entity through various methods such as teaching training or data exchange.</obo:IAO_0000115>
        <oboInOwl:hasExactSynonym>Inductive Transfer</oboInOwl:hasExactSynonym>
        <oboInOwl:hasExactSynonym>Skill Acquisition</oboInOwl:hasExactSynonym>
        <oboInOwl:hasRelatedSynonym>Adaptation</oboInOwl:hasRelatedSynonym>
        <oboInOwl:hasRelatedSynonym>Pretrained models</oboInOwl:hasRelatedSynonym>
        <oboInOwl:inSubset rdf:resource="https://w3id.org/aio/PreprocessingSubset"/>
        <rdfs:label>Knowledge Transfer</rdfs:label>
    </owl:Class>
    <owl:Axiom>
        <owl:annotatedSource rdf:resource="https://w3id.org/aio/KnowledgeTransfer"/>
        <owl:annotatedProperty rdf:resource="http://purl.obolibrary.org/obo/IAO_0000115"/>
        <owl:annotatedTarget>The process by which knowledge is passed from one entity such as a person organization or system to another facilitating learning and adaptation in the receiving entity through various methods such as teaching training or data exchange.</owl:annotatedTarget>
        <oboInOwl:hasDbXref rdf:resource="https://doi.org/10.1016/j.knosys.2015.01.010"/>
    </owl:Axiom>
    


    <!-- https://w3id.org/aio/KohonenNetwork -->

    <owl:Class rdf:about="https://w3id.org/aio/KohonenNetwork">
        <rdfs:subClassOf rdf:resource="https://w3id.org/aio/Network"/>
        <rdfs:subClassOf>
            <owl:Restriction>
                <owl:onProperty rdf:resource="http://purl.obolibrary.org/obo/BFO_0000051"/>
                <owl:someValuesFrom rdf:resource="https://w3id.org/aio/HiddenLayer"/>
            </owl:Restriction>
        </rdfs:subClassOf>
        <rdfs:subClassOf>
            <owl:Restriction>
                <owl:onProperty rdf:resource="http://purl.obolibrary.org/obo/BFO_0000051"/>
                <owl:someValuesFrom rdf:resource="https://w3id.org/aio/InputLayer"/>
            </owl:Restriction>
        </rdfs:subClassOf>
        <obo:IAO_0000115>A network that is an unsupervised technique producing a low-dimensional representation of high-dimensional data preserving topological structure.</obo:IAO_0000115>
        <oboInOwl:hasExactSynonym>KN</oboInOwl:hasExactSynonym>
        <oboInOwl:hasExactSynonym>SOFM</oboInOwl:hasExactSynonym>
        <oboInOwl:hasExactSynonym>SOM</oboInOwl:hasExactSynonym>
        <oboInOwl:hasExactSynonym>Self-Organizing Feature Map</oboInOwl:hasExactSynonym>
        <oboInOwl:hasExactSynonym>Self-Organizing Map</oboInOwl:hasExactSynonym>
        <oboInOwl:inSubset rdf:resource="https://w3id.org/aio/NetworkSubset"/>
        <rdfs:comment>Layers: Input, Hidden</rdfs:comment>
        <rdfs:label>Kohonen Network</rdfs:label>
    </owl:Class>
    <owl:Axiom>
        <owl:annotatedSource rdf:resource="https://w3id.org/aio/KohonenNetwork"/>
        <owl:annotatedProperty rdf:resource="http://purl.obolibrary.org/obo/IAO_0000115"/>
        <owl:annotatedTarget>A network that is an unsupervised technique producing a low-dimensional representation of high-dimensional data preserving topological structure.</owl:annotatedTarget>
        <oboInOwl:hasDbXref rdf:resource="https://en.wikipedia.org/wiki/Self-organizing_map"/>
    </owl:Axiom>
    


    <!-- https://w3id.org/aio/LPPool1DLayer -->

    <owl:Class rdf:about="https://w3id.org/aio/LPPool1DLayer">
        <rdfs:subClassOf rdf:resource="https://w3id.org/aio/PoolingLayer"/>
        <obo:IAO_0000115>A pooling layer that applies 1D power-average pooling over an input signal composed of several input planes.</obo:IAO_0000115>
        <oboInOwl:hasExactSynonym>LPPool1D</oboInOwl:hasExactSynonym>
        <oboInOwl:inSubset rdf:resource="https://w3id.org/aio/LayerSubset"/>
        <rdfs:label>LPPool1D Layer</rdfs:label>
    </owl:Class>
    <owl:Axiom>
        <owl:annotatedSource rdf:resource="https://w3id.org/aio/LPPool1DLayer"/>
        <owl:annotatedProperty rdf:resource="http://purl.obolibrary.org/obo/IAO_0000115"/>
        <owl:annotatedTarget>A pooling layer that applies 1D power-average pooling over an input signal composed of several input planes.</owl:annotatedTarget>
        <oboInOwl:hasDbXref rdf:resource="https://pytorch.org/docs/stable/nn.html#pooling-layers"/>
    </owl:Axiom>
    


    <!-- https://w3id.org/aio/LPPool2DLayer -->

    <owl:Class rdf:about="https://w3id.org/aio/LPPool2DLayer">
        <rdfs:subClassOf rdf:resource="https://w3id.org/aio/PoolingLayer"/>
        <obo:IAO_0000115>A pooling layer that applies 2D power-average pooling over an input signal composed of several input planes.</obo:IAO_0000115>
        <oboInOwl:hasExactSynonym>LPPool2D</oboInOwl:hasExactSynonym>
        <oboInOwl:inSubset rdf:resource="https://w3id.org/aio/LayerSubset"/>
        <rdfs:label>LPPool2D Layer</rdfs:label>
    </owl:Class>
    <owl:Axiom>
        <owl:annotatedSource rdf:resource="https://w3id.org/aio/LPPool2DLayer"/>
        <owl:annotatedProperty rdf:resource="http://purl.obolibrary.org/obo/IAO_0000115"/>
        <owl:annotatedTarget>A pooling layer that applies 2D power-average pooling over an input signal composed of several input planes.</owl:annotatedTarget>
        <oboInOwl:hasDbXref rdf:resource="https://pytorch.org/docs/stable/nn.html#pooling-layers"/>
    </owl:Axiom>
    


    <!-- https://w3id.org/aio/LSTMCellLayer -->

    <owl:Class rdf:about="https://w3id.org/aio/LSTMCellLayer">
        <rdfs:subClassOf rdf:resource="https://w3id.org/aio/Layer"/>
        <obo:IAO_0000115>A layer that processes one step within the whole time sequence input for an LSTM layer.</obo:IAO_0000115>
        <oboInOwl:inSubset rdf:resource="https://w3id.org/aio/LayerSubset"/>
        <rdfs:comment>Cell class for the LSTM layer.</rdfs:comment>
        <rdfs:label>LSTMCell Layer</rdfs:label>
    </owl:Class>
    <owl:Axiom>
        <owl:annotatedSource rdf:resource="https://w3id.org/aio/LSTMCellLayer"/>
        <owl:annotatedProperty rdf:resource="http://purl.obolibrary.org/obo/IAO_0000115"/>
        <owl:annotatedTarget>A layer that processes one step within the whole time sequence input for an LSTM layer.</owl:annotatedTarget>
        <oboInOwl:hasDbXref rdf:resource="https://www.tensorflow.org/api_docs/python/tf/keras/layers/LSTMCell"/>
    </owl:Axiom>
    


    <!-- https://w3id.org/aio/LSTMLayer -->

    <owl:Class rdf:about="https://w3id.org/aio/LSTMLayer">
        <rdfs:subClassOf rdf:resource="https://w3id.org/aio/RecurrentLayer"/>
        <obo:IAO_0000115>A recurrent layer that implements the Long Short-Term Memory architecture.</obo:IAO_0000115>
        <oboInOwl:inSubset rdf:resource="https://w3id.org/aio/LayerSubset"/>
        <rdfs:comment>Long Short-Term Memory layer - Hochreiter 1997. Based on available runtime hardware and constraints, this layer will choose different implementations (cuDNN-based or pure-TensorFlow) to maximize the performance. If a GPU is available and all the arguments to the layer meet the requirement of the cuDNN kernel (see below for details), the layer will use a fast cuDNN implementation. The requirements to use the cuDNN implementation are: 1. activation == tanh, 2. recurrent_activation == sigmoid, 3. recurrent_dropout == 0, 4. unroll is False, 5. use_bias is True, 6. Inputs, if use masking, are strictly right-padded, 7. Eager execution is enabled in the outermost context.</rdfs:comment>
        <rdfs:label>LSTM Layer</rdfs:label>
    </owl:Class>
    <owl:Axiom>
        <owl:annotatedSource rdf:resource="https://w3id.org/aio/LSTMLayer"/>
        <owl:annotatedProperty rdf:resource="http://purl.obolibrary.org/obo/IAO_0000115"/>
        <owl:annotatedTarget>A recurrent layer that implements the Long Short-Term Memory architecture.</owl:annotatedTarget>
        <oboInOwl:hasDbXref rdf:resource="https://www.tensorflow.org/api_docs/python/tf/keras/layers/LSTM"/>
    </owl:Axiom>
    


    <!-- https://w3id.org/aio/LambdaLayer -->

    <owl:Class rdf:about="https://w3id.org/aio/LambdaLayer">
        <rdfs:subClassOf rdf:resource="https://w3id.org/aio/Layer"/>
        <obo:IAO_0000115>A layer that wraps arbitrary expressions as a Layer object.</obo:IAO_0000115>
        <oboInOwl:inSubset rdf:resource="https://w3id.org/aio/LayerSubset"/>
        <rdfs:comment>Wraps arbitrary expressions as a Layer object.</rdfs:comment>
        <rdfs:label>Lambda Layer</rdfs:label>
    </owl:Class>
    <owl:Axiom>
        <owl:annotatedSource rdf:resource="https://w3id.org/aio/LambdaLayer"/>
        <owl:annotatedProperty rdf:resource="http://purl.obolibrary.org/obo/IAO_0000115"/>
        <owl:annotatedTarget>A layer that wraps arbitrary expressions as a Layer object.</owl:annotatedTarget>
        <oboInOwl:hasDbXref rdf:resource="https://www.tensorflow.org/api_docs/python/tf/keras/layers/Lambda"/>
    </owl:Axiom>
    


    <!-- https://w3id.org/aio/LanguageInterfaceLLM -->

    <owl:Class rdf:about="https://w3id.org/aio/LanguageInterfaceLLM">
        <rdfs:subClassOf rdf:resource="https://w3id.org/aio/LargeLanguageModel"/>
        <obo:IAO_0000115>A large language model that supports interactive semantic parsing enabling users to provide feedback and corrections to dynamically refine and update the language model.</obo:IAO_0000115>
        <oboInOwl:hasRelatedSynonym>Interactive learning</oboInOwl:hasRelatedSynonym>
        <oboInOwl:inSubset rdf:resource="https://w3id.org/aio/ModelSubset"/>
        <rdfs:label>Language Interface LLM</rdfs:label>
    </owl:Class>
    


    <!-- https://w3id.org/aio/LanguageModel -->

    <owl:Class rdf:about="https://w3id.org/aio/LanguageModel">
        <rdfs:subClassOf rdf:resource="https://w3id.org/aio/Model"/>
        <obo:IAO_0000115>A model designed to predict the next word in a sequence or assign probabilities to sequences of words in natural language.</obo:IAO_0000115>
        <oboInOwl:inSubset rdf:resource="https://w3id.org/aio/ModelSubset"/>
        <rdfs:label>Language Model</rdfs:label>
    </owl:Class>
    <owl:Axiom>
        <owl:annotatedSource rdf:resource="https://w3id.org/aio/LanguageModel"/>
        <owl:annotatedProperty rdf:resource="http://purl.obolibrary.org/obo/IAO_0000115"/>
        <owl:annotatedTarget>A model designed to predict the next word in a sequence or assign probabilities to sequences of words in natural language.</owl:annotatedTarget>
        <oboInOwl:hasDbXref rdf:resource="https://en.wikipedia.org/wiki/Language_model"/>
    </owl:Axiom>
    


    <!-- https://w3id.org/aio/LargeLanguageModel -->

    <owl:Class rdf:about="https://w3id.org/aio/LargeLanguageModel">
        <rdfs:subClassOf rdf:resource="https://w3id.org/aio/LanguageModel"/>
        <obo:IAO_0000115>A language model consisting of a neural network with many parameters (typically billions of weights or more) trained on large quantities of unlabeled text using self-supervised learning or semi-supervised learning.</obo:IAO_0000115>
        <oboInOwl:hasExactSynonym>LLM</oboInOwl:hasExactSynonym>
        <oboInOwl:inSubset rdf:resource="https://w3id.org/aio/ModelSubset"/>
        <rdfs:label>Large Language Model</rdfs:label>
    </owl:Class>
    <owl:Axiom>
        <owl:annotatedSource rdf:resource="https://w3id.org/aio/LargeLanguageModel"/>
        <owl:annotatedProperty rdf:resource="http://purl.obolibrary.org/obo/IAO_0000115"/>
        <owl:annotatedTarget>A language model consisting of a neural network with many parameters (typically billions of weights or more) trained on large quantities of unlabeled text using self-supervised learning or semi-supervised learning.</owl:annotatedTarget>
        <oboInOwl:hasDbXref rdf:resource="https://en.wikipedia.org/wiki/Large_language_model"/>
    </owl:Axiom>
    


    <!-- https://w3id.org/aio/LassoRegression -->

    <owl:Class rdf:about="https://w3id.org/aio/LassoRegression">
        <rdfs:subClassOf rdf:resource="https://w3id.org/aio/RegressionAnalysis"/>
        <obo:IAO_0000115>A regression analysis method that performs both variable selection and regularization to enhance prediction accuracy and interpretability.</obo:IAO_0000115>
        <oboInOwl:inSubset rdf:resource="https://w3id.org/aio/MachineLearningSubset"/>
        <rdfs:label>Lasso Regression</rdfs:label>
    </owl:Class>
    <owl:Axiom>
        <owl:annotatedSource rdf:resource="https://w3id.org/aio/LassoRegression"/>
        <owl:annotatedProperty rdf:resource="http://purl.obolibrary.org/obo/IAO_0000115"/>
        <owl:annotatedTarget>A regression analysis method that performs both variable selection and regularization to enhance prediction accuracy and interpretability.</owl:annotatedTarget>
        <oboInOwl:hasDbXref rdf:resource="https://en.wikipedia.org/wiki/Lasso_(statistics)"/>
    </owl:Axiom>
    


    <!-- https://w3id.org/aio/Layer -->

    <owl:Class rdf:about="https://w3id.org/aio/Layer">
        <rdfs:subClassOf rdf:resource="http://www.w3.org/2002/07/owl#Thing"/>
        <obo:IAO_0000115>A structure or network topology in a deep learning model that takes information from previous layers and passes it to the next layer.</obo:IAO_0000115>
        <oboInOwl:inSubset rdf:resource="https://w3id.org/aio/ClassSubset"/>
        <rdfs:label>Layer</rdfs:label>
    </owl:Class>
    <owl:Axiom>
        <owl:annotatedSource rdf:resource="https://w3id.org/aio/Layer"/>
        <owl:annotatedProperty rdf:resource="http://purl.obolibrary.org/obo/IAO_0000115"/>
        <owl:annotatedTarget>A structure or network topology in a deep learning model that takes information from previous layers and passes it to the next layer.</owl:annotatedTarget>
        <oboInOwl:hasDbXref rdf:resource="https://en.wikipedia.org/wiki/Layer_(deep_learning)"/>
    </owl:Axiom>
    


    <!-- https://w3id.org/aio/LayerLayer -->

    <owl:Class rdf:about="https://w3id.org/aio/LayerLayer">
        <rdfs:subClassOf rdf:resource="https://w3id.org/aio/Layer"/>
        <obo:IAO_0000115>The base class from which all layers inherit.</obo:IAO_0000115>
        <oboInOwl:inSubset rdf:resource="https://w3id.org/aio/LayerSubset"/>
        <rdfs:comment>This is the class from which all layers inherit. A layer is a callable object that takes as input one or more tensors and that outputs one or more tensors. It involves computation, defined in the call() method, and a state (weight variables). State can be created in various places, at the convenience of the subclass implementer: in __init__(); in the optional build() method, which is invoked by the first __call__() to the layer, and supplies the shape(s) of the input(s), which may not have been known at initialization time; in the first invocation of call(), with some caveats discussed below. Users will just instantiate a layer and then treat it as a callable.</rdfs:comment>
        <rdfs:label>Layer Layer</rdfs:label>
    </owl:Class>
    <owl:Axiom>
        <owl:annotatedSource rdf:resource="https://w3id.org/aio/LayerLayer"/>
        <owl:annotatedProperty rdf:resource="http://purl.obolibrary.org/obo/IAO_0000115"/>
        <owl:annotatedTarget>The base class from which all layers inherit.</owl:annotatedTarget>
        <oboInOwl:hasDbXref rdf:resource="https://www.tensorflow.org/api_docs/python/tf/keras/layers/Layer"/>
    </owl:Axiom>
    


    <!-- https://w3id.org/aio/LayerNormLayer -->

    <owl:Class rdf:about="https://w3id.org/aio/LayerNormLayer">
        <rdfs:subClassOf rdf:resource="https://w3id.org/aio/NormalizationLayer"/>
        <obo:IAO_0000115>A normalization layer that applies Layer Normalization over a mini-batch of inputs.</obo:IAO_0000115>
        <oboInOwl:hasExactSynonym>LayerNorm</oboInOwl:hasExactSynonym>
        <oboInOwl:inSubset rdf:resource="https://w3id.org/aio/LayerSubset"/>
        <rdfs:comment>Applies Layer Normalization over a mini-batch of inputs as described in the paper Layer Normalization</rdfs:comment>
        <rdfs:label>LayerNorm Layer</rdfs:label>
    </owl:Class>
    <owl:Axiom>
        <owl:annotatedSource rdf:resource="https://w3id.org/aio/LayerNormLayer"/>
        <owl:annotatedProperty rdf:resource="http://purl.obolibrary.org/obo/IAO_0000115"/>
        <owl:annotatedTarget>A normalization layer that applies Layer Normalization over a mini-batch of inputs.</owl:annotatedTarget>
        <oboInOwl:hasDbXref rdf:resource="https://pytorch.org/docs/stable/nn.html#normalization-layers"/>
    </owl:Axiom>
    


    <!-- https://w3id.org/aio/LayerNormalizationLayer -->

    <owl:Class rdf:about="https://w3id.org/aio/LayerNormalizationLayer">
        <rdfs:subClassOf rdf:resource="https://w3id.org/aio/NormalizationLayer"/>
        <obo:IAO_0000115>A normalization layer that applies Layer Normalization over the inputs.</obo:IAO_0000115>
        <oboInOwl:inSubset rdf:resource="https://w3id.org/aio/LayerSubset"/>
        <rdfs:comment>Layer normalization layer (Ba et al., 2016). Normalize the activations of the previous layer for each given example in a batch independently, rather than across a batch like Batch Normalization. i.e. applies a transformation that maintains the mean activation within each example close to 0 and the activation standard deviation close to 1. Given a tensor inputs, moments are calculated and normalization is performed across the axes specified in axis.</rdfs:comment>
        <rdfs:label>LayerNormalization Layer</rdfs:label>
    </owl:Class>
    <owl:Axiom>
        <owl:annotatedSource rdf:resource="https://w3id.org/aio/LayerNormalizationLayer"/>
        <owl:annotatedProperty rdf:resource="http://purl.obolibrary.org/obo/IAO_0000115"/>
        <owl:annotatedTarget>A normalization layer that applies Layer Normalization over the inputs.</owl:annotatedTarget>
        <oboInOwl:hasDbXref rdf:resource="https://www.tensorflow.org/api_docs/python/tf/keras/layers/LayerNormalization"/>
    </owl:Axiom>
    


    <!-- https://w3id.org/aio/LazyBatchNorm1DLayer -->

    <owl:Class rdf:about="https://w3id.org/aio/LazyBatchNorm1DLayer">
        <rdfs:subClassOf rdf:resource="https://w3id.org/aio/BatchNormalizationLayer"/>
        <obo:IAO_0000115>A batch normalization layer that lazily initializes the num_features argument from the input size for 1D data.</obo:IAO_0000115>
        <oboInOwl:hasExactSynonym>LazyBatchNorm1D</oboInOwl:hasExactSynonym>
        <oboInOwl:inSubset rdf:resource="https://w3id.org/aio/LayerSubset"/>
        <rdfs:comment>A torch.nn.BatchNorm1D module with lazy initialization of the num_features argument of the BatchNorm1D that is inferred from the input.size(1).</rdfs:comment>
        <rdfs:label>LazyBatchNorm1D Layer</rdfs:label>
    </owl:Class>
    <owl:Axiom>
        <owl:annotatedSource rdf:resource="https://w3id.org/aio/LazyBatchNorm1DLayer"/>
        <owl:annotatedProperty rdf:resource="http://purl.obolibrary.org/obo/IAO_0000115"/>
        <owl:annotatedTarget>A batch normalization layer that lazily initializes the num_features argument from the input size for 1D data.</owl:annotatedTarget>
        <oboInOwl:hasDbXref rdf:resource="https://pytorch.org/docs/stable/nn.html#normalization-layers"/>
    </owl:Axiom>
    


    <!-- https://w3id.org/aio/LazyBatchNorm2DLayer -->

    <owl:Class rdf:about="https://w3id.org/aio/LazyBatchNorm2DLayer">
        <rdfs:subClassOf rdf:resource="https://w3id.org/aio/BatchNormalizationLayer"/>
        <obo:IAO_0000115>A batch normalization layer that lazily initializes the num_features argument from the input size for 2D data.</obo:IAO_0000115>
        <oboInOwl:hasExactSynonym>LazyBatchNorm2D</oboInOwl:hasExactSynonym>
        <oboInOwl:inSubset rdf:resource="https://w3id.org/aio/LayerSubset"/>
        <rdfs:comment>A torch.nn.BatchNorm2D module with lazy initialization of the num_features argument of the BatchNorm2D that is inferred from the input.size(1).</rdfs:comment>
        <rdfs:label>LazyBatchNorm2D Layer</rdfs:label>
    </owl:Class>
    <owl:Axiom>
        <owl:annotatedSource rdf:resource="https://w3id.org/aio/LazyBatchNorm2DLayer"/>
        <owl:annotatedProperty rdf:resource="http://purl.obolibrary.org/obo/IAO_0000115"/>
        <owl:annotatedTarget>A batch normalization layer that lazily initializes the num_features argument from the input size for 2D data.</owl:annotatedTarget>
        <oboInOwl:hasDbXref rdf:resource="https://pytorch.org/docs/stable/nn.html#normalization-layers"/>
    </owl:Axiom>
    


    <!-- https://w3id.org/aio/LazyBatchNorm3DLayer -->

    <owl:Class rdf:about="https://w3id.org/aio/LazyBatchNorm3DLayer">
        <rdfs:subClassOf rdf:resource="https://w3id.org/aio/BatchNormalizationLayer"/>
        <obo:IAO_0000115>A batch normalization layer that lazily initializes the num_features argument from the input size for 3D data.</obo:IAO_0000115>
        <oboInOwl:hasExactSynonym>LazyBatchNorm3D</oboInOwl:hasExactSynonym>
        <oboInOwl:inSubset rdf:resource="https://w3id.org/aio/LayerSubset"/>
        <rdfs:comment>A torch.nn.BatchNorm3D module with lazy initialization of the num_features argument of the BatchNorm3D that is inferred from the input.size(1).</rdfs:comment>
        <rdfs:label>LazyBatchNorm3D Layer</rdfs:label>
    </owl:Class>
    <owl:Axiom>
        <owl:annotatedSource rdf:resource="https://w3id.org/aio/LazyBatchNorm3DLayer"/>
        <owl:annotatedProperty rdf:resource="http://purl.obolibrary.org/obo/IAO_0000115"/>
        <owl:annotatedTarget>A batch normalization layer that lazily initializes the num_features argument from the input size for 3D data.</owl:annotatedTarget>
        <oboInOwl:hasDbXref rdf:resource="https://pytorch.org/docs/stable/nn.html#normalization-layers"/>
    </owl:Axiom>
    


    <!-- https://w3id.org/aio/LazyInstanceNorm1DLayer -->

    <owl:Class rdf:about="https://w3id.org/aio/LazyInstanceNorm1DLayer">
        <rdfs:subClassOf rdf:resource="https://w3id.org/aio/NormalizationLayer"/>
        <obo:IAO_0000115>An instance normalization layer that lazily initializes the num_features argument from the input size for 1D data.</obo:IAO_0000115>
        <oboInOwl:hasExactSynonym>LazyInstanceNorm1D</oboInOwl:hasExactSynonym>
        <oboInOwl:inSubset rdf:resource="https://w3id.org/aio/LayerSubset"/>
        <rdfs:comment>A torch.nn.InstanceNorm1D module with lazy initialization of the num_features argument of the InstanceNorm1D that is inferred from the input.size(1).</rdfs:comment>
        <rdfs:label>LazyInstanceNorm1D Layer</rdfs:label>
    </owl:Class>
    <owl:Axiom>
        <owl:annotatedSource rdf:resource="https://w3id.org/aio/LazyInstanceNorm1DLayer"/>
        <owl:annotatedProperty rdf:resource="http://purl.obolibrary.org/obo/IAO_0000115"/>
        <owl:annotatedTarget>An instance normalization layer that lazily initializes the num_features argument from the input size for 1D data.</owl:annotatedTarget>
        <oboInOwl:hasDbXref rdf:resource="https://pytorch.org/docs/stable/nn.html#normalization-layers"/>
    </owl:Axiom>
    


    <!-- https://w3id.org/aio/LazyInstanceNorm2DLayer -->

    <owl:Class rdf:about="https://w3id.org/aio/LazyInstanceNorm2DLayer">
        <rdfs:subClassOf rdf:resource="https://w3id.org/aio/NormalizationLayer"/>
        <obo:IAO_0000115>An instance normalization layer that lazily initializes the num_features argument from the input size for 2D data.</obo:IAO_0000115>
        <oboInOwl:hasExactSynonym>LazyInstanceNorm2D</oboInOwl:hasExactSynonym>
        <oboInOwl:inSubset rdf:resource="https://w3id.org/aio/LayerSubset"/>
        <rdfs:comment>A torch.nn.InstanceNorm2D module with lazy initialization of the num_features argument of the InstanceNorm2D that is inferred from the input.size(1).</rdfs:comment>
        <rdfs:label>LazyInstanceNorm2D Layer</rdfs:label>
    </owl:Class>
    <owl:Axiom>
        <owl:annotatedSource rdf:resource="https://w3id.org/aio/LazyInstanceNorm2DLayer"/>
        <owl:annotatedProperty rdf:resource="http://purl.obolibrary.org/obo/IAO_0000115"/>
        <owl:annotatedTarget>An instance normalization layer that lazily initializes the num_features argument from the input size for 2D data.</owl:annotatedTarget>
        <oboInOwl:hasDbXref rdf:resource="https://pytorch.org/docs/stable/nn.html#normalization-layers"/>
    </owl:Axiom>
    


    <!-- https://w3id.org/aio/LazyInstanceNorm3DLayer -->

    <owl:Class rdf:about="https://w3id.org/aio/LazyInstanceNorm3DLayer">
        <rdfs:subClassOf rdf:resource="https://w3id.org/aio/NormalizationLayer"/>
        <obo:IAO_0000115>An instance normalization layer that lazily initializes the num_features argument from the input size for 3D data.</obo:IAO_0000115>
        <oboInOwl:hasExactSynonym>LazyInstanceNorm3D</oboInOwl:hasExactSynonym>
        <oboInOwl:inSubset rdf:resource="https://w3id.org/aio/LayerSubset"/>
        <rdfs:comment>A torch.nn.InstanceNorm3D module with lazy initialization of the num_features argument of the InstanceNorm3D that is inferred from the input.size(1).</rdfs:comment>
        <rdfs:label>LazyInstanceNorm3D Layer</rdfs:label>
    </owl:Class>
    <owl:Axiom>
        <owl:annotatedSource rdf:resource="https://w3id.org/aio/LazyInstanceNorm3DLayer"/>
        <owl:annotatedProperty rdf:resource="http://purl.obolibrary.org/obo/IAO_0000115"/>
        <owl:annotatedTarget>An instance normalization layer that lazily initializes the num_features argument from the input size for 3D data.</owl:annotatedTarget>
        <oboInOwl:hasDbXref rdf:resource="https://pytorch.org/docs/stable/nn.html#normalization-layers"/>
    </owl:Axiom>
    


    <!-- https://w3id.org/aio/LeakyReLULayer -->

    <owl:Class rdf:about="https://w3id.org/aio/LeakyReLULayer">
        <rdfs:subClassOf rdf:resource="https://w3id.org/aio/ActivationLayer"/>
        <obo:IAO_0000115>An activation layer that applies the leaky rectified linear unit function element-wise.</obo:IAO_0000115>
        <oboInOwl:inSubset rdf:resource="https://w3id.org/aio/LayerSubset"/>
        <rdfs:comment>Leaky version of a Rectified Linear Unit.</rdfs:comment>
        <rdfs:label>LeakyReLU Layer</rdfs:label>
    </owl:Class>
    <owl:Axiom>
        <owl:annotatedSource rdf:resource="https://w3id.org/aio/LeakyReLULayer"/>
        <owl:annotatedProperty rdf:resource="http://purl.obolibrary.org/obo/IAO_0000115"/>
        <owl:annotatedTarget>An activation layer that applies the leaky rectified linear unit function element-wise.</owl:annotatedTarget>
        <oboInOwl:hasDbXref rdf:resource="https://www.tensorflow.org/api_docs/python/tf/keras/layers/LeakyReLU"/>
    </owl:Axiom>
    


    <!-- https://w3id.org/aio/LeastsquaresAnalysis -->

    <owl:Class rdf:about="https://w3id.org/aio/LeastsquaresAnalysis">
        <rdfs:subClassOf rdf:resource="https://w3id.org/aio/RegressionAnalysis"/>
        <obo:IAO_0000115>A regression analysis which approximates the solution of overdetermined systems by minimizing the sum of the squares of the residuals.</obo:IAO_0000115>
        <oboInOwl:inSubset rdf:resource="https://w3id.org/aio/MachineLearningSubset"/>
        <rdfs:label>Least-squares Analysis</rdfs:label>
    </owl:Class>
    <owl:Axiom>
        <owl:annotatedSource rdf:resource="https://w3id.org/aio/LeastsquaresAnalysis"/>
        <owl:annotatedProperty rdf:resource="http://purl.obolibrary.org/obo/IAO_0000115"/>
        <owl:annotatedTarget>A regression analysis which approximates the solution of overdetermined systems by minimizing the sum of the squares of the residuals.</owl:annotatedTarget>
        <oboInOwl:hasDbXref rdf:resource="https://en.wikipedia.org/wiki/Least_squares"/>
    </owl:Axiom>
    


    <!-- https://w3id.org/aio/LifelongLearningLLM -->

    <owl:Class rdf:about="https://w3id.org/aio/LifelongLearningLLM">
        <rdfs:subClassOf rdf:resource="https://w3id.org/aio/LargeLanguageModel"/>
        <obo:IAO_0000115>A large language model that continually acquires new knowledge over time without forgetting previously learned information maintaining a balance between plasticity and stability.</obo:IAO_0000115>
        <oboInOwl:hasExactSynonym>Continual Learning LLM</oboInOwl:hasExactSynonym>
        <oboInOwl:hasExactSynonym>Forever Learning</oboInOwl:hasExactSynonym>
        <oboInOwl:hasRelatedSynonym>Catastrophic forgetting</oboInOwl:hasRelatedSynonym>
        <oboInOwl:hasRelatedSynonym>Plasticity-Stability balance</oboInOwl:hasRelatedSynonym>
        <oboInOwl:inSubset rdf:resource="https://w3id.org/aio/ModelSubset"/>
        <rdfs:label>Lifelong Learning LLM</rdfs:label>
    </owl:Class>
    


    <!-- https://w3id.org/aio/LinearFunction -->

    <owl:Class rdf:about="https://w3id.org/aio/LinearFunction">
        <rdfs:subClassOf rdf:resource="https://w3id.org/aio/Function"/>
        <obo:IAO_0000115>An activation function that has the form f(x) = a + bx.</obo:IAO_0000115>
        <oboInOwl:inSubset rdf:resource="https://w3id.org/aio/FunctionSubset"/>
        <rdfs:label>Linear Function</rdfs:label>
    </owl:Class>
    <owl:Axiom>
        <owl:annotatedSource rdf:resource="https://w3id.org/aio/LinearFunction"/>
        <owl:annotatedProperty rdf:resource="http://purl.obolibrary.org/obo/IAO_0000115"/>
        <owl:annotatedTarget>An activation function that has the form f(x) = a + bx.</owl:annotatedTarget>
        <oboInOwl:hasDbXref rdf:resource="https://www.tensorflow.org/api_docs/python/tf/keras/activations/linear"/>
    </owl:Axiom>
    


    <!-- https://w3id.org/aio/LinearRegression -->

    <owl:Class rdf:about="https://w3id.org/aio/LinearRegression">
        <rdfs:subClassOf rdf:resource="https://w3id.org/aio/RegressionAnalysis"/>
        <obo:IAO_0000115>A regression analysis model that is a linear approach for modeling the relationship between a scalar response and one or more explanatory variables.</obo:IAO_0000115>
        <oboInOwl:inSubset rdf:resource="https://w3id.org/aio/MachineLearningSubset"/>
        <rdfs:label>Linear Regression</rdfs:label>
    </owl:Class>
    <owl:Axiom>
        <owl:annotatedSource rdf:resource="https://w3id.org/aio/LinearRegression"/>
        <owl:annotatedProperty rdf:resource="http://purl.obolibrary.org/obo/IAO_0000115"/>
        <owl:annotatedTarget>A regression analysis model that is a linear approach for modeling the relationship between a scalar response and one or more explanatory variables.</owl:annotatedTarget>
        <oboInOwl:hasDbXref rdf:resource="https://en.wikipedia.org/wiki/Linear_regression"/>
    </owl:Axiom>
    


    <!-- https://w3id.org/aio/LinkingBias -->

    <owl:Class rdf:about="https://w3id.org/aio/LinkingBias">
        <rdfs:subClassOf rdf:resource="https://w3id.org/aio/UseAndInterpretationBias"/>
        <obo:IAO_0000115>A use and interpretation bias arising when network attributes obtained from user connections activities or interactions misrepresent true user behavior.</obo:IAO_0000115>
        <oboInOwl:inSubset rdf:resource="https://w3id.org/aio/BiasSubset"/>
        <rdfs:comment>Bias arising when network attributes obtained from user connections, activities, or interactions misrepresent true user behavior.</rdfs:comment>
        <rdfs:label>Linking Bias</rdfs:label>
    </owl:Class>
    <owl:Axiom>
        <owl:annotatedSource rdf:resource="https://w3id.org/aio/LinkingBias"/>
        <owl:annotatedProperty rdf:resource="http://purl.obolibrary.org/obo/IAO_0000115"/>
        <owl:annotatedTarget>A use and interpretation bias arising when network attributes obtained from user connections activities or interactions misrepresent true user behavior.</owl:annotatedTarget>
        <oboInOwl:hasDbXref rdf:resource="https://doi.org/10.6028/NIST.SP.1270"/>
    </owl:Axiom>
    


    <!-- https://w3id.org/aio/LiquidStateMachineNetwork -->

    <owl:Class rdf:about="https://w3id.org/aio/LiquidStateMachineNetwork">
        <rdfs:subClassOf rdf:resource="https://w3id.org/aio/Network"/>
        <rdfs:subClassOf>
            <owl:Restriction>
                <owl:onProperty rdf:resource="http://purl.obolibrary.org/obo/BFO_0000051"/>
                <owl:someValuesFrom rdf:resource="https://w3id.org/aio/InputLayer"/>
            </owl:Restriction>
        </rdfs:subClassOf>
        <rdfs:subClassOf>
            <owl:Restriction>
                <owl:onProperty rdf:resource="http://purl.obolibrary.org/obo/BFO_0000051"/>
                <owl:someValuesFrom rdf:resource="https://w3id.org/aio/OutputLayer"/>
            </owl:Restriction>
        </rdfs:subClassOf>
        <rdfs:subClassOf>
            <owl:Restriction>
                <owl:onProperty rdf:resource="http://purl.obolibrary.org/obo/BFO_0000051"/>
                <owl:someValuesFrom rdf:resource="https://w3id.org/aio/SpikingHiddenLayer"/>
            </owl:Restriction>
        </rdfs:subClassOf>
        <obo:IAO_0000115>A network that is a type of reservoir computer turning time-varying input into spatio-temporal activation patterns.</obo:IAO_0000115>
        <oboInOwl:hasExactSynonym>LSM</oboInOwl:hasExactSynonym>
        <oboInOwl:inSubset rdf:resource="https://w3id.org/aio/NetworkSubset"/>
        <rdfs:comment>Layers: Input, Spiking Hidden, Output</rdfs:comment>
        <rdfs:label>Liquid State Machine Network</rdfs:label>
    </owl:Class>
    <owl:Axiom>
        <owl:annotatedSource rdf:resource="https://w3id.org/aio/LiquidStateMachineNetwork"/>
        <owl:annotatedProperty rdf:resource="http://purl.obolibrary.org/obo/IAO_0000115"/>
        <owl:annotatedTarget>A network that is a type of reservoir computer turning time-varying input into spatio-temporal activation patterns.</owl:annotatedTarget>
        <oboInOwl:hasDbXref rdf:resource="https://en.wikipedia.org/wiki/Liquid_state_machine"/>
    </owl:Axiom>
    


    <!-- https://w3id.org/aio/LocalResponseNormLayer -->

    <owl:Class rdf:about="https://w3id.org/aio/LocalResponseNormLayer">
        <rdfs:subClassOf rdf:resource="https://w3id.org/aio/NormalizationLayer"/>
        <obo:IAO_0000115>A normalization layer that applies local response normalization over an input signal composed of several input planes.</obo:IAO_0000115>
        <oboInOwl:hasExactSynonym>LocalResponseNorm</oboInOwl:hasExactSynonym>
        <oboInOwl:inSubset rdf:resource="https://w3id.org/aio/LayerSubset"/>
        <rdfs:comment>Applies local response normalization over an input signal composed of several input planes, where channels occupy the second dimension.</rdfs:comment>
        <rdfs:label>LocalResponseNorm Layer</rdfs:label>
    </owl:Class>
    <owl:Axiom>
        <owl:annotatedSource rdf:resource="https://w3id.org/aio/LocalResponseNormLayer"/>
        <owl:annotatedProperty rdf:resource="http://purl.obolibrary.org/obo/IAO_0000115"/>
        <owl:annotatedTarget>A normalization layer that applies local response normalization over an input signal composed of several input planes.</owl:annotatedTarget>
        <oboInOwl:hasDbXref rdf:resource="https://pytorch.org/docs/stable/nn.html#normalization-layers"/>
    </owl:Axiom>
    


    <!-- https://w3id.org/aio/LocallyConnected1DLayer -->

    <owl:Class rdf:about="https://w3id.org/aio/LocallyConnected1DLayer">
        <rdfs:subClassOf rdf:resource="https://w3id.org/aio/LocallyconnectedLayer"/>
        <obo:IAO_0000115>A locally-connected layer for 1D inputs where each patch of the input is convolved with a different set of filters.</obo:IAO_0000115>
        <oboInOwl:inSubset rdf:resource="https://w3id.org/aio/LayerSubset"/>
        <rdfs:comment>Locally-connected layer for 1D inputs. The LocallyConnected1D layer works similarly to the Conv1D layer, except that weights are unshared, that is, a different set of filters is applied at each different patch of the input.</rdfs:comment>
        <rdfs:label>LocallyConnected1D Layer</rdfs:label>
    </owl:Class>
    <owl:Axiom>
        <owl:annotatedSource rdf:resource="https://w3id.org/aio/LocallyConnected1DLayer"/>
        <owl:annotatedProperty rdf:resource="http://purl.obolibrary.org/obo/IAO_0000115"/>
        <owl:annotatedTarget>A locally-connected layer for 1D inputs where each patch of the input is convolved with a different set of filters.</owl:annotatedTarget>
        <oboInOwl:hasDbXref rdf:resource="https://www.tensorflow.org/api_docs/python/tf/keras/layers/LocallyConnected1D"/>
    </owl:Axiom>
    


    <!-- https://w3id.org/aio/LocallyConnected2DLayer -->

    <owl:Class rdf:about="https://w3id.org/aio/LocallyConnected2DLayer">
        <rdfs:subClassOf rdf:resource="https://w3id.org/aio/LocallyconnectedLayer"/>
        <obo:IAO_0000115>A locally-connected layer for 2D inputs where each patch of the input is convolved with a different set of filters.</obo:IAO_0000115>
        <oboInOwl:inSubset rdf:resource="https://w3id.org/aio/LayerSubset"/>
        <rdfs:comment>Locally-connected layer for 2D inputs. The LocallyConnected2D layer works similarly to the Conv2D layer, except that weights are unshared, that is, a different set of filters is applied at each different patch of the input.</rdfs:comment>
        <rdfs:label>LocallyConnected2D Layer</rdfs:label>
    </owl:Class>
    <owl:Axiom>
        <owl:annotatedSource rdf:resource="https://w3id.org/aio/LocallyConnected2DLayer"/>
        <owl:annotatedProperty rdf:resource="http://purl.obolibrary.org/obo/IAO_0000115"/>
        <owl:annotatedTarget>A locally-connected layer for 2D inputs where each patch of the input is convolved with a different set of filters.</owl:annotatedTarget>
        <oboInOwl:hasDbXref rdf:resource="https://www.tensorflow.org/api_docs/python/tf/keras/layers/LocallyConnected2D"/>
    </owl:Axiom>
    


    <!-- https://w3id.org/aio/LocallyconnectedLayer -->

    <owl:Class rdf:about="https://w3id.org/aio/LocallyconnectedLayer">
        <rdfs:subClassOf rdf:resource="https://w3id.org/aio/Layer"/>
        <obo:IAO_0000115>A layer that works similarly to the Convolution1D layer, except that weights are unshared, that is, a different set of filters is applied at each different patch of the input.</obo:IAO_0000115>
        <oboInOwl:inSubset rdf:resource="https://w3id.org/aio/LayerSubset"/>
        <rdfs:label>Locally-connected Layer</rdfs:label>
    </owl:Class>
    <owl:Axiom>
        <owl:annotatedSource rdf:resource="https://w3id.org/aio/LocallyconnectedLayer"/>
        <owl:annotatedProperty rdf:resource="http://purl.obolibrary.org/obo/IAO_0000115"/>
        <owl:annotatedTarget>A layer that works similarly to the Convolution1D layer, except that weights are unshared, that is, a different set of filters is applied at each different patch of the input.</owl:annotatedTarget>
        <oboInOwl:hasDbXref rdf:resource="https://faroit.com/keras-docs/1.2.2/layers/local/"/>
    </owl:Axiom>
    


    <!-- https://w3id.org/aio/LogisticRegression -->

    <owl:Class rdf:about="https://w3id.org/aio/LogisticRegression">
        <rdfs:subClassOf rdf:resource="https://w3id.org/aio/RegressionAnalysis"/>
        <obo:IAO_0000115>A regression analysis model that estimates the probability of an event occurring by modeling the log-odds of the event as a linear combination of one or more independent variables.</obo:IAO_0000115>
        <oboInOwl:inSubset rdf:resource="https://w3id.org/aio/MachineLearningSubset"/>
        <rdfs:label>Logistic Regression</rdfs:label>
    </owl:Class>
    <owl:Axiom>
        <owl:annotatedSource rdf:resource="https://w3id.org/aio/LogisticRegression"/>
        <owl:annotatedProperty rdf:resource="http://purl.obolibrary.org/obo/IAO_0000115"/>
        <owl:annotatedTarget>A regression analysis model that estimates the probability of an event occurring by modeling the log-odds of the event as a linear combination of one or more independent variables.</owl:annotatedTarget>
        <oboInOwl:hasDbXref rdf:resource="https://en.wikipedia.org/wiki/Logistic_regression"/>
    </owl:Axiom>
    


    <!-- https://w3id.org/aio/LongShortTermMemory -->

    <owl:Class rdf:about="https://w3id.org/aio/LongShortTermMemory">
        <rdfs:subClassOf rdf:resource="https://w3id.org/aio/RecurrentNeuralNetwork"/>
        <rdfs:subClassOf>
            <owl:Restriction>
                <owl:onProperty rdf:resource="http://purl.obolibrary.org/obo/BFO_0000051"/>
                <owl:someValuesFrom rdf:resource="https://w3id.org/aio/InputLayer"/>
            </owl:Restriction>
        </rdfs:subClassOf>
        <rdfs:subClassOf>
            <owl:Restriction>
                <owl:onProperty rdf:resource="http://purl.obolibrary.org/obo/BFO_0000051"/>
                <owl:someValuesFrom rdf:resource="https://w3id.org/aio/MemoryCellLayer"/>
            </owl:Restriction>
        </rdfs:subClassOf>
        <rdfs:subClassOf>
            <owl:Restriction>
                <owl:onProperty rdf:resource="http://purl.obolibrary.org/obo/BFO_0000051"/>
                <owl:someValuesFrom rdf:resource="https://w3id.org/aio/OutputLayer"/>
            </owl:Restriction>
        </rdfs:subClassOf>
        <obo:IAO_0000115>A recurrent neural network with feedback connections that processes entire sequences of data.</obo:IAO_0000115>
        <oboInOwl:hasExactSynonym>LSTM</oboInOwl:hasExactSynonym>
        <oboInOwl:inSubset rdf:resource="https://w3id.org/aio/NetworkSubset"/>
        <rdfs:comment>Layers: Input, Memory Cell, Output</rdfs:comment>
        <rdfs:label>Long Short Term Memory</rdfs:label>
    </owl:Class>
    <owl:Axiom>
        <owl:annotatedSource rdf:resource="https://w3id.org/aio/LongShortTermMemory"/>
        <owl:annotatedProperty rdf:resource="http://purl.obolibrary.org/obo/IAO_0000115"/>
        <owl:annotatedTarget>A recurrent neural network with feedback connections that processes entire sequences of data.</owl:annotatedTarget>
        <oboInOwl:hasDbXref rdf:resource="https://en.wikipedia.org/wiki/Long_short-term_memory"/>
    </owl:Axiom>
    


    <!-- https://w3id.org/aio/LossOfSituationalAwarenessBias -->

    <owl:Class rdf:about="https://w3id.org/aio/LossOfSituationalAwarenessBias">
        <rdfs:subClassOf rdf:resource="https://w3id.org/aio/IndividualBias"/>
        <obo:IAO_0000115>An individual bias occurring when automation leads to humans being unaware of their situation making them unprepared to assume control in cooperative systems.</obo:IAO_0000115>
        <oboInOwl:inSubset rdf:resource="https://w3id.org/aio/BiasSubset"/>
        <rdfs:label>Loss Of Situational Awareness Bias</rdfs:label>
    </owl:Class>
    <owl:Axiom>
        <owl:annotatedSource rdf:resource="https://w3id.org/aio/LossOfSituationalAwarenessBias"/>
        <owl:annotatedProperty rdf:resource="http://purl.obolibrary.org/obo/IAO_0000115"/>
        <owl:annotatedTarget>An individual bias occurring when automation leads to humans being unaware of their situation making them unprepared to assume control in cooperative systems.</owl:annotatedTarget>
        <oboInOwl:hasDbXref rdf:resource="https://doi.org/10.6028/NIST.SP.1270"/>
    </owl:Axiom>
    


    <!-- https://w3id.org/aio/LowResourceLLM -->

    <owl:Class rdf:about="https://w3id.org/aio/LowResourceLLM">
        <rdfs:subClassOf rdf:resource="https://w3id.org/aio/LargeLanguageModel"/>
        <obo:IAO_0000115>A LLM which is optimized for performance in scenarios with limited data, computational resources, or for languages with sparse datasets.</obo:IAO_0000115>
        <oboInOwl:hasExactSynonym>Low-Resource Language Model</oboInOwl:hasExactSynonym>
        <oboInOwl:hasRelatedSynonym>low-resource languages</oboInOwl:hasRelatedSynonym>
        <oboInOwl:hasRelatedSynonym>resource-efficient</oboInOwl:hasRelatedSynonym>
        <oboInOwl:inSubset rdf:resource="https://w3id.org/aio/ModelSubset"/>
        <rdfs:label>Low-Resource LLM</rdfs:label>
    </owl:Class>
    


    <!-- https://w3id.org/aio/MachineLearning -->

    <owl:Class rdf:about="https://w3id.org/aio/MachineLearning">
        <rdfs:subClassOf rdf:resource="http://www.w3.org/2002/07/owl#Thing"/>
        <obo:IAO_0000115>A field of inquiry devoted to understanding and building methods that learn from data to improve performance on a set of tasks.</obo:IAO_0000115>
        <oboInOwl:inSubset rdf:resource="https://w3id.org/aio/MachineLearningSubset"/>
        <rdfs:label>Machine Learning</rdfs:label>
    </owl:Class>
    <owl:Axiom>
        <owl:annotatedSource rdf:resource="https://w3id.org/aio/MachineLearning"/>
        <owl:annotatedProperty rdf:resource="http://purl.obolibrary.org/obo/IAO_0000115"/>
        <owl:annotatedTarget>A field of inquiry devoted to understanding and building methods that learn from data to improve performance on a set of tasks.</owl:annotatedTarget>
        <oboInOwl:hasDbXref rdf:resource="https://doi.org/10.6028/NIST.SP.1270"/>
    </owl:Axiom>
    


    <!-- https://w3id.org/aio/ManifoldLearning -->

    <owl:Class rdf:about="https://w3id.org/aio/ManifoldLearning">
        <rdfs:subClassOf rdf:resource="https://w3id.org/aio/DimensionalityReduction"/>
        <obo:IAO_0000115>A dimensionality reduction method based on the assumption that observed data lie on a low-dimensional manifold embedded in a higher-dimensional space.</obo:IAO_0000115>
        <oboInOwl:inSubset rdf:resource="https://w3id.org/aio/MachineLearningSubset"/>
        <rdfs:label>Manifold Learning</rdfs:label>
    </owl:Class>
    <owl:Axiom>
        <owl:annotatedSource rdf:resource="https://w3id.org/aio/ManifoldLearning"/>
        <owl:annotatedProperty rdf:resource="http://purl.obolibrary.org/obo/IAO_0000115"/>
        <owl:annotatedTarget>A dimensionality reduction method based on the assumption that observed data lie on a low-dimensional manifold embedded in a higher-dimensional space.</owl:annotatedTarget>
        <oboInOwl:hasDbXref rdf:resource="https://arxiv.org/abs/2011.01307"/>
    </owl:Axiom>
    


    <!-- https://w3id.org/aio/MarkovChain -->

    <owl:Class rdf:about="https://w3id.org/aio/MarkovChain">
        <rdfs:subClassOf rdf:resource="https://w3id.org/aio/Network"/>
        <rdfs:subClassOf>
            <owl:Restriction>
                <owl:onProperty rdf:resource="http://purl.obolibrary.org/obo/BFO_0000051"/>
                <owl:someValuesFrom rdf:resource="https://w3id.org/aio/ProbabilisticHiddenLayer"/>
            </owl:Restriction>
        </rdfs:subClassOf>
        <obo:IAO_0000115>A network that is a stochastic model describing a sequence of possible events where the probability of each event depends only on the previous event&apos;s state.</obo:IAO_0000115>
        <oboInOwl:hasExactSynonym>MC</oboInOwl:hasExactSynonym>
        <oboInOwl:hasExactSynonym>MP</oboInOwl:hasExactSynonym>
        <oboInOwl:hasExactSynonym>Markov Process</oboInOwl:hasExactSynonym>
        <oboInOwl:inSubset rdf:resource="https://w3id.org/aio/ModelSubset"/>
        <rdfs:comment>Layers: Probalistic Hidden</rdfs:comment>
        <rdfs:label>Markov Chain</rdfs:label>
    </owl:Class>
    <owl:Axiom>
        <owl:annotatedSource rdf:resource="https://w3id.org/aio/MarkovChain"/>
        <owl:annotatedProperty rdf:resource="http://purl.obolibrary.org/obo/IAO_0000115"/>
        <owl:annotatedTarget>A network that is a stochastic model describing a sequence of possible events where the probability of each event depends only on the previous event&apos;s state.</owl:annotatedTarget>
        <oboInOwl:hasDbXref rdf:resource="https://en.wikipedia.org/wiki/Markov_chain"/>
    </owl:Axiom>
    


    <!-- https://w3id.org/aio/MaskedLanguageModel -->

    <owl:Class rdf:about="https://w3id.org/aio/MaskedLanguageModel">
        <rdfs:subClassOf rdf:resource="https://w3id.org/aio/LanguageModel"/>
        <obo:IAO_0000115>A language model that is trained to predict randomly masked tokens in a sequence based on the remaining unmasked tokens allowing it to build deep bidirectional representations that can be effectively transferred to various NLP tasks via fine-tuning.</obo:IAO_0000115>
        <oboInOwl:hasRelatedSynonym>bidirectional encoder</oboInOwl:hasRelatedSynonym>
        <oboInOwl:hasRelatedSynonym>denoising autoencoder</oboInOwl:hasRelatedSynonym>
        <oboInOwl:inSubset rdf:resource="https://w3id.org/aio/ModelSubset"/>
        <rdfs:label>Masked Language Model</rdfs:label>
    </owl:Class>
    


    <!-- https://w3id.org/aio/MaskingLayer -->

    <owl:Class rdf:about="https://w3id.org/aio/MaskingLayer">
        <rdfs:subClassOf rdf:resource="https://w3id.org/aio/Layer"/>
        <obo:IAO_0000115>A layer that masks a sequence by using a mask value to skip timesteps.</obo:IAO_0000115>
        <oboInOwl:inSubset rdf:resource="https://w3id.org/aio/LayerSubset"/>
        <rdfs:comment>Masks a sequence by using a mask value to skip timesteps. For each timestep in the input tensor (dimension #1 in the tensor), if all values in the input tensor at that timestep are equal to mask_value, then the timestep will be masked (skipped) in all downstream layers (as long as they support masking). If any downstream layer does not support masking yet receives such an input mask, an exception will be raised.</rdfs:comment>
        <rdfs:label>Masking Layer</rdfs:label>
    </owl:Class>
    <owl:Axiom>
        <owl:annotatedSource rdf:resource="https://w3id.org/aio/MaskingLayer"/>
        <owl:annotatedProperty rdf:resource="http://purl.obolibrary.org/obo/IAO_0000115"/>
        <owl:annotatedTarget>A layer that masks a sequence by using a mask value to skip timesteps.</owl:annotatedTarget>
        <oboInOwl:hasDbXref rdf:resource="https://www.tensorflow.org/api_docs/python/tf/keras/layers/Masking"/>
    </owl:Axiom>
    


    <!-- https://w3id.org/aio/MatchedInputOutputLayer -->

    <owl:Class rdf:about="https://w3id.org/aio/MatchedInputOutputLayer">
        <rdfs:subClassOf rdf:resource="https://w3id.org/aio/InputLayer"/>
        <obo:IAO_0000115>An input layer with a shape corresponding to that of the output layer.</obo:IAO_0000115>
        <oboInOwl:inSubset rdf:resource="https://w3id.org/aio/LayerSubset"/>
        <rdfs:label>Matched Input-Output Layer</rdfs:label>
    </owl:Class>
    


    <!-- https://w3id.org/aio/MaxPooling1DLayer -->

    <owl:Class rdf:about="https://w3id.org/aio/MaxPooling1DLayer">
        <rdfs:subClassOf rdf:resource="https://w3id.org/aio/PoolingLayer"/>
        <obo:IAO_0000115>A pooling layer that performs max pooling operation for temporal data.</obo:IAO_0000115>
        <oboInOwl:hasExactSynonym>MaxPool1D</oboInOwl:hasExactSynonym>
        <oboInOwl:hasExactSynonym>MaxPooling1D</oboInOwl:hasExactSynonym>
        <oboInOwl:inSubset rdf:resource="https://w3id.org/aio/LayerSubset"/>
        <rdfs:comment>Max pooling operation for 1D temporal data. Downsamples the input representation by taking the maximum value over a spatial window of size pool_size. The window is shifted by strides. The resulting output, when using the &quot;valid&quot; padding option, has a shape of: output_shape = (input_shape - pool_size + 1) / strides) The resulting output shape when using the &quot;same&quot; padding option is: output_shape = input_shape / strides.</rdfs:comment>
        <rdfs:label>MaxPooling1D Layer</rdfs:label>
    </owl:Class>
    <owl:Axiom>
        <owl:annotatedSource rdf:resource="https://w3id.org/aio/MaxPooling1DLayer"/>
        <owl:annotatedProperty rdf:resource="http://purl.obolibrary.org/obo/IAO_0000115"/>
        <owl:annotatedTarget>A pooling layer that performs max pooling operation for temporal data.</owl:annotatedTarget>
        <oboInOwl:hasDbXref rdf:resource="https://www.tensorflow.org/api_docs/python/tf/keras/layers/MaxPool1D"/>
    </owl:Axiom>
    


    <!-- https://w3id.org/aio/MaxPooling2DLayer -->

    <owl:Class rdf:about="https://w3id.org/aio/MaxPooling2DLayer">
        <rdfs:subClassOf rdf:resource="https://w3id.org/aio/PoolingLayer"/>
        <obo:IAO_0000115>A pooling layer that performs max pooling operation for spatial data.</obo:IAO_0000115>
        <oboInOwl:hasExactSynonym>MaxPool2D</oboInOwl:hasExactSynonym>
        <oboInOwl:hasExactSynonym>MaxPooling2D</oboInOwl:hasExactSynonym>
        <oboInOwl:inSubset rdf:resource="https://w3id.org/aio/LayerSubset"/>
        <rdfs:comment>Max pooling operation for 2D spatial data.</rdfs:comment>
        <rdfs:label>MaxPooling2D Layer</rdfs:label>
    </owl:Class>
    <owl:Axiom>
        <owl:annotatedSource rdf:resource="https://w3id.org/aio/MaxPooling2DLayer"/>
        <owl:annotatedProperty rdf:resource="http://purl.obolibrary.org/obo/IAO_0000115"/>
        <owl:annotatedTarget>A pooling layer that performs max pooling operation for spatial data.</owl:annotatedTarget>
        <oboInOwl:hasDbXref rdf:resource="https://www.tensorflow.org/api_docs/python/tf/keras/layers/MaxPool2D"/>
    </owl:Axiom>
    


    <!-- https://w3id.org/aio/MaxPooling3DLayer -->

    <owl:Class rdf:about="https://w3id.org/aio/MaxPooling3DLayer">
        <rdfs:subClassOf rdf:resource="https://w3id.org/aio/PoolingLayer"/>
        <obo:IAO_0000115>A pooling layer that performs max pooling operation for 3D data (spatial or spatio-temporal).</obo:IAO_0000115>
        <oboInOwl:hasExactSynonym>MaxPool3D</oboInOwl:hasExactSynonym>
        <oboInOwl:hasExactSynonym>MaxPooling3D</oboInOwl:hasExactSynonym>
        <oboInOwl:inSubset rdf:resource="https://w3id.org/aio/LayerSubset"/>
        <rdfs:comment>Max pooling operation for 3D data (spatial or spatio-temporal). Downsamples the input along its spatial dimensions (depth, height, and width) by taking the maximum value over an input window (of size defined by pool_size) for each channel of the input. The window is shifted by strides along each dimension.</rdfs:comment>
        <rdfs:label>MaxPooling3D Layer</rdfs:label>
    </owl:Class>
    <owl:Axiom>
        <owl:annotatedSource rdf:resource="https://w3id.org/aio/MaxPooling3DLayer"/>
        <owl:annotatedProperty rdf:resource="http://purl.obolibrary.org/obo/IAO_0000115"/>
        <owl:annotatedTarget>A pooling layer that performs max pooling operation for 3D data (spatial or spatio-temporal).</owl:annotatedTarget>
        <oboInOwl:hasDbXref rdf:resource="https://www.tensorflow.org/api_docs/python/tf/keras/layers/MaxPool3D"/>
    </owl:Axiom>
    


    <!-- https://w3id.org/aio/MaxUnpool1DLayer -->

    <owl:Class rdf:about="https://w3id.org/aio/MaxUnpool1DLayer">
        <rdfs:subClassOf rdf:resource="https://w3id.org/aio/PoolingLayer"/>
        <obo:IAO_0000115>A pooling layer that computes a partial inverse of MaxPool1D.</obo:IAO_0000115>
        <oboInOwl:hasExactSynonym>MaxUnpool1D</oboInOwl:hasExactSynonym>
        <oboInOwl:inSubset rdf:resource="https://w3id.org/aio/LayerSubset"/>
        <rdfs:comment>Computes a partial inverse of MaxPool1D.</rdfs:comment>
        <rdfs:label>MaxUnpool1D Layer</rdfs:label>
    </owl:Class>
    <owl:Axiom>
        <owl:annotatedSource rdf:resource="https://w3id.org/aio/MaxUnpool1DLayer"/>
        <owl:annotatedProperty rdf:resource="http://purl.obolibrary.org/obo/IAO_0000115"/>
        <owl:annotatedTarget>A pooling layer that computes a partial inverse of MaxPool1D.</owl:annotatedTarget>
        <oboInOwl:hasDbXref rdf:resource="https://pytorch.org/docs/stable/nn.html#pooling-layers"/>
    </owl:Axiom>
    


    <!-- https://w3id.org/aio/MaxUnpool2DLayer -->

    <owl:Class rdf:about="https://w3id.org/aio/MaxUnpool2DLayer">
        <rdfs:subClassOf rdf:resource="https://w3id.org/aio/PoolingLayer"/>
        <obo:IAO_0000115>A pooling layer that computes a partial inverse of MaxPool2D.</obo:IAO_0000115>
        <oboInOwl:hasExactSynonym>MaxUnpool2D</oboInOwl:hasExactSynonym>
        <oboInOwl:inSubset rdf:resource="https://w3id.org/aio/LayerSubset"/>
        <rdfs:comment>Computes a partial inverse of MaxPool2D.</rdfs:comment>
        <rdfs:label>MaxUnpool2D Layer</rdfs:label>
    </owl:Class>
    <owl:Axiom>
        <owl:annotatedSource rdf:resource="https://w3id.org/aio/MaxUnpool2DLayer"/>
        <owl:annotatedProperty rdf:resource="http://purl.obolibrary.org/obo/IAO_0000115"/>
        <owl:annotatedTarget>A pooling layer that computes a partial inverse of MaxPool2D.</owl:annotatedTarget>
        <oboInOwl:hasDbXref rdf:resource="https://pytorch.org/docs/stable/nn.html#pooling-layers"/>
    </owl:Axiom>
    


    <!-- https://w3id.org/aio/MaxUnpool3DLayer -->

    <owl:Class rdf:about="https://w3id.org/aio/MaxUnpool3DLayer">
        <rdfs:subClassOf rdf:resource="https://w3id.org/aio/PoolingLayer"/>
        <obo:IAO_0000115>A pooling layer that computes a partial inverse of MaxPool3D.</obo:IAO_0000115>
        <oboInOwl:hasExactSynonym>MaxUnpool3D</oboInOwl:hasExactSynonym>
        <oboInOwl:inSubset rdf:resource="https://w3id.org/aio/LayerSubset"/>
        <rdfs:comment>Computes a partial inverse of MaxPool3D.</rdfs:comment>
        <rdfs:label>MaxUnpool3D Layer</rdfs:label>
    </owl:Class>
    <owl:Axiom>
        <owl:annotatedSource rdf:resource="https://w3id.org/aio/MaxUnpool3DLayer"/>
        <owl:annotatedProperty rdf:resource="http://purl.obolibrary.org/obo/IAO_0000115"/>
        <owl:annotatedTarget>A pooling layer that computes a partial inverse of MaxPool3D.</owl:annotatedTarget>
        <oboInOwl:hasDbXref rdf:resource="https://pytorch.org/docs/stable/nn.html#pooling-layers"/>
    </owl:Axiom>
    


    <!-- https://w3id.org/aio/MaximumLayer -->

    <owl:Class rdf:about="https://w3id.org/aio/MaximumLayer">
        <rdfs:subClassOf rdf:resource="https://w3id.org/aio/MergingLayer"/>
        <obo:IAO_0000115>A merging layer that computes the maximum (element-wise) of a list of inputs.</obo:IAO_0000115>
        <oboInOwl:inSubset rdf:resource="https://w3id.org/aio/LayerSubset"/>
        <rdfs:comment>Layer that computes the maximum (element-wise) a list of inputs. It takes as input a list of tensors, all of the same shape, and returns a single tensor (also of the same shape).</rdfs:comment>
        <rdfs:label>Maximum Layer</rdfs:label>
    </owl:Class>
    <owl:Axiom>
        <owl:annotatedSource rdf:resource="https://w3id.org/aio/MaximumLayer"/>
        <owl:annotatedProperty rdf:resource="http://purl.obolibrary.org/obo/IAO_0000115"/>
        <owl:annotatedTarget>A merging layer that computes the maximum (element-wise) of a list of inputs.</owl:annotatedTarget>
        <oboInOwl:hasDbXref rdf:resource="https://www.tensorflow.org/api_docs/python/tf/keras/layers/Maximum"/>
    </owl:Axiom>
    


    <!-- https://w3id.org/aio/MeasurementBias -->

    <owl:Class rdf:about="https://w3id.org/aio/MeasurementBias">
        <rdfs:subClassOf rdf:resource="https://w3id.org/aio/SelectionAndSamplingBias"/>
        <obo:IAO_0000115>A selection and sampling bias arising when features and labels are proxies for desired quantities potentially leading to differential performance.</obo:IAO_0000115>
        <oboInOwl:inSubset rdf:resource="https://w3id.org/aio/BiasSubset"/>
        <rdfs:label>Measurement Bias</rdfs:label>
    </owl:Class>
    <owl:Axiom>
        <owl:annotatedSource rdf:resource="https://w3id.org/aio/MeasurementBias"/>
        <owl:annotatedProperty rdf:resource="http://purl.obolibrary.org/obo/IAO_0000115"/>
        <owl:annotatedTarget>A selection and sampling bias arising when features and labels are proxies for desired quantities potentially leading to differential performance.</owl:annotatedTarget>
        <oboInOwl:hasDbXref rdf:resource="https://doi.org/10.6028/NIST.SP.1270"/>
    </owl:Axiom>
    


    <!-- https://w3id.org/aio/MemoryAugmentedLLM -->

    <owl:Class rdf:about="https://w3id.org/aio/MemoryAugmentedLLM">
        <rdfs:subClassOf rdf:resource="https://w3id.org/aio/LargeLanguageModel"/>
        <obo:IAO_0000115>A LLM which incorporates external writable and readable memory components, allowing it to store and retrieve information over long contexts.</obo:IAO_0000115>
        <oboInOwl:hasExactSynonym>Memory-Augmented Large Language Model</oboInOwl:hasExactSynonym>
        <oboInOwl:hasRelatedSynonym>external memory</oboInOwl:hasRelatedSynonym>
        <oboInOwl:inSubset rdf:resource="https://w3id.org/aio/ModelSubset"/>
        <rdfs:label>Memory-Augmented LLM</rdfs:label>
    </owl:Class>
    <owl:Axiom>
        <owl:annotatedSource rdf:resource="https://w3id.org/aio/MemoryAugmentedLLM"/>
        <owl:annotatedProperty rdf:resource="http://purl.obolibrary.org/obo/IAO_0000115"/>
        <owl:annotatedTarget>A LLM which incorporates external writable and readable memory components, allowing it to store and retrieve information over long contexts.</owl:annotatedTarget>
        <oboInOwl:hasDbXref rdf:resource="https://arxiv.org/abs/2306.07174"/>
    </owl:Axiom>
    


    <!-- https://w3id.org/aio/MemoryCellLayer -->

    <owl:Class rdf:about="https://w3id.org/aio/MemoryCellLayer">
        <rdfs:subClassOf rdf:resource="https://w3id.org/aio/Layer"/>
        <obo:IAO_0000115>A layer of cells, each with an internal state or weights.</obo:IAO_0000115>
        <oboInOwl:inSubset rdf:resource="https://w3id.org/aio/LayerSubset"/>
        <rdfs:label>Memory Cell Layer</rdfs:label>
    </owl:Class>
    <owl:Axiom>
        <owl:annotatedSource rdf:resource="https://w3id.org/aio/MemoryCellLayer"/>
        <owl:annotatedProperty rdf:resource="http://purl.obolibrary.org/obo/IAO_0000115"/>
        <owl:annotatedTarget>A layer of cells, each with an internal state or weights.</owl:annotatedTarget>
        <oboInOwl:hasDbXref rdf:resource="https://doi.org/10.1162/neco.1997.9.8.1735"/>
    </owl:Axiom>
    


    <!-- https://w3id.org/aio/MergingLayer -->

    <owl:Class rdf:about="https://w3id.org/aio/MergingLayer">
        <rdfs:subClassOf rdf:resource="https://w3id.org/aio/Layer"/>
        <obo:IAO_0000115>A layer used to merge a list of inputs.</obo:IAO_0000115>
        <oboInOwl:inSubset rdf:resource="https://w3id.org/aio/LayerSubset"/>
        <rdfs:label>Merging Layer</rdfs:label>
    </owl:Class>
    <owl:Axiom>
        <owl:annotatedSource rdf:resource="https://w3id.org/aio/MergingLayer"/>
        <owl:annotatedProperty rdf:resource="http://purl.obolibrary.org/obo/IAO_0000115"/>
        <owl:annotatedTarget>A layer used to merge a list of inputs.</owl:annotatedTarget>
        <oboInOwl:hasDbXref rdf:resource="https://www.tutorialspoint.com/keras/keras_merge_layer.htm"/>
    </owl:Axiom>
    


    <!-- https://w3id.org/aio/MetaLearning -->

    <owl:Class rdf:about="https://w3id.org/aio/MetaLearning">
        <rdfs:subClassOf rdf:resource="https://w3id.org/aio/MachineLearning"/>
        <obo:IAO_0000115>A machine learning that automatically learns from metadata about machine learning experiments.</obo:IAO_0000115>
        <oboInOwl:inSubset rdf:resource="https://w3id.org/aio/NetworkSubset"/>
        <rdfs:label>Meta-Learning</rdfs:label>
    </owl:Class>
    <owl:Axiom>
        <owl:annotatedSource rdf:resource="https://w3id.org/aio/MetaLearning"/>
        <owl:annotatedProperty rdf:resource="http://purl.obolibrary.org/obo/IAO_0000115"/>
        <owl:annotatedTarget>A machine learning that automatically learns from metadata about machine learning experiments.</owl:annotatedTarget>
        <oboInOwl:hasDbXref rdf:resource="https://doi.org/10.6028/NIST.SP.1270"/>
    </owl:Axiom>
    


    <!-- https://w3id.org/aio/MetaLearningLLM -->

    <owl:Class rdf:about="https://w3id.org/aio/MetaLearningLLM">
        <rdfs:subClassOf rdf:resource="https://w3id.org/aio/LargeLanguageModel"/>
        <obo:IAO_0000115>A LLM which is trained in a way that allows it to quickly adapt to new tasks or datasets through only a few examples or fine-tuning steps, leveraging meta-learned priors about how to efficiently learn.</obo:IAO_0000115>
        <oboInOwl:hasExactSynonym>Meta-Learning Large Language Model</oboInOwl:hasExactSynonym>
        <oboInOwl:hasRelatedSynonym>few-shot adaptation</oboInOwl:hasRelatedSynonym>
        <oboInOwl:hasRelatedSynonym>learning to learn</oboInOwl:hasRelatedSynonym>
        <oboInOwl:inSubset rdf:resource="https://w3id.org/aio/ModelSubset"/>
        <rdfs:label>Meta-Learning LLM</rdfs:label>
    </owl:Class>
    


    <!-- https://w3id.org/aio/MetricLearning -->

    <owl:Class rdf:about="https://w3id.org/aio/MetricLearning">
        <rdfs:subClassOf rdf:resource="https://w3id.org/aio/DeepNeuralNetwork"/>
        <obo:IAO_0000115>A deep neural network that learns a representation function mapping objects into an embedded space.</obo:IAO_0000115>
        <oboInOwl:hasExactSynonym>Distance Metric Learning</oboInOwl:hasExactSynonym>
        <oboInOwl:inSubset rdf:resource="https://w3id.org/aio/NetworkSubset"/>
        <rdfs:comment>Learning a representation function that maps objects into an embedded space.</rdfs:comment>
        <rdfs:label>Metric Learning</rdfs:label>
    </owl:Class>
    <owl:Axiom>
        <owl:annotatedSource rdf:resource="https://w3id.org/aio/MetricLearning"/>
        <owl:annotatedProperty rdf:resource="http://purl.obolibrary.org/obo/IAO_0000115"/>
        <owl:annotatedTarget>A deep neural network that learns a representation function mapping objects into an embedded space.</owl:annotatedTarget>
        <oboInOwl:hasDbXref rdf:resource="https://paperswithcode.com/task/metric-learning"/>
    </owl:Axiom>
    


    <!-- https://w3id.org/aio/MinimumLayer -->

    <owl:Class rdf:about="https://w3id.org/aio/MinimumLayer">
        <rdfs:subClassOf rdf:resource="https://w3id.org/aio/MergingLayer"/>
        <obo:IAO_0000115>A merging layer that computes the minimum (element-wise) of a list of inputs.</obo:IAO_0000115>
        <oboInOwl:inSubset rdf:resource="https://w3id.org/aio/LayerSubset"/>
        <rdfs:comment>Layer that computes the minimum (element-wise) a list of inputs. It takes as input a list of tensors, all of the same shape, and returns a single tensor (also of the same shape).</rdfs:comment>
        <rdfs:label>Minimum Layer</rdfs:label>
    </owl:Class>
    <owl:Axiom>
        <owl:annotatedSource rdf:resource="https://w3id.org/aio/MinimumLayer"/>
        <owl:annotatedProperty rdf:resource="http://purl.obolibrary.org/obo/IAO_0000115"/>
        <owl:annotatedTarget>A merging layer that computes the minimum (element-wise) of a list of inputs.</owl:annotatedTarget>
        <oboInOwl:hasDbXref rdf:resource="https://www.tensorflow.org/api_docs/python/tf/keras/layers/Minimum"/>
    </owl:Axiom>
    


    <!-- https://w3id.org/aio/MixtureofExpertsLLM -->

    <owl:Class rdf:about="https://w3id.org/aio/MixtureofExpertsLLM">
        <rdfs:subClassOf rdf:resource="https://w3id.org/aio/LargeLanguageModel"/>
        <obo:IAO_0000115>A LLM which dynamically selects and combines outputs from multiple expert submodels, allowing for efficient scaling by conditionally activating only a subset of model components for each input.</obo:IAO_0000115>
        <oboInOwl:hasExactSynonym>Mixture-of-Experts Large Language Model</oboInOwl:hasExactSynonym>
        <oboInOwl:hasExactSynonym>MoE Large Language Model</oboInOwl:hasExactSynonym>
        <oboInOwl:hasRelatedSynonym>conditional computation</oboInOwl:hasRelatedSynonym>
        <oboInOwl:hasRelatedSynonym>model parallelism</oboInOwl:hasRelatedSynonym>
        <oboInOwl:inSubset rdf:resource="https://w3id.org/aio/ModelSubset"/>
        <rdfs:label>Mixture-of-Experts LLM</rdfs:label>
    </owl:Class>
    <owl:Axiom>
        <owl:annotatedSource rdf:resource="https://w3id.org/aio/MixtureofExpertsLLM"/>
        <owl:annotatedProperty rdf:resource="http://purl.obolibrary.org/obo/IAO_0000115"/>
        <owl:annotatedTarget>A LLM which dynamically selects and combines outputs from multiple expert submodels, allowing for efficient scaling by conditionally activating only a subset of model components for each input.</owl:annotatedTarget>
        <oboInOwl:hasDbXref rdf:resource="https://proceedings.mlr.press/v162/du22c.html"/>
    </owl:Axiom>
    


    <!-- https://w3id.org/aio/ModeConfusionBias -->

    <owl:Class rdf:about="https://w3id.org/aio/ModeConfusionBias">
        <rdfs:subClassOf rdf:resource="https://w3id.org/aio/IndividualBias"/>
        <obo:IAO_0000115>A bias occurring when modal interfaces confuse human operators causing actions appropriate for a different mode but incorrect for the current situation.</obo:IAO_0000115>
        <oboInOwl:inSubset rdf:resource="https://w3id.org/aio/BiasSubset"/>
        <rdfs:label>Mode Confusion Bias</rdfs:label>
    </owl:Class>
    <owl:Axiom>
        <owl:annotatedSource rdf:resource="https://w3id.org/aio/ModeConfusionBias"/>
        <owl:annotatedProperty rdf:resource="http://purl.obolibrary.org/obo/IAO_0000115"/>
        <owl:annotatedTarget>A bias occurring when modal interfaces confuse human operators causing actions appropriate for a different mode but incorrect for the current situation.</owl:annotatedTarget>
        <oboInOwl:hasDbXref rdf:resource="https://doi.org/10.6028/NIST.SP.1270"/>
    </owl:Axiom>
    


    <!-- https://w3id.org/aio/Model -->

    <owl:Class rdf:about="https://w3id.org/aio/Model">
        <rdfs:subClassOf rdf:resource="http://www.w3.org/2002/07/owl#Thing"/>
        <obo:IAO_0000115>An abstract representation of a complex system generally assembled as a set of logical mathematical or conceptual properties to simulate or understand the system&apos;s behavior.</obo:IAO_0000115>
        <oboInOwl:inSubset rdf:resource="https://w3id.org/aio/ModelSubset"/>
        <rdfs:label>Model</rdfs:label>
    </owl:Class>
    <owl:Axiom>
        <owl:annotatedSource rdf:resource="https://w3id.org/aio/Model"/>
        <owl:annotatedProperty rdf:resource="http://purl.obolibrary.org/obo/IAO_0000115"/>
        <owl:annotatedTarget>An abstract representation of a complex system generally assembled as a set of logical mathematical or conceptual properties to simulate or understand the system&apos;s behavior.</owl:annotatedTarget>
        <oboInOwl:hasDbXref rdf:resource="https://en.wikipedia.org/wiki/Mathematical_model"/>
    </owl:Axiom>
    


    <!-- https://w3id.org/aio/ModelEfficiency -->

    <owl:Class rdf:about="https://w3id.org/aio/ModelEfficiency">
        <rdfs:subClassOf rdf:resource="https://w3id.org/aio/Preprocessing"/>
        <obo:IAO_0000115>Techniques aimed at making models more efficient such as knowledge distillation.</obo:IAO_0000115>
        <oboInOwl:hasExactSynonym>Computational Efficiency</oboInOwl:hasExactSynonym>
        <oboInOwl:hasExactSynonym>Model Optimization</oboInOwl:hasExactSynonym>
        <oboInOwl:inSubset rdf:resource="https://w3id.org/aio/PreprocessingSubset"/>
        <rdfs:label>Model Efficiency</rdfs:label>
    </owl:Class>
    <owl:Axiom>
        <owl:annotatedSource rdf:resource="https://w3id.org/aio/ModelEfficiency"/>
        <owl:annotatedProperty rdf:resource="http://purl.obolibrary.org/obo/IAO_0000115"/>
        <owl:annotatedTarget>Techniques aimed at making models more efficient such as knowledge distillation.</owl:annotatedTarget>
        <oboInOwl:hasDbXref rdf:resource="https://doi.org/10.1145/3578938"/>
    </owl:Axiom>
    


    <!-- https://w3id.org/aio/ModelSelectionBias -->

    <owl:Class rdf:about="https://w3id.org/aio/ModelSelectionBias">
        <rdfs:subClassOf rdf:resource="https://w3id.org/aio/ProcessingBias"/>
        <obo:IAO_0000115>A processing bias introduced when using data to select a single &quot;best&quot; model from many or when an explanatory variable has a weak relationship with the response variable.</obo:IAO_0000115>
        <oboInOwl:inSubset rdf:resource="https://w3id.org/aio/BiasSubset"/>
        <rdfs:label>Model Selection Bias</rdfs:label>
    </owl:Class>
    <owl:Axiom>
        <owl:annotatedSource rdf:resource="https://w3id.org/aio/ModelSelectionBias"/>
        <owl:annotatedProperty rdf:resource="http://purl.obolibrary.org/obo/IAO_0000115"/>
        <owl:annotatedTarget>A processing bias introduced when using data to select a single &quot;best&quot; model from many or when an explanatory variable has a weak relationship with the response variable.</owl:annotatedTarget>
        <oboInOwl:hasDbXref rdf:resource="https://doi.org/10.6028/NIST.SP.1270"/>
    </owl:Axiom>
    


    <!-- https://w3id.org/aio/ModularLLM -->

    <owl:Class rdf:about="https://w3id.org/aio/ModularLLM">
        <rdfs:subClassOf rdf:resource="https://w3id.org/aio/ModularLanguageModel"/>
        <obo:IAO_0000115>A modular large language model that consists of multiple specialized components or skills that can be dynamically composed and recombined to solve complex tasks mimicking the modular structure of human cognition.</obo:IAO_0000115>
        <oboInOwl:hasExactSynonym>Modular Large Language Model</oboInOwl:hasExactSynonym>
        <oboInOwl:hasRelatedSynonym>component skills</oboInOwl:hasRelatedSynonym>
        <oboInOwl:hasRelatedSynonym>skill composition</oboInOwl:hasRelatedSynonym>
        <oboInOwl:inSubset rdf:resource="https://w3id.org/aio/ModelSubset"/>
        <rdfs:label>Modular LLM</rdfs:label>
    </owl:Class>
    <owl:Axiom>
        <owl:annotatedSource rdf:resource="https://w3id.org/aio/ModularLLM"/>
        <owl:annotatedProperty rdf:resource="http://purl.obolibrary.org/obo/IAO_0000115"/>
        <owl:annotatedTarget>A modular large language model that consists of multiple specialized components or skills that can be dynamically composed and recombined to solve complex tasks mimicking the modular structure of human cognition.</owl:annotatedTarget>
        <oboInOwl:hasDbXref rdf:resource="https://arxiv.org/abs/2302.11529v2"/>
    </owl:Axiom>
    


    <!-- https://w3id.org/aio/ModularLanguageModel -->

    <owl:Class rdf:about="https://w3id.org/aio/ModularLanguageModel">
        <rdfs:subClassOf rdf:resource="https://w3id.org/aio/LanguageModel"/>
        <obo:IAO_0000115>A language model that consists of multiple specialized components or skills that can be dynamically composed and recombined to solve complex tasks mimicking the modular structure of human cognition.</obo:IAO_0000115>
        <oboInOwl:hasExactSynonym>Modular LM</oboInOwl:hasExactSynonym>
        <oboInOwl:inSubset rdf:resource="https://w3id.org/aio/ModelSubset"/>
        <rdfs:label>Modular Language Model</rdfs:label>
    </owl:Class>
    <owl:Axiom>
        <owl:annotatedSource rdf:resource="https://w3id.org/aio/ModularLanguageModel"/>
        <owl:annotatedProperty rdf:resource="http://purl.obolibrary.org/obo/IAO_0000115"/>
        <owl:annotatedTarget>A language model that consists of multiple specialized components or skills that can be dynamically composed and recombined to solve complex tasks mimicking the modular structure of human cognition.</owl:annotatedTarget>
        <oboInOwl:hasDbXref rdf:resource="https://arxiv.org/abs/2302.11529v2"/>
    </owl:Axiom>
    


    <!-- https://w3id.org/aio/MultiHeadAttentionLayer -->

    <owl:Class rdf:about="https://w3id.org/aio/MultiHeadAttentionLayer">
        <rdfs:subClassOf rdf:resource="https://w3id.org/aio/AttentionLayer"/>
        <obo:IAO_0000115>An attention layer that allows the model to attend to information from different representation subspaces.</obo:IAO_0000115>
        <oboInOwl:inSubset rdf:resource="https://w3id.org/aio/LayerSubset"/>
        <rdfs:comment>MultiHeadAttention layer. This is an implementation of multi-headed attention as described in the paper &quot;Attention is all you Need&quot; (Vaswani et al., 2017). If query, key, value are the same, then this is self-attention. Each timestep in query attends to the corresponding sequence in key, and returns a fixed-width vector.This layer first projects query, key and value. These are (effectively) a list of tensors of length num_attention_heads, where the corresponding shapes are (batch_size, &lt;query dimensions&gt;, key_dim), (batch_size, &lt;key/value dimensions&gt;, key_dim), (batch_size, &lt;key/value dimensions&gt;, value_dim).Then, the query and key tensors are dot-producted and scaled. These are softmaxed to obtain attention probabilities. The value tensors are then interpolated by these probabilities, then concatenated back to a single tensor. Finally, the result tensor with the last dimension as value_dim can take an linear projection and return. When using MultiHeadAttention inside a custom Layer, the custom Layer must implement build() and call MultiHeadAttention&apos;s _build_from_signature(). This enables weights to be restored correctly when the model is loaded.</rdfs:comment>
        <rdfs:label>MultiHeadAttention Layer</rdfs:label>
    </owl:Class>
    <owl:Axiom>
        <owl:annotatedSource rdf:resource="https://w3id.org/aio/MultiHeadAttentionLayer"/>
        <owl:annotatedProperty rdf:resource="http://purl.obolibrary.org/obo/IAO_0000115"/>
        <owl:annotatedTarget>An attention layer that allows the model to attend to information from different representation subspaces.</owl:annotatedTarget>
        <oboInOwl:hasDbXref rdf:resource="https://www.tensorflow.org/api_docs/python/tf/keras/layers/MultiHeadAttention"/>
    </owl:Axiom>
    


    <!-- https://w3id.org/aio/MultiTaskLLM -->

    <owl:Class rdf:about="https://w3id.org/aio/MultiTaskLLM">
        <rdfs:subClassOf rdf:resource="https://w3id.org/aio/LargeLanguageModel"/>
        <obo:IAO_0000115>A LLM which is trained jointly on multiple language tasks simultaneously, learning shared representations that transfer across tasks.</obo:IAO_0000115>
        <oboInOwl:hasExactSynonym>Multi-Task Large Language Model</oboInOwl:hasExactSynonym>
        <oboInOwl:hasRelatedSynonym>transfer learning</oboInOwl:hasRelatedSynonym>
        <oboInOwl:inSubset rdf:resource="https://w3id.org/aio/ModelSubset"/>
        <rdfs:label>Multi-Task LLM</rdfs:label>
    </owl:Class>
    


    <!-- https://w3id.org/aio/MulticlassClassification -->

    <owl:Class rdf:about="https://w3id.org/aio/MulticlassClassification">
        <rdfs:subClassOf rdf:resource="https://w3id.org/aio/Classification"/>
        <obo:IAO_0000115>A machine learning task focused on methods that classify instances into one of three or more classes.</obo:IAO_0000115>
        <oboInOwl:hasExactSynonym>Multinomial Classification</oboInOwl:hasExactSynonym>
        <oboInOwl:inSubset rdf:resource="https://w3id.org/aio/MachineLearningSubset"/>
        <rdfs:comment>Methods that classify instances into one of three or more classes.</rdfs:comment>
        <rdfs:label>Multiclass Classification</rdfs:label>
    </owl:Class>
    <owl:Axiom>
        <owl:annotatedSource rdf:resource="https://w3id.org/aio/MulticlassClassification"/>
        <owl:annotatedProperty rdf:resource="http://purl.obolibrary.org/obo/IAO_0000115"/>
        <owl:annotatedTarget>A machine learning task focused on methods that classify instances into one of three or more classes.</owl:annotatedTarget>
        <oboInOwl:hasDbXref rdf:resource="https://en.wikipedia.org/wiki/Multiclass_classification"/>
    </owl:Axiom>
    


    <!-- https://w3id.org/aio/MultidimensionalScaling -->

    <owl:Class rdf:about="https://w3id.org/aio/MultidimensionalScaling">
        <rdfs:subClassOf rdf:resource="https://w3id.org/aio/DimensionalityReduction"/>
        <obo:IAO_0000115>A dimensionality reduction method that translates information about the pairwise distances among a set of objects or individuals into a configuration of points mapped into an abstract Cartesian space.</obo:IAO_0000115>
        <oboInOwl:hasExactSynonym>MDS</oboInOwl:hasExactSynonym>
        <oboInOwl:inSubset rdf:resource="https://w3id.org/aio/MachineLearningSubset"/>
        <rdfs:label>Multidimensional Scaling</rdfs:label>
    </owl:Class>
    <owl:Axiom>
        <owl:annotatedSource rdf:resource="https://w3id.org/aio/MultidimensionalScaling"/>
        <owl:annotatedProperty rdf:resource="http://purl.obolibrary.org/obo/IAO_0000115"/>
        <owl:annotatedTarget>A dimensionality reduction method that translates information about the pairwise distances among a set of objects or individuals into a configuration of points mapped into an abstract Cartesian space.</owl:annotatedTarget>
        <oboInOwl:hasDbXref rdf:resource="https://en.wikipedia.org/wiki/Multidimensional_scaling"/>
    </owl:Axiom>
    


    <!-- https://w3id.org/aio/MultilingualLLM -->

    <owl:Class rdf:about="https://w3id.org/aio/MultilingualLLM">
        <rdfs:subClassOf rdf:resource="https://w3id.org/aio/LargeLanguageModel"/>
        <obo:IAO_0000115>A large language model that is trained on text from multiple languages learning shared representations that enable zero-shot or few-shot transfer to new languages.</obo:IAO_0000115>
        <oboInOwl:hasExactSynonym>Multilingual Large Language Model</oboInOwl:hasExactSynonym>
        <oboInOwl:hasRelatedSynonym>cross-lingual transfer</oboInOwl:hasRelatedSynonym>
        <oboInOwl:inSubset rdf:resource="https://w3id.org/aio/ModelSubset"/>
        <rdfs:label>Multilingual LLM</rdfs:label>
    </owl:Class>
    


    <!-- https://w3id.org/aio/MultimodalDeepLearning -->

    <owl:Class rdf:about="https://w3id.org/aio/MultimodalDeepLearning">
        <rdfs:subClassOf rdf:resource="https://w3id.org/aio/DeepNeuralNetwork"/>
        <obo:IAO_0000115>A deep neural network that processes and links information using various modalities.</obo:IAO_0000115>
        <oboInOwl:inSubset rdf:resource="https://w3id.org/aio/NetworkSubset"/>
        <rdfs:comment>Creating models that process and link information using various modalities.</rdfs:comment>
        <rdfs:label>Multimodal Deep Learning</rdfs:label>
    </owl:Class>
    <owl:Axiom>
        <owl:annotatedSource rdf:resource="https://w3id.org/aio/MultimodalDeepLearning"/>
        <owl:annotatedProperty rdf:resource="http://purl.obolibrary.org/obo/IAO_0000115"/>
        <owl:annotatedTarget>A deep neural network that processes and links information using various modalities.</owl:annotatedTarget>
        <oboInOwl:hasDbXref rdf:resource="https://arxiv.org/abs/2105.11087"/>
    </owl:Axiom>
    


    <!-- https://w3id.org/aio/MultimodalFusionLLM -->

    <owl:Class rdf:about="https://w3id.org/aio/MultimodalFusionLLM">
        <rdfs:subClassOf rdf:resource="https://w3id.org/aio/LargeLanguageModel"/>
        <obo:IAO_0000115>A large language model that learns joint representations across different modalities like text vision and audio in an end-to-end fashion for better cross-modal understanding and generation.</obo:IAO_0000115>
        <oboInOwl:hasRelatedSynonym>cross-modal grounding</oboInOwl:hasRelatedSynonym>
        <oboInOwl:inSubset rdf:resource="https://w3id.org/aio/ModelSubset"/>
        <rdfs:label>Multimodal Fusion LLM</rdfs:label>
    </owl:Class>
    


    <!-- https://w3id.org/aio/MultimodalLLM -->

    <owl:Class rdf:about="https://w3id.org/aio/MultimodalLLM">
        <rdfs:subClassOf rdf:resource="https://w3id.org/aio/MultimodalLanguageModel"/>
        <obo:IAO_0000115>A multimodal large language model that learns joint representations across different modalities like text vision and audio in an end-to-end fashion for better cross-modal understanding and generation.</obo:IAO_0000115>
        <oboInOwl:hasExactSynonym>Multimodal Large Language Model</oboInOwl:hasExactSynonym>
        <oboInOwl:hasRelatedSynonym>cross-modal grounding</oboInOwl:hasRelatedSynonym>
        <oboInOwl:inSubset rdf:resource="https://w3id.org/aio/ModelSubset"/>
        <rdfs:label>Multimodal LLM</rdfs:label>
    </owl:Class>
    <owl:Axiom>
        <owl:annotatedSource rdf:resource="https://w3id.org/aio/MultimodalLLM"/>
        <owl:annotatedProperty rdf:resource="http://purl.obolibrary.org/obo/IAO_0000115"/>
        <owl:annotatedTarget>A multimodal large language model that learns joint representations across different modalities like text vision and audio in an end-to-end fashion for better cross-modal understanding and generation.</owl:annotatedTarget>
        <oboInOwl:hasDbXref rdf:resource="https://arxiv.org/abs/2303.17580"/>
    </owl:Axiom>
    


    <!-- https://w3id.org/aio/MultimodalLanguageModel -->

    <owl:Class rdf:about="https://w3id.org/aio/MultimodalLanguageModel">
        <rdfs:subClassOf rdf:resource="https://w3id.org/aio/LanguageModel"/>
        <obo:IAO_0000115>A language model that learns joint representations across different modalities like text vision and audio in an end-to-end fashion for better cross-modal understanding and generation.</obo:IAO_0000115>
        <oboInOwl:hasExactSynonym>Mulimodal LM</oboInOwl:hasExactSynonym>
        <oboInOwl:inSubset rdf:resource="https://w3id.org/aio/ModelSubset"/>
        <rdfs:label>Multimodal Language Model</rdfs:label>
    </owl:Class>
    <owl:Axiom>
        <owl:annotatedSource rdf:resource="https://w3id.org/aio/MultimodalLanguageModel"/>
        <owl:annotatedProperty rdf:resource="http://purl.obolibrary.org/obo/IAO_0000115"/>
        <owl:annotatedTarget>A language model that learns joint representations across different modalities like text vision and audio in an end-to-end fashion for better cross-modal understanding and generation.</owl:annotatedTarget>
        <oboInOwl:hasDbXref rdf:resource="https://arxiv.org/abs/2205.12630"/>
    </owl:Axiom>
    


    <!-- https://w3id.org/aio/MultimodalLearning -->

    <owl:Class rdf:about="https://w3id.org/aio/MultimodalLearning">
        <rdfs:subClassOf rdf:resource="https://w3id.org/aio/MachineLearning"/>
        <obo:IAO_0000115>A type of machine learning that uses multiple modalities of data such as text audio and images to improve learning outcomes.</obo:IAO_0000115>
        <oboInOwl:inSubset rdf:resource="https://w3id.org/aio/NetworkSubset"/>
        <rdfs:comment>A type of deep learning that uses multiple modalities of data, such as text, audio, and images, to improve learning outcomes.</rdfs:comment>
        <rdfs:label>Multimodal Learning</rdfs:label>
    </owl:Class>
    <owl:Axiom>
        <owl:annotatedSource rdf:resource="https://w3id.org/aio/MultimodalLearning"/>
        <owl:annotatedProperty rdf:resource="http://purl.obolibrary.org/obo/IAO_0000115"/>
        <owl:annotatedTarget>A type of machine learning that uses multiple modalities of data such as text audio and images to improve learning outcomes.</owl:annotatedTarget>
        <oboInOwl:hasDbXref rdf:resource="https://doi.org/10.6028/NIST.SP.1270"/>
    </owl:Axiom>
    


    <!-- https://w3id.org/aio/MultimodalPromptbasedLanguageModel -->

    <owl:Class rdf:about="https://w3id.org/aio/MultimodalPromptbasedLanguageModel">
        <rdfs:subClassOf rdf:resource="https://w3id.org/aio/MultimodalLanguageModel"/>
        <obo:IAO_0000115>A multimodal LLM which processes prompts that include multiple modalities, such as both text and images, to generate relevant responses.</obo:IAO_0000115>
        <oboInOwl:inSubset rdf:resource="https://w3id.org/aio/ModelSubset"/>
        <rdfs:label>Multimodal Prompt-based Language Model</rdfs:label>
    </owl:Class>
    <owl:Axiom>
        <owl:annotatedSource rdf:resource="https://w3id.org/aio/MultimodalPromptbasedLanguageModel"/>
        <owl:annotatedProperty rdf:resource="http://purl.obolibrary.org/obo/IAO_0000115"/>
        <owl:annotatedTarget>A multimodal LLM which processes prompts that include multiple modalities, such as both text and images, to generate relevant responses.</owl:annotatedTarget>
        <oboInOwl:hasDbXref rdf:resource="https://arxiv.org/abs/2210.03094"/>
    </owl:Axiom>
    


    <!-- https://w3id.org/aio/MultimodalTransformer -->

    <owl:Class rdf:about="https://w3id.org/aio/MultimodalTransformer">
        <rdfs:subClassOf rdf:resource="https://w3id.org/aio/TransformerNetwork"/>
        <obo:IAO_0000115>A transformer network that processes and relates information from different modalities such as text images and audio using a shared embedding space and attention mechanism to learn joint representations across modalities.</obo:IAO_0000115>
        <oboInOwl:hasRelatedSynonym>unified encoder</oboInOwl:hasRelatedSynonym>
        <oboInOwl:hasRelatedSynonym>vision-language model</oboInOwl:hasRelatedSynonym>
        <oboInOwl:inSubset rdf:resource="https://w3id.org/aio/ModelSubset"/>
        <rdfs:label>Multimodal Transformer</rdfs:label>
    </owl:Class>
    


    <!-- https://w3id.org/aio/MultiplyLayer -->

    <owl:Class rdf:about="https://w3id.org/aio/MultiplyLayer">
        <rdfs:subClassOf rdf:resource="https://w3id.org/aio/MergingLayer"/>
        <obo:IAO_0000115>A merging layer that multiplies (element-wise) a list of inputs.</obo:IAO_0000115>
        <oboInOwl:inSubset rdf:resource="https://w3id.org/aio/LayerSubset"/>
        <rdfs:comment>Layer that multiplies (element-wise) a list of inputs. It takes as input a list of tensors, all of the same shape, and returns a single tensor (also of the same shape).</rdfs:comment>
        <rdfs:label>Multiply Layer</rdfs:label>
    </owl:Class>
    <owl:Axiom>
        <owl:annotatedSource rdf:resource="https://w3id.org/aio/MultiplyLayer"/>
        <owl:annotatedProperty rdf:resource="http://purl.obolibrary.org/obo/IAO_0000115"/>
        <owl:annotatedTarget>A merging layer that multiplies (element-wise) a list of inputs.</owl:annotatedTarget>
        <oboInOwl:hasDbXref rdf:resource="https://www.tensorflow.org/api_docs/python/tf/keras/layers/Multiply"/>
    </owl:Axiom>
    


    <!-- https://w3id.org/aio/NaturalLanguageProcessing -->

    <owl:Class rdf:about="https://w3id.org/aio/NaturalLanguageProcessing">
        <rdfs:subClassOf rdf:resource="https://w3id.org/aio/MachineLearning"/>
        <obo:IAO_0000115>A subfield of machine learning focused on the interactions between computers and human language including programming computers to process and analyze large amounts of natural language data.</obo:IAO_0000115>
        <oboInOwl:hasExactSynonym>NLP</oboInOwl:hasExactSynonym>
        <oboInOwl:inSubset rdf:resource="https://w3id.org/aio/MachineLearningSubset"/>
        <rdfs:label>Natural Language Processing</rdfs:label>
    </owl:Class>
    <owl:Axiom>
        <owl:annotatedSource rdf:resource="https://w3id.org/aio/NaturalLanguageProcessing"/>
        <owl:annotatedProperty rdf:resource="http://purl.obolibrary.org/obo/IAO_0000115"/>
        <owl:annotatedTarget>A subfield of machine learning focused on the interactions between computers and human language including programming computers to process and analyze large amounts of natural language data.</owl:annotatedTarget>
        <oboInOwl:hasDbXref rdf:resource="https://en.wikipedia.org/wiki/Natural_language_processing"/>
    </owl:Axiom>
    


    <!-- https://w3id.org/aio/Network -->

    <owl:Class rdf:about="https://w3id.org/aio/Network">
        <rdfs:subClassOf rdf:resource="http://www.w3.org/2002/07/owl#Thing"/>
        <obo:IAO_0000115>A system of interconnected nodes or entities for communication computation or data exchange.</obo:IAO_0000115>
        <oboInOwl:inSubset rdf:resource="https://w3id.org/aio/ClassSubset"/>
        <rdfs:label>Network</rdfs:label>
    </owl:Class>
    


    <!-- https://w3id.org/aio/NeuralTuringMachineNetwork -->

    <owl:Class rdf:about="https://w3id.org/aio/NeuralTuringMachineNetwork">
        <rdfs:subClassOf rdf:resource="https://w3id.org/aio/DeepFeedForwardNetwork"/>
        <rdfs:subClassOf rdf:resource="https://w3id.org/aio/LongShortTermMemory"/>
        <rdfs:subClassOf>
            <owl:Restriction>
                <owl:onProperty rdf:resource="http://purl.obolibrary.org/obo/BFO_0000051"/>
                <owl:someValuesFrom rdf:resource="https://w3id.org/aio/SpikingHiddenLayer"/>
            </owl:Restriction>
        </rdfs:subClassOf>
        <obo:IAO_0000115>A deep feedforward network that combines neural network pattern matching with the algorithmic power of programmable computers.</obo:IAO_0000115>
        <oboInOwl:hasExactSynonym>NTM</oboInOwl:hasExactSynonym>
        <oboInOwl:inSubset rdf:resource="https://w3id.org/aio/NetworkSubset"/>
        <rdfs:comment>Layers: Input, Hidden, Spiking Hidden, Output</rdfs:comment>
        <rdfs:label>Neural Turing Machine Network</rdfs:label>
    </owl:Class>
    <owl:Axiom>
        <owl:annotatedSource rdf:resource="https://w3id.org/aio/NeuralTuringMachineNetwork"/>
        <owl:annotatedProperty rdf:resource="http://purl.obolibrary.org/obo/IAO_0000115"/>
        <owl:annotatedTarget>A deep feedforward network that combines neural network pattern matching with the algorithmic power of programmable computers.</owl:annotatedTarget>
        <oboInOwl:hasDbXref rdf:resource="https://en.wikipedia.org/wiki/Neural_Turing_machine"/>
    </owl:Axiom>
    


    <!-- https://w3id.org/aio/NeuroSymbolicLLM -->

    <owl:Class rdf:about="https://w3id.org/aio/NeuroSymbolicLLM">
        <rdfs:subClassOf rdf:resource="https://w3id.org/aio/LargeLanguageModel"/>
        <obo:IAO_0000115>A LLM which combines neural language modeling with symbolic reasoning components, leveraging structured knowledge representations and logical inferences to improve reasoning capabilities.</obo:IAO_0000115>
        <oboInOwl:hasExactSynonym>Neuro-Symbolic Large Language Model</oboInOwl:hasExactSynonym>
        <oboInOwl:hasRelatedSynonym>knowledge reasoning</oboInOwl:hasRelatedSynonym>
        <oboInOwl:hasRelatedSynonym>symbolic grounding</oboInOwl:hasRelatedSynonym>
        <oboInOwl:inSubset rdf:resource="https://w3id.org/aio/ModelSubset"/>
        <rdfs:label>Neuro-Symbolic LLM</rdfs:label>
    </owl:Class>
    


    <!-- https://w3id.org/aio/NoiseDenseLayer -->

    <owl:Class rdf:about="https://w3id.org/aio/NoiseDenseLayer">
        <rdfs:subClassOf rdf:resource="https://w3id.org/aio/Layer"/>
        <obo:IAO_0000115>A layer that is a densely-connected neural network layer with added noise for regularization.</obo:IAO_0000115>
        <oboInOwl:inSubset rdf:resource="https://w3id.org/aio/LayerSubset"/>
        <rdfs:comment>Noisy dense layer that injects random noise to the weights of dense layer. Noisy dense layers are fully connected layers whose weights and biases are augmented by factorised Gaussian noise. The factorised Gaussian noise is controlled through gradient descent by a second weights layer. A NoisyDense layer implements the operation: $$ mathrm{NoisyDense}(x) = mathrm{activation}(mathrm{dot}(x, mu + (sigma cdot epsilon)) mathrm{bias}) $$ where mu is the standard weights layer, epsilon is the factorised Gaussian noise, and delta is a second weights layer which controls epsilon.</rdfs:comment>
        <rdfs:label>Noise Dense Layer</rdfs:label>
    </owl:Class>
    <owl:Axiom>
        <owl:annotatedSource rdf:resource="https://w3id.org/aio/NoiseDenseLayer"/>
        <owl:annotatedProperty rdf:resource="http://purl.obolibrary.org/obo/IAO_0000115"/>
        <owl:annotatedTarget>A layer that is a densely-connected neural network layer with added noise for regularization.</owl:annotatedTarget>
        <oboInOwl:hasDbXref rdf:resource="https://www.tensorflow.org/addons/api_docs/python/tfa/layers/NoisyDense"/>
    </owl:Axiom>
    


    <!-- https://w3id.org/aio/NoisyInputLayer -->

    <owl:Class rdf:about="https://w3id.org/aio/NoisyInputLayer">
        <rdfs:subClassOf rdf:resource="https://w3id.org/aio/InputLayer"/>
        <obo:IAO_0000115>An input layer that adds noise to each value.</obo:IAO_0000115>
        <oboInOwl:inSubset rdf:resource="https://w3id.org/aio/LayerSubset"/>
        <rdfs:label>Noisy Input Layer</rdfs:label>
    </owl:Class>
    <owl:Axiom>
        <owl:annotatedSource rdf:resource="https://w3id.org/aio/NoisyInputLayer"/>
        <owl:annotatedProperty rdf:resource="http://purl.obolibrary.org/obo/IAO_0000115"/>
        <owl:annotatedTarget>An input layer that adds noise to each value.</owl:annotatedTarget>
        <oboInOwl:hasDbXref rdf:resource="https://doi.org/10.1109/21.155944"/>
    </owl:Axiom>
    


    <!-- https://w3id.org/aio/Normalization -->

    <owl:Class rdf:about="https://w3id.org/aio/Normalization">
        <rdfs:subClassOf rdf:resource="https://w3id.org/aio/DataPreparation"/>
        <obo:IAO_0000115>The technique of transforming data into a standard format or scale typically to reduce redundancy and improve consistency often involving the adjustment of values measured on different scales to a common scale.</obo:IAO_0000115>
        <oboInOwl:inSubset rdf:resource="https://w3id.org/aio/PreprocessingSubset"/>
        <rdfs:label>Normalization</rdfs:label>
    </owl:Class>
    


    <!-- https://w3id.org/aio/NormalizationLayer -->

    <owl:Class rdf:about="https://w3id.org/aio/NormalizationLayer">
        <rdfs:subClassOf rdf:resource="https://w3id.org/aio/NumericalFeaturesPreprocessingLayer"/>
        <obo:IAO_0000115>A preprocessing layer that normalizes continuous features.</obo:IAO_0000115>
        <oboInOwl:inSubset rdf:resource="https://w3id.org/aio/LayerSubset"/>
        <rdfs:label>Normalization Layer</rdfs:label>
    </owl:Class>
    <owl:Axiom>
        <owl:annotatedSource rdf:resource="https://w3id.org/aio/NormalizationLayer"/>
        <owl:annotatedProperty rdf:resource="http://purl.obolibrary.org/obo/IAO_0000115"/>
        <owl:annotatedTarget>A preprocessing layer that normalizes continuous features.</owl:annotatedTarget>
        <oboInOwl:hasDbXref rdf:resource="https://www.tensorflow.org/api_docs/python/tf/keras/layers/Normalization"/>
    </owl:Axiom>
    


    <!-- https://w3id.org/aio/NumericalFeaturesPreprocessingLayer -->

    <owl:Class rdf:about="https://w3id.org/aio/NumericalFeaturesPreprocessingLayer">
        <rdfs:subClassOf rdf:resource="https://w3id.org/aio/Layer"/>
        <obo:IAO_0000115>A layer that performs numerical data preprocessing operations.</obo:IAO_0000115>
        <oboInOwl:inSubset rdf:resource="https://w3id.org/aio/LayerSubset"/>
        <rdfs:label>Numerical Features Preprocessing Layer</rdfs:label>
    </owl:Class>
    <owl:Axiom>
        <owl:annotatedSource rdf:resource="https://w3id.org/aio/NumericalFeaturesPreprocessingLayer"/>
        <owl:annotatedProperty rdf:resource="http://purl.obolibrary.org/obo/IAO_0000115"/>
        <owl:annotatedTarget>A layer that performs numerical data preprocessing operations.</owl:annotatedTarget>
        <oboInOwl:hasDbXref rdf:resource="https://keras.io/guides/preprocessing_layers/"/>
    </owl:Axiom>
    


    <!-- https://w3id.org/aio/OneshotLearning -->

    <owl:Class rdf:about="https://w3id.org/aio/OneshotLearning">
        <rdfs:subClassOf rdf:resource="https://w3id.org/aio/DeepNeuralNetwork"/>
        <obo:IAO_0000115>A deep neural network that classified objects from one or only a few examples.</obo:IAO_0000115>
        <oboInOwl:hasExactSynonym>OSL</oboInOwl:hasExactSynonym>
        <oboInOwl:inSubset rdf:resource="https://w3id.org/aio/NetworkSubset"/>
        <rdfs:label>One-shot Learning</rdfs:label>
    </owl:Class>
    <owl:Axiom>
        <owl:annotatedSource rdf:resource="https://w3id.org/aio/OneshotLearning"/>
        <owl:annotatedProperty rdf:resource="http://purl.obolibrary.org/obo/IAO_0000115"/>
        <owl:annotatedTarget>A deep neural network that classified objects from one or only a few examples.</owl:annotatedTarget>
        <oboInOwl:hasDbXref rdf:resource="https://en.wikipedia.org/wiki/One-shot_learning"/>
    </owl:Axiom>
    


    <!-- https://w3id.org/aio/OrdinalLLM -->

    <owl:Class rdf:about="https://w3id.org/aio/OrdinalLLM">
        <rdfs:subClassOf rdf:resource="https://w3id.org/aio/LargeLanguageModel"/>
        <obo:IAO_0000115>A large language model that is trained to model ordinal relationships and rank outputs rather than model probability distributions over text sequences directly.</obo:IAO_0000115>
        <oboInOwl:hasExactSynonym>Ordinal Large Language Model</oboInOwl:hasExactSynonym>
        <oboInOwl:hasRelatedSynonym>preference modeling</oboInOwl:hasRelatedSynonym>
        <oboInOwl:hasRelatedSynonym>ranking</oboInOwl:hasRelatedSynonym>
        <oboInOwl:inSubset rdf:resource="https://w3id.org/aio/ModelSubset"/>
        <rdfs:label>Ordinal LLM</rdfs:label>
    </owl:Class>
    


    <!-- https://w3id.org/aio/OutputLayer -->

    <owl:Class rdf:about="https://w3id.org/aio/OutputLayer">
        <rdfs:subClassOf rdf:resource="https://w3id.org/aio/Layer"/>
        <obo:IAO_0000115>A layer containing the last neurons in the network that produces given outputs for the program.</obo:IAO_0000115>
        <oboInOwl:inSubset rdf:resource="https://w3id.org/aio/LayerSubset"/>
        <rdfs:comment>The output layer in an artificial neural network is the last layer of neurons that produces given outputs for the program. Though they are made much like other artificial neurons in the neural network, output layer neurons may be built or observed in a different way, given that they are the last “actor” nodes on the network.</rdfs:comment>
        <rdfs:label>Output Layer</rdfs:label>
    </owl:Class>
    <owl:Axiom>
        <owl:annotatedSource rdf:resource="https://w3id.org/aio/OutputLayer"/>
        <owl:annotatedProperty rdf:resource="http://purl.obolibrary.org/obo/IAO_0000115"/>
        <owl:annotatedTarget>A layer containing the last neurons in the network that produces given outputs for the program.</owl:annotatedTarget>
        <oboInOwl:hasDbXref rdf:resource="https://www.techopedia.com/definition/33263/output-layer-neural-networks"/>
    </owl:Axiom>
    


    <!-- https://w3id.org/aio/PReLULayer -->

    <owl:Class rdf:about="https://w3id.org/aio/PReLULayer">
        <rdfs:subClassOf rdf:resource="https://w3id.org/aio/ActivationLayer"/>
        <obo:IAO_0000115>An activation layer that applies parametric rectified linear unit function element-wise.</obo:IAO_0000115>
        <oboInOwl:inSubset rdf:resource="https://w3id.org/aio/LayerSubset"/>
        <rdfs:comment>Parametric Rectified Linear Unit.</rdfs:comment>
        <rdfs:label>PReLU Layer</rdfs:label>
    </owl:Class>
    <owl:Axiom>
        <owl:annotatedSource rdf:resource="https://w3id.org/aio/PReLULayer"/>
        <owl:annotatedProperty rdf:resource="http://purl.obolibrary.org/obo/IAO_0000115"/>
        <owl:annotatedTarget>An activation layer that applies parametric rectified linear unit function element-wise.</owl:annotatedTarget>
        <oboInOwl:hasDbXref rdf:resource="https://www.tensorflow.org/api_docs/python/tf/keras/layers/PReLU"/>
    </owl:Axiom>
    


    <!-- https://w3id.org/aio/Perceptron -->

    <owl:Class rdf:about="https://w3id.org/aio/Perceptron">
        <rdfs:subClassOf rdf:resource="https://w3id.org/aio/ArtificialNeuralNetwork"/>
        <rdfs:subClassOf>
            <owl:Restriction>
                <owl:onProperty rdf:resource="http://purl.obolibrary.org/obo/BFO_0000051"/>
                <owl:someValuesFrom rdf:resource="https://w3id.org/aio/InputLayer"/>
            </owl:Restriction>
        </rdfs:subClassOf>
        <rdfs:subClassOf>
            <owl:Restriction>
                <owl:onProperty rdf:resource="http://purl.obolibrary.org/obo/BFO_0000051"/>
                <owl:someValuesFrom rdf:resource="https://w3id.org/aio/OutputLayer"/>
            </owl:Restriction>
        </rdfs:subClassOf>
        <obo:IAO_0000115>An artificial neural network with a supervised learning algorithm for binary classification using a linear predictor function.</obo:IAO_0000115>
        <oboInOwl:hasExactSynonym>FFN</oboInOwl:hasExactSynonym>
        <oboInOwl:hasExactSynonym>Feed-Forward Network</oboInOwl:hasExactSynonym>
        <oboInOwl:hasExactSynonym>SLP</oboInOwl:hasExactSynonym>
        <oboInOwl:hasExactSynonym>Single Layer Perceptron</oboInOwl:hasExactSynonym>
        <oboInOwl:inSubset rdf:resource="https://w3id.org/aio/NetworkSubset"/>
        <rdfs:comment>Layers: Input, Output</rdfs:comment>
        <rdfs:label>Perceptron</rdfs:label>
    </owl:Class>
    


    <!-- https://w3id.org/aio/PermuteLayer -->

    <owl:Class rdf:about="https://w3id.org/aio/PermuteLayer">
        <rdfs:subClassOf rdf:resource="https://w3id.org/aio/ReshapingLayer"/>
        <obo:IAO_0000115>A layer that permutes the dimensions of the input according to a given pattern.</obo:IAO_0000115>
        <oboInOwl:inSubset rdf:resource="https://w3id.org/aio/LayerSubset"/>
        <rdfs:comment>Permutes the dimensions of the input according to a given pattern. Useful e.g. connecting RNNs and convnets.</rdfs:comment>
        <rdfs:label>Permute Layer</rdfs:label>
    </owl:Class>
    <owl:Axiom>
        <owl:annotatedSource rdf:resource="https://w3id.org/aio/PermuteLayer"/>
        <owl:annotatedProperty rdf:resource="http://purl.obolibrary.org/obo/IAO_0000115"/>
        <owl:annotatedTarget>A layer that permutes the dimensions of the input according to a given pattern.</owl:annotatedTarget>
        <oboInOwl:hasDbXref rdf:resource="https://www.tensorflow.org/api_docs/python/tf/keras/layers/Permute"/>
    </owl:Axiom>
    


    <!-- https://w3id.org/aio/PersonalizedLLM -->

    <owl:Class rdf:about="https://w3id.org/aio/PersonalizedLLM">
        <rdfs:subClassOf rdf:resource="https://w3id.org/aio/LargeLanguageModel"/>
        <obo:IAO_0000115>A large language model that adapts its language modeling and generation to the preferences style and persona of individual users or audiences.</obo:IAO_0000115>
        <oboInOwl:hasExactSynonym>Personalized Large Language Model</oboInOwl:hasExactSynonym>
        <oboInOwl:hasRelatedSynonym>user adaptation LLM</oboInOwl:hasRelatedSynonym>
        <oboInOwl:inSubset rdf:resource="https://w3id.org/aio/ModelSubset"/>
        <rdfs:label>Personalized LLM</rdfs:label>
    </owl:Class>
    


    <!-- https://w3id.org/aio/PolicyLayer -->

    <owl:Class rdf:about="https://w3id.org/aio/PolicyLayer">
        <rdfs:subClassOf rdf:resource="https://w3id.org/aio/Layer"/>
        <obo:IAO_0000115>A layer that, after taking a set of states or values as input, predicts a probability distribution of actions to take.</obo:IAO_0000115>
        <oboInOwl:inSubset rdf:resource="https://w3id.org/aio/LayerSubset"/>
        <rdfs:label>Policy Layer</rdfs:label>
    </owl:Class>
    


    <!-- https://w3id.org/aio/PoolingLayer -->

    <owl:Class rdf:about="https://w3id.org/aio/PoolingLayer">
        <rdfs:subClassOf rdf:resource="https://w3id.org/aio/Layer"/>
        <obo:IAO_0000115>A layer that serves to mitigate the sensitivity of convolutional layers to location and spatially downsample representations.</obo:IAO_0000115>
        <oboInOwl:inSubset rdf:resource="https://w3id.org/aio/LayerSubset"/>
        <rdfs:comment>Pooling layers serve the dual purposes of mitigating the sensitivity of convolutional layers to location and of spatially downsampling representations.</rdfs:comment>
        <rdfs:label>Pooling Layer</rdfs:label>
    </owl:Class>
    <owl:Axiom>
        <owl:annotatedSource rdf:resource="https://w3id.org/aio/PoolingLayer"/>
        <owl:annotatedProperty rdf:resource="http://purl.obolibrary.org/obo/IAO_0000115"/>
        <owl:annotatedTarget>A layer that serves to mitigate the sensitivity of convolutional layers to location and spatially downsample representations.</owl:annotatedTarget>
        <oboInOwl:hasDbXref rdf:resource="https://d2l.ai/chapter_convolutional-neural-networks/pooling.html"/>
    </owl:Axiom>
    


    <!-- https://w3id.org/aio/PopularityBias -->

    <owl:Class rdf:about="https://w3id.org/aio/PopularityBias">
        <rdfs:subClassOf rdf:resource="https://w3id.org/aio/SelectionAndSamplingBias"/>
        <obo:IAO_0000115>A selection and sampling bias where more popular items are more exposed under-representing less popular items.</obo:IAO_0000115>
        <oboInOwl:inSubset rdf:resource="https://w3id.org/aio/BiasSubset"/>
        <rdfs:comment>Selection bias where more popular items are more exposed, under-representing less popular items.</rdfs:comment>
        <rdfs:label>Popularity Bias</rdfs:label>
    </owl:Class>
    <owl:Axiom>
        <owl:annotatedSource rdf:resource="https://w3id.org/aio/PopularityBias"/>
        <owl:annotatedProperty rdf:resource="http://purl.obolibrary.org/obo/IAO_0000115"/>
        <owl:annotatedTarget>A selection and sampling bias where more popular items are more exposed under-representing less popular items.</owl:annotatedTarget>
        <oboInOwl:hasDbXref rdf:resource="https://doi.org/10.6028/NIST.SP.1270"/>
    </owl:Axiom>
    


    <!-- https://w3id.org/aio/PopulationBias -->

    <owl:Class rdf:about="https://w3id.org/aio/PopulationBias">
        <rdfs:subClassOf rdf:resource="https://w3id.org/aio/SelectionAndSamplingBias"/>
        <obo:IAO_0000115>A selection and sampling bias characterized by systematic distortions in demographics or other user characteristics between represented users and the target population.</obo:IAO_0000115>
        <oboInOwl:inSubset rdf:resource="https://w3id.org/aio/BiasSubset"/>
        <rdfs:label>Population Bias</rdfs:label>
    </owl:Class>
    <owl:Axiom>
        <owl:annotatedSource rdf:resource="https://w3id.org/aio/PopulationBias"/>
        <owl:annotatedProperty rdf:resource="http://purl.obolibrary.org/obo/IAO_0000115"/>
        <owl:annotatedTarget>A selection and sampling bias characterized by systematic distortions in demographics or other user characteristics between represented users and the target population.</owl:annotatedTarget>
        <oboInOwl:hasDbXref rdf:resource="https://doi.org/10.6028/NIST.SP.1270"/>
    </owl:Axiom>
    


    <!-- https://w3id.org/aio/Preprocessing -->

    <owl:Class rdf:about="https://w3id.org/aio/Preprocessing">
        <rdfs:subClassOf rdf:resource="http://www.w3.org/2002/07/owl#Thing"/>
        <obo:IAO_0000115>The series of steps applied to raw data before it is used in a machine learning model including tasks such as normalization scaling encoding and transformation to ensure the data is in an appropriate format and quality for analysis.</obo:IAO_0000115>
        <oboInOwl:inSubset rdf:resource="https://w3id.org/aio/PreprocessingSubset"/>
        <rdfs:label>Preprocessing</rdfs:label>
    </owl:Class>
    <owl:Axiom>
        <owl:annotatedSource rdf:resource="https://w3id.org/aio/Preprocessing"/>
        <owl:annotatedProperty rdf:resource="http://purl.obolibrary.org/obo/IAO_0000115"/>
        <owl:annotatedTarget>The series of steps applied to raw data before it is used in a machine learning model including tasks such as normalization scaling encoding and transformation to ensure the data is in an appropriate format and quality for analysis.</owl:annotatedTarget>
        <oboInOwl:hasDbXref rdf:resource="https://doi.org/10.1109/ICDE.2019.00245"/>
    </owl:Axiom>
    


    <!-- https://w3id.org/aio/PreprocessingLayer -->

    <owl:Class rdf:about="https://w3id.org/aio/PreprocessingLayer">
        <rdfs:subClassOf rdf:resource="https://w3id.org/aio/Layer"/>
        <obo:IAO_0000115>A layer that performs data preprocessing operations.</obo:IAO_0000115>
        <oboInOwl:inSubset rdf:resource="https://w3id.org/aio/LayerSubset"/>
        <rdfs:label>Preprocessing Layer</rdfs:label>
    </owl:Class>
    <owl:Axiom>
        <owl:annotatedSource rdf:resource="https://w3id.org/aio/PreprocessingLayer"/>
        <owl:annotatedProperty rdf:resource="http://purl.obolibrary.org/obo/IAO_0000115"/>
        <owl:annotatedTarget>A layer that performs data preprocessing operations.</owl:annotatedTarget>
        <oboInOwl:hasDbXref rdf:resource="https://www.tensorflow.org/guide/keras/preprocessing_layers"/>
    </owl:Axiom>
    


    <!-- https://w3id.org/aio/PresentationBias -->

    <owl:Class rdf:about="https://w3id.org/aio/PresentationBias">
        <rdfs:subClassOf rdf:resource="https://w3id.org/aio/IndividualBias"/>
        <obo:IAO_0000115>An individual bias arising from how information is presented on the Web via a user interface due to rating or ranking of output or through users&apos; self-selected biased interaction.</obo:IAO_0000115>
        <oboInOwl:inSubset rdf:resource="https://w3id.org/aio/BiasSubset"/>
        <rdfs:label>Presentation Bias</rdfs:label>
    </owl:Class>
    <owl:Axiom>
        <owl:annotatedSource rdf:resource="https://w3id.org/aio/PresentationBias"/>
        <owl:annotatedProperty rdf:resource="http://purl.obolibrary.org/obo/IAO_0000115"/>
        <owl:annotatedTarget>An individual bias arising from how information is presented on the Web via a user interface due to rating or ranking of output or through users&apos; self-selected biased interaction.</owl:annotatedTarget>
        <oboInOwl:hasDbXref rdf:resource="https://doi.org/10.6028/NIST.SP.1270"/>
    </owl:Axiom>
    


    <!-- https://w3id.org/aio/PrincipalComponentAnalysis -->

    <owl:Class rdf:about="https://w3id.org/aio/PrincipalComponentAnalysis">
        <rdfs:subClassOf rdf:resource="https://w3id.org/aio/DimensionalityReduction"/>
        <obo:IAO_0000115>A dimensionality reduction method for analyzing large datasets with high-dimensional features per observation increasing data interpretability while preserving maximum information and enabling visualization.</obo:IAO_0000115>
        <oboInOwl:hasExactSynonym>PCA</oboInOwl:hasExactSynonym>
        <oboInOwl:inSubset rdf:resource="https://w3id.org/aio/MachineLearningSubset"/>
        <rdfs:label>Principal Component Analysis</rdfs:label>
    </owl:Class>
    <owl:Axiom>
        <owl:annotatedSource rdf:resource="https://w3id.org/aio/PrincipalComponentAnalysis"/>
        <owl:annotatedProperty rdf:resource="http://purl.obolibrary.org/obo/IAO_0000115"/>
        <owl:annotatedTarget>A dimensionality reduction method for analyzing large datasets with high-dimensional features per observation increasing data interpretability while preserving maximum information and enabling visualization.</owl:annotatedTarget>
        <oboInOwl:hasDbXref rdf:resource="https://en.wikipedia.org/wiki/Principal_component_analysis"/>
    </owl:Axiom>
    


    <!-- https://w3id.org/aio/ProbabilisticGraphicalModel -->

    <owl:Class rdf:about="https://w3id.org/aio/ProbabilisticGraphicalModel">
        <rdfs:subClassOf rdf:resource="https://w3id.org/aio/MachineLearning"/>
        <obo:IAO_0000115>A machine learning model in which a graph expresses the conditional dependence structure between random variables.</obo:IAO_0000115>
        <oboInOwl:hasExactSynonym>Graphical Model</oboInOwl:hasExactSynonym>
        <oboInOwl:hasExactSynonym>PGM</oboInOwl:hasExactSynonym>
        <oboInOwl:hasExactSynonym>Structure Probabilistic Model</oboInOwl:hasExactSynonym>
        <oboInOwl:inSubset rdf:resource="https://w3id.org/aio/MachineLearningSubset"/>
        <rdfs:label>Probabilistic Graphical Model</rdfs:label>
    </owl:Class>
    <owl:Axiom>
        <owl:annotatedSource rdf:resource="https://w3id.org/aio/ProbabilisticGraphicalModel"/>
        <owl:annotatedProperty rdf:resource="http://purl.obolibrary.org/obo/IAO_0000115"/>
        <owl:annotatedTarget>A machine learning model in which a graph expresses the conditional dependence structure between random variables.</owl:annotatedTarget>
        <oboInOwl:hasDbXref rdf:resource="https://en.wikipedia.org/wiki/Graphical_model"/>
    </owl:Axiom>
    


    <!-- https://w3id.org/aio/ProbabilisticHiddenLayer -->

    <owl:Class rdf:about="https://w3id.org/aio/ProbabilisticHiddenLayer">
        <rdfs:subClassOf rdf:resource="https://w3id.org/aio/HiddenLayer"/>
        <obo:IAO_0000115>A hidden layer that estimates the probability of a sample being within a certain category.</obo:IAO_0000115>
        <oboInOwl:inSubset rdf:resource="https://w3id.org/aio/LayerSubset"/>
        <rdfs:label>Probabilistic Hidden Layer</rdfs:label>
    </owl:Class>
    


    <!-- https://w3id.org/aio/ProbabilisticTopicModel -->

    <owl:Class rdf:about="https://w3id.org/aio/ProbabilisticTopicModel">
        <rdfs:subClassOf rdf:resource="https://w3id.org/aio/ProbabilisticGraphicalModel"/>
        <obo:IAO_0000115>A probabilistic graphical model that uses statistical techniques to analyze the words in each text to discover common themes their connections and their changes over time.</obo:IAO_0000115>
        <oboInOwl:inSubset rdf:resource="https://w3id.org/aio/MachineLearningSubset"/>
        <rdfs:label>Probabilistic Topic Model</rdfs:label>
    </owl:Class>
    <owl:Axiom>
        <owl:annotatedSource rdf:resource="https://w3id.org/aio/ProbabilisticTopicModel"/>
        <owl:annotatedProperty rdf:resource="http://purl.obolibrary.org/obo/IAO_0000115"/>
        <owl:annotatedTarget>A probabilistic graphical model that uses statistical techniques to analyze the words in each text to discover common themes their connections and their changes over time.</owl:annotatedTarget>
        <oboInOwl:hasDbXref rdf:resource="https://pyro.ai/examples/prodlda.html"/>
    </owl:Axiom>
    


    <!-- https://w3id.org/aio/ProcessingBias -->

    <owl:Class rdf:about="https://w3id.org/aio/ProcessingBias">
        <rdfs:subClassOf rdf:resource="https://w3id.org/aio/ComputationalBias"/>
        <obo:IAO_0000115>A computational bias resulting from judgment modulated by affect influenced by the level of efficacy and efficiency in information processing.</obo:IAO_0000115>
        <oboInOwl:hasExactSynonym>Validation Bias</oboInOwl:hasExactSynonym>
        <oboInOwl:inSubset rdf:resource="https://w3id.org/aio/BiasSubset"/>
        <rdfs:comment>Judgment modulated by affect, influenced by the level of efficacy and efficiency in information processing; often referred to as aesthetic judgment in cognitive sciences.</rdfs:comment>
        <rdfs:label>Processing Bias</rdfs:label>
    </owl:Class>
    <owl:Axiom>
        <owl:annotatedSource rdf:resource="https://w3id.org/aio/ProcessingBias"/>
        <owl:annotatedProperty rdf:resource="http://purl.obolibrary.org/obo/IAO_0000115"/>
        <owl:annotatedTarget>A computational bias resulting from judgment modulated by affect influenced by the level of efficacy and efficiency in information processing.</owl:annotatedTarget>
        <oboInOwl:hasDbXref rdf:resource="https://en.wikipedia.org/wiki/Bias_(statistics)"/>
    </owl:Axiom>
    


    <!-- https://w3id.org/aio/PromptbasedFineTuningLLM -->

    <owl:Class rdf:about="https://w3id.org/aio/PromptbasedFineTuningLLM">
        <rdfs:subClassOf rdf:resource="https://w3id.org/aio/LargeLanguageModel"/>
        <obo:IAO_0000115>A LLM which is fine-tuned on a small number of examples or prompts, rather than full task datasets. This allows for rapid adaptation to new tasks with limited data, leveraging the model&apos;s few-shot learning capabilities.</obo:IAO_0000115>
        <oboInOwl:hasExactSynonym>Prompt-based Fine-Tuning Large Language Model</oboInOwl:hasExactSynonym>
        <oboInOwl:hasExactSynonym>Prompt-tuned Large Language Model</oboInOwl:hasExactSynonym>
        <oboInOwl:hasRelatedSynonym>few-shot learning</oboInOwl:hasRelatedSynonym>
        <oboInOwl:hasRelatedSynonym>in-context learning</oboInOwl:hasRelatedSynonym>
        <oboInOwl:inSubset rdf:resource="https://w3id.org/aio/ModelSubset"/>
        <rdfs:label>Prompt-based Fine-Tuning LLM</rdfs:label>
    </owl:Class>
    


    <!-- https://w3id.org/aio/ProportionalHazardsModel -->

    <owl:Class rdf:about="https://w3id.org/aio/ProportionalHazardsModel">
        <rdfs:subClassOf rdf:resource="https://w3id.org/aio/RegressionAnalysis"/>
        <rdfs:subClassOf rdf:resource="https://w3id.org/aio/SurvivalAnalysis"/>
        <obo:IAO_0000115>A regression analysis method for survival analysis where the unique effect of a unit increase in a covariate is multiplicative with respect to the hazard rate.</obo:IAO_0000115>
        <oboInOwl:inSubset rdf:resource="https://w3id.org/aio/MachineLearningSubset"/>
        <rdfs:label>Proportional Hazards Model</rdfs:label>
    </owl:Class>
    <owl:Axiom>
        <owl:annotatedSource rdf:resource="https://w3id.org/aio/ProportionalHazardsModel"/>
        <owl:annotatedProperty rdf:resource="http://purl.obolibrary.org/obo/IAO_0000115"/>
        <owl:annotatedTarget>A regression analysis method for survival analysis where the unique effect of a unit increase in a covariate is multiplicative with respect to the hazard rate.</owl:annotatedTarget>
        <oboInOwl:hasDbXref rdf:resource="https://en.wikipedia.org/wiki/Proportional_hazards_model"/>
    </owl:Axiom>
    


    <!-- https://w3id.org/aio/RNNLayer -->

    <owl:Class rdf:about="https://w3id.org/aio/RNNLayer">
        <rdfs:subClassOf rdf:resource="https://w3id.org/aio/RecurrentLayer"/>
        <obo:IAO_0000115>The base class for recurrent layers.</obo:IAO_0000115>
        <oboInOwl:inSubset rdf:resource="https://w3id.org/aio/LayerSubset"/>
        <rdfs:comment>Base class for recurrent layers.</rdfs:comment>
        <rdfs:label>RNN Layer</rdfs:label>
    </owl:Class>
    <owl:Axiom>
        <owl:annotatedSource rdf:resource="https://w3id.org/aio/RNNLayer"/>
        <owl:annotatedProperty rdf:resource="http://purl.obolibrary.org/obo/IAO_0000115"/>
        <owl:annotatedTarget>The base class for recurrent layers.</owl:annotatedTarget>
        <oboInOwl:hasDbXref rdf:resource="https://www.tensorflow.org/api_docs/python/tf/keras/layers/RNN"/>
    </owl:Axiom>
    


    <!-- https://w3id.org/aio/RadialBasisNetwork -->

    <owl:Class rdf:about="https://w3id.org/aio/RadialBasisNetwork">
        <rdfs:subClassOf rdf:resource="https://w3id.org/aio/DeepFeedForwardNetwork"/>
        <obo:IAO_0000115>A deep feedforward network that uses radial basis functions as activation functions for pattern recognition and interpolation.</obo:IAO_0000115>
        <oboInOwl:hasExactSynonym>RBFN</oboInOwl:hasExactSynonym>
        <oboInOwl:hasExactSynonym>RBN</oboInOwl:hasExactSynonym>
        <oboInOwl:hasExactSynonym>Radial Basis Function Network</oboInOwl:hasExactSynonym>
        <oboInOwl:inSubset rdf:resource="https://w3id.org/aio/NetworkSubset"/>
        <rdfs:comment>Layers: Input, Hidden, Output</rdfs:comment>
        <rdfs:label>Radial Basis Network</rdfs:label>
    </owl:Class>
    <owl:Axiom>
        <owl:annotatedSource rdf:resource="https://w3id.org/aio/RadialBasisNetwork"/>
        <owl:annotatedProperty rdf:resource="http://purl.obolibrary.org/obo/IAO_0000115"/>
        <owl:annotatedTarget>A deep feedforward network that uses radial basis functions as activation functions for pattern recognition and interpolation.</owl:annotatedTarget>
        <oboInOwl:hasDbXref rdf:resource="https://en.wikipedia.org/wiki/Radial_basis_function_network"/>
    </owl:Axiom>
    


    <!-- https://w3id.org/aio/RandomBrightnessLayer -->

    <owl:Class rdf:about="https://w3id.org/aio/RandomBrightnessLayer">
        <rdfs:subClassOf rdf:resource="https://w3id.org/aio/Layer"/>
        <obo:IAO_0000115>An image preprocessing layer that randomly adjusts brightness during training.</obo:IAO_0000115>
        <oboInOwl:inSubset rdf:resource="https://w3id.org/aio/LayerSubset"/>
        <rdfs:comment>A preprocessing layer which randomly adjusts brightness during training. This layer will randomly increase/reduce the brightness for the input RGB images. At inference time, the output will be identical to the input. Call the layer with training=True to adjust the brightness of the input. Note that different brightness adjustment factors will be apply to each the images in the batch.</rdfs:comment>
        <rdfs:label>RandomBrightness Layer</rdfs:label>
    </owl:Class>
    <owl:Axiom>
        <owl:annotatedSource rdf:resource="https://w3id.org/aio/RandomBrightnessLayer"/>
        <owl:annotatedProperty rdf:resource="http://purl.obolibrary.org/obo/IAO_0000115"/>
        <owl:annotatedTarget>An image preprocessing layer that randomly adjusts brightness during training.</owl:annotatedTarget>
        <oboInOwl:hasDbXref rdf:resource="https://www.tensorflow.org/api_docs/python/tf/keras/layers/RandomBrightness"/>
    </owl:Axiom>
    


    <!-- https://w3id.org/aio/RandomContrastLayer -->

    <owl:Class rdf:about="https://w3id.org/aio/RandomContrastLayer">
        <rdfs:subClassOf rdf:resource="https://w3id.org/aio/Layer"/>
        <obo:IAO_0000115>An image preprocessing layer that randomly adjusts contrast during training.</obo:IAO_0000115>
        <oboInOwl:inSubset rdf:resource="https://w3id.org/aio/LayerSubset"/>
        <rdfs:comment>A preprocessing layer which randomly adjusts contrast during training. This layer will randomly adjust the contrast of an image or images by a random factor. Contrast is adjusted independently for each channel of each image during training. For each channel, this layer computes the mean of the image pixels in the channel and then adjusts each component x of each pixel to (x - mean) * contrast_factor + mean. Input pixel values can be of any range (e.g. [0., 1.) or [0, 255]) and in integer or floating point dtype. By default, the layer will output floats. The output value will be clipped to the range [0, 255], the valid range of RGB colors.</rdfs:comment>
        <rdfs:label>RandomContrast Layer</rdfs:label>
    </owl:Class>
    <owl:Axiom>
        <owl:annotatedSource rdf:resource="https://w3id.org/aio/RandomContrastLayer"/>
        <owl:annotatedProperty rdf:resource="http://purl.obolibrary.org/obo/IAO_0000115"/>
        <owl:annotatedTarget>An image preprocessing layer that randomly adjusts contrast during training.</owl:annotatedTarget>
        <oboInOwl:hasDbXref rdf:resource="https://www.tensorflow.org/api_docs/python/tf/keras/layers/RandomContrast"/>
    </owl:Axiom>
    


    <!-- https://w3id.org/aio/RandomCropLayer -->

    <owl:Class rdf:about="https://w3id.org/aio/RandomCropLayer">
        <rdfs:subClassOf rdf:resource="https://w3id.org/aio/Layer"/>
        <obo:IAO_0000115>An image preprocessing layer that randomly crops images during training.</obo:IAO_0000115>
        <oboInOwl:inSubset rdf:resource="https://w3id.org/aio/LayerSubset"/>
        <rdfs:comment>A preprocessing layer which randomly crops images during training. During training, this layer will randomly choose a location to crop images down to a target size. The layer will crop all the images in the same batch to the same cropping location. At inference time, and during training if an input image is smaller than the target size, the input will be resized and cropped so as to return the largest possible window in the image that matches the target aspect ratio. If you need to apply random cropping at inference time, set training to True when calling the layer. Input pixel values can be of any range (e.g. [0., 1.) or [0, 255]) and of interger or floating point dtype. By default, the layer will output floats.</rdfs:comment>
        <rdfs:label>RandomCrop Layer</rdfs:label>
    </owl:Class>
    <owl:Axiom>
        <owl:annotatedSource rdf:resource="https://w3id.org/aio/RandomCropLayer"/>
        <owl:annotatedProperty rdf:resource="http://purl.obolibrary.org/obo/IAO_0000115"/>
        <owl:annotatedTarget>An image preprocessing layer that randomly crops images during training.</owl:annotatedTarget>
        <oboInOwl:hasDbXref rdf:resource="https://www.tensorflow.org/api_docs/python/tf/keras/layers/RandomCrop"/>
    </owl:Axiom>
    


    <!-- https://w3id.org/aio/RandomEffectsModel -->

    <owl:Class rdf:about="https://w3id.org/aio/RandomEffectsModel">
        <rdfs:subClassOf rdf:resource="https://w3id.org/aio/RegressionAnalysis"/>
        <obo:IAO_0000115>A regression analysis model where the model parameters are random variables.</obo:IAO_0000115>
        <oboInOwl:hasExactSynonym>REM</oboInOwl:hasExactSynonym>
        <oboInOwl:inSubset rdf:resource="https://w3id.org/aio/MachineLearningSubset"/>
        <rdfs:label>Random Effects Model</rdfs:label>
    </owl:Class>
    <owl:Axiom>
        <owl:annotatedSource rdf:resource="https://w3id.org/aio/RandomEffectsModel"/>
        <owl:annotatedProperty rdf:resource="http://purl.obolibrary.org/obo/IAO_0000115"/>
        <owl:annotatedTarget>A regression analysis model where the model parameters are random variables.</owl:annotatedTarget>
        <oboInOwl:hasDbXref rdf:resource="https://en.wikipedia.org/wiki/Random_effects_model"/>
    </owl:Axiom>
    


    <!-- https://w3id.org/aio/RandomFlipLayer -->

    <owl:Class rdf:about="https://w3id.org/aio/RandomFlipLayer">
        <rdfs:subClassOf rdf:resource="https://w3id.org/aio/Layer"/>
        <obo:IAO_0000115>An image preprocessing layer that randomly flips images during training.</obo:IAO_0000115>
        <oboInOwl:inSubset rdf:resource="https://w3id.org/aio/LayerSubset"/>
        <rdfs:comment>A preprocessing layer which randomly flips images during training. This layer will flip the images horizontally and or vertically based on the mode attribute. During inference time, the output will be identical to input. Call the layer with training=True to flip the input. Input pixel values can be of any range (e.g. [0., 1.) or [0, 255]) and of interger or floating point dtype. By default, the layer will output floats.</rdfs:comment>
        <rdfs:label>RandomFlip Layer</rdfs:label>
    </owl:Class>
    <owl:Axiom>
        <owl:annotatedSource rdf:resource="https://w3id.org/aio/RandomFlipLayer"/>
        <owl:annotatedProperty rdf:resource="http://purl.obolibrary.org/obo/IAO_0000115"/>
        <owl:annotatedTarget>An image preprocessing layer that randomly flips images during training.</owl:annotatedTarget>
        <oboInOwl:hasDbXref rdf:resource="https://www.tensorflow.org/api_docs/python/tf/keras/layers/RandomFlip"/>
    </owl:Axiom>
    


    <!-- https://w3id.org/aio/RandomForest -->

    <owl:Class rdf:about="https://w3id.org/aio/RandomForest">
        <rdfs:subClassOf rdf:resource="https://w3id.org/aio/EnsembleLearning"/>
        <obo:IAO_0000115>An ensemble learning method for classification regression and other tasks that constructs a multitude of decision trees during training.</obo:IAO_0000115>
        <oboInOwl:inSubset rdf:resource="https://w3id.org/aio/MachineLearningSubset"/>
        <rdfs:label>Random Forest</rdfs:label>
    </owl:Class>
    <owl:Axiom>
        <owl:annotatedSource rdf:resource="https://w3id.org/aio/RandomForest"/>
        <owl:annotatedProperty rdf:resource="http://purl.obolibrary.org/obo/IAO_0000115"/>
        <owl:annotatedTarget>An ensemble learning method for classification regression and other tasks that constructs a multitude of decision trees during training.</owl:annotatedTarget>
        <oboInOwl:hasDbXref rdf:resource="https://en.wikipedia.org/wiki/Random_forest"/>
    </owl:Axiom>
    


    <!-- https://w3id.org/aio/RandomHeightLayer -->

    <owl:Class rdf:about="https://w3id.org/aio/RandomHeightLayer">
        <rdfs:subClassOf rdf:resource="https://w3id.org/aio/Layer"/>
        <obo:IAO_0000115>An image preprocessing layer that randomly varies image height during training.</obo:IAO_0000115>
        <oboInOwl:inSubset rdf:resource="https://w3id.org/aio/LayerSubset"/>
        <rdfs:comment>A preprocessing layer which randomly varies image height during training. This layer adjusts the height of a batch of images by a random factor. The input should be a 3D (unbatched) or 4D (batched) tensor in the &quot;channels_last&quot; image data format. Input pixel values can be of any range (e.g. [0., 1.) or [0, 255]) and of interger or floating point dtype. By default, the layer will output floats. By default, this layer is inactive during inference.</rdfs:comment>
        <rdfs:label>RandomHeight Layer</rdfs:label>
    </owl:Class>
    <owl:Axiom>
        <owl:annotatedSource rdf:resource="https://w3id.org/aio/RandomHeightLayer"/>
        <owl:annotatedProperty rdf:resource="http://purl.obolibrary.org/obo/IAO_0000115"/>
        <owl:annotatedTarget>An image preprocessing layer that randomly varies image height during training.</owl:annotatedTarget>
        <oboInOwl:hasDbXref rdf:resource="https://www.tensorflow.org/api_docs/python/tf/keras/layers/RandomHeight"/>
    </owl:Axiom>
    


    <!-- https://w3id.org/aio/RandomRotationLayer -->

    <owl:Class rdf:about="https://w3id.org/aio/RandomRotationLayer">
        <rdfs:subClassOf rdf:resource="https://w3id.org/aio/Layer"/>
        <obo:IAO_0000115>An image preprocessing layer that randomly rotates images during training.</obo:IAO_0000115>
        <oboInOwl:inSubset rdf:resource="https://w3id.org/aio/LayerSubset"/>
        <rdfs:comment>A preprocessing layer which randomly rotates images during training.</rdfs:comment>
        <rdfs:label>RandomRotation Layer</rdfs:label>
    </owl:Class>
    <owl:Axiom>
        <owl:annotatedSource rdf:resource="https://w3id.org/aio/RandomRotationLayer"/>
        <owl:annotatedProperty rdf:resource="http://purl.obolibrary.org/obo/IAO_0000115"/>
        <owl:annotatedTarget>An image preprocessing layer that randomly rotates images during training.</owl:annotatedTarget>
        <oboInOwl:hasDbXref rdf:resource="https://www.tensorflow.org/api_docs/python/tf/keras/layers/RandomRotation"/>
    </owl:Axiom>
    


    <!-- https://w3id.org/aio/RandomTranslationLayer -->

    <owl:Class rdf:about="https://w3id.org/aio/RandomTranslationLayer">
        <rdfs:subClassOf rdf:resource="https://w3id.org/aio/Layer"/>
        <obo:IAO_0000115>An image preprocessing layer that randomly translates images during training.</obo:IAO_0000115>
        <oboInOwl:inSubset rdf:resource="https://w3id.org/aio/LayerSubset"/>
        <rdfs:comment>A preprocessing layer which randomly translates images during training. This layer will apply random translations to each image during training, filling empty space according to fill_mode. aInput pixel values can be of any range (e.g. [0., 1.) or [0, 255]) and of interger or floating point dtype. By default, the layer will output floats.</rdfs:comment>
        <rdfs:label>RandomTranslation Layer</rdfs:label>
    </owl:Class>
    <owl:Axiom>
        <owl:annotatedSource rdf:resource="https://w3id.org/aio/RandomTranslationLayer"/>
        <owl:annotatedProperty rdf:resource="http://purl.obolibrary.org/obo/IAO_0000115"/>
        <owl:annotatedTarget>An image preprocessing layer that randomly translates images during training.</owl:annotatedTarget>
        <oboInOwl:hasDbXref rdf:resource="https://www.tensorflow.org/api_docs/python/tf/keras/layers/RandomTranslation"/>
    </owl:Axiom>
    


    <!-- https://w3id.org/aio/RandomWidthLayer -->

    <owl:Class rdf:about="https://w3id.org/aio/RandomWidthLayer">
        <rdfs:subClassOf rdf:resource="https://w3id.org/aio/Layer"/>
        <obo:IAO_0000115>An image preprocessing layer that randomly varies image width during training.</obo:IAO_0000115>
        <oboInOwl:inSubset rdf:resource="https://w3id.org/aio/LayerSubset"/>
        <rdfs:comment>A preprocessing layer which randomly varies image width during training. This layer will randomly adjusts the width of a batch of images of a batch of images by a random factor. The input should be a 3D (unbatched) or 4D (batched) tensor in the &quot;channels_last&quot; image data format. Input pixel values can be of any range (e.g. [0., 1.) or [0, 255]) and of interger or floating point dtype. By default, the layer will output floats. By default, this layer is inactive during inference.</rdfs:comment>
        <rdfs:label>RandomWidth Layer</rdfs:label>
    </owl:Class>
    <owl:Axiom>
        <owl:annotatedSource rdf:resource="https://w3id.org/aio/RandomWidthLayer"/>
        <owl:annotatedProperty rdf:resource="http://purl.obolibrary.org/obo/IAO_0000115"/>
        <owl:annotatedTarget>An image preprocessing layer that randomly varies image width during training.</owl:annotatedTarget>
        <oboInOwl:hasDbXref rdf:resource="https://www.tensorflow.org/api_docs/python/tf/keras/layers/RandomWidth"/>
    </owl:Axiom>
    


    <!-- https://w3id.org/aio/RandomZoomLayer -->

    <owl:Class rdf:about="https://w3id.org/aio/RandomZoomLayer">
        <rdfs:subClassOf rdf:resource="https://w3id.org/aio/Layer"/>
        <obo:IAO_0000115>An image preprocessing layer that randomly zooms in or out on images during training.</obo:IAO_0000115>
        <oboInOwl:inSubset rdf:resource="https://w3id.org/aio/LayerSubset"/>
        <rdfs:comment>A preprocessing layer which randomly zooms images during training. This layer will randomly zoom in or out on each axis of an image independently, filling empty space according to fill_mode.Input pixel values can be of any range (e.g. [0., 1.) or [0, 255]) and of interger or floating point dtype. By default, the layer will output floats.</rdfs:comment>
        <rdfs:label>RandomZoom Layer</rdfs:label>
    </owl:Class>
    <owl:Axiom>
        <owl:annotatedSource rdf:resource="https://w3id.org/aio/RandomZoomLayer"/>
        <owl:annotatedProperty rdf:resource="http://purl.obolibrary.org/obo/IAO_0000115"/>
        <owl:annotatedTarget>An image preprocessing layer that randomly zooms in or out on images during training.</owl:annotatedTarget>
        <oboInOwl:hasDbXref rdf:resource="https://www.tensorflow.org/api_docs/python/tf/keras/layers/RandomZoom"/>
    </owl:Axiom>
    


    <!-- https://w3id.org/aio/RankingBias -->

    <owl:Class rdf:about="https://w3id.org/aio/RankingBias">
        <rdfs:subClassOf rdf:resource="https://w3id.org/aio/AnchoringBias"/>
        <obo:IAO_0000115>An anchoring bias characterized by the idea that top-ranked results are the most relevant and important leading to more clicks than other results.</obo:IAO_0000115>
        <oboInOwl:inSubset rdf:resource="https://w3id.org/aio/BiasSubset"/>
        <rdfs:label>Ranking Bias</rdfs:label>
    </owl:Class>
    <owl:Axiom>
        <owl:annotatedSource rdf:resource="https://w3id.org/aio/RankingBias"/>
        <owl:annotatedProperty rdf:resource="http://purl.obolibrary.org/obo/IAO_0000115"/>
        <owl:annotatedTarget>An anchoring bias characterized by the idea that top-ranked results are the most relevant and important leading to more clicks than other results.</owl:annotatedTarget>
        <oboInOwl:hasDbXref rdf:resource="https://doi.org/10.6028/NIST.SP.1270"/>
    </owl:Axiom>
    


    <!-- https://w3id.org/aio/RashomonEffectBias -->

    <owl:Class rdf:about="https://w3id.org/aio/RashomonEffectBias">
        <rdfs:subClassOf rdf:resource="https://w3id.org/aio/IndividualBias"/>
        <obo:IAO_0000115>An individual bias characterized by differences in perspective memory recall interpretation and reporting of the same event by multiple persons or witnesses.</obo:IAO_0000115>
        <oboInOwl:hasExactSynonym>Rashomon Effect</oboInOwl:hasExactSynonym>
        <oboInOwl:hasExactSynonym>Rashomon Principle</oboInOwl:hasExactSynonym>
        <oboInOwl:inSubset rdf:resource="https://w3id.org/aio/BiasSubset"/>
        <rdfs:comment>Differences in perspective, memory, recall, interpretation, and reporting of the same event by multiple persons or witnesses.</rdfs:comment>
        <rdfs:label>Rashomon Effect Bias</rdfs:label>
    </owl:Class>
    <owl:Axiom>
        <owl:annotatedSource rdf:resource="https://w3id.org/aio/RashomonEffectBias"/>
        <owl:annotatedProperty rdf:resource="http://purl.obolibrary.org/obo/IAO_0000115"/>
        <owl:annotatedTarget>An individual bias characterized by differences in perspective memory recall interpretation and reporting of the same event by multiple persons or witnesses.</owl:annotatedTarget>
        <oboInOwl:hasDbXref rdf:resource="https://doi.org/10.6028/NIST.SP.1270"/>
    </owl:Axiom>
    


    <!-- https://w3id.org/aio/ReLUFunction -->

    <owl:Class rdf:about="https://w3id.org/aio/ReLUFunction">
        <rdfs:subClassOf rdf:resource="https://w3id.org/aio/Function"/>
        <obo:IAO_0000115>An activation function that returns max(x 0) the element-wise maximum of 0 and the input tensor.</obo:IAO_0000115>
        <oboInOwl:hasExactSynonym>ReLU</oboInOwl:hasExactSynonym>
        <oboInOwl:hasExactSynonym>Rectified Linear Unit</oboInOwl:hasExactSynonym>
        <oboInOwl:inSubset rdf:resource="https://w3id.org/aio/FunctionSubset"/>
        <rdfs:comment>The ReLU activation function returns: max(x, 0), the element-wise maximum of 0 and the input tensor.</rdfs:comment>
        <rdfs:label>ReLU Function</rdfs:label>
    </owl:Class>
    <owl:Axiom>
        <owl:annotatedSource rdf:resource="https://w3id.org/aio/ReLUFunction"/>
        <owl:annotatedProperty rdf:resource="http://purl.obolibrary.org/obo/IAO_0000115"/>
        <owl:annotatedTarget>An activation function that returns max(x 0) the element-wise maximum of 0 and the input tensor.</owl:annotatedTarget>
        <oboInOwl:hasDbXref rdf:resource="https://www.tensorflow.org/api_docs/python/tf/keras/activations/relu"/>
    </owl:Axiom>
    


    <!-- https://w3id.org/aio/ReLULayer -->

    <owl:Class rdf:about="https://w3id.org/aio/ReLULayer">
        <rdfs:subClassOf rdf:resource="https://w3id.org/aio/ActivationLayer"/>
        <obo:IAO_0000115>An activation layer that applies the rectified linear unit function element-wise.</obo:IAO_0000115>
        <oboInOwl:inSubset rdf:resource="https://w3id.org/aio/LayerSubset"/>
        <rdfs:comment>Rectified Linear Unit activation function. With default values, it returns element-wise max(x, 0).</rdfs:comment>
        <rdfs:label>ReLU Layer</rdfs:label>
    </owl:Class>
    <owl:Axiom>
        <owl:annotatedSource rdf:resource="https://w3id.org/aio/ReLULayer"/>
        <owl:annotatedProperty rdf:resource="http://purl.obolibrary.org/obo/IAO_0000115"/>
        <owl:annotatedTarget>An activation layer that applies the rectified linear unit function element-wise.</owl:annotatedTarget>
        <oboInOwl:hasDbXref rdf:resource="https://www.tensorflow.org/api_docs/python/tf/keras/layers/ReLU"/>
    </owl:Axiom>
    


    <!-- https://w3id.org/aio/ReasoningLLM -->

    <owl:Class rdf:about="https://w3id.org/aio/ReasoningLLM">
        <rdfs:subClassOf rdf:resource="https://w3id.org/aio/LargeLanguageModel"/>
        <obo:IAO_0000115>A large language model that incorporates explicit reasoning capabilities leveraging logical rules axioms or external knowledge to make deductive inferences during language tasks.</obo:IAO_0000115>
        <oboInOwl:hasExactSynonym>Rational Large Language Model</oboInOwl:hasExactSynonym>
        <oboInOwl:hasExactSynonym>Reasoning Large Language Model</oboInOwl:hasExactSynonym>
        <oboInOwl:hasRelatedSynonym>logical inferences</oboInOwl:hasRelatedSynonym>
        <oboInOwl:hasRelatedSynonym>reasoning</oboInOwl:hasRelatedSynonym>
        <oboInOwl:inSubset rdf:resource="https://w3id.org/aio/ModelSubset"/>
        <rdfs:label>Reasoning LLM</rdfs:label>
    </owl:Class>
    <owl:Axiom>
        <owl:annotatedSource rdf:resource="https://w3id.org/aio/ReasoningLLM"/>
        <owl:annotatedProperty rdf:resource="http://purl.obolibrary.org/obo/IAO_0000115"/>
        <owl:annotatedTarget>A large language model that incorporates explicit reasoning capabilities leveraging logical rules axioms or external knowledge to make deductive inferences during language tasks.</owl:annotatedTarget>
        <oboInOwl:hasDbXref rdf:resource="https://doi.org/10.18653/v1/2023.acl-long.347"/>
    </owl:Axiom>
    


    <!-- https://w3id.org/aio/RecurrentLayer -->

    <owl:Class rdf:about="https://w3id.org/aio/RecurrentLayer">
        <rdfs:subClassOf rdf:resource="https://w3id.org/aio/Layer"/>
        <obo:IAO_0000115>A layer composed of recurrent units with the number equal to the hidden size of the layer.</obo:IAO_0000115>
        <oboInOwl:inSubset rdf:resource="https://w3id.org/aio/LayerSubset"/>
        <rdfs:label>Recurrent Layer</rdfs:label>
    </owl:Class>
    <owl:Axiom>
        <owl:annotatedSource rdf:resource="https://w3id.org/aio/RecurrentLayer"/>
        <owl:annotatedProperty rdf:resource="http://purl.obolibrary.org/obo/IAO_0000115"/>
        <owl:annotatedTarget>A layer composed of recurrent units with the number equal to the hidden size of the layer.</owl:annotatedTarget>
        <oboInOwl:hasDbXref rdf:resource="https://docs.nvidia.com/deepLearning/performance/dl-performance-recurrent/index.html#recurrent-layer"/>
    </owl:Axiom>
    


    <!-- https://w3id.org/aio/RecurrentNeuralNetwork -->

    <owl:Class rdf:about="https://w3id.org/aio/RecurrentNeuralNetwork">
        <rdfs:subClassOf rdf:resource="https://w3id.org/aio/Network"/>
        <obo:IAO_0000115>A deep neural network with connections forming a directed graph along a temporal sequence enabling dynamic behavior.</obo:IAO_0000115>
        <oboInOwl:hasExactSynonym>RN</oboInOwl:hasExactSynonym>
        <oboInOwl:hasExactSynonym>RecNN</oboInOwl:hasExactSynonym>
        <oboInOwl:hasExactSynonym>Recurrent Network</oboInOwl:hasExactSynonym>
        <oboInOwl:inSubset rdf:resource="https://w3id.org/aio/NetworkSubset"/>
        <rdfs:label>Recurrent Neural Network</rdfs:label>
    </owl:Class>
    


    <!-- https://w3id.org/aio/RecursiveLLM -->

    <owl:Class rdf:about="https://w3id.org/aio/RecursiveLLM">
        <rdfs:subClassOf rdf:resource="https://w3id.org/aio/LanguageModel"/>
        <obo:IAO_0000115>A large language model that uses recursive neural network architectures like TreeLSTMs to learn syntactic composition functions improving systematic generalization abilities.</obo:IAO_0000115>
        <oboInOwl:hasExactSynonym>Recursive Large Language Model</oboInOwl:hasExactSynonym>
        <oboInOwl:hasExactSynonym>Self-Attending Large Language Model</oboInOwl:hasExactSynonym>
        <oboInOwl:hasRelatedSynonym>iterative refinement</oboInOwl:hasRelatedSynonym>
        <oboInOwl:hasRelatedSynonym>self-attention</oboInOwl:hasRelatedSynonym>
        <oboInOwl:inSubset rdf:resource="https://w3id.org/aio/ModelSubset"/>
        <rdfs:label>Recursive LLM</rdfs:label>
    </owl:Class>
    <owl:Axiom>
        <owl:annotatedSource rdf:resource="https://w3id.org/aio/RecursiveLLM"/>
        <owl:annotatedProperty rdf:resource="http://purl.obolibrary.org/obo/IAO_0000115"/>
        <owl:annotatedTarget>A large language model that uses recursive neural network architectures like TreeLSTMs to learn syntactic composition functions improving systematic generalization abilities.</owl:annotatedTarget>
        <oboInOwl:hasDbXref rdf:resource="https://doi.org/10.1609/aaai.v33i01.33017450"/>
    </owl:Axiom>
    


    <!-- https://w3id.org/aio/RecursiveLanguageModel -->

    <owl:Class rdf:about="https://w3id.org/aio/RecursiveLanguageModel">
        <rdfs:subClassOf rdf:resource="https://w3id.org/aio/DeepNeuralNetwork"/>
        <rdfs:subClassOf>
            <owl:Restriction>
                <owl:onProperty rdf:resource="http://purl.obolibrary.org/obo/BFO_0000051"/>
                <owl:someValuesFrom rdf:resource="https://w3id.org/aio/InputLayer"/>
            </owl:Restriction>
        </rdfs:subClassOf>
        <rdfs:subClassOf>
            <owl:Restriction>
                <owl:onProperty rdf:resource="http://purl.obolibrary.org/obo/BFO_0000051"/>
                <owl:someValuesFrom rdf:resource="https://w3id.org/aio/MemoryCellLayer"/>
            </owl:Restriction>
        </rdfs:subClassOf>
        <rdfs:subClassOf>
            <owl:Restriction>
                <owl:onProperty rdf:resource="http://purl.obolibrary.org/obo/BFO_0000051"/>
                <owl:someValuesFrom rdf:resource="https://w3id.org/aio/OutputLayer"/>
            </owl:Restriction>
        </rdfs:subClassOf>
        <obo:IAO_0000115>A language model that uses recursive neural network architectures like TreeLSTMs to learn syntactic composition functions improving systematic generalization abilities.</obo:IAO_0000115>
        <oboInOwl:hasExactSynonym>RLM</oboInOwl:hasExactSynonym>
        <oboInOwl:hasRelatedSynonym>Compositional generalization</oboInOwl:hasRelatedSynonym>
        <oboInOwl:inSubset rdf:resource="https://w3id.org/aio/ModelSubset"/>
        <rdfs:comment>Layers: Input, Memory Cell, Output</rdfs:comment>
        <rdfs:label>Recursive Language Model</rdfs:label>
    </owl:Class>
    <owl:Axiom>
        <owl:annotatedSource rdf:resource="https://w3id.org/aio/RecursiveLanguageModel"/>
        <owl:annotatedProperty rdf:resource="http://purl.obolibrary.org/obo/IAO_0000115"/>
        <owl:annotatedTarget>A language model that uses recursive neural network architectures like TreeLSTMs to learn syntactic composition functions improving systematic generalization abilities.</owl:annotatedTarget>
        <oboInOwl:hasDbXref rdf:resource="https://en.wikipedia.org/wiki/Recurrent_neural_network"/>
    </owl:Axiom>
    


    <!-- https://w3id.org/aio/RecursiveNeuralNetwork -->

    <owl:Class rdf:about="https://w3id.org/aio/RecursiveNeuralNetwork">
        <rdfs:subClassOf rdf:resource="https://w3id.org/aio/DeepNeuralNetwork"/>
        <obo:IAO_0000115>A deep neural network that recursively applies weights over structured input to generate structured or scalar predictions.</obo:IAO_0000115>
        <oboInOwl:hasExactSynonym>RecuNN</oboInOwl:hasExactSynonym>
        <oboInOwl:hasExactSynonym>RvNN</oboInOwl:hasExactSynonym>
        <oboInOwl:inSubset rdf:resource="https://w3id.org/aio/NetworkSubset"/>
        <rdfs:label>Recursive Neural Network</rdfs:label>
    </owl:Class>
    <owl:Axiom>
        <owl:annotatedSource rdf:resource="https://w3id.org/aio/RecursiveNeuralNetwork"/>
        <owl:annotatedProperty rdf:resource="http://purl.obolibrary.org/obo/IAO_0000115"/>
        <owl:annotatedTarget>A deep neural network that recursively applies weights over structured input to generate structured or scalar predictions.</owl:annotatedTarget>
        <oboInOwl:hasDbXref rdf:resource="https://en.wikipedia.org/wiki/Recursive_neural_network"/>
    </owl:Axiom>
    


    <!-- https://w3id.org/aio/RegressionAnalysis -->

    <owl:Class rdf:about="https://w3id.org/aio/RegressionAnalysis">
        <rdfs:subClassOf rdf:resource="https://w3id.org/aio/SupervisedLearning"/>
        <obo:IAO_0000115>A set of statistical processes for estimating the relationships between a dependent variable and one or more independent variables.</obo:IAO_0000115>
        <oboInOwl:hasExactSynonym>Regression analysis</oboInOwl:hasExactSynonym>
        <oboInOwl:hasExactSynonym>Regression model</oboInOwl:hasExactSynonym>
        <oboInOwl:inSubset rdf:resource="https://w3id.org/aio/MachineLearningSubset"/>
        <rdfs:label>Regression Analysis</rdfs:label>
    </owl:Class>
    <owl:Axiom>
        <owl:annotatedSource rdf:resource="https://w3id.org/aio/RegressionAnalysis"/>
        <owl:annotatedProperty rdf:resource="http://purl.obolibrary.org/obo/IAO_0000115"/>
        <owl:annotatedTarget>A set of statistical processes for estimating the relationships between a dependent variable and one or more independent variables.</owl:annotatedTarget>
        <oboInOwl:hasDbXref rdf:resource="https://en.wikipedia.org/wiki/Regression_analysis"/>
    </owl:Axiom>
    


    <!-- https://w3id.org/aio/RegularizationLayer -->

    <owl:Class rdf:about="https://w3id.org/aio/RegularizationLayer">
        <rdfs:subClassOf rdf:resource="https://w3id.org/aio/Layer"/>
        <obo:IAO_0000115>A layer that applies penalties on layer parameters or layer activity during optimization summed into the loss function that the network optimizes.</obo:IAO_0000115>
        <oboInOwl:inSubset rdf:resource="https://w3id.org/aio/LayerSubset"/>
        <rdfs:comment>Regularizers allow you to apply penalties on layer parameters or layer activity during optimization. These penalties are summed into the loss function that the network optimizes. Regularization penalties are applied on a per-layer basis.</rdfs:comment>
        <rdfs:label>Regularization Layer</rdfs:label>
    </owl:Class>
    <owl:Axiom>
        <owl:annotatedSource rdf:resource="https://w3id.org/aio/RegularizationLayer"/>
        <owl:annotatedProperty rdf:resource="http://purl.obolibrary.org/obo/IAO_0000115"/>
        <owl:annotatedTarget>A layer that applies penalties on layer parameters or layer activity during optimization summed into the loss function that the network optimizes.</owl:annotatedTarget>
        <oboInOwl:hasDbXref rdf:resource="https://keras.io/api/layers/regularizers/"/>
    </owl:Axiom>
    


    <!-- https://w3id.org/aio/ReinforcementLearning -->

    <owl:Class rdf:about="https://w3id.org/aio/ReinforcementLearning">
        <rdfs:subClassOf rdf:resource="https://w3id.org/aio/MachineLearning"/>
        <obo:IAO_0000115>A type of machine learning focused on methods that do not require labeled input/output pairs or explicit correction of sub-optimal actions focusing instead on balancing exploration and exploitation to optimize performance over time.</obo:IAO_0000115>
        <oboInOwl:inSubset rdf:resource="https://w3id.org/aio/MachineLearningSubset"/>
        <rdfs:label>Reinforcement Learning</rdfs:label>
    </owl:Class>
    <owl:Axiom>
        <owl:annotatedSource rdf:resource="https://w3id.org/aio/ReinforcementLearning"/>
        <owl:annotatedProperty rdf:resource="http://purl.obolibrary.org/obo/IAO_0000115"/>
        <owl:annotatedTarget>A type of machine learning focused on methods that do not require labeled input/output pairs or explicit correction of sub-optimal actions focusing instead on balancing exploration and exploitation to optimize performance over time.</owl:annotatedTarget>
        <oboInOwl:hasDbXref rdf:resource="https://en.wikipedia.org/wiki/Reinforcement_learning"/>
    </owl:Axiom>
    


    <!-- https://w3id.org/aio/ReinforcementLearningLLM -->

    <owl:Class rdf:about="https://w3id.org/aio/ReinforcementLearningLLM">
        <rdfs:subClassOf rdf:resource="https://w3id.org/aio/LargeLanguageModel"/>
        <obo:IAO_0000115>A large language model that is fine-tuned using reinforcement learning where the model receives rewards for generating text that satisfies certain desired properties or objectives improving the quality safety or alignment of generated text.</obo:IAO_0000115>
        <oboInOwl:hasExactSynonym>RL-Large Language Model</oboInOwl:hasExactSynonym>
        <oboInOwl:hasExactSynonym>Reinforcement Learning Large Language Model</oboInOwl:hasExactSynonym>
        <oboInOwl:hasRelatedSynonym>decision transformers</oboInOwl:hasRelatedSynonym>
        <oboInOwl:hasRelatedSynonym>reward modeling</oboInOwl:hasRelatedSynonym>
        <oboInOwl:inSubset rdf:resource="https://w3id.org/aio/ModelSubset"/>
        <rdfs:comment>An RL-LLM is a language model fine-tuned using reinforcement learning, where the model receives rewards for generating text that satisfies certain desired properties or objectives. This can improve the quality, safety, or alignment of generated text.</rdfs:comment>
        <rdfs:label>Reinforcement Learning LLM</rdfs:label>
    </owl:Class>
    


    <!-- https://w3id.org/aio/RepeatVectorLayer -->

    <owl:Class rdf:about="https://w3id.org/aio/RepeatVectorLayer">
        <rdfs:subClassOf rdf:resource="https://w3id.org/aio/ReshapingLayer"/>
        <obo:IAO_0000115>A layer that repeats the input n times.</obo:IAO_0000115>
        <oboInOwl:inSubset rdf:resource="https://w3id.org/aio/LayerSubset"/>
        <rdfs:comment>Repeats the input n times.</rdfs:comment>
        <rdfs:label>RepeatVector Layer</rdfs:label>
    </owl:Class>
    <owl:Axiom>
        <owl:annotatedSource rdf:resource="https://w3id.org/aio/RepeatVectorLayer"/>
        <owl:annotatedProperty rdf:resource="http://purl.obolibrary.org/obo/IAO_0000115"/>
        <owl:annotatedTarget>A layer that repeats the input n times.</owl:annotatedTarget>
        <oboInOwl:hasDbXref rdf:resource="https://www.tensorflow.org/api_docs/python/tf/keras/layers/RepeatVector"/>
    </owl:Axiom>
    


    <!-- https://w3id.org/aio/RepresentationBias -->

    <owl:Class rdf:about="https://w3id.org/aio/RepresentationBias">
        <rdfs:subClassOf rdf:resource="https://w3id.org/aio/SelectionAndSamplingBias"/>
        <obo:IAO_0000115>A selection and sampling bias due to non-random sampling of subgroups making trends non-generalizable to new populations.</obo:IAO_0000115>
        <oboInOwl:inSubset rdf:resource="https://w3id.org/aio/BiasSubset"/>
        <rdfs:comment>Bias due to non-random sampling of subgroups, making trends non-generalizable to new populations.</rdfs:comment>
        <rdfs:label>Representation Bias</rdfs:label>
    </owl:Class>
    <owl:Axiom>
        <owl:annotatedSource rdf:resource="https://w3id.org/aio/RepresentationBias"/>
        <owl:annotatedProperty rdf:resource="http://purl.obolibrary.org/obo/IAO_0000115"/>
        <owl:annotatedTarget>A selection and sampling bias due to non-random sampling of subgroups making trends non-generalizable to new populations.</owl:annotatedTarget>
        <oboInOwl:hasDbXref rdf:resource="https://doi.org/10.6028/NIST.SP.1270"/>
    </owl:Axiom>
    


    <!-- https://w3id.org/aio/RepresentationLearning -->

    <owl:Class rdf:about="https://w3id.org/aio/RepresentationLearning">
        <rdfs:subClassOf rdf:resource="https://w3id.org/aio/DeepNeuralNetwork"/>
        <obo:IAO_0000115>A deep neural network that discovers representations required for feature detection or classification from raw data.</obo:IAO_0000115>
        <oboInOwl:hasExactSynonym>Feature Learning</oboInOwl:hasExactSynonym>
        <oboInOwl:inSubset rdf:resource="https://w3id.org/aio/NetworkSubset"/>
        <rdfs:comment>Discovering representations required for feature detection or classification from raw data.</rdfs:comment>
        <rdfs:label>Representation Learning</rdfs:label>
    </owl:Class>
    <owl:Axiom>
        <owl:annotatedSource rdf:resource="https://w3id.org/aio/RepresentationLearning"/>
        <owl:annotatedProperty rdf:resource="http://purl.obolibrary.org/obo/IAO_0000115"/>
        <owl:annotatedTarget>A deep neural network that discovers representations required for feature detection or classification from raw data.</owl:annotatedTarget>
        <oboInOwl:hasDbXref rdf:resource="https://en.wikipedia.org/wiki/Feature_learning"/>
    </owl:Axiom>
    


    <!-- https://w3id.org/aio/RescalingLayer -->

    <owl:Class rdf:about="https://w3id.org/aio/RescalingLayer">
        <rdfs:subClassOf rdf:resource="https://w3id.org/aio/ImagePreprocessingLayer"/>
        <obo:IAO_0000115>A preprocessing layer that rescales input values to a new range.</obo:IAO_0000115>
        <oboInOwl:inSubset rdf:resource="https://w3id.org/aio/LayerSubset"/>
        <rdfs:label>Rescaling Layer</rdfs:label>
    </owl:Class>
    <owl:Axiom>
        <owl:annotatedSource rdf:resource="https://w3id.org/aio/RescalingLayer"/>
        <owl:annotatedProperty rdf:resource="http://purl.obolibrary.org/obo/IAO_0000115"/>
        <owl:annotatedTarget>A preprocessing layer that rescales input values to a new range.</owl:annotatedTarget>
        <oboInOwl:hasDbXref rdf:resource="https://www.tensorflow.org/api_docs/python/tf/keras/layers/Rescaling"/>
    </owl:Axiom>
    


    <!-- https://w3id.org/aio/ReshapeLayer -->

    <owl:Class rdf:about="https://w3id.org/aio/ReshapeLayer">
        <rdfs:subClassOf rdf:resource="https://w3id.org/aio/ReshapingLayer"/>
        <obo:IAO_0000115>A layer that reshapes the inputs into the given shape.</obo:IAO_0000115>
        <oboInOwl:inSubset rdf:resource="https://w3id.org/aio/LayerSubset"/>
        <rdfs:label>Reshape Layer</rdfs:label>
    </owl:Class>
    <owl:Axiom>
        <owl:annotatedSource rdf:resource="https://w3id.org/aio/ReshapeLayer"/>
        <owl:annotatedProperty rdf:resource="http://purl.obolibrary.org/obo/IAO_0000115"/>
        <owl:annotatedTarget>A layer that reshapes the inputs into the given shape.</owl:annotatedTarget>
        <oboInOwl:hasDbXref rdf:resource="https://www.tensorflow.org/api_docs/python/tf/keras/layers/Reshape"/>
    </owl:Axiom>
    


    <!-- https://w3id.org/aio/ReshapingLayer -->

    <owl:Class rdf:about="https://w3id.org/aio/ReshapingLayer">
        <rdfs:subClassOf rdf:resource="https://w3id.org/aio/Layer"/>
        <obo:IAO_0000115>A layer that is used to change the shape of the input.</obo:IAO_0000115>
        <oboInOwl:hasExactSynonym>Reshape Layer</oboInOwl:hasExactSynonym>
        <oboInOwl:inSubset rdf:resource="https://w3id.org/aio/LayerSubset"/>
        <rdfs:comment>Reshape layers are used to change the shape of the input.</rdfs:comment>
        <rdfs:label>Reshaping Layer</rdfs:label>
    </owl:Class>
    <owl:Axiom>
        <owl:annotatedSource rdf:resource="https://w3id.org/aio/ReshapingLayer"/>
        <owl:annotatedProperty rdf:resource="http://purl.obolibrary.org/obo/IAO_0000115"/>
        <owl:annotatedTarget>A layer that is used to change the shape of the input.</owl:annotatedTarget>
        <oboInOwl:hasDbXref rdf:resource="https://keras.io/api/layers/reshaping_layers/reshape/"/>
    </owl:Axiom>
    


    <!-- https://w3id.org/aio/ResidualNeuralNetwork -->

    <owl:Class rdf:about="https://w3id.org/aio/ResidualNeuralNetwork">
        <rdfs:subClassOf rdf:resource="https://w3id.org/aio/DeepNeuralNetwork"/>
        <rdfs:subClassOf>
            <owl:Restriction>
                <owl:onProperty rdf:resource="http://purl.obolibrary.org/obo/BFO_0000051"/>
                <owl:someValuesFrom rdf:resource="https://w3id.org/aio/AdditionLayer"/>
            </owl:Restriction>
        </rdfs:subClassOf>
        <rdfs:subClassOf>
            <owl:Restriction>
                <owl:onProperty rdf:resource="http://purl.obolibrary.org/obo/BFO_0000051"/>
                <owl:someValuesFrom rdf:resource="https://w3id.org/aio/BatchNormalizationLayer"/>
            </owl:Restriction>
        </rdfs:subClassOf>
        <rdfs:subClassOf>
            <owl:Restriction>
                <owl:onProperty rdf:resource="http://purl.obolibrary.org/obo/BFO_0000051"/>
                <owl:someValuesFrom rdf:resource="https://w3id.org/aio/InputLayer"/>
            </owl:Restriction>
        </rdfs:subClassOf>
        <rdfs:subClassOf>
            <owl:Restriction>
                <owl:onProperty rdf:resource="http://purl.obolibrary.org/obo/BFO_0000051"/>
                <owl:someValuesFrom rdf:resource="https://w3id.org/aio/ReLULayer"/>
            </owl:Restriction>
        </rdfs:subClassOf>
        <rdfs:subClassOf>
            <owl:Restriction>
                <owl:onProperty rdf:resource="http://purl.obolibrary.org/obo/BFO_0000051"/>
                <owl:someValuesFrom rdf:resource="https://w3id.org/aio/WeightedLayer"/>
            </owl:Restriction>
        </rdfs:subClassOf>
        <obo:IAO_0000115>A deep neural network that employs skip connections to bypass layers facilitating learning of residual functions.</obo:IAO_0000115>
        <oboInOwl:hasExactSynonym>DRN</oboInOwl:hasExactSynonym>
        <oboInOwl:hasExactSynonym>Deep Residual Network</oboInOwl:hasExactSynonym>
        <oboInOwl:hasExactSynonym>ResNN</oboInOwl:hasExactSynonym>
        <oboInOwl:hasExactSynonym>ResNet</oboInOwl:hasExactSynonym>
        <oboInOwl:inSubset rdf:resource="https://w3id.org/aio/NetworkSubset"/>
        <rdfs:comment>Layers: Input, Weight, BN, ReLU, Weight, BN, Addition, ReLU</rdfs:comment>
        <rdfs:label>Residual Neural Network</rdfs:label>
    </owl:Class>
    <owl:Axiom>
        <owl:annotatedSource rdf:resource="https://w3id.org/aio/ResidualNeuralNetwork"/>
        <owl:annotatedProperty rdf:resource="http://purl.obolibrary.org/obo/IAO_0000115"/>
        <owl:annotatedTarget>A deep neural network that employs skip connections to bypass layers facilitating learning of residual functions.</owl:annotatedTarget>
        <oboInOwl:hasDbXref rdf:resource="https://en.wikipedia.org/wiki/Residual_neural_network"/>
    </owl:Axiom>
    


    <!-- https://w3id.org/aio/ResizingLayer -->

    <owl:Class rdf:about="https://w3id.org/aio/ResizingLayer">
        <rdfs:subClassOf rdf:resource="https://w3id.org/aio/ImagePreprocessingLayer"/>
        <obo:IAO_0000115>A preprocessing layer that resizes images to a target size.</obo:IAO_0000115>
        <oboInOwl:inSubset rdf:resource="https://w3id.org/aio/LayerSubset"/>
        <rdfs:comment>A preprocessing layer which resizes images. This layer resizes an image input to a target height and width. The input should be a 4D (batched) or 3D (unbatched) tensor in &quot;channels_last&quot; format. Input pixel values can be of any range (e.g. [0., 1.) or [0, 255]) and of interger or floating point dtype. By default, the layer will output floats. This layer can be called on tf.RaggedTensor batches of input images of distinct sizes, and will resize the outputs to dense tensors of uniform size.</rdfs:comment>
        <rdfs:label>Resizing Layer</rdfs:label>
    </owl:Class>
    <owl:Axiom>
        <owl:annotatedSource rdf:resource="https://w3id.org/aio/ResizingLayer"/>
        <owl:annotatedProperty rdf:resource="http://purl.obolibrary.org/obo/IAO_0000115"/>
        <owl:annotatedTarget>A preprocessing layer that resizes images to a target size.</owl:annotatedTarget>
        <oboInOwl:hasDbXref rdf:resource="https://www.tensorflow.org/api_docs/python/tf/keras/layers/Resizing"/>
    </owl:Axiom>
    


    <!-- https://w3id.org/aio/RestrictedBoltzmannMachine -->

    <owl:Class rdf:about="https://w3id.org/aio/RestrictedBoltzmannMachine">
        <rdfs:subClassOf rdf:resource="https://w3id.org/aio/BoltzmannMachineNetwork"/>
        <obo:IAO_0000115>A Boltzmann machine network that learns the probability distribution of its input data.</obo:IAO_0000115>
        <oboInOwl:hasExactSynonym>RBM</oboInOwl:hasExactSynonym>
        <oboInOwl:inSubset rdf:resource="https://w3id.org/aio/NetworkSubset"/>
        <rdfs:comment>Layers: Backfed Input, Probabilistic Hidden</rdfs:comment>
        <rdfs:label>Restricted Boltzmann Machine</rdfs:label>
    </owl:Class>
    <owl:Axiom>
        <owl:annotatedSource rdf:resource="https://w3id.org/aio/RestrictedBoltzmannMachine"/>
        <owl:annotatedProperty rdf:resource="http://purl.obolibrary.org/obo/IAO_0000115"/>
        <owl:annotatedTarget>A Boltzmann machine network that learns the probability distribution of its input data.</owl:annotatedTarget>
        <oboInOwl:hasDbXref rdf:resource="https://en.wikipedia.org/wiki/Restricted_Boltzmann_machine"/>
    </owl:Axiom>
    


    <!-- https://w3id.org/aio/RetrievalAugmentedLLM -->

    <owl:Class rdf:about="https://w3id.org/aio/RetrievalAugmentedLLM">
        <rdfs:subClassOf rdf:resource="https://w3id.org/aio/LargeLanguageModel"/>
        <obo:IAO_0000115>A LLM which combines a pre-trained language model with a retrieval system that can access external knowledge sources. This allows the model to condition its generation on relevant retrieved knowledge, improving factual accuracy and knowledge grounding.</obo:IAO_0000115>
        <oboInOwl:hasExactSynonym>Retrieval-Augmented Large Language Model</oboInOwl:hasExactSynonym>
        <oboInOwl:hasRelatedSynonym>knowledge grounding</oboInOwl:hasRelatedSynonym>
        <oboInOwl:hasRelatedSynonym>open-book question answering</oboInOwl:hasRelatedSynonym>
        <oboInOwl:inSubset rdf:resource="https://w3id.org/aio/ModelSubset"/>
        <rdfs:label>Retrieval-Augmented LLM</rdfs:label>
    </owl:Class>
    


    <!-- https://w3id.org/aio/RidgeRegression -->

    <owl:Class rdf:about="https://w3id.org/aio/RidgeRegression">
        <rdfs:subClassOf rdf:resource="https://w3id.org/aio/RegressionAnalysis"/>
        <obo:IAO_0000115>A regression analysis method that estimates the coefficients of multiple regression models in scenarios where the independent variables are highly correlated.</obo:IAO_0000115>
        <oboInOwl:inSubset rdf:resource="https://w3id.org/aio/MachineLearningSubset"/>
        <rdfs:label>Ridge Regression</rdfs:label>
    </owl:Class>
    <owl:Axiom>
        <owl:annotatedSource rdf:resource="https://w3id.org/aio/RidgeRegression"/>
        <owl:annotatedProperty rdf:resource="http://purl.obolibrary.org/obo/IAO_0000115"/>
        <owl:annotatedTarget>A regression analysis method that estimates the coefficients of multiple regression models in scenarios where the independent variables are highly correlated.</owl:annotatedTarget>
        <oboInOwl:hasDbXref rdf:resource="https://en.wikipedia.org/wiki/Ridge_regression"/>
    </owl:Axiom>
    


    <!-- https://w3id.org/aio/SELUFunction -->

    <owl:Class rdf:about="https://w3id.org/aio/SELUFunction">
        <rdfs:subClassOf rdf:resource="https://w3id.org/aio/Function"/>
        <obo:IAO_0000115>An activation function that multiplies scale (&gt; 1) with the output of the ELU function to ensure a slope larger than one for positive inputs.</obo:IAO_0000115>
        <oboInOwl:hasExactSynonym>SELU</oboInOwl:hasExactSynonym>
        <oboInOwl:hasExactSynonym>Scaled Exponential Linear Unit</oboInOwl:hasExactSynonym>
        <oboInOwl:inSubset rdf:resource="https://w3id.org/aio/FunctionSubset"/>
        <rdfs:label>SELU Function</rdfs:label>
    </owl:Class>
    <owl:Axiom>
        <owl:annotatedSource rdf:resource="https://w3id.org/aio/SELUFunction"/>
        <owl:annotatedProperty rdf:resource="http://purl.obolibrary.org/obo/IAO_0000115"/>
        <owl:annotatedTarget>An activation function that multiplies scale (&gt; 1) with the output of the ELU function to ensure a slope larger than one for positive inputs.</owl:annotatedTarget>
        <oboInOwl:hasDbXref rdf:resource="https://www.tensorflow.org/api_docs/python/tf/keras/activations/selu"/>
    </owl:Axiom>
    


    <!-- https://w3id.org/aio/SeasonalAutoregressiveIntegratedMovingAverage -->

    <owl:Class rdf:about="https://w3id.org/aio/SeasonalAutoregressiveIntegratedMovingAverage">
        <rdfs:subClassOf rdf:resource="https://w3id.org/aio/Model"/>
        <obo:IAO_0000115>A model that extends ARIMA, explicitly supporting univariate time series data with a seasonal component, combining seasonal differencing with ARIMA modeling.</obo:IAO_0000115>
        <oboInOwl:hasExactSynonym>SARIMA</oboInOwl:hasExactSynonym>
        <oboInOwl:inSubset rdf:resource="https://w3id.org/aio/ModelSubset"/>
        <rdfs:label>Seasonal Autoregressive Integrated Moving-Average</rdfs:label>
    </owl:Class>
    


    <!-- https://w3id.org/aio/SelectionAndSamplingBias -->

    <owl:Class rdf:about="https://w3id.org/aio/SelectionAndSamplingBias">
        <rdfs:subClassOf rdf:resource="https://w3id.org/aio/ComputationalBias"/>
        <obo:IAO_0000115>A computational bias introduced by non-random selection of individuals groups or data failing to ensure representativeness.</obo:IAO_0000115>
        <oboInOwl:hasExactSynonym>Sampling Bias</oboInOwl:hasExactSynonym>
        <oboInOwl:hasExactSynonym>Selection Bias</oboInOwl:hasExactSynonym>
        <oboInOwl:hasExactSynonym>Selection Effect</oboInOwl:hasExactSynonym>
        <oboInOwl:inSubset rdf:resource="https://w3id.org/aio/BiasSubset"/>
        <rdfs:comment>Bias introduced by non-random selection of individuals, groups, or data, failing to ensure representativeness.</rdfs:comment>
        <rdfs:label>Selection And Sampling Bias</rdfs:label>
    </owl:Class>
    <owl:Axiom>
        <owl:annotatedSource rdf:resource="https://w3id.org/aio/SelectionAndSamplingBias"/>
        <owl:annotatedProperty rdf:resource="http://purl.obolibrary.org/obo/IAO_0000115"/>
        <owl:annotatedTarget>A computational bias introduced by non-random selection of individuals groups or data failing to ensure representativeness.</owl:annotatedTarget>
        <oboInOwl:hasDbXref rdf:resource="https://doi.org/10.6028/NIST.SP.1270"/>
    </owl:Axiom>
    


    <!-- https://w3id.org/aio/SelectiveAdherenceBias -->

    <owl:Class rdf:about="https://w3id.org/aio/SelectiveAdherenceBias">
        <rdfs:subClassOf rdf:resource="https://w3id.org/aio/IndividualBias"/>
        <obo:IAO_0000115>An individual bias characterized by the tendency to selectively adopt algorithmic advice that matches pre-existing beliefs and stereotypes.</obo:IAO_0000115>
        <oboInOwl:inSubset rdf:resource="https://w3id.org/aio/BiasSubset"/>
        <rdfs:label>Selective Adherence Bias</rdfs:label>
    </owl:Class>
    <owl:Axiom>
        <owl:annotatedSource rdf:resource="https://w3id.org/aio/SelectiveAdherenceBias"/>
        <owl:annotatedProperty rdf:resource="http://purl.obolibrary.org/obo/IAO_0000115"/>
        <owl:annotatedTarget>An individual bias characterized by the tendency to selectively adopt algorithmic advice that matches pre-existing beliefs and stereotypes.</owl:annotatedTarget>
        <oboInOwl:hasDbXref rdf:resource="https://doi.org/10.6028/NIST.SP.1270"/>
    </owl:Axiom>
    


    <!-- https://w3id.org/aio/SelfSupervisedLLM -->

    <owl:Class rdf:about="https://w3id.org/aio/SelfSupervisedLLM">
        <rdfs:subClassOf rdf:resource="https://w3id.org/aio/LargeLanguageModel"/>
        <obo:IAO_0000115>A LLM which learns rich representations by solving pretext tasks that involve predicting parts of the input from other observed parts of the data, without relying on human-annotated labels.</obo:IAO_0000115>
        <oboInOwl:hasRelatedSynonym>Pretext tasks</oboInOwl:hasRelatedSynonym>
        <oboInOwl:inSubset rdf:resource="https://w3id.org/aio/ModelSubset"/>
        <rdfs:label>Self-Supervised LLM</rdfs:label>
    </owl:Class>
    


    <!-- https://w3id.org/aio/SelfsupervisedLearning -->

    <owl:Class rdf:about="https://w3id.org/aio/SelfsupervisedLearning">
        <rdfs:subClassOf rdf:resource="https://w3id.org/aio/MachineLearning"/>
        <obo:IAO_0000115>A machine learning that is intermediate between supervised and unsupervised learning and predicts parts of the input data from other observed parts without relying on human-annotated labels.</obo:IAO_0000115>
        <oboInOwl:inSubset rdf:resource="https://w3id.org/aio/MachineLearningSubset"/>
        <rdfs:label>Self-supervised Learning</rdfs:label>
    </owl:Class>
    <owl:Axiom>
        <owl:annotatedSource rdf:resource="https://w3id.org/aio/SelfsupervisedLearning"/>
        <owl:annotatedProperty rdf:resource="http://purl.obolibrary.org/obo/IAO_0000115"/>
        <owl:annotatedTarget>A machine learning that is intermediate between supervised and unsupervised learning and predicts parts of the input data from other observed parts without relying on human-annotated labels.</owl:annotatedTarget>
        <oboInOwl:hasDbXref rdf:resource="https://en.wikipedia.org/wiki/Self-supervised_learning"/>
    </owl:Axiom>
    


    <!-- https://w3id.org/aio/SemiSupervisedLLM -->

    <owl:Class rdf:about="https://w3id.org/aio/SemiSupervisedLLM">
        <rdfs:subClassOf rdf:resource="https://w3id.org/aio/LargeLanguageModel"/>
        <obo:IAO_0000115>A LLM which combines self-supervised pretraining on unlabeled data with supervised fine-tuning on labeled task data.</obo:IAO_0000115>
        <oboInOwl:hasExactSynonym>Semi-Supervised Large Language Model</oboInOwl:hasExactSynonym>
        <oboInOwl:hasRelatedSynonym>self-training</oboInOwl:hasRelatedSynonym>
        <oboInOwl:inSubset rdf:resource="https://w3id.org/aio/ModelSubset"/>
        <rdfs:label>Semi-Supervised LLM</rdfs:label>
    </owl:Class>
    


    <!-- https://w3id.org/aio/SeparableConvolution1DLayer -->

    <owl:Class rdf:about="https://w3id.org/aio/SeparableConvolution1DLayer">
        <rdfs:subClassOf rdf:resource="https://w3id.org/aio/ConvolutionalLayer"/>
        <obo:IAO_0000115>A layer that performs depthwise separable 1D convolution.</obo:IAO_0000115>
        <oboInOwl:hasExactSynonym>SeparableConv1D Layer</oboInOwl:hasExactSynonym>
        <oboInOwl:inSubset rdf:resource="https://w3id.org/aio/LayerSubset"/>
        <rdfs:comment>Depthwise separable 1D convolution. This layer performs a depthwise convolution that acts separately on channels, followed by a pointwise convolution that mixes channels. If use_bias is True and a bias initializer is provided, it adds a bias vector to the output. It then optionally applies an activation function to produce the final output.a</rdfs:comment>
        <rdfs:label>SeparableConvolution1D Layer</rdfs:label>
    </owl:Class>
    <owl:Axiom>
        <owl:annotatedSource rdf:resource="https://w3id.org/aio/SeparableConvolution1DLayer"/>
        <owl:annotatedProperty rdf:resource="http://purl.obolibrary.org/obo/IAO_0000115"/>
        <owl:annotatedTarget>A layer that performs depthwise separable 1D convolution.</owl:annotatedTarget>
        <oboInOwl:hasDbXref rdf:resource="https://www.tensorflow.org/api_docs/python/tf/keras/layers/SeparableConv1D"/>
    </owl:Axiom>
    


    <!-- https://w3id.org/aio/SeparableConvolution2DLayer -->

    <owl:Class rdf:about="https://w3id.org/aio/SeparableConvolution2DLayer">
        <rdfs:subClassOf rdf:resource="https://w3id.org/aio/ConvolutionalLayer"/>
        <obo:IAO_0000115>A layer that performs depthwise separable 2D convolution.</obo:IAO_0000115>
        <oboInOwl:hasExactSynonym>SeparableConv2D Layer</oboInOwl:hasExactSynonym>
        <oboInOwl:inSubset rdf:resource="https://w3id.org/aio/LayerSubset"/>
        <rdfs:comment>Depthwise separable 2D convolution. Separable convolutions consist of first performing a depthwise spatial convolution (which acts on each input channel separately) followed by a pointwise convolution which mixes the resulting output channels. The depth_multiplier argument controls how many output channels are generated per input channel in the depthwise step. Intuitively, separable convolutions can be understood as a way to factorize a convolution kernel into two smaller kernels, or as an extreme version of an Inception block.</rdfs:comment>
        <rdfs:label>SeparableConvolution2D Layer</rdfs:label>
    </owl:Class>
    <owl:Axiom>
        <owl:annotatedSource rdf:resource="https://w3id.org/aio/SeparableConvolution2DLayer"/>
        <owl:annotatedProperty rdf:resource="http://purl.obolibrary.org/obo/IAO_0000115"/>
        <owl:annotatedTarget>A layer that performs depthwise separable 2D convolution.</owl:annotatedTarget>
        <oboInOwl:hasDbXref rdf:resource="https://www.tensorflow.org/api_docs/python/tf/keras/layers/SeparableConv2D"/>
    </owl:Axiom>
    


    <!-- https://w3id.org/aio/SigmoidFunction -->

    <owl:Class rdf:about="https://w3id.org/aio/SigmoidFunction">
        <rdfs:subClassOf rdf:resource="https://w3id.org/aio/Function"/>
        <obo:IAO_0000115>An activation function that applies the sigmoid activation function sigmoid(x) = 1 / (1 + exp(-x)) always returning a value between 0 and 1.</obo:IAO_0000115>
        <oboInOwl:inSubset rdf:resource="https://w3id.org/aio/FunctionSubset"/>
        <rdfs:comment>Applies the sigmoid activation function sigmoid(x) = 1 / (1 + exp(-x)). For small values (&lt;-5), sigmoid returns a value close to zero, and for large values (&gt;5) the result of the function gets close to 1. Sigmoid is equivalent to a 2-element Softmax, where the second element is assumed to be zero. The sigmoid function always returns a value between 0 and 1.</rdfs:comment>
        <rdfs:label>Sigmoid Function</rdfs:label>
    </owl:Class>
    <owl:Axiom>
        <owl:annotatedSource rdf:resource="https://w3id.org/aio/SigmoidFunction"/>
        <owl:annotatedProperty rdf:resource="http://purl.obolibrary.org/obo/IAO_0000115"/>
        <owl:annotatedTarget>An activation function that applies the sigmoid activation function sigmoid(x) = 1 / (1 + exp(-x)) always returning a value between 0 and 1.</owl:annotatedTarget>
        <oboInOwl:hasDbXref rdf:resource="https://www.tensorflow.org/api_docs/python/tf/keras/activations/sigmoid"/>
    </owl:Axiom>
    


    <!-- https://w3id.org/aio/SimpleRNNCellLayer -->

    <owl:Class rdf:about="https://w3id.org/aio/SimpleRNNCellLayer">
        <rdfs:subClassOf rdf:resource="https://w3id.org/aio/Layer"/>
        <obo:IAO_0000115>A layer that processes one step within the whole time sequence input for a SimpleRNN layer.</obo:IAO_0000115>
        <oboInOwl:inSubset rdf:resource="https://w3id.org/aio/LayerSubset"/>
        <rdfs:comment>Cell class for SimpleRNN. This class processes one step within the whole time sequence input, whereas tf.keras.layer.SimpleRNN processes the whole sequence.</rdfs:comment>
        <rdfs:label>SimpleRNNCell Layer</rdfs:label>
    </owl:Class>
    <owl:Axiom>
        <owl:annotatedSource rdf:resource="https://w3id.org/aio/SimpleRNNCellLayer"/>
        <owl:annotatedProperty rdf:resource="http://purl.obolibrary.org/obo/IAO_0000115"/>
        <owl:annotatedTarget>A layer that processes one step within the whole time sequence input for a SimpleRNN layer.</owl:annotatedTarget>
        <oboInOwl:hasDbXref rdf:resource="https://www.tensorflow.org/api_docs/python/tf/keras/layers/SimpleRNNCell"/>
    </owl:Axiom>
    


    <!-- https://w3id.org/aio/SimpleRNNLayer -->

    <owl:Class rdf:about="https://w3id.org/aio/SimpleRNNLayer">
        <rdfs:subClassOf rdf:resource="https://w3id.org/aio/RecurrentLayer"/>
        <obo:IAO_0000115>A recurrent layer that implements a fully-connected RNN where the output is to be fed back to input.</obo:IAO_0000115>
        <oboInOwl:inSubset rdf:resource="https://w3id.org/aio/LayerSubset"/>
        <rdfs:comment>Fully-connected RNN where the output is to be fed back to input.</rdfs:comment>
        <rdfs:label>SimpleRNN Layer</rdfs:label>
    </owl:Class>
    <owl:Axiom>
        <owl:annotatedSource rdf:resource="https://w3id.org/aio/SimpleRNNLayer"/>
        <owl:annotatedProperty rdf:resource="http://purl.obolibrary.org/obo/IAO_0000115"/>
        <owl:annotatedTarget>A recurrent layer that implements a fully-connected RNN where the output is to be fed back to input.</owl:annotatedTarget>
        <oboInOwl:hasDbXref rdf:resource="https://www.tensorflow.org/api_docs/python/tf/keras/layers/SimpleRNN"/>
    </owl:Axiom>
    


    <!-- https://w3id.org/aio/SimponsParadoxBias -->

    <owl:Class rdf:about="https://w3id.org/aio/SimponsParadoxBias">
        <rdfs:subClassOf rdf:resource="https://w3id.org/aio/SelectionAndSamplingBias"/>
        <obo:IAO_0000115>Ahere the association between two variables changes when controlling for another variable.</obo:IAO_0000115>
        <oboInOwl:hasExactSynonym>Simpson&apos;s Paradox</oboInOwl:hasExactSynonym>
        <oboInOwl:inSubset rdf:resource="https://w3id.org/aio/BiasSubset"/>
        <rdfs:label>Simpon&apos;s Paradox Bias</rdfs:label>
    </owl:Class>
    <owl:Axiom>
        <owl:annotatedSource rdf:resource="https://w3id.org/aio/SimponsParadoxBias"/>
        <owl:annotatedProperty rdf:resource="http://purl.obolibrary.org/obo/IAO_0000115"/>
        <owl:annotatedTarget>Ahere the association between two variables changes when controlling for another variable.</owl:annotatedTarget>
        <oboInOwl:hasDbXref rdf:resource="https://doi.org/10.6028/NIST.SP.1270"/>
    </owl:Axiom>
    


    <!-- https://w3id.org/aio/SocietalBias -->

    <owl:Class rdf:about="https://w3id.org/aio/SocietalBias">
        <rdfs:subClassOf rdf:resource="https://w3id.org/aio/Bias"/>
        <obo:IAO_0000115>A bias characterized by being for or against groups or individuals based on social identities demographic factors or immutable physical characteristics often manifesting as stereotypes.</obo:IAO_0000115>
        <oboInOwl:inSubset rdf:resource="https://w3id.org/aio/BiasSubset"/>
        <rdfs:label>Societal Bias</rdfs:label>
    </owl:Class>
    <owl:Axiom>
        <owl:annotatedSource rdf:resource="https://w3id.org/aio/SocietalBias"/>
        <owl:annotatedProperty rdf:resource="http://purl.obolibrary.org/obo/IAO_0000115"/>
        <owl:annotatedTarget>A bias characterized by being for or against groups or individuals based on social identities demographic factors or immutable physical characteristics often manifesting as stereotypes.</owl:annotatedTarget>
        <oboInOwl:hasDbXref rdf:resource="https://doi.org/10.6028/NIST.SP.1270"/>
    </owl:Axiom>
    


    <!-- https://w3id.org/aio/SoftmaxFunction -->

    <owl:Class rdf:about="https://w3id.org/aio/SoftmaxFunction">
        <rdfs:subClassOf rdf:resource="https://w3id.org/aio/Function"/>
        <obo:IAO_0000115>An activation function where the elements of the output vector are in range (0 1) and sum to 1 and each vector is handled independently.</obo:IAO_0000115>
        <oboInOwl:inSubset rdf:resource="https://w3id.org/aio/FunctionSubset"/>
        <rdfs:comment>The elements of the output vector are in range (0, 1) and sum to 1. Each vector is handled independently. The axis argument sets which axis of the input the function is applied along. Softmax is often used as the activation for the last layer of a classification network because the result could be interpreted as a probability distribution. The softmax of each vector x is computed as exp(x) / tf.reduce_sum(exp(x)). The input values in are the log-odds of the resulting probability.</rdfs:comment>
        <rdfs:label>Softmax Function</rdfs:label>
    </owl:Class>
    <owl:Axiom>
        <owl:annotatedSource rdf:resource="https://w3id.org/aio/SoftmaxFunction"/>
        <owl:annotatedProperty rdf:resource="http://purl.obolibrary.org/obo/IAO_0000115"/>
        <owl:annotatedTarget>An activation function where the elements of the output vector are in range (0 1) and sum to 1 and each vector is handled independently.</owl:annotatedTarget>
        <oboInOwl:hasDbXref rdf:resource="https://www.tensorflow.org/api_docs/python/tf/keras/activations/softmax"/>
    </owl:Axiom>
    


    <!-- https://w3id.org/aio/SoftmaxLayer -->

    <owl:Class rdf:about="https://w3id.org/aio/SoftmaxLayer">
        <rdfs:subClassOf rdf:resource="https://w3id.org/aio/ActivationLayer"/>
        <obo:IAO_0000115>An activation layer that applies the softmax function to the inputs.</obo:IAO_0000115>
        <oboInOwl:inSubset rdf:resource="https://w3id.org/aio/LayerSubset"/>
        <rdfs:comment>Softmax activation function.</rdfs:comment>
        <rdfs:label>Softmax Layer</rdfs:label>
    </owl:Class>
    <owl:Axiom>
        <owl:annotatedSource rdf:resource="https://w3id.org/aio/SoftmaxLayer"/>
        <owl:annotatedProperty rdf:resource="http://purl.obolibrary.org/obo/IAO_0000115"/>
        <owl:annotatedTarget>An activation layer that applies the softmax function to the inputs.</owl:annotatedTarget>
        <oboInOwl:hasDbXref rdf:resource="https://www.tensorflow.org/api_docs/python/tf/keras/layers/Softmax"/>
    </owl:Axiom>
    


    <!-- https://w3id.org/aio/SoftplusFunction -->

    <owl:Class rdf:about="https://w3id.org/aio/SoftplusFunction">
        <rdfs:subClassOf rdf:resource="https://w3id.org/aio/Function"/>
        <obo:IAO_0000115>An activation function that is softplus(x) = log(exp(x) + 1).</obo:IAO_0000115>
        <oboInOwl:inSubset rdf:resource="https://w3id.org/aio/FunctionSubset"/>
        <rdfs:comment>softplus(x) = log(exp(x) + 1)</rdfs:comment>
        <rdfs:label>Softplus Function</rdfs:label>
    </owl:Class>
    <owl:Axiom>
        <owl:annotatedSource rdf:resource="https://w3id.org/aio/SoftplusFunction"/>
        <owl:annotatedProperty rdf:resource="http://purl.obolibrary.org/obo/IAO_0000115"/>
        <owl:annotatedTarget>An activation function that is softplus(x) = log(exp(x) + 1).</owl:annotatedTarget>
        <oboInOwl:hasDbXref rdf:resource="https://www.tensorflow.org/api_docs/python/tf/keras/activations/softplus"/>
    </owl:Axiom>
    


    <!-- https://w3id.org/aio/SoftsignFunction -->

    <owl:Class rdf:about="https://w3id.org/aio/SoftsignFunction">
        <rdfs:subClassOf rdf:resource="https://w3id.org/aio/Function"/>
        <obo:IAO_0000115>An activation function that is softsign(x) = x / (abs(x) + 1).</obo:IAO_0000115>
        <oboInOwl:inSubset rdf:resource="https://w3id.org/aio/FunctionSubset"/>
        <rdfs:comment>softsign(x) = x / (abs(x) + 1)</rdfs:comment>
        <rdfs:label>Softsign Function</rdfs:label>
    </owl:Class>
    <owl:Axiom>
        <owl:annotatedSource rdf:resource="https://w3id.org/aio/SoftsignFunction"/>
        <owl:annotatedProperty rdf:resource="http://purl.obolibrary.org/obo/IAO_0000115"/>
        <owl:annotatedTarget>An activation function that is softsign(x) = x / (abs(x) + 1).</owl:annotatedTarget>
        <oboInOwl:hasDbXref rdf:resource="https://www.tensorflow.org/api_docs/python/tf/keras/activations/softsign"/>
    </owl:Axiom>
    


    <!-- https://w3id.org/aio/SparseAutoEncoder -->

    <owl:Class rdf:about="https://w3id.org/aio/SparseAutoEncoder">
        <rdfs:subClassOf rdf:resource="https://w3id.org/aio/AutoEncoderNetwork"/>
        <obo:IAO_0000115>An autoencoder network with more hidden units than inputs that constrains only a few hidden units to be active at once.</obo:IAO_0000115>
        <oboInOwl:hasExactSynonym>SAE</oboInOwl:hasExactSynonym>
        <oboInOwl:hasExactSynonym>Sparse AE</oboInOwl:hasExactSynonym>
        <oboInOwl:hasExactSynonym>Sparse Autoencoder</oboInOwl:hasExactSynonym>
        <oboInOwl:inSubset rdf:resource="https://w3id.org/aio/NetworkSubset"/>
        <rdfs:comment>Layers: Input, Hidden, Matched Output-Input</rdfs:comment>
        <rdfs:label>Sparse Auto Encoder</rdfs:label>
    </owl:Class>
    


    <!-- https://w3id.org/aio/SparseLLM -->

    <owl:Class rdf:about="https://w3id.org/aio/SparseLLM">
        <rdfs:subClassOf rdf:resource="https://w3id.org/aio/LargeLanguageModel"/>
        <obo:IAO_0000115>A large language model that uses techniques like pruning or quantization to reduce the number of non-zero parameters in the model making it more parameter-efficient and easier to deploy on resource-constrained devices.</obo:IAO_0000115>
        <oboInOwl:hasExactSynonym>Sparse Large Language Model</oboInOwl:hasExactSynonym>
        <oboInOwl:hasRelatedSynonym>model compression</oboInOwl:hasRelatedSynonym>
        <oboInOwl:hasRelatedSynonym>parameter efficiency</oboInOwl:hasRelatedSynonym>
        <oboInOwl:inSubset rdf:resource="https://w3id.org/aio/ModelSubset"/>
        <rdfs:label>Sparse LLM</rdfs:label>
    </owl:Class>
    


    <!-- https://w3id.org/aio/SparseLearning -->

    <owl:Class rdf:about="https://w3id.org/aio/SparseLearning">
        <rdfs:subClassOf rdf:resource="https://w3id.org/aio/RepresentationLearning"/>
        <obo:IAO_0000115>A representation learning network that finds sparse representations of input data as a linear combination of basic elements and identifies those elements.</obo:IAO_0000115>
        <oboInOwl:hasExactSynonym>Sparse coding</oboInOwl:hasExactSynonym>
        <oboInOwl:hasExactSynonym>Sparse dictionary Learning</oboInOwl:hasExactSynonym>
        <oboInOwl:inSubset rdf:resource="https://w3id.org/aio/NetworkSubset"/>
        <rdfs:label>Sparse Learning</rdfs:label>
    </owl:Class>
    <owl:Axiom>
        <owl:annotatedSource rdf:resource="https://w3id.org/aio/SparseLearning"/>
        <owl:annotatedProperty rdf:resource="http://purl.obolibrary.org/obo/IAO_0000115"/>
        <owl:annotatedTarget>A representation learning network that finds sparse representations of input data as a linear combination of basic elements and identifies those elements.</owl:annotatedTarget>
        <oboInOwl:hasDbXref rdf:resource="https://en.wikipedia.org/wiki/Sparse_dictionary_learning"/>
    </owl:Axiom>
    


    <!-- https://w3id.org/aio/SpatialDropout1DLayer -->

    <owl:Class rdf:about="https://w3id.org/aio/SpatialDropout1DLayer">
        <rdfs:subClassOf rdf:resource="https://w3id.org/aio/RegularizationLayer"/>
        <obo:IAO_0000115>A regularization layer that performs the same function as Dropout but drops entire 1D feature maps instead of individual elements.</obo:IAO_0000115>
        <oboInOwl:inSubset rdf:resource="https://w3id.org/aio/LayerSubset"/>
        <rdfs:comment>Spatial 1D version of Dropout. This version performs the same function as Dropout, however, it drops entire 1D feature maps instead of individual elements. If adjacent frames within feature maps are strongly correlated (as is normally the case in early convolution layers) then regular dropout will not regularize the activations and will otherwise just result in an effective Learning rate decrease. In this case, SpatialDropout1D will help promote independence between feature maps and should be used instead.</rdfs:comment>
        <rdfs:label>SpatialDropout1D Layer</rdfs:label>
    </owl:Class>
    <owl:Axiom>
        <owl:annotatedSource rdf:resource="https://w3id.org/aio/SpatialDropout1DLayer"/>
        <owl:annotatedProperty rdf:resource="http://purl.obolibrary.org/obo/IAO_0000115"/>
        <owl:annotatedTarget>A regularization layer that performs the same function as Dropout but drops entire 1D feature maps instead of individual elements.</owl:annotatedTarget>
        <oboInOwl:hasDbXref rdf:resource="https://www.tensorflow.org/api_docs/python/tf/keras/layers/SpatialDropout1D"/>
    </owl:Axiom>
    


    <!-- https://w3id.org/aio/SpatialDropout2DLayer -->

    <owl:Class rdf:about="https://w3id.org/aio/SpatialDropout2DLayer">
        <rdfs:subClassOf rdf:resource="https://w3id.org/aio/RegularizationLayer"/>
        <obo:IAO_0000115>A regularization layer that performs the same function as Dropout but drops entire 2D feature maps instead of individual elements.</obo:IAO_0000115>
        <oboInOwl:inSubset rdf:resource="https://w3id.org/aio/LayerSubset"/>
        <rdfs:comment>Spatial 2D version of Dropout. This version performs the same function as Dropout, however, it drops entire 2D feature maps instead of individual elements. If adjacent pixels within feature maps are strongly correlated (as is normally the case in early convolution layers) then regular dropout will not regularize the activations and will otherwise just result in an effective Learning rate decrease. In this case, SpatialDropout2D will help promote independence between feature maps and should be used instead.a</rdfs:comment>
        <rdfs:label>SpatialDropout2D Layer</rdfs:label>
    </owl:Class>
    <owl:Axiom>
        <owl:annotatedSource rdf:resource="https://w3id.org/aio/SpatialDropout2DLayer"/>
        <owl:annotatedProperty rdf:resource="http://purl.obolibrary.org/obo/IAO_0000115"/>
        <owl:annotatedTarget>A regularization layer that performs the same function as Dropout but drops entire 2D feature maps instead of individual elements.</owl:annotatedTarget>
        <oboInOwl:hasDbXref rdf:resource="https://www.tensorflow.org/api_docs/python/tf/keras/layers/SpatialDropout2D"/>
    </owl:Axiom>
    


    <!-- https://w3id.org/aio/SpatialDropout3DLayer -->

    <owl:Class rdf:about="https://w3id.org/aio/SpatialDropout3DLayer">
        <rdfs:subClassOf rdf:resource="https://w3id.org/aio/RegularizationLayer"/>
        <obo:IAO_0000115>A regularization layer that performs the same function as Dropout but drops entire 3D feature maps instead of individual elements.</obo:IAO_0000115>
        <oboInOwl:inSubset rdf:resource="https://w3id.org/aio/LayerSubset"/>
        <rdfs:comment>Spatial 3D version of Dropout. This version performs the same function as Dropout, however, it drops entire 3D feature maps instead of individual elements. If adjacent voxels within feature maps are strongly correlated (as is normally the case in early convolution layers) then regular dropout will not regularize the activations and will otherwise just result in an effective Learning rate decrease. In this case, SpatialDropout3D will help promote independence between feature maps and should be used instead.</rdfs:comment>
        <rdfs:label>SpatialDropout3D Layer</rdfs:label>
    </owl:Class>
    <owl:Axiom>
        <owl:annotatedSource rdf:resource="https://w3id.org/aio/SpatialDropout3DLayer"/>
        <owl:annotatedProperty rdf:resource="http://purl.obolibrary.org/obo/IAO_0000115"/>
        <owl:annotatedTarget>A regularization layer that performs the same function as Dropout but drops entire 3D feature maps instead of individual elements.</owl:annotatedTarget>
        <oboInOwl:hasDbXref rdf:resource="https://www.tensorflow.org/api_docs/python/tf/keras/layers/SpatialDropout3D"/>
    </owl:Axiom>
    


    <!-- https://w3id.org/aio/SpatialRegression -->

    <owl:Class rdf:about="https://w3id.org/aio/SpatialRegression">
        <rdfs:subClassOf rdf:resource="https://w3id.org/aio/RegressionAnalysis"/>
        <obo:IAO_0000115>A regression analysis method used to model spatial relationships.</obo:IAO_0000115>
        <oboInOwl:inSubset rdf:resource="https://w3id.org/aio/MachineLearningSubset"/>
        <rdfs:label>Spatial Regression</rdfs:label>
    </owl:Class>
    <owl:Axiom>
        <owl:annotatedSource rdf:resource="https://w3id.org/aio/SpatialRegression"/>
        <owl:annotatedProperty rdf:resource="http://purl.obolibrary.org/obo/IAO_0000115"/>
        <owl:annotatedTarget>A regression analysis method used to model spatial relationships.</owl:annotatedTarget>
        <oboInOwl:hasDbXref rdf:resource="https://gisgeography.com/spatial-regression-models-arcgis/"/>
    </owl:Axiom>
    


    <!-- https://w3id.org/aio/SpikingHiddenLayer -->

    <owl:Class rdf:about="https://w3id.org/aio/SpikingHiddenLayer">
        <rdfs:subClassOf rdf:resource="https://w3id.org/aio/HiddenLayer"/>
        <obo:IAO_0000115>A hidden layer that makes connections to an additional, heterogeneous hidden layer; modeled after biological neural networks.</obo:IAO_0000115>
        <oboInOwl:inSubset rdf:resource="https://w3id.org/aio/LayerSubset"/>
        <rdfs:label>Spiking Hidden Layer</rdfs:label>
    </owl:Class>
    <owl:Axiom>
        <owl:annotatedSource rdf:resource="https://w3id.org/aio/SpikingHiddenLayer"/>
        <owl:annotatedProperty rdf:resource="http://purl.obolibrary.org/obo/IAO_0000115"/>
        <owl:annotatedTarget>A hidden layer that makes connections to an additional, heterogeneous hidden layer; modeled after biological neural networks.</owl:annotatedTarget>
        <oboInOwl:hasDbXref rdf:resource="https://doi.org/10.1016/S0893-6080(97)00011-7"/>
    </owl:Axiom>
    


    <!-- https://w3id.org/aio/StackedRNNCellsLayer -->

    <owl:Class rdf:about="https://w3id.org/aio/StackedRNNCellsLayer">
        <rdfs:subClassOf rdf:resource="https://w3id.org/aio/Layer"/>
        <obo:IAO_0000115>A layer that allows a stack of RNN cells to behave as a single cell.</obo:IAO_0000115>
        <oboInOwl:inSubset rdf:resource="https://w3id.org/aio/LayerSubset"/>
        <rdfs:comment>Wrapper allowing a stack of RNN cells to behave as a single cell. Used to implement efficient stacked RNNs.</rdfs:comment>
        <rdfs:label>StackedRNNCells Layer</rdfs:label>
    </owl:Class>
    <owl:Axiom>
        <owl:annotatedSource rdf:resource="https://w3id.org/aio/StackedRNNCellsLayer"/>
        <owl:annotatedProperty rdf:resource="http://purl.obolibrary.org/obo/IAO_0000115"/>
        <owl:annotatedTarget>A layer that allows a stack of RNN cells to behave as a single cell.</owl:annotatedTarget>
        <oboInOwl:hasDbXref rdf:resource="https://www.tensorflow.org/api_docs/python/tf/keras/layers/StackedRNNCells"/>
    </owl:Axiom>
    


    <!-- https://w3id.org/aio/StreetlightEffectBias -->

    <owl:Class rdf:about="https://w3id.org/aio/StreetlightEffectBias">
        <rdfs:subClassOf rdf:resource="https://w3id.org/aio/IndividualBias"/>
        <obo:IAO_0000115>An individual bias where people search only where it is easiest to look.</obo:IAO_0000115>
        <oboInOwl:hasExactSynonym>Streetlight Effect</oboInOwl:hasExactSynonym>
        <oboInOwl:inSubset rdf:resource="https://w3id.org/aio/BiasSubset"/>
        <rdfs:label>Streetlight Effect Bias</rdfs:label>
    </owl:Class>
    <owl:Axiom>
        <owl:annotatedSource rdf:resource="https://w3id.org/aio/StreetlightEffectBias"/>
        <owl:annotatedProperty rdf:resource="http://purl.obolibrary.org/obo/IAO_0000115"/>
        <owl:annotatedTarget>An individual bias where people search only where it is easiest to look.</owl:annotatedTarget>
        <oboInOwl:hasDbXref rdf:resource="https://doi.org/10.6028/NIST.SP.1270"/>
    </owl:Axiom>
    


    <!-- https://w3id.org/aio/StringLookupLayer -->

    <owl:Class rdf:about="https://w3id.org/aio/StringLookupLayer">
        <rdfs:subClassOf rdf:resource="https://w3id.org/aio/CategoricalFeaturesPreprocessingLayer"/>
        <obo:IAO_0000115>A categorical features preprocessing layer that maps string features to integer indices.</obo:IAO_0000115>
        <oboInOwl:inSubset rdf:resource="https://w3id.org/aio/LayerSubset"/>
        <rdfs:label>StringLookup Layer</rdfs:label>
    </owl:Class>
    <owl:Axiom>
        <owl:annotatedSource rdf:resource="https://w3id.org/aio/StringLookupLayer"/>
        <owl:annotatedProperty rdf:resource="http://purl.obolibrary.org/obo/IAO_0000115"/>
        <owl:annotatedTarget>A categorical features preprocessing layer that maps string features to integer indices.</owl:annotatedTarget>
        <oboInOwl:hasDbXref rdf:resource="https://www.tensorflow.org/api_docs/python/tf/keras/layers/StringLookup"/>
    </owl:Axiom>
    


    <!-- https://w3id.org/aio/SubtractLayer -->

    <owl:Class rdf:about="https://w3id.org/aio/SubtractLayer">
        <rdfs:subClassOf rdf:resource="https://w3id.org/aio/MergingLayer"/>
        <obo:IAO_0000115>A merging layer that subtracts two inputs.</obo:IAO_0000115>
        <oboInOwl:inSubset rdf:resource="https://w3id.org/aio/LayerSubset"/>
        <rdfs:comment>Layer that subtracts two inputs. It takes as input a list of tensors of size 2, both of the same shape, and returns a single tensor, (inputs[0] - inputs[1]), also of the same shape.</rdfs:comment>
        <rdfs:label>Subtract Layer</rdfs:label>
    </owl:Class>
    <owl:Axiom>
        <owl:annotatedSource rdf:resource="https://w3id.org/aio/SubtractLayer"/>
        <owl:annotatedProperty rdf:resource="http://purl.obolibrary.org/obo/IAO_0000115"/>
        <owl:annotatedTarget>A merging layer that subtracts two inputs.</owl:annotatedTarget>
        <oboInOwl:hasDbXref rdf:resource="https://www.tensorflow.org/api_docs/python/tf/keras/layers/Subtract"/>
    </owl:Axiom>
    


    <!-- https://w3id.org/aio/SubwordSegmentation -->

    <owl:Class rdf:about="https://w3id.org/aio/SubwordSegmentation">
        <rdfs:subClassOf rdf:resource="https://w3id.org/aio/DataPreparation"/>
        <obo:IAO_0000115>The process of dividing text into subword units which are smaller than words but larger than individual characters to improve the efficiency and effectiveness of natural language processing models by capturing meaningful subunits of words.</obo:IAO_0000115>
        <oboInOwl:hasExactSynonym>Fragmentation</oboInOwl:hasExactSynonym>
        <oboInOwl:hasExactSynonym>Part-word Division</oboInOwl:hasExactSynonym>
        <oboInOwl:hasRelatedSynonym>Byte Pair Encoding</oboInOwl:hasRelatedSynonym>
        <oboInOwl:hasRelatedSynonym>SentencePiece</oboInOwl:hasRelatedSynonym>
        <oboInOwl:inSubset rdf:resource="https://w3id.org/aio/PreprocessingSubset"/>
        <rdfs:label>Subword Segmentation</rdfs:label>
    </owl:Class>
    


    <!-- https://w3id.org/aio/SunkCostFallacyBias -->

    <owl:Class rdf:about="https://w3id.org/aio/SunkCostFallacyBias">
        <rdfs:subClassOf rdf:resource="https://w3id.org/aio/Bias"/>
        <obo:IAO_0000115>A bias characterized by the tendency to continue an endeavor due to previously invested resources despite costs outweighing benefits.</obo:IAO_0000115>
        <oboInOwl:hasExactSynonym>Sunk Cost Fallacy</oboInOwl:hasExactSynonym>
        <oboInOwl:inSubset rdf:resource="https://w3id.org/aio/BiasSubset"/>
        <rdfs:comment>The tendency to continue an endeavor due to previously invested resources, despite costs outweighing benefits.</rdfs:comment>
        <rdfs:label>Sunk Cost Fallacy Bias</rdfs:label>
    </owl:Class>
    <owl:Axiom>
        <owl:annotatedSource rdf:resource="https://w3id.org/aio/SunkCostFallacyBias"/>
        <owl:annotatedProperty rdf:resource="http://purl.obolibrary.org/obo/IAO_0000115"/>
        <owl:annotatedTarget>A bias characterized by the tendency to continue an endeavor due to previously invested resources despite costs outweighing benefits.</owl:annotatedTarget>
        <oboInOwl:hasDbXref rdf:resource="https://doi.org/10.6028/NIST.SP.1270"/>
    </owl:Axiom>
    


    <!-- https://w3id.org/aio/SupervisedBiclustering -->

    <owl:Class rdf:about="https://w3id.org/aio/SupervisedBiclustering">
        <rdfs:subClassOf rdf:resource="https://w3id.org/aio/Biclustering"/>
        <obo:IAO_0000115>A biclustering task focused on methods that simultaneously cluster the rows and columns of a labeled matrix considering data labels to enhance cluster coherence.</obo:IAO_0000115>
        <oboInOwl:hasExactSynonym>Supervised Block Clustering</oboInOwl:hasExactSynonym>
        <oboInOwl:hasExactSynonym>Supervised Co-clustering</oboInOwl:hasExactSynonym>
        <oboInOwl:hasExactSynonym>Supervised Joint Clustering</oboInOwl:hasExactSynonym>
        <oboInOwl:hasExactSynonym>Supervised Two-mode Clustering</oboInOwl:hasExactSynonym>
        <oboInOwl:hasExactSynonym>Supervised Two-way Clustering</oboInOwl:hasExactSynonym>
        <oboInOwl:inSubset rdf:resource="https://w3id.org/aio/MachineLearningSubset"/>
        <rdfs:label>Supervised Biclustering</rdfs:label>
    </owl:Class>
    <owl:Axiom>
        <owl:annotatedSource rdf:resource="https://w3id.org/aio/SupervisedBiclustering"/>
        <owl:annotatedProperty rdf:resource="http://purl.obolibrary.org/obo/IAO_0000115"/>
        <owl:annotatedTarget>A biclustering task focused on methods that simultaneously cluster the rows and columns of a labeled matrix considering data labels to enhance cluster coherence.</owl:annotatedTarget>
        <oboInOwl:hasDbXref rdf:resource="https://en.wikipedia.org/wiki/Biclustering"/>
    </owl:Axiom>
    


    <!-- https://w3id.org/aio/SupervisedClustering -->

    <owl:Class rdf:about="https://w3id.org/aio/SupervisedClustering">
        <rdfs:subClassOf rdf:resource="https://w3id.org/aio/Clustering"/>
        <obo:IAO_0000115>A clustering task focused on methods that group labeled objects such that objects in the same group have similar labels relative to those in other groups.</obo:IAO_0000115>
        <oboInOwl:hasExactSynonym>Cluster analysis</oboInOwl:hasExactSynonym>
        <oboInOwl:inSubset rdf:resource="https://w3id.org/aio/MachineLearningSubset"/>
        <rdfs:label>Supervised Clustering</rdfs:label>
    </owl:Class>
    <owl:Axiom>
        <owl:annotatedSource rdf:resource="https://w3id.org/aio/SupervisedClustering"/>
        <owl:annotatedProperty rdf:resource="http://purl.obolibrary.org/obo/IAO_0000115"/>
        <owl:annotatedTarget>A clustering task focused on methods that group labeled objects such that objects in the same group have similar labels relative to those in other groups.</owl:annotatedTarget>
        <oboInOwl:hasDbXref rdf:resource="https://en.wikipedia.org/wiki/Cluster_analysis"/>
    </owl:Axiom>
    


    <!-- https://w3id.org/aio/SupervisedLearning -->

    <owl:Class rdf:about="https://w3id.org/aio/SupervisedLearning">
        <rdfs:subClassOf rdf:resource="https://w3id.org/aio/MachineLearning"/>
        <obo:IAO_0000115>A type of machine learning focused on methods that learn a function mapping input to output based on example input-output pairs.</obo:IAO_0000115>
        <oboInOwl:inSubset rdf:resource="https://w3id.org/aio/MachineLearningSubset"/>
        <rdfs:label>Supervised Learning</rdfs:label>
    </owl:Class>
    <owl:Axiom>
        <owl:annotatedSource rdf:resource="https://w3id.org/aio/SupervisedLearning"/>
        <owl:annotatedProperty rdf:resource="http://purl.obolibrary.org/obo/IAO_0000115"/>
        <owl:annotatedTarget>A type of machine learning focused on methods that learn a function mapping input to output based on example input-output pairs.</owl:annotatedTarget>
        <oboInOwl:hasDbXref rdf:resource="https://en.wikipedia.org/wiki/Supervised_learning"/>
    </owl:Axiom>
    


    <!-- https://w3id.org/aio/SupportVectorMachine -->

    <owl:Class rdf:about="https://w3id.org/aio/SupportVectorMachine">
        <rdfs:subClassOf rdf:resource="https://w3id.org/aio/Network"/>
        <rdfs:subClassOf>
            <owl:Restriction>
                <owl:onProperty rdf:resource="http://purl.obolibrary.org/obo/BFO_0000051"/>
                <owl:someValuesFrom rdf:resource="https://w3id.org/aio/HiddenLayer"/>
            </owl:Restriction>
        </rdfs:subClassOf>
        <rdfs:subClassOf>
            <owl:Restriction>
                <owl:onProperty rdf:resource="http://purl.obolibrary.org/obo/BFO_0000051"/>
                <owl:someValuesFrom rdf:resource="https://w3id.org/aio/InputLayer"/>
            </owl:Restriction>
        </rdfs:subClassOf>
        <rdfs:subClassOf>
            <owl:Restriction>
                <owl:onProperty rdf:resource="http://purl.obolibrary.org/obo/BFO_0000051"/>
                <owl:someValuesFrom rdf:resource="https://w3id.org/aio/OutputLayer"/>
            </owl:Restriction>
        </rdfs:subClassOf>
        <obo:IAO_0000115>A network with supervised learning models for classification and regression that maps training examples to points in space maximizing the gap between categories.</obo:IAO_0000115>
        <oboInOwl:hasExactSynonym>SVM</oboInOwl:hasExactSynonym>
        <oboInOwl:hasExactSynonym>SVN</oboInOwl:hasExactSynonym>
        <oboInOwl:hasExactSynonym>Supper Vector Network</oboInOwl:hasExactSynonym>
        <oboInOwl:inSubset rdf:resource="https://w3id.org/aio/NetworkSubset"/>
        <rdfs:comment>Layers: Input, Hidden, Output</rdfs:comment>
        <rdfs:label>Support Vector Machine</rdfs:label>
    </owl:Class>
    <owl:Axiom>
        <owl:annotatedSource rdf:resource="https://w3id.org/aio/SupportVectorMachine"/>
        <owl:annotatedProperty rdf:resource="http://purl.obolibrary.org/obo/IAO_0000115"/>
        <owl:annotatedTarget>A network with supervised learning models for classification and regression that maps training examples to points in space maximizing the gap between categories.</owl:annotatedTarget>
        <oboInOwl:hasDbXref rdf:resource="https://en.wikipedia.org/wiki/Support-vector_machine"/>
    </owl:Axiom>
    


    <!-- https://w3id.org/aio/SurvivalAnalysis -->

    <owl:Class rdf:about="https://w3id.org/aio/SurvivalAnalysis">
        <rdfs:subClassOf rdf:resource="https://w3id.org/aio/MachineLearning"/>
        <obo:IAO_0000115>A machine learning task focused on methods for analyzing the expected duration of time until one or more events occur such as death in biological organisms or failure in mechanical systems.</obo:IAO_0000115>
        <oboInOwl:inSubset rdf:resource="https://w3id.org/aio/MachineLearningSubset"/>
        <rdfs:label>Survival Analysis</rdfs:label>
    </owl:Class>
    <owl:Axiom>
        <owl:annotatedSource rdf:resource="https://w3id.org/aio/SurvivalAnalysis"/>
        <owl:annotatedProperty rdf:resource="http://purl.obolibrary.org/obo/IAO_0000115"/>
        <owl:annotatedTarget>A machine learning task focused on methods for analyzing the expected duration of time until one or more events occur such as death in biological organisms or failure in mechanical systems.</owl:annotatedTarget>
        <oboInOwl:hasDbXref rdf:resource="https://en.wikipedia.org/wiki/Survival_analysis"/>
    </owl:Axiom>
    


    <!-- https://w3id.org/aio/SurvivorshipBias -->

    <owl:Class rdf:about="https://w3id.org/aio/SurvivorshipBias">
        <rdfs:subClassOf rdf:resource="https://w3id.org/aio/ProcessingBias"/>
        <obo:IAO_0000115>A processing bias characterized by the tendency to focus on items observations or people that &quot;survive&quot; a selection process overlooking those that did not.</obo:IAO_0000115>
        <oboInOwl:inSubset rdf:resource="https://w3id.org/aio/BiasSubset"/>
        <rdfs:comment>The tendency to focus on items, observations, or people that &quot;survive&quot; a selection process, overlooking those that did not.</rdfs:comment>
        <rdfs:label>Survivorship Bias</rdfs:label>
    </owl:Class>
    <owl:Axiom>
        <owl:annotatedSource rdf:resource="https://w3id.org/aio/SurvivorshipBias"/>
        <owl:annotatedProperty rdf:resource="http://purl.obolibrary.org/obo/IAO_0000115"/>
        <owl:annotatedTarget>A processing bias characterized by the tendency to focus on items observations or people that &quot;survive&quot; a selection process overlooking those that did not.</owl:annotatedTarget>
        <oboInOwl:hasDbXref rdf:resource="https://doi.org/10.6028/NIST.SP.1270"/>
    </owl:Axiom>
    


    <!-- https://w3id.org/aio/SwishFunction -->

    <owl:Class rdf:about="https://w3id.org/aio/SwishFunction">
        <rdfs:subClassOf rdf:resource="https://w3id.org/aio/Function"/>
        <obo:IAO_0000115>An activation function that is x*sigmoid(x) a smooth non-monotonic function that consistently matches or outperforms ReLU on deep networks.</obo:IAO_0000115>
        <oboInOwl:inSubset rdf:resource="https://w3id.org/aio/FunctionSubset"/>
        <rdfs:comment>x*sigmoid(x). It is a smooth, non-monotonic function that consistently matches or outperforms ReLU on deep networks, it is unbounded above and bounded below.</rdfs:comment>
        <rdfs:label>Swish Function</rdfs:label>
    </owl:Class>
    <owl:Axiom>
        <owl:annotatedSource rdf:resource="https://w3id.org/aio/SwishFunction"/>
        <owl:annotatedProperty rdf:resource="http://purl.obolibrary.org/obo/IAO_0000115"/>
        <owl:annotatedTarget>An activation function that is x*sigmoid(x) a smooth non-monotonic function that consistently matches or outperforms ReLU on deep networks.</owl:annotatedTarget>
        <oboInOwl:hasDbXref rdf:resource="https://www.tensorflow.org/api_docs/python/tf/keras/activations/swish"/>
    </owl:Axiom>
    


    <!-- https://w3id.org/aio/SymmetricallyConnectedNetwork -->

    <owl:Class rdf:about="https://w3id.org/aio/SymmetricallyConnectedNetwork">
        <rdfs:subClassOf rdf:resource="https://w3id.org/aio/Network"/>
        <obo:IAO_0000115>A network that is a type of recurrent neural network where connections between units are symmetrical with equal weights in both directions.</obo:IAO_0000115>
        <oboInOwl:hasExactSynonym>SCN</oboInOwl:hasExactSynonym>
        <oboInOwl:inSubset rdf:resource="https://w3id.org/aio/NetworkSubset"/>
        <rdfs:comment>Symmetrically connected networks are a type of recurrent neural network where connections between units are symmetrical, meaning they have equal weights in both directions. This structure allows the network to maintain consistent information flow and equilibrium.</rdfs:comment>
        <rdfs:label>Symmetrically Connected Network</rdfs:label>
    </owl:Class>
    <owl:Axiom>
        <owl:annotatedSource rdf:resource="https://w3id.org/aio/SymmetricallyConnectedNetwork"/>
        <owl:annotatedProperty rdf:resource="http://purl.obolibrary.org/obo/IAO_0000115"/>
        <owl:annotatedTarget>A network that is a type of recurrent neural network where connections between units are symmetrical with equal weights in both directions.</owl:annotatedTarget>
        <oboInOwl:hasDbXref rdf:resource="https://ieeexplore.ieee.org/document/287176"/>
    </owl:Axiom>
    


    <!-- https://w3id.org/aio/SyncBatchNormLayer -->

    <owl:Class rdf:about="https://w3id.org/aio/SyncBatchNormLayer">
        <rdfs:subClassOf rdf:resource="https://w3id.org/aio/BatchNormalizationLayer"/>
        <obo:IAO_0000115>A batch normalization layer that applies synchronous Batch Normalization across multiple devices.</obo:IAO_0000115>
        <oboInOwl:hasExactSynonym>SyncBatchNorm</oboInOwl:hasExactSynonym>
        <oboInOwl:inSubset rdf:resource="https://w3id.org/aio/LayerSubset"/>
        <rdfs:comment>Applies Batch Normalization over a N-Dimensional input (a mini-batch of [N-2]D inputs with additional channel dimension) as described in the paper Batch Normalization: Accelerating Deep Network Training by Reducing Internal Covariate Shift .</rdfs:comment>
        <rdfs:label>SyncBatchNorm Layer</rdfs:label>
    </owl:Class>
    <owl:Axiom>
        <owl:annotatedSource rdf:resource="https://w3id.org/aio/SyncBatchNormLayer"/>
        <owl:annotatedProperty rdf:resource="http://purl.obolibrary.org/obo/IAO_0000115"/>
        <owl:annotatedTarget>A batch normalization layer that applies synchronous Batch Normalization across multiple devices.</owl:annotatedTarget>
        <oboInOwl:hasDbXref rdf:resource="https://pytorch.org/docs/stable/nn.html#normalization-layers"/>
    </owl:Axiom>
    


    <!-- https://w3id.org/aio/SystemicBias -->

    <owl:Class rdf:about="https://w3id.org/aio/SystemicBias">
        <rdfs:subClassOf rdf:resource="https://w3id.org/aio/Bias"/>
        <obo:IAO_0000115>A bias resulting from procedures and practices of institutions that operate in ways which result in certain social groups being advantaged or favored and others being disadvantaged or devalued.</obo:IAO_0000115>
        <oboInOwl:hasExactSynonym>Institutional Bias</oboInOwl:hasExactSynonym>
        <oboInOwl:hasExactSynonym>Societal Bias</oboInOwl:hasExactSynonym>
        <oboInOwl:inSubset rdf:resource="https://w3id.org/aio/BiasSubset"/>
        <rdfs:label>Systemic Bias</rdfs:label>
    </owl:Class>
    <owl:Axiom>
        <owl:annotatedSource rdf:resource="https://w3id.org/aio/SystemicBias"/>
        <owl:annotatedProperty rdf:resource="http://purl.obolibrary.org/obo/IAO_0000115"/>
        <owl:annotatedTarget>A bias resulting from procedures and practices of institutions that operate in ways which result in certain social groups being advantaged or favored and others being disadvantaged or devalued.</owl:annotatedTarget>
        <oboInOwl:hasDbXref rdf:resource="https://doi.org/10.6028/NIST.SP.1270"/>
    </owl:Axiom>
    


    <!-- https://w3id.org/aio/TanhFunction -->

    <owl:Class rdf:about="https://w3id.org/aio/TanhFunction">
        <rdfs:subClassOf rdf:resource="https://w3id.org/aio/Function"/>
        <obo:IAO_0000115>An activation function that is the hyperbolic tangent activation function.</obo:IAO_0000115>
        <oboInOwl:hasExactSynonym>hyperbolic tangent</oboInOwl:hasExactSynonym>
        <oboInOwl:inSubset rdf:resource="https://w3id.org/aio/FunctionSubset"/>
        <rdfs:comment>Hyperbolic tangent activation function.</rdfs:comment>
        <rdfs:label>Tanh Function</rdfs:label>
    </owl:Class>
    <owl:Axiom>
        <owl:annotatedSource rdf:resource="https://w3id.org/aio/TanhFunction"/>
        <owl:annotatedProperty rdf:resource="http://purl.obolibrary.org/obo/IAO_0000115"/>
        <owl:annotatedTarget>An activation function that is the hyperbolic tangent activation function.</owl:annotatedTarget>
        <oboInOwl:hasDbXref rdf:resource="https://www.tensorflow.org/api_docs/python/tf/keras/activations/tanh"/>
    </owl:Axiom>
    


    <!-- https://w3id.org/aio/TemporalBias -->

    <owl:Class rdf:about="https://w3id.org/aio/TemporalBias">
        <rdfs:subClassOf rdf:resource="https://w3id.org/aio/SelectionAndSamplingBias"/>
        <obo:IAO_0000115>A selection and sampling bias arising from differences in populations and behaviors over time.</obo:IAO_0000115>
        <oboInOwl:inSubset rdf:resource="https://w3id.org/aio/BiasSubset"/>
        <rdfs:label>Temporal Bias</rdfs:label>
    </owl:Class>
    <owl:Axiom>
        <owl:annotatedSource rdf:resource="https://w3id.org/aio/TemporalBias"/>
        <owl:annotatedProperty rdf:resource="http://purl.obolibrary.org/obo/IAO_0000115"/>
        <owl:annotatedTarget>A selection and sampling bias arising from differences in populations and behaviors over time.</owl:annotatedTarget>
        <oboInOwl:hasDbXref rdf:resource="https://doi.org/10.6028/NIST.SP.1270"/>
    </owl:Axiom>
    


    <!-- https://w3id.org/aio/TextPreprocessingLayer -->

    <owl:Class rdf:about="https://w3id.org/aio/TextPreprocessingLayer">
        <rdfs:subClassOf rdf:resource="https://w3id.org/aio/Layer"/>
        <obo:IAO_0000115>A layer that performs text data preprocessing operations.</obo:IAO_0000115>
        <oboInOwl:inSubset rdf:resource="https://w3id.org/aio/LayerSubset"/>
        <rdfs:label>Text Preprocessing Layer</rdfs:label>
    </owl:Class>
    <owl:Axiom>
        <owl:annotatedSource rdf:resource="https://w3id.org/aio/TextPreprocessingLayer"/>
        <owl:annotatedProperty rdf:resource="http://purl.obolibrary.org/obo/IAO_0000115"/>
        <owl:annotatedTarget>A layer that performs text data preprocessing operations.</owl:annotatedTarget>
        <oboInOwl:hasDbXref rdf:resource="https://keras.io/guides/preprocessing_layers/"/>
    </owl:Axiom>
    


    <!-- https://w3id.org/aio/TextVectorizationLayer -->

    <owl:Class rdf:about="https://w3id.org/aio/TextVectorizationLayer">
        <rdfs:subClassOf rdf:resource="https://w3id.org/aio/TextPreprocessingLayer"/>
        <obo:IAO_0000115>A preprocessing layer that maps text features to integer sequences.</obo:IAO_0000115>
        <oboInOwl:inSubset rdf:resource="https://w3id.org/aio/LayerSubset"/>
        <rdfs:label>TextVectorization Layer</rdfs:label>
    </owl:Class>
    <owl:Axiom>
        <owl:annotatedSource rdf:resource="https://w3id.org/aio/TextVectorizationLayer"/>
        <owl:annotatedProperty rdf:resource="http://purl.obolibrary.org/obo/IAO_0000115"/>
        <owl:annotatedTarget>A preprocessing layer that maps text features to integer sequences.</owl:annotatedTarget>
        <oboInOwl:hasDbXref rdf:resource="https://www.tensorflow.org/api_docs/python/tf/keras/layers/TextVectorization"/>
    </owl:Axiom>
    


    <!-- https://w3id.org/aio/ThresholdAutoregressive -->

    <owl:Class rdf:about="https://w3id.org/aio/ThresholdAutoregressive">
        <rdfs:subClassOf rdf:resource="https://w3id.org/aio/Model"/>
        <obo:IAO_0000115>A model that allows for different autoregressive processes depending on the regime or state of the time series, enabling the capture of nonlinear behaviors.</obo:IAO_0000115>
        <oboInOwl:hasExactSynonym>TAR</oboInOwl:hasExactSynonym>
        <oboInOwl:inSubset rdf:resource="https://w3id.org/aio/ModelSubset"/>
        <rdfs:label>Threshold Autoregressive</rdfs:label>
    </owl:Class>
    


    <!-- https://w3id.org/aio/ThresholdedReLULayer -->

    <owl:Class rdf:about="https://w3id.org/aio/ThresholdedReLULayer">
        <rdfs:subClassOf rdf:resource="https://w3id.org/aio/ActivationLayer"/>
        <obo:IAO_0000115>An activation layer that applies the thresholded rectified linear unit function element-wise.</obo:IAO_0000115>
        <oboInOwl:inSubset rdf:resource="https://w3id.org/aio/LayerSubset"/>
        <rdfs:comment>Thresholded Rectified Linear Unit.</rdfs:comment>
        <rdfs:label>ThresholdedReLU Layer</rdfs:label>
    </owl:Class>
    <owl:Axiom>
        <owl:annotatedSource rdf:resource="https://w3id.org/aio/ThresholdedReLULayer"/>
        <owl:annotatedProperty rdf:resource="http://purl.obolibrary.org/obo/IAO_0000115"/>
        <owl:annotatedTarget>An activation layer that applies the thresholded rectified linear unit function element-wise.</owl:annotatedTarget>
        <oboInOwl:hasDbXref rdf:resource="https://www.tensorflow.org/api_docs/python/tf/keras/layers/ThresholdedReLU"/>
    </owl:Axiom>
    


    <!-- https://w3id.org/aio/TimeDistributedLayer -->

    <owl:Class rdf:about="https://w3id.org/aio/TimeDistributedLayer">
        <rdfs:subClassOf rdf:resource="https://w3id.org/aio/RecurrentLayer"/>
        <obo:IAO_0000115>A wrapper layer that applies a layer to every temporal slice of an input.</obo:IAO_0000115>
        <oboInOwl:inSubset rdf:resource="https://w3id.org/aio/LayerSubset"/>
        <rdfs:comment>This wrapper allows to apply a layer to every temporal slice of an input. Every input should be at least 3D, and the dimension of index one of the first input will be considered to be the temporal dimension. Consider a batch of 32 video samples, where each sample is a 128x128 RGB image with channels_last data format, across 10 timesteps. The batch input shape is (32, 10, 128, 128, 3). You can then use TimeDistributed to apply the same Conv2D layer to each of the 10 timesteps, independently:</rdfs:comment>
        <rdfs:label>TimeDistributed Layer</rdfs:label>
    </owl:Class>
    <owl:Axiom>
        <owl:annotatedSource rdf:resource="https://w3id.org/aio/TimeDistributedLayer"/>
        <owl:annotatedProperty rdf:resource="http://purl.obolibrary.org/obo/IAO_0000115"/>
        <owl:annotatedTarget>A wrapper layer that applies a layer to every temporal slice of an input.</owl:annotatedTarget>
        <oboInOwl:hasDbXref rdf:resource="https://www.tensorflow.org/api_docs/python/tf/keras/layers/TimeDistributed"/>
    </owl:Axiom>
    


    <!-- https://w3id.org/aio/TimeSeriesAnalysis -->

    <owl:Class rdf:about="https://w3id.org/aio/TimeSeriesAnalysis">
        <rdfs:subClassOf rdf:resource="https://w3id.org/aio/MachineLearning"/>
        <obo:IAO_0000115>A machine learning task focused on methods for analyzing time series data to extract meaningful statistics and characteristics.</obo:IAO_0000115>
        <oboInOwl:inSubset rdf:resource="https://w3id.org/aio/MachineLearningSubset"/>
        <rdfs:comment>Methods for analyzing time series data to extract meaningful statistics and characteristics.</rdfs:comment>
        <rdfs:label>Time Series Analysis</rdfs:label>
    </owl:Class>
    <owl:Axiom>
        <owl:annotatedSource rdf:resource="https://w3id.org/aio/TimeSeriesAnalysis"/>
        <owl:annotatedProperty rdf:resource="http://purl.obolibrary.org/obo/IAO_0000115"/>
        <owl:annotatedTarget>A machine learning task focused on methods for analyzing time series data to extract meaningful statistics and characteristics.</owl:annotatedTarget>
        <oboInOwl:hasDbXref rdf:resource="https://en.wikipedia.org/wiki/Time_series"/>
    </owl:Axiom>
    


    <!-- https://w3id.org/aio/TimeSeriesForecasting -->

    <owl:Class rdf:about="https://w3id.org/aio/TimeSeriesForecasting">
        <rdfs:subClassOf rdf:resource="https://w3id.org/aio/MachineLearning"/>
        <obo:IAO_0000115>A machine learning task focused on methods that predict future values based on previously observed values.</obo:IAO_0000115>
        <oboInOwl:inSubset rdf:resource="https://w3id.org/aio/MachineLearningSubset"/>
        <rdfs:comment>Methods that predict future values based on previously observed values.</rdfs:comment>
        <rdfs:label>Time Series Forecasting</rdfs:label>
    </owl:Class>
    <owl:Axiom>
        <owl:annotatedSource rdf:resource="https://w3id.org/aio/TimeSeriesForecasting"/>
        <owl:annotatedProperty rdf:resource="http://purl.obolibrary.org/obo/IAO_0000115"/>
        <owl:annotatedTarget>A machine learning task focused on methods that predict future values based on previously observed values.</owl:annotatedTarget>
        <oboInOwl:hasDbXref rdf:resource="https://en.wikipedia.org/wiki/Time_series"/>
    </owl:Axiom>
    


    <!-- https://w3id.org/aio/Tokenization -->

    <owl:Class rdf:about="https://w3id.org/aio/Tokenization">
        <rdfs:subClassOf rdf:resource="https://w3id.org/aio/DataPreparation"/>
        <obo:IAO_0000115>The process of converting a sequence of text into smaller meaningful units called tokens typically words or subwords for the purpose of analysis or processing by language models.</obo:IAO_0000115>
        <oboInOwl:hasExactSynonym>Lexical Analysis</oboInOwl:hasExactSynonym>
        <oboInOwl:hasExactSynonym>Text Segmentation</oboInOwl:hasExactSynonym>
        <oboInOwl:inSubset rdf:resource="https://w3id.org/aio/PreprocessingSubset"/>
        <rdfs:label>Tokenization</rdfs:label>
    </owl:Class>
    


    <!-- https://w3id.org/aio/TrainingStrategies -->

    <owl:Class rdf:about="https://w3id.org/aio/TrainingStrategies">
        <rdfs:subClassOf rdf:resource="https://w3id.org/aio/Preprocessing"/>
        <obo:IAO_0000115>The methodologies and approaches used to train machine learning models including techniques such as supervised learning unsupervised learning reinforcement learning and transfer learning aimed at optimizing model performance.</obo:IAO_0000115>
        <oboInOwl:hasExactSynonym>Instructional Methods</oboInOwl:hasExactSynonym>
        <oboInOwl:hasExactSynonym>Learning Techniques</oboInOwl:hasExactSynonym>
        <oboInOwl:inSubset rdf:resource="https://w3id.org/aio/PreprocessingSubset"/>
        <rdfs:label>Training Strategies</rdfs:label>
    </owl:Class>
    


    <!-- https://w3id.org/aio/TransferLearning -->

    <owl:Class rdf:about="https://w3id.org/aio/TransferLearning">
        <rdfs:subClassOf rdf:resource="https://w3id.org/aio/MachineLearning"/>
        <obo:IAO_0000115>A type of machine learning focused on methods that reuse or transfer information from previously learned tasks to facilitate the learning of new tasks.</obo:IAO_0000115>
        <oboInOwl:inSubset rdf:resource="https://w3id.org/aio/NetworkSubset"/>
        <rdfs:label>Transfer Learning</rdfs:label>
    </owl:Class>
    <owl:Axiom>
        <owl:annotatedSource rdf:resource="https://w3id.org/aio/TransferLearning"/>
        <owl:annotatedProperty rdf:resource="http://purl.obolibrary.org/obo/IAO_0000115"/>
        <owl:annotatedTarget>A type of machine learning focused on methods that reuse or transfer information from previously learned tasks to facilitate the learning of new tasks.</owl:annotatedTarget>
        <oboInOwl:hasDbXref rdf:resource="https://en.wikipedia.org/wiki/Transfer_learning"/>
    </owl:Axiom>
    


    <!-- https://w3id.org/aio/TransferLearningLLM -->

    <owl:Class rdf:about="https://w3id.org/aio/TransferLearningLLM">
        <rdfs:subClassOf rdf:resource="https://w3id.org/aio/LargeLanguageModel"/>
        <obo:IAO_0000115>A large language model that leverages knowledge acquired during training on one task to improve performance on different but related tasks facilitating more efficient learning and adaptation.</obo:IAO_0000115>
        <oboInOwl:hasExactSynonym>Transfer LLM</oboInOwl:hasExactSynonym>
        <oboInOwl:hasRelatedSynonym>transfer learning</oboInOwl:hasRelatedSynonym>
        <oboInOwl:inSubset rdf:resource="https://w3id.org/aio/ModelSubset"/>
        <rdfs:label>Transfer Learning LLM</rdfs:label>
    </owl:Class>
    


    <!-- https://w3id.org/aio/TransformerLLM -->

    <owl:Class rdf:about="https://w3id.org/aio/TransformerLLM">
        <rdfs:subClassOf rdf:resource="https://w3id.org/aio/TransformerLanguageModel"/>
        <obo:IAO_0000115>A transformer language model with large training corpuses and sets of parameters that uses the transformer architecture based on multi-head attention mechanisms allowing it to contextualize tokens within a context window for effective language understanding and generation.</obo:IAO_0000115>
        <oboInOwl:hasExactSynonym>Transformer Large Language Model</oboInOwl:hasExactSynonym>
        <oboInOwl:inSubset rdf:resource="https://w3id.org/aio/ModelSubset"/>
        <rdfs:label>Transformer LLM</rdfs:label>
    </owl:Class>
    <owl:Axiom>
        <owl:annotatedSource rdf:resource="https://w3id.org/aio/TransformerLLM"/>
        <owl:annotatedProperty rdf:resource="http://purl.obolibrary.org/obo/IAO_0000115"/>
        <owl:annotatedTarget>A transformer language model with large training corpuses and sets of parameters that uses the transformer architecture based on multi-head attention mechanisms allowing it to contextualize tokens within a context window for effective language understanding and generation.</owl:annotatedTarget>
        <oboInOwl:hasDbXref rdf:resource="https://en.wikipedia.org/wiki/Transformer_(deep_learning_architecture)"/>
    </owl:Axiom>
    


    <!-- https://w3id.org/aio/TransformerLanguageModel -->

    <owl:Class rdf:about="https://w3id.org/aio/TransformerLanguageModel">
        <rdfs:subClassOf rdf:resource="https://w3id.org/aio/LanguageModel"/>
        <obo:IAO_0000115>A language model that uses the transformer architecture based on multi-head attention mechanisms allowing it to contextualize tokens within a context window for effective language understanding and generation.</obo:IAO_0000115>
        <oboInOwl:hasExactSynonym>Transformer LM</oboInOwl:hasExactSynonym>
        <oboInOwl:inSubset rdf:resource="https://w3id.org/aio/ModelSubset"/>
        <rdfs:label>Transformer Language Model</rdfs:label>
    </owl:Class>
    <owl:Axiom>
        <owl:annotatedSource rdf:resource="https://w3id.org/aio/TransformerLanguageModel"/>
        <owl:annotatedProperty rdf:resource="http://purl.obolibrary.org/obo/IAO_0000115"/>
        <owl:annotatedTarget>A language model that uses the transformer architecture based on multi-head attention mechanisms allowing it to contextualize tokens within a context window for effective language understanding and generation.</owl:annotatedTarget>
        <oboInOwl:hasDbXref rdf:resource="https://arxiv.org/abs/1706.03762"/>
    </owl:Axiom>
    


    <!-- https://w3id.org/aio/TransformerNetwork -->

    <owl:Class rdf:about="https://w3id.org/aio/TransformerNetwork">
        <rdfs:subClassOf rdf:resource="https://w3id.org/aio/DeepNeuralNetwork"/>
        <obo:IAO_0000115>A deep neural network that utilizes attention mechanisms to weigh the significance of input data.</obo:IAO_0000115>
        <oboInOwl:inSubset rdf:resource="https://w3id.org/aio/NetworkSubset"/>
        <rdfs:comment>A transformer network utilizes attention mechanisms to weigh the significance of each part of the input data, widely used in natural language processing (NLP) and computer vision (CV).</rdfs:comment>
        <rdfs:label>Transformer Network</rdfs:label>
    </owl:Class>
    <owl:Axiom>
        <owl:annotatedSource rdf:resource="https://w3id.org/aio/TransformerNetwork"/>
        <owl:annotatedProperty rdf:resource="http://purl.obolibrary.org/obo/IAO_0000115"/>
        <owl:annotatedTarget>A deep neural network that utilizes attention mechanisms to weigh the significance of input data.</owl:annotatedTarget>
        <oboInOwl:hasDbXref rdf:resource="https://en.wikipedia.org/wiki/Transformer_(machine_Learning_model)"/>
    </owl:Axiom>
    


    <!-- https://w3id.org/aio/UncertaintyBias -->

    <owl:Class rdf:about="https://w3id.org/aio/UncertaintyBias">
        <rdfs:subClassOf rdf:resource="https://w3id.org/aio/SelectionAndSamplingBias"/>
        <obo:IAO_0000115>A selection and sampling bias favoring groups better represented in training data due to less prediction uncertainty.</obo:IAO_0000115>
        <oboInOwl:inSubset rdf:resource="https://w3id.org/aio/BiasSubset"/>
        <rdfs:comment>Bias favoring groups better represented in training data, due to less prediction uncertainty.</rdfs:comment>
        <rdfs:label>Uncertainty Bias</rdfs:label>
    </owl:Class>
    <owl:Axiom>
        <owl:annotatedSource rdf:resource="https://w3id.org/aio/UncertaintyBias"/>
        <owl:annotatedProperty rdf:resource="http://purl.obolibrary.org/obo/IAO_0000115"/>
        <owl:annotatedTarget>A selection and sampling bias favoring groups better represented in training data due to less prediction uncertainty.</owl:annotatedTarget>
        <oboInOwl:hasDbXref rdf:resource="https://doi.org/10.6028/NIST.SP.1270"/>
    </owl:Axiom>
    


    <!-- https://w3id.org/aio/UnitNormalizationLayer -->

    <owl:Class rdf:about="https://w3id.org/aio/UnitNormalizationLayer">
        <rdfs:subClassOf rdf:resource="https://w3id.org/aio/RecurrentLayer"/>
        <obo:IAO_0000115>A normalization layer that normalizes a batch of inputs so that each input in the batch has a L2 norm equal to 1.</obo:IAO_0000115>
        <oboInOwl:inSubset rdf:resource="https://w3id.org/aio/LayerSubset"/>
        <rdfs:comment>Unit normalization layer. Normalize a batch of inputs so that each input in the batch has a L2 norm equal to 1 (across the axes specified in axis).</rdfs:comment>
        <rdfs:label>UnitNormalization Layer</rdfs:label>
    </owl:Class>
    <owl:Axiom>
        <owl:annotatedSource rdf:resource="https://w3id.org/aio/UnitNormalizationLayer"/>
        <owl:annotatedProperty rdf:resource="http://purl.obolibrary.org/obo/IAO_0000115"/>
        <owl:annotatedTarget>A normalization layer that normalizes a batch of inputs so that each input in the batch has a L2 norm equal to 1.</owl:annotatedTarget>
        <oboInOwl:hasDbXref rdf:resource="https://www.tensorflow.org/api_docs/python/tf/keras/layers/UnitNormalization"/>
    </owl:Axiom>
    


    <!-- https://w3id.org/aio/UnsupervisedBiclustering -->

    <owl:Class rdf:about="https://w3id.org/aio/UnsupervisedBiclustering">
        <rdfs:subClassOf rdf:resource="https://w3id.org/aio/Biclustering"/>
        <obo:IAO_0000115>A biclustering task focused on methods that simultaneously cluster the rows and columns of an unlabeled input matrix to identify submatrices with coherent patterns.</obo:IAO_0000115>
        <oboInOwl:hasExactSynonym>Block Clustering</oboInOwl:hasExactSynonym>
        <oboInOwl:hasExactSynonym>Co-clustering</oboInOwl:hasExactSynonym>
        <oboInOwl:hasExactSynonym>Joint Clustering</oboInOwl:hasExactSynonym>
        <oboInOwl:hasExactSynonym>Two-mode Clustering</oboInOwl:hasExactSynonym>
        <oboInOwl:hasExactSynonym>Two-way Clustering</oboInOwl:hasExactSynonym>
        <oboInOwl:inSubset rdf:resource="https://w3id.org/aio/MachineLearningSubset"/>
        <rdfs:label>Unsupervised Biclustering</rdfs:label>
    </owl:Class>
    <owl:Axiom>
        <owl:annotatedSource rdf:resource="https://w3id.org/aio/UnsupervisedBiclustering"/>
        <owl:annotatedProperty rdf:resource="http://purl.obolibrary.org/obo/IAO_0000115"/>
        <owl:annotatedTarget>A biclustering task focused on methods that simultaneously cluster the rows and columns of an unlabeled input matrix to identify submatrices with coherent patterns.</owl:annotatedTarget>
        <oboInOwl:hasDbXref rdf:resource="https://en.wikipedia.org/wiki/Biclustering"/>
    </owl:Axiom>
    


    <!-- https://w3id.org/aio/UnsupervisedClustering -->

    <owl:Class rdf:about="https://w3id.org/aio/UnsupervisedClustering">
        <rdfs:subClassOf rdf:resource="https://w3id.org/aio/Clustering"/>
        <obo:IAO_0000115>A clustering task focused on methods that group a set of unlabeled objects such that objects in the same group are more similar to each other than to those in other groups.</obo:IAO_0000115>
        <oboInOwl:hasExactSynonym>Cluster analysis</oboInOwl:hasExactSynonym>
        <oboInOwl:inSubset rdf:resource="https://w3id.org/aio/MachineLearningSubset"/>
        <rdfs:label>Unsupervised Clustering</rdfs:label>
    </owl:Class>
    <owl:Axiom>
        <owl:annotatedSource rdf:resource="https://w3id.org/aio/UnsupervisedClustering"/>
        <owl:annotatedProperty rdf:resource="http://purl.obolibrary.org/obo/IAO_0000115"/>
        <owl:annotatedTarget>A clustering task focused on methods that group a set of unlabeled objects such that objects in the same group are more similar to each other than to those in other groups.</owl:annotatedTarget>
        <oboInOwl:hasDbXref rdf:resource="https://en.wikipedia.org/wiki/Cluster_analysis"/>
    </owl:Axiom>
    


    <!-- https://w3id.org/aio/UnsupervisedLLM -->

    <owl:Class rdf:about="https://w3id.org/aio/UnsupervisedLLM">
        <rdfs:subClassOf rdf:resource="https://w3id.org/aio/LargeLanguageModel"/>
        <obo:IAO_0000115>A large language model that is trained solely on unlabeled data using self-supervised objectives like masked language modeling without any supervised fine-tuning.</obo:IAO_0000115>
        <oboInOwl:hasExactSynonym>Unsupervised Large Language Model</oboInOwl:hasExactSynonym>
        <oboInOwl:hasRelatedSynonym>self-supervised</oboInOwl:hasRelatedSynonym>
        <oboInOwl:inSubset rdf:resource="https://w3id.org/aio/ModelSubset"/>
        <rdfs:label>Unsupervised LLM</rdfs:label>
    </owl:Class>
    


    <!-- https://w3id.org/aio/UnsupervisedLearning -->

    <owl:Class rdf:about="https://w3id.org/aio/UnsupervisedLearning">
        <rdfs:subClassOf rdf:resource="https://w3id.org/aio/MachineLearning"/>
        <obo:IAO_0000115>A type of machine learning focused on algorithms that learn patterns from unlabeled data.</obo:IAO_0000115>
        <oboInOwl:inSubset rdf:resource="https://w3id.org/aio/MachineLearningSubset"/>
        <rdfs:comment>Algorithms that learn patterns from unlabeled data.</rdfs:comment>
        <rdfs:label>Unsupervised Learning</rdfs:label>
    </owl:Class>
    <owl:Axiom>
        <owl:annotatedSource rdf:resource="https://w3id.org/aio/UnsupervisedLearning"/>
        <owl:annotatedProperty rdf:resource="http://purl.obolibrary.org/obo/IAO_0000115"/>
        <owl:annotatedTarget>A type of machine learning focused on algorithms that learn patterns from unlabeled data.</owl:annotatedTarget>
        <oboInOwl:hasDbXref rdf:resource="https://en.wikipedia.org/wiki/Unsupervised_learning"/>
    </owl:Axiom>
    


    <!-- https://w3id.org/aio/UnsupervisedPretrainedNetwork -->

    <owl:Class rdf:about="https://w3id.org/aio/UnsupervisedPretrainedNetwork">
        <rdfs:subClassOf rdf:resource="https://w3id.org/aio/Network"/>
        <obo:IAO_0000115>A network that initializes a discriminative neural net from one trained using an unsupervised criterion.</obo:IAO_0000115>
        <oboInOwl:hasExactSynonym>UPN</oboInOwl:hasExactSynonym>
        <oboInOwl:inSubset rdf:resource="https://w3id.org/aio/NetworkSubset"/>
        <rdfs:comment>Unsupervised pre-training initializes a discriminative neural net from one trained using an unsupervised criterion, aiding in optimization and overfitting issues.</rdfs:comment>
        <rdfs:label>Unsupervised Pretrained Network</rdfs:label>
    </owl:Class>
    <owl:Axiom>
        <owl:annotatedSource rdf:resource="https://w3id.org/aio/UnsupervisedPretrainedNetwork"/>
        <owl:annotatedProperty rdf:resource="http://purl.obolibrary.org/obo/IAO_0000115"/>
        <owl:annotatedTarget>A network that initializes a discriminative neural net from one trained using an unsupervised criterion.</owl:annotatedTarget>
        <oboInOwl:hasDbXref rdf:resource="https://metacademy.org/graphs/concepts/unsupervised_pre_training"/>
    </owl:Axiom>
    


    <!-- https://w3id.org/aio/UpSampling1DLayer -->

    <owl:Class rdf:about="https://w3id.org/aio/UpSampling1DLayer">
        <rdfs:subClassOf rdf:resource="https://w3id.org/aio/ReshapingLayer"/>
        <obo:IAO_0000115>A layer that upsamples the input by repeating each temporal step size times along the time axis.</obo:IAO_0000115>
        <oboInOwl:inSubset rdf:resource="https://w3id.org/aio/LayerSubset"/>
        <rdfs:comment>Upsampling layer for 1D inputs. Repeats each temporal step size times along the time axis.</rdfs:comment>
        <rdfs:label>UpSampling1D Layer</rdfs:label>
    </owl:Class>
    <owl:Axiom>
        <owl:annotatedSource rdf:resource="https://w3id.org/aio/UpSampling1DLayer"/>
        <owl:annotatedProperty rdf:resource="http://purl.obolibrary.org/obo/IAO_0000115"/>
        <owl:annotatedTarget>A layer that upsamples the input by repeating each temporal step size times along the time axis.</owl:annotatedTarget>
        <oboInOwl:hasDbXref rdf:resource="https://www.tensorflow.org/api_docs/python/tf/keras/layers/UpSampling1D"/>
    </owl:Axiom>
    


    <!-- https://w3id.org/aio/UpSampling2DLayer -->

    <owl:Class rdf:about="https://w3id.org/aio/UpSampling2DLayer">
        <rdfs:subClassOf rdf:resource="https://w3id.org/aio/Layer"/>
        <obo:IAO_0000115>A layer that upsamples the input by repeating each row and column size times.</obo:IAO_0000115>
        <oboInOwl:inSubset rdf:resource="https://w3id.org/aio/LayerSubset"/>
        <rdfs:comment>Upsampling layer for 2D inputs. Repeats the rows and columns of the data by size[0] and size[1] respectively.</rdfs:comment>
        <rdfs:label>UpSampling2D Layer</rdfs:label>
    </owl:Class>
    <owl:Axiom>
        <owl:annotatedSource rdf:resource="https://w3id.org/aio/UpSampling2DLayer"/>
        <owl:annotatedProperty rdf:resource="http://purl.obolibrary.org/obo/IAO_0000115"/>
        <owl:annotatedTarget>A layer that upsamples the input by repeating each row and column size times.</owl:annotatedTarget>
        <oboInOwl:hasDbXref rdf:resource="https://www.tensorflow.org/api_docs/python/tf/keras/layers/UpSampling2D"/>
    </owl:Axiom>
    


    <!-- https://w3id.org/aio/UpSampling3DLayer -->

    <owl:Class rdf:about="https://w3id.org/aio/UpSampling3DLayer">
        <rdfs:subClassOf rdf:resource="https://w3id.org/aio/Layer"/>
        <obo:IAO_0000115>A layer that upsamples the input by repeating each depth</obo:IAO_0000115>
        <oboInOwl:inSubset rdf:resource="https://w3id.org/aio/LayerSubset"/>
        <rdfs:comment>Upsampling layer for 3D inputs.</rdfs:comment>
        <rdfs:label>UpSampling3D Layer</rdfs:label>
    </owl:Class>
    <owl:Axiom>
        <owl:annotatedSource rdf:resource="https://w3id.org/aio/UpSampling3DLayer"/>
        <owl:annotatedProperty rdf:resource="http://purl.obolibrary.org/obo/IAO_0000115"/>
        <owl:annotatedTarget>A layer that upsamples the input by repeating each depth</owl:annotatedTarget>
        <oboInOwl:hasDbXref rdf:resource="https://www.tensorflow.org/api_docs/python/tf/keras/layers/UpSampling3D"/>
    </owl:Axiom>
    


    <!-- https://w3id.org/aio/UseAndInterpretationBias -->

    <owl:Class rdf:about="https://w3id.org/aio/UseAndInterpretationBias">
        <rdfs:subClassOf rdf:resource="https://w3id.org/aio/ComputationalBias"/>
        <obo:IAO_0000115>A computational bias characterized by inappropriately analyzing ambiguous stimuli scenarios and events.</obo:IAO_0000115>
        <oboInOwl:hasExactSynonym>Interpretive Bias</oboInOwl:hasExactSynonym>
        <oboInOwl:inSubset rdf:resource="https://w3id.org/aio/BiasSubset"/>
        <rdfs:comment>Bias inappropriately analyzing ambiguous stimuli, scenarios, and events.</rdfs:comment>
        <rdfs:label>Use And Interpretation Bias</rdfs:label>
    </owl:Class>
    <owl:Axiom>
        <owl:annotatedSource rdf:resource="https://w3id.org/aio/UseAndInterpretationBias"/>
        <owl:annotatedProperty rdf:resource="http://purl.obolibrary.org/obo/IAO_0000115"/>
        <owl:annotatedTarget>A computational bias characterized by inappropriately analyzing ambiguous stimuli scenarios and events.</owl:annotatedTarget>
        <oboInOwl:hasDbXref rdf:resource="https://doi.org/10.6028/NIST.SP.1270"/>
    </owl:Axiom>
    


    <!-- https://w3id.org/aio/UserInteractionBias -->

    <owl:Class rdf:about="https://w3id.org/aio/UserInteractionBias">
        <rdfs:subClassOf rdf:resource="https://w3id.org/aio/IndividualBias"/>
        <obo:IAO_0000115>An individual bias arising when a user imposes their own biases during interaction with data output results etc.</obo:IAO_0000115>
        <oboInOwl:inSubset rdf:resource="https://w3id.org/aio/BiasSubset"/>
        <rdfs:comment>Bias arising when a user imposes their own biases during interaction with data, output, results, etc.</rdfs:comment>
        <rdfs:label>User Interaction Bias</rdfs:label>
    </owl:Class>
    <owl:Axiom>
        <owl:annotatedSource rdf:resource="https://w3id.org/aio/UserInteractionBias"/>
        <owl:annotatedProperty rdf:resource="http://purl.obolibrary.org/obo/IAO_0000115"/>
        <owl:annotatedTarget>An individual bias arising when a user imposes their own biases during interaction with data output results etc.</owl:annotatedTarget>
        <oboInOwl:hasDbXref rdf:resource="https://doi.org/10.6028/NIST.SP.1270"/>
    </owl:Axiom>
    


    <!-- https://w3id.org/aio/VariationalAutoEncoder -->

    <owl:Class rdf:about="https://w3id.org/aio/VariationalAutoEncoder">
        <rdfs:subClassOf rdf:resource="https://w3id.org/aio/AutoEncoderNetwork"/>
        <rdfs:subClassOf>
            <owl:Restriction>
                <owl:onProperty rdf:resource="http://purl.obolibrary.org/obo/BFO_0000051"/>
                <owl:someValuesFrom rdf:resource="https://w3id.org/aio/ProbabilisticHiddenLayer"/>
            </owl:Restriction>
        </rdfs:subClassOf>
        <obo:IAO_0000115>An autoencoder network that imposes a probabilistic structure on the latent space for unsupervised learning.</obo:IAO_0000115>
        <oboInOwl:hasExactSynonym>VAE</oboInOwl:hasExactSynonym>
        <oboInOwl:inSubset rdf:resource="https://w3id.org/aio/NetworkSubset"/>
        <rdfs:comment>Layers: Input, Probabilistic Hidden, Matched Output-Input</rdfs:comment>
        <rdfs:label>Variational Auto Encoder</rdfs:label>
    </owl:Class>
    


    <!-- https://w3id.org/aio/VectorAutoregression -->

    <owl:Class rdf:about="https://w3id.org/aio/VectorAutoregression">
        <rdfs:subClassOf rdf:resource="https://w3id.org/aio/Model"/>
        <obo:IAO_0000115>A model that captures the linear interdependencies among multiple time series, where each variable is modeled as a linear function of its own past values and the past values of all other variables in the system.</obo:IAO_0000115>
        <oboInOwl:hasExactSynonym>VAR</oboInOwl:hasExactSynonym>
        <oboInOwl:inSubset rdf:resource="https://w3id.org/aio/ModelSubset"/>
        <rdfs:label>Vector Autoregression</rdfs:label>
    </owl:Class>
    


    <!-- https://w3id.org/aio/VocabularyReduction -->

    <owl:Class rdf:about="https://w3id.org/aio/VocabularyReduction">
        <rdfs:subClassOf rdf:resource="https://w3id.org/aio/DataPreparation"/>
        <obo:IAO_0000115>The technique of limiting the number of unique tokens in a language model&apos;s vocabulary by merging or eliminating less frequent tokens thereby optimizing computational efficiency and resource usage.</obo:IAO_0000115>
        <oboInOwl:hasExactSynonym>Lexical Simplification</oboInOwl:hasExactSynonym>
        <oboInOwl:hasExactSynonym>Lexicon Pruning</oboInOwl:hasExactSynonym>
        <oboInOwl:hasExactSynonym>Vocabulary Condensation</oboInOwl:hasExactSynonym>
        <oboInOwl:inSubset rdf:resource="https://w3id.org/aio/PreprocessingSubset"/>
        <rdfs:label>Vocabulary Reduction</rdfs:label>
    </owl:Class>
    


    <!-- https://w3id.org/aio/WeightedLayer -->

    <owl:Class rdf:about="https://w3id.org/aio/WeightedLayer">
        <rdfs:subClassOf rdf:resource="https://w3id.org/aio/Layer"/>
        <obo:IAO_0000115>A layer of values to be applied to other cells or neurons in a network.</obo:IAO_0000115>
        <oboInOwl:inSubset rdf:resource="https://w3id.org/aio/LayerSubset"/>
        <rdfs:label>Weighted Layer</rdfs:label>
    </owl:Class>
    


    <!-- https://w3id.org/aio/WrapperLayer -->

    <owl:Class rdf:about="https://w3id.org/aio/WrapperLayer">
        <rdfs:subClassOf rdf:resource="https://w3id.org/aio/Layer"/>
        <obo:IAO_0000115>An abstract base class for wrappers that augment the functionality of another layer.</obo:IAO_0000115>
        <oboInOwl:inSubset rdf:resource="https://w3id.org/aio/LayerSubset"/>
        <rdfs:comment>Abstract wrapper base class. Wrappers take another layer and augment it in various ways. Do not use this class as a layer, it is only an abstract base class. Two usable wrappers are the TimeDistributed and Bidirectional wrappers.</rdfs:comment>
        <rdfs:label>Wrapper Layer</rdfs:label>
    </owl:Class>
    <owl:Axiom>
        <owl:annotatedSource rdf:resource="https://w3id.org/aio/WrapperLayer"/>
        <owl:annotatedProperty rdf:resource="http://purl.obolibrary.org/obo/IAO_0000115"/>
        <owl:annotatedTarget>An abstract base class for wrappers that augment the functionality of another layer.</owl:annotatedTarget>
        <oboInOwl:hasDbXref rdf:resource="https://www.tensorflow.org/api_docs/python/tf/keras/layers/Wrapper"/>
    </owl:Axiom>
    


    <!-- https://w3id.org/aio/ZeroPadding1DLayer -->

    <owl:Class rdf:about="https://w3id.org/aio/ZeroPadding1DLayer">
        <rdfs:subClassOf rdf:resource="https://w3id.org/aio/ReshapingLayer"/>
        <obo:IAO_0000115>A layer that zero-pads the input along the time axis.</obo:IAO_0000115>
        <oboInOwl:inSubset rdf:resource="https://w3id.org/aio/LayerSubset"/>
        <rdfs:comment>Zero-padding layer for 1D input (e.g. temporal sequence).</rdfs:comment>
        <rdfs:label>ZeroPadding1D Layer</rdfs:label>
    </owl:Class>
    <owl:Axiom>
        <owl:annotatedSource rdf:resource="https://w3id.org/aio/ZeroPadding1DLayer"/>
        <owl:annotatedProperty rdf:resource="http://purl.obolibrary.org/obo/IAO_0000115"/>
        <owl:annotatedTarget>A layer that zero-pads the input along the time axis.</owl:annotatedTarget>
        <oboInOwl:hasDbXref rdf:resource="https://www.tensorflow.org/api_docs/python/tf/keras/layers/ZeroPadding1D"/>
    </owl:Axiom>
    


    <!-- https://w3id.org/aio/ZeroPadding2DLayer -->

    <owl:Class rdf:about="https://w3id.org/aio/ZeroPadding2DLayer">
        <rdfs:subClassOf rdf:resource="https://w3id.org/aio/ReshapingLayer"/>
        <obo:IAO_0000115>A layer that zero-pads the input along the height and width dimensions.</obo:IAO_0000115>
        <oboInOwl:inSubset rdf:resource="https://w3id.org/aio/LayerSubset"/>
        <rdfs:comment>Zero-padding layer for 2D input (e.g. picture). This layer can add rows and columns of zeros at the top, bottom, left and right side of an image tensor.</rdfs:comment>
        <rdfs:label>ZeroPadding2D Layer</rdfs:label>
    </owl:Class>
    <owl:Axiom>
        <owl:annotatedSource rdf:resource="https://w3id.org/aio/ZeroPadding2DLayer"/>
        <owl:annotatedProperty rdf:resource="http://purl.obolibrary.org/obo/IAO_0000115"/>
        <owl:annotatedTarget>A layer that zero-pads the input along the height and width dimensions.</owl:annotatedTarget>
        <oboInOwl:hasDbXref rdf:resource="https://www.tensorflow.org/api_docs/python/tf/keras/layers/ZeroPadding2D"/>
    </owl:Axiom>
    


    <!-- https://w3id.org/aio/ZeroPadding3DLayer -->

    <owl:Class rdf:about="https://w3id.org/aio/ZeroPadding3DLayer">
        <rdfs:subClassOf rdf:resource="https://w3id.org/aio/ReshapingLayer"/>
        <obo:IAO_0000115>A layer that zero-pads the input along the depth</obo:IAO_0000115>
        <oboInOwl:inSubset rdf:resource="https://w3id.org/aio/LayerSubset"/>
        <rdfs:comment>Zero-padding layer for 3D data (spatial or spatio-temporal).</rdfs:comment>
        <rdfs:label>ZeroPadding3D Layer</rdfs:label>
    </owl:Class>
    <owl:Axiom>
        <owl:annotatedSource rdf:resource="https://w3id.org/aio/ZeroPadding3DLayer"/>
        <owl:annotatedProperty rdf:resource="http://purl.obolibrary.org/obo/IAO_0000115"/>
        <owl:annotatedTarget>A layer that zero-pads the input along the depth</owl:annotatedTarget>
        <oboInOwl:hasDbXref rdf:resource="https://www.tensorflow.org/api_docs/python/tf/keras/layers/ZeroPadding3D"/>
    </owl:Axiom>
    


    <!-- https://w3id.org/aio/ZeroShotLearningLLM -->

    <owl:Class rdf:about="https://w3id.org/aio/ZeroShotLearningLLM">
        <rdfs:subClassOf rdf:resource="https://w3id.org/aio/LargeLanguageModel"/>
        <obo:IAO_0000115>A LLM which performs tasks or understands concepts it has not explicitly been trained on, demonstrating a high degree of generalization and understanding.</obo:IAO_0000115>
        <oboInOwl:hasExactSynonym>Zero-Shot LLM</oboInOwl:hasExactSynonym>
        <oboInOwl:hasRelatedSynonym>zero-shot learning</oboInOwl:hasRelatedSynonym>
        <oboInOwl:inSubset rdf:resource="https://w3id.org/aio/ModelSubset"/>
        <rdfs:label>Zero-Shot Learning LLM</rdfs:label>
    </owl:Class>
    


    <!-- https://w3id.org/aio/ZeroshotLearning -->

    <owl:Class rdf:about="https://w3id.org/aio/ZeroshotLearning">
        <rdfs:subClassOf rdf:resource="https://w3id.org/aio/DeepNeuralNetwork"/>
        <obo:IAO_0000115>A deep neural network that predicts classes at test time from classes not observed during training.</obo:IAO_0000115>
        <oboInOwl:hasExactSynonym>ZSL</oboInOwl:hasExactSynonym>
        <oboInOwl:inSubset rdf:resource="https://w3id.org/aio/NetworkSubset"/>
        <rdfs:label>Zero-shot Learning</rdfs:label>
    </owl:Class>
    <owl:Axiom>
        <owl:annotatedSource rdf:resource="https://w3id.org/aio/ZeroshotLearning"/>
        <owl:annotatedProperty rdf:resource="http://purl.obolibrary.org/obo/IAO_0000115"/>
        <owl:annotatedTarget>A deep neural network that predicts classes at test time from classes not observed during training.</owl:annotatedTarget>
        <oboInOwl:hasDbXref rdf:resource="https://en.wikipedia.org/wiki/Zero-shot_learning"/>
    </owl:Axiom>
    


    <!-- https://w3id.org/aio/node2vec -->

    <owl:Class rdf:about="https://w3id.org/aio/node2vec">
        <rdfs:subClassOf rdf:resource="https://w3id.org/aio/MachineLearning"/>
        <rdfs:subClassOf>
            <owl:Restriction>
                <owl:onProperty rdf:resource="http://purl.obolibrary.org/obo/BFO_0000051"/>
                <owl:someValuesFrom rdf:resource="https://w3id.org/aio/HiddenLayer"/>
            </owl:Restriction>
        </rdfs:subClassOf>
        <rdfs:subClassOf>
            <owl:Restriction>
                <owl:onProperty rdf:resource="http://purl.obolibrary.org/obo/BFO_0000051"/>
                <owl:someValuesFrom rdf:resource="https://w3id.org/aio/InputLayer"/>
            </owl:Restriction>
        </rdfs:subClassOf>
        <rdfs:subClassOf>
            <owl:Restriction>
                <owl:onProperty rdf:resource="http://purl.obolibrary.org/obo/BFO_0000051"/>
                <owl:someValuesFrom rdf:resource="https://w3id.org/aio/OutputLayer"/>
            </owl:Restriction>
        </rdfs:subClassOf>
        <obo:IAO_0000115>A machine learning designed to learn continuous feature representations for nodes in a graph by optimizing a neighborhood-preserving objective.</obo:IAO_0000115>
        <oboInOwl:hasExactSynonym>N2V</oboInOwl:hasExactSynonym>
        <oboInOwl:inSubset rdf:resource="https://w3id.org/aio/NetworkSubset"/>
        <rdfs:comment>Layers: Input, Hidden, Output</rdfs:comment>
        <rdfs:label>node2vec</rdfs:label>
    </owl:Class>
    <owl:Axiom>
        <owl:annotatedSource rdf:resource="https://w3id.org/aio/node2vec"/>
        <owl:annotatedProperty rdf:resource="http://purl.obolibrary.org/obo/IAO_0000115"/>
        <owl:annotatedTarget>A machine learning designed to learn continuous feature representations for nodes in a graph by optimizing a neighborhood-preserving objective.</owl:annotatedTarget>
        <oboInOwl:hasDbXref rdf:resource="https://en.wikipedia.org/wiki/Node2vec"/>
    </owl:Axiom>
    


    <!-- https://w3id.org/aio/node2vecCBOW -->

    <owl:Class rdf:about="https://w3id.org/aio/node2vecCBOW">
        <rdfs:subClassOf rdf:resource="https://w3id.org/aio/word2vec"/>
        <obo:IAO_0000115>A node2vec that predicts the current node from a window of surrounding context nodes, with the order of context nodes not influencing prediction.</obo:IAO_0000115>
        <oboInOwl:hasExactSynonym>N2V-CBOW</oboInOwl:hasExactSynonym>
        <oboInOwl:hasRelatedSynonym>CBOW</oboInOwl:hasRelatedSynonym>
        <oboInOwl:inSubset rdf:resource="https://w3id.org/aio/NetworkSubset"/>
        <rdfs:comment>Layers: Input, Hidden, Output</rdfs:comment>
        <rdfs:label>node2vec-CBOW</rdfs:label>
    </owl:Class>
    <owl:Axiom>
        <owl:annotatedSource rdf:resource="https://w3id.org/aio/node2vecCBOW"/>
        <owl:annotatedProperty rdf:resource="http://purl.obolibrary.org/obo/IAO_0000115"/>
        <owl:annotatedTarget>A node2vec that predicts the current node from a window of surrounding context nodes, with the order of context nodes not influencing prediction.</owl:annotatedTarget>
        <oboInOwl:hasDbXref rdf:resource="https://en.wikipedia.org/wiki/Word2vec"/>
    </owl:Axiom>
    


    <!-- https://w3id.org/aio/node2vecSkipGram -->

    <owl:Class rdf:about="https://w3id.org/aio/node2vecSkipGram">
        <rdfs:subClassOf rdf:resource="https://w3id.org/aio/node2vec"/>
        <obo:IAO_0000115>A node2vec that uses the current node to predict the surrounding window of context nodes, weighing nearby context nodes more heavily than distant ones.</obo:IAO_0000115>
        <oboInOwl:hasExactSynonym>N2V-SkipGram</oboInOwl:hasExactSynonym>
        <oboInOwl:hasRelatedSynonym>SkipGram</oboInOwl:hasRelatedSynonym>
        <oboInOwl:inSubset rdf:resource="https://w3id.org/aio/NetworkSubset"/>
        <rdfs:comment>Layers: Input, Hidden, Output</rdfs:comment>
        <rdfs:label>node2vec-SkipGram</rdfs:label>
    </owl:Class>
    <owl:Axiom>
        <owl:annotatedSource rdf:resource="https://w3id.org/aio/node2vecSkipGram"/>
        <owl:annotatedProperty rdf:resource="http://purl.obolibrary.org/obo/IAO_0000115"/>
        <owl:annotatedTarget>A node2vec that uses the current node to predict the surrounding window of context nodes, weighing nearby context nodes more heavily than distant ones.</owl:annotatedTarget>
        <oboInOwl:hasDbXref rdf:resource="https://en.wikipedia.org/wiki/Word2vec"/>
    </owl:Axiom>
    


    <!-- https://w3id.org/aio/tDistributedStochasticNeighborembedding -->

    <owl:Class rdf:about="https://w3id.org/aio/tDistributedStochasticNeighborembedding">
        <rdfs:subClassOf rdf:resource="https://w3id.org/aio/DimensionalityReduction"/>
        <obo:IAO_0000115>A dimensionality reduction for visualizing high-dimensional data by giving each datapoint a location in a two or three-dimensional map.</obo:IAO_0000115>
        <oboInOwl:hasExactSynonym>t-SNE</oboInOwl:hasExactSynonym>
        <oboInOwl:hasExactSynonym>tSNE</oboInOwl:hasExactSynonym>
        <oboInOwl:inSubset rdf:resource="https://w3id.org/aio/MachineLearningSubset"/>
        <rdfs:label>t-Distributed Stochastic Neighbor embedding</rdfs:label>
    </owl:Class>
    <owl:Axiom>
        <owl:annotatedSource rdf:resource="https://w3id.org/aio/tDistributedStochasticNeighborembedding"/>
        <owl:annotatedProperty rdf:resource="http://purl.obolibrary.org/obo/IAO_0000115"/>
        <owl:annotatedTarget>A dimensionality reduction for visualizing high-dimensional data by giving each datapoint a location in a two or three-dimensional map.</owl:annotatedTarget>
        <oboInOwl:hasDbXref rdf:resource="https://en.wikipedia.org/wiki/T-distributed_stochastic_neighbor_embedding"/>
    </owl:Axiom>
    


    <!-- https://w3id.org/aio/word2vec -->

    <owl:Class rdf:about="https://w3id.org/aio/word2vec">
        <rdfs:subClassOf rdf:resource="https://w3id.org/aio/MachineLearning"/>
        <rdfs:subClassOf>
            <owl:Restriction>
                <owl:onProperty rdf:resource="http://purl.obolibrary.org/obo/BFO_0000051"/>
                <owl:someValuesFrom rdf:resource="https://w3id.org/aio/HiddenLayer"/>
            </owl:Restriction>
        </rdfs:subClassOf>
        <rdfs:subClassOf>
            <owl:Restriction>
                <owl:onProperty rdf:resource="http://purl.obolibrary.org/obo/BFO_0000051"/>
                <owl:someValuesFrom rdf:resource="https://w3id.org/aio/InputLayer"/>
            </owl:Restriction>
        </rdfs:subClassOf>
        <rdfs:subClassOf>
            <owl:Restriction>
                <owl:onProperty rdf:resource="http://purl.obolibrary.org/obo/BFO_0000051"/>
                <owl:someValuesFrom rdf:resource="https://w3id.org/aio/OutputLayer"/>
            </owl:Restriction>
        </rdfs:subClassOf>
        <obo:IAO_0000115>A machine learning that generates distributed representations of words by training a shallow neural network model, which aims to predict the context of each word within a corpus. This algorithm captures semantic meanings of words through their contextual usage in the text.</obo:IAO_0000115>
        <oboInOwl:hasExactSynonym>W2V</oboInOwl:hasExactSynonym>
        <oboInOwl:inSubset rdf:resource="https://w3id.org/aio/NetworkSubset"/>
        <rdfs:comment>Layers: Input, Hidden, Output</rdfs:comment>
        <rdfs:label>word2vec</rdfs:label>
    </owl:Class>
    <owl:Axiom>
        <owl:annotatedSource rdf:resource="https://w3id.org/aio/word2vec"/>
        <owl:annotatedProperty rdf:resource="http://purl.obolibrary.org/obo/IAO_0000115"/>
        <owl:annotatedTarget>A machine learning that generates distributed representations of words by training a shallow neural network model, which aims to predict the context of each word within a corpus. This algorithm captures semantic meanings of words through their contextual usage in the text.</owl:annotatedTarget>
        <oboInOwl:hasDbXref rdf:resource="https://en.wikipedia.org/wiki/Word2vec"/>
    </owl:Axiom>
    


    <!-- https://w3id.org/aio/word2vecCBOW -->

    <owl:Class rdf:about="https://w3id.org/aio/word2vecCBOW">
        <rdfs:subClassOf rdf:resource="https://w3id.org/aio/word2vec"/>
        <obo:IAO_0000115>A word2vec that predicts the current word from a window of surrounding context words, ignoring the order of context words.</obo:IAO_0000115>
        <oboInOwl:hasExactSynonym>W2V-CBOW</oboInOwl:hasExactSynonym>
        <oboInOwl:hasRelatedSynonym>CBOW</oboInOwl:hasRelatedSynonym>
        <oboInOwl:inSubset rdf:resource="https://w3id.org/aio/NetworkSubset"/>
        <rdfs:comment>Layers: Input, Hidden, Output</rdfs:comment>
        <rdfs:label>word2vec-CBOW</rdfs:label>
    </owl:Class>
    <owl:Axiom>
        <owl:annotatedSource rdf:resource="https://w3id.org/aio/word2vecCBOW"/>
        <owl:annotatedProperty rdf:resource="http://purl.obolibrary.org/obo/IAO_0000115"/>
        <owl:annotatedTarget>A word2vec that predicts the current word from a window of surrounding context words, ignoring the order of context words.</owl:annotatedTarget>
        <oboInOwl:hasDbXref rdf:resource="https://en.wikipedia.org/wiki/Word2vec"/>
    </owl:Axiom>
    


    <!-- https://w3id.org/aio/word2vecSkipGram -->

    <owl:Class rdf:about="https://w3id.org/aio/word2vecSkipGram">
        <rdfs:subClassOf rdf:resource="https://w3id.org/aio/word2vec"/>
        <obo:IAO_0000115>A word2vec that predicts surrounding context words from the current word, giving more weight to nearby context words than distant ones.</obo:IAO_0000115>
        <oboInOwl:hasExactSynonym>W2V-SkipGram</oboInOwl:hasExactSynonym>
        <oboInOwl:hasRelatedSynonym>SkipGram</oboInOwl:hasRelatedSynonym>
        <oboInOwl:inSubset rdf:resource="https://w3id.org/aio/NetworkSubset"/>
        <rdfs:comment>Layers: Input, Hidden, Output</rdfs:comment>
        <rdfs:label>word2vec-SkipGram</rdfs:label>
    </owl:Class>
    <owl:Axiom>
        <owl:annotatedSource rdf:resource="https://w3id.org/aio/word2vecSkipGram"/>
        <owl:annotatedProperty rdf:resource="http://purl.obolibrary.org/obo/IAO_0000115"/>
        <owl:annotatedTarget>A word2vec that predicts surrounding context words from the current word, giving more weight to nearby context words than distant ones.</owl:annotatedTarget>
        <oboInOwl:hasDbXref rdf:resource="https://en.wikipedia.org/wiki/Word2vec"/>
    </owl:Axiom>
    


    <!-- 
    ///////////////////////////////////////////////////////////////////////////////////////
    //
    // Annotations
    //
    ///////////////////////////////////////////////////////////////////////////////////////
     -->

    <rdf:Description rdf:about="http://purl.obolibrary.org/obo/BFO_0000051">
        <obo:IAO_0000115 xml:lang="en">A core relation that holds between a whole and its part</obo:IAO_0000115>
        <rdfs:label xml:lang="en">has part</rdfs:label>
    </rdf:Description>
</rdf:RDF>



<!-- Generated by the OWL API (version 4.5.26) https://github.com/owlcs/owlapi -->

